<?xml version="1.0"?>
<rdf:RDF xmlns="http://www.semanticweb.org/oberreb4/ontologies/2018/9/INTRO#"
     xml:base="http://www.semanticweb.org/oberreb4/ontologies/2018/9/INTRO"
     xmlns:rdf="http://www.w3.org/1999/02/22-rdf-syntax-ns#"
     xmlns:owl="http://www.w3.org/2002/07/owl#"
     xmlns:xml="http://www.w3.org/XML/1998/namespace"
     xmlns:xsd="http://www.w3.org/2001/XMLSchema#"
     xmlns:skos="http://www.w3.org/2004/02/skos/core#"
     xmlns:rdfs="http://www.w3.org/2000/01/rdf-schema#"
     xmlns:dc="http://purl.org/dc/elements/1.1/">
    <owl:Ontology rdf:about="http://www.semanticweb.org/oberreb4/ontologies/2018/9/INTRO">
        <owl:imports rdf:resource="http://erlangen-crm.org/efrbroo/"/>
        <dc:title xml:lang="en">INTRO - the Intertextual Relationships Ontology</dc:title>
        <rdfs:label rdf:datatype="http://www.w3.org/2001/XMLSchema#string">INTRO</rdfs:label>
        <owl:versionInfo rdf:datatype="http://www.w3.org/2001/XMLSchema#string">BETA</owl:versionInfo>
        <dc:creator rdf:datatype="http://www.w3.org/2001/XMLSchema#string"> Bernhard Oberreither </dc:creator>
    </owl:Ontology>
    


    <!-- 
    ///////////////////////////////////////////////////////////////////////////////////////
    //
    // Annotation properties
    //
    ///////////////////////////////////////////////////////////////////////////////////////
     -->

    


    <!-- http://purl.org/dc/elements/1.1/description -->

    <owl:AnnotationProperty rdf:about="http://purl.org/dc/elements/1.1/description"/>
    


    <!-- 
    ///////////////////////////////////////////////////////////////////////////////////////
    //
    // Object Properties
    //
    ///////////////////////////////////////////////////////////////////////////////////////
     -->

    


    <!-- http://www.semanticweb.org/oberreb4/ontologies/2018/9/INTRO#R10_has_Text_Passage -->

    <owl:ObjectProperty rdf:about="http://www.semanticweb.org/oberreb4/ontologies/2018/9/INTRO#R10_has_Text_Passage">
        <owl:inverseOf rdf:resource="http://www.semanticweb.org/oberreb4/ontologies/2018/9/INTRO#R10_is_Text_Passage_of"/>
        <rdfs:domain>
            <owl:Class>
                <owl:unionOf rdf:parseType="Collection">
                    <rdf:Description rdf:about="http://erlangen-crm.org/efrbroo/F1_Work"/>
                    <rdf:Description rdf:about="http://erlangen-crm.org/efrbroo/F2_Expression"/>
                </owl:unionOf>
            </owl:Class>
        </rdfs:domain>
        <rdfs:range rdf:resource="http://www.semanticweb.org/oberreb4/ontologies/2018/9/INTRO#INT1_Text_Passage"/>
        <rdfs:comment>Links a F24 Publication Expression to a INT1 Text passage from that F24 Publication Expression, e.g. the book with the ISBN 978-0307278630 to a passage on page three of this book.</rdfs:comment>
    </owl:ObjectProperty>
    


    <!-- http://www.semanticweb.org/oberreb4/ontologies/2018/9/INTRO#R10_is_Text_Passage_of -->

    <owl:ObjectProperty rdf:about="http://www.semanticweb.org/oberreb4/ontologies/2018/9/INTRO#R10_is_Text_Passage_of">
        <rdfs:domain rdf:resource="http://www.semanticweb.org/oberreb4/ontologies/2018/9/INTRO#INT1_Text_Passage"/>
        <rdfs:range>
            <owl:Class>
                <owl:unionOf rdf:parseType="Collection">
                    <rdf:Description rdf:about="http://erlangen-crm.org/efrbroo/F1_Work"/>
                    <rdf:Description rdf:about="http://erlangen-crm.org/efrbroo/F2_Expression"/>
                </owl:unionOf>
            </owl:Class>
        </rdfs:range>
        <rdfs:comment>Links an INT1 Text Passage from a F24 Publication Expression  to that F24 Publication Expression, e.g. a passage on page three of the book with the ISBN 978-0307278630 to that book.</rdfs:comment>
    </owl:ObjectProperty>
    


    <!-- http://www.semanticweb.org/oberreb4/ontologies/2018/9/INTRO#R11_has_fragment -->

    <owl:ObjectProperty rdf:about="http://www.semanticweb.org/oberreb4/ontologies/2018/9/INTRO#R11_has_fragment">
        <owl:inverseOf rdf:resource="http://www.semanticweb.org/oberreb4/ontologies/2018/9/INTRO#R11_is_fragment_of"/>
        <rdfs:domain rdf:resource="http://www.semanticweb.org/oberreb4/ontologies/2018/9/INTRO#INT1_Text_Passage"/>
        <rdfs:range rdf:resource="http://www.semanticweb.org/oberreb4/ontologies/2018/9/INTRO#INT1_Text_Passage"/>
        <rdfs:comment>Links a INT1 Text Passage to shorter INT1 Text Passages it contains.</rdfs:comment>
    </owl:ObjectProperty>
    


    <!-- http://www.semanticweb.org/oberreb4/ontologies/2018/9/INTRO#R11_is_fragment_of -->

    <owl:ObjectProperty rdf:about="http://www.semanticweb.org/oberreb4/ontologies/2018/9/INTRO#R11_is_fragment_of">
        <rdfs:domain rdf:resource="http://www.semanticweb.org/oberreb4/ontologies/2018/9/INTRO#INT1_Text_Passage"/>
        <rdfs:range rdf:resource="http://www.semanticweb.org/oberreb4/ontologies/2018/9/INTRO#INT1_Text_Passage"/>
        <rdfs:comment>Links a INT1 Text Passage to a larger INT1 Text Passage it is a part of.</rdfs:comment>
    </owl:ObjectProperty>
    


    <!-- http://www.semanticweb.org/oberreb4/ontologies/2018/9/INTRO#R12_has_referred_to_entity -->

    <owl:ObjectProperty rdf:about="http://www.semanticweb.org/oberreb4/ontologies/2018/9/INTRO#R12_has_referred_to_entity">
        <rdfs:subPropertyOf rdf:resource="http://www.semanticweb.org/oberreb4/ontologies/2018/9/INTRO#R24_has_related_entity"/>
        <owl:inverseOf rdf:resource="http://www.semanticweb.org/oberreb4/ontologies/2018/9/INTRO#R12_is_referred_to_entity"/>
        <rdfs:domain rdf:resource="http://www.semanticweb.org/oberreb4/ontologies/2018/9/INTRO#INT4_Intertextual_Relationship"/>
        <rdfs:range>
            <owl:Class>
                <owl:unionOf rdf:parseType="Collection">
                    <rdf:Description rdf:about="http://erlangen-crm.org/efrbroo/F1_Work"/>
                    <rdf:Description rdf:about="http://erlangen-crm.org/efrbroo/F2_Expression"/>
                    <rdf:Description rdf:about="http://www.semanticweb.org/oberreb4/ontologies/2018/9/INTRO#INT3_Architextual_Entity"/>
                    <rdf:Description rdf:about="http://www.semanticweb.org/oberreb4/ontologies/2018/9/INTRO#INT5_Actualization_of_Feature"/>
                </owl:unionOf>
            </owl:Class>
        </rdfs:range>
    </owl:ObjectProperty>
    


    <!-- http://www.semanticweb.org/oberreb4/ontologies/2018/9/INTRO#R12_is_referred_to_entity -->

    <owl:ObjectProperty rdf:about="http://www.semanticweb.org/oberreb4/ontologies/2018/9/INTRO#R12_is_referred_to_entity">
        <rdfs:subPropertyOf rdf:resource="http://www.semanticweb.org/oberreb4/ontologies/2018/9/INTRO#R24_is_related_entity"/>
        <rdfs:domain>
            <owl:Class>
                <owl:unionOf rdf:parseType="Collection">
                    <rdf:Description rdf:about="http://erlangen-crm.org/efrbroo/F1_Work"/>
                    <rdf:Description rdf:about="http://erlangen-crm.org/efrbroo/F2_Expression"/>
                    <rdf:Description rdf:about="http://www.semanticweb.org/oberreb4/ontologies/2018/9/INTRO#INT3_Architextual_Entity"/>
                    <rdf:Description rdf:about="http://www.semanticweb.org/oberreb4/ontologies/2018/9/INTRO#INT5_Actualization_of_Feature"/>
                </owl:unionOf>
            </owl:Class>
        </rdfs:domain>
        <rdfs:range rdf:resource="http://www.semanticweb.org/oberreb4/ontologies/2018/9/INTRO#INT4_Intertextual_Relationship"/>
    </owl:ObjectProperty>
    


    <!-- http://www.semanticweb.org/oberreb4/ontologies/2018/9/INTRO#R13_has_referring_entity -->

    <owl:ObjectProperty rdf:about="http://www.semanticweb.org/oberreb4/ontologies/2018/9/INTRO#R13_has_referring_entity">
        <rdfs:subPropertyOf rdf:resource="http://www.semanticweb.org/oberreb4/ontologies/2018/9/INTRO#R24_has_related_entity"/>
        <owl:inverseOf rdf:resource="http://www.semanticweb.org/oberreb4/ontologies/2018/9/INTRO#R13_is_referring_entity"/>
        <rdfs:domain rdf:resource="http://www.semanticweb.org/oberreb4/ontologies/2018/9/INTRO#INT4_Intertextual_Relationship"/>
        <rdfs:range>
            <owl:Class>
                <owl:unionOf rdf:parseType="Collection">
                    <rdf:Description rdf:about="http://erlangen-crm.org/efrbroo/F1_Work"/>
                    <rdf:Description rdf:about="http://erlangen-crm.org/efrbroo/F2_Expression"/>
                    <rdf:Description rdf:about="http://www.semanticweb.org/oberreb4/ontologies/2018/9/INTRO#INT3_Architextual_Entity"/>
                    <rdf:Description rdf:about="http://www.semanticweb.org/oberreb4/ontologies/2018/9/INTRO#INT5_Actualization_of_Feature"/>
                </owl:unionOf>
            </owl:Class>
        </rdfs:range>
        <rdfs:comment>Links an INT4 Reference to a referring entity (a text on any ontological level).</rdfs:comment>
    </owl:ObjectProperty>
    


    <!-- http://www.semanticweb.org/oberreb4/ontologies/2018/9/INTRO#R13_is_referring_entity -->

    <owl:ObjectProperty rdf:about="http://www.semanticweb.org/oberreb4/ontologies/2018/9/INTRO#R13_is_referring_entity">
        <rdfs:subPropertyOf rdf:resource="http://www.semanticweb.org/oberreb4/ontologies/2018/9/INTRO#R24_is_related_entity"/>
        <rdfs:domain>
            <owl:Class>
                <owl:unionOf rdf:parseType="Collection">
                    <rdf:Description rdf:about="http://erlangen-crm.org/efrbroo/F1_Work"/>
                    <rdf:Description rdf:about="http://erlangen-crm.org/efrbroo/F2_Expression"/>
                    <rdf:Description rdf:about="http://www.semanticweb.org/oberreb4/ontologies/2018/9/INTRO#INT3_Architextual_Entity"/>
                    <rdf:Description rdf:about="http://www.semanticweb.org/oberreb4/ontologies/2018/9/INTRO#INT5_Actualization_of_Feature"/>
                </owl:unionOf>
            </owl:Class>
        </rdfs:domain>
        <rdfs:range rdf:resource="http://www.semanticweb.org/oberreb4/ontologies/2018/9/INTRO#INT4_Intertextual_Relationship"/>
        <rdfs:comment>Links the referring entity (a text on any ontological level) to the INT4 Reference it constitutes.</rdfs:comment>
    </owl:ObjectProperty>
    


    <!-- http://www.semanticweb.org/oberreb4/ontologies/2018/9/INTRO#R14_likeness_supported_by -->

    <owl:ObjectProperty rdf:about="http://www.semanticweb.org/oberreb4/ontologies/2018/9/INTRO#R14_likeness_supported_by">
        <owl:inverseOf rdf:resource="http://www.semanticweb.org/oberreb4/ontologies/2018/9/INTRO#R14_supports_likeness"/>
        <rdfs:domain rdf:resource="http://www.semanticweb.org/oberreb4/ontologies/2018/9/INTRO#INT3_Architextual_Entity"/>
        <rdfs:range rdf:resource="http://www.semanticweb.org/oberreb4/ontologies/2018/9/INTRO#INT6_Characteristic"/>
        <rdfs:comment>Links an INT3 Architextual Entity to an INT6 Characteristic that, found on a text, establishes a likeness to the INT3 Architextual Entity. For Example: The appearance of a ghost in a text establishes a likeness to the &apos;Gothic novel&apos;.</rdfs:comment>
    </owl:ObjectProperty>
    


    <!-- http://www.semanticweb.org/oberreb4/ontologies/2018/9/INTRO#R14_supports_likeness -->

    <owl:ObjectProperty rdf:about="http://www.semanticweb.org/oberreb4/ontologies/2018/9/INTRO#R14_supports_likeness">
        <rdfs:domain rdf:resource="http://www.semanticweb.org/oberreb4/ontologies/2018/9/INTRO#INT6_Characteristic"/>
        <rdfs:range rdf:resource="http://www.semanticweb.org/oberreb4/ontologies/2018/9/INTRO#INT3_Architextual_Entity"/>
    </owl:ObjectProperty>
    


    <!-- http://www.semanticweb.org/oberreb4/ontologies/2018/9/INTRO#R15_non-affiliation_supported_by -->

    <owl:ObjectProperty rdf:about="http://www.semanticweb.org/oberreb4/ontologies/2018/9/INTRO#R15_non-affiliation_supported_by">
        <owl:inverseOf rdf:resource="http://www.semanticweb.org/oberreb4/ontologies/2018/9/INTRO#R15_supports_non-affiliation"/>
        <rdfs:domain rdf:resource="http://www.semanticweb.org/oberreb4/ontologies/2018/9/INTRO#INT3_Architextual_Entity"/>
        <rdfs:range rdf:resource="http://www.semanticweb.org/oberreb4/ontologies/2018/9/INTRO#INT6_Characteristic"/>
        <rdfs:comment>Links an INT3 Architextual Entity to a INT6 Characteristic that, found on a text, is a reason to consider the text not an element of the INT3 Architextual Entity. For Example: The appearance of a teenage vampire could be a reason to consider a text not a representative of a &apos;Bildungsroman&apos;.</rdfs:comment>
    </owl:ObjectProperty>
    


    <!-- http://www.semanticweb.org/oberreb4/ontologies/2018/9/INTRO#R15_supports_non-affiliation -->

    <owl:ObjectProperty rdf:about="http://www.semanticweb.org/oberreb4/ontologies/2018/9/INTRO#R15_supports_non-affiliation">
        <rdfs:domain rdf:resource="http://www.semanticweb.org/oberreb4/ontologies/2018/9/INTRO#INT6_Characteristic"/>
        <rdfs:range rdf:resource="http://www.semanticweb.org/oberreb4/ontologies/2018/9/INTRO#INT3_Architextual_Entity"/>
        <rdfs:comment>Links to a INT6 Characteristic, that, found on a text, is a reason to consider the text not an element of a specific INT3 Architextual Entity, to that INT3 Architextual Entity. For example: The appearance of a ghost is a reason not to consider a text a representative of the genre &apos;crime fiction&apos;.</rdfs:comment>
    </owl:ObjectProperty>
    


    <!-- http://www.semanticweb.org/oberreb4/ontologies/2018/9/INTRO#R16_supports_unlikeness -->

    <owl:ObjectProperty rdf:about="http://www.semanticweb.org/oberreb4/ontologies/2018/9/INTRO#R16_supports_unlikeness">
        <owl:inverseOf rdf:resource="http://www.semanticweb.org/oberreb4/ontologies/2018/9/INTRO#R16_unlikeness_supported_by"/>
        <rdfs:domain rdf:resource="http://www.semanticweb.org/oberreb4/ontologies/2018/9/INTRO#INT6_Characteristic"/>
        <rdfs:range rdf:resource="http://www.semanticweb.org/oberreb4/ontologies/2018/9/INTRO#INT3_Architextual_Entity"/>
    </owl:ObjectProperty>
    


    <!-- http://www.semanticweb.org/oberreb4/ontologies/2018/9/INTRO#R16_unlikeness_supported_by -->

    <owl:ObjectProperty rdf:about="http://www.semanticweb.org/oberreb4/ontologies/2018/9/INTRO#R16_unlikeness_supported_by">
        <rdfs:domain rdf:resource="http://www.semanticweb.org/oberreb4/ontologies/2018/9/INTRO#INT3_Architextual_Entity"/>
        <rdfs:range rdf:resource="http://www.semanticweb.org/oberreb4/ontologies/2018/9/INTRO#INT6_Characteristic"/>
    </owl:ObjectProperty>
    


    <!-- http://www.semanticweb.org/oberreb4/ontologies/2018/9/INTRO#R17_actualizes_feature -->

    <owl:ObjectProperty rdf:about="http://www.semanticweb.org/oberreb4/ontologies/2018/9/INTRO#R17_actualizes_feature">
        <owl:inverseOf rdf:resource="http://www.semanticweb.org/oberreb4/ontologies/2018/9/INTRO#R17_feature_actualized_in"/>
        <rdfs:domain rdf:resource="http://www.semanticweb.org/oberreb4/ontologies/2018/9/INTRO#INT5_Actualization_of_Feature"/>
        <rdfs:range rdf:resource="http://www.semanticweb.org/oberreb4/ontologies/2018/9/INTRO#INT2_Receptional_Entity"/>
        <rdfs:comment>Links the specific INT5 Actualization of Feature to the (abstract concept of the) feature it actualizes, a INT2 Receptional Entity.</rdfs:comment>
    </owl:ObjectProperty>
    


    <!-- http://www.semanticweb.org/oberreb4/ontologies/2018/9/INTRO#R17_feature_actualized_in -->

    <owl:ObjectProperty rdf:about="http://www.semanticweb.org/oberreb4/ontologies/2018/9/INTRO#R17_feature_actualized_in">
        <rdfs:domain rdf:resource="http://www.semanticweb.org/oberreb4/ontologies/2018/9/INTRO#INT2_Receptional_Entity"/>
        <rdfs:range rdf:resource="http://www.semanticweb.org/oberreb4/ontologies/2018/9/INTRO#INT5_Actualization_of_Feature"/>
        <rdfs:comment>Links the INT2 Receptional Entity, the feature, to an INT5 Actualization of Feature (that is itself linked to a specific text).</rdfs:comment>
    </owl:ObjectProperty>
    


    <!-- http://www.semanticweb.org/oberreb4/ontologies/2018/9/INTRO#R18_actualization_found_on -->

    <owl:ObjectProperty rdf:about="http://www.semanticweb.org/oberreb4/ontologies/2018/9/INTRO#R18_actualization_found_on">
        <owl:inverseOf rdf:resource="http://www.semanticweb.org/oberreb4/ontologies/2018/9/INTRO#R18_shows_actualization"/>
        <rdfs:domain rdf:resource="http://www.semanticweb.org/oberreb4/ontologies/2018/9/INTRO#INT5_Actualization_of_Feature"/>
        <rdfs:range>
            <owl:Class>
                <owl:unionOf rdf:parseType="Collection">
                    <rdf:Description rdf:about="http://erlangen-crm.org/efrbroo/F1_Work"/>
                    <rdf:Description rdf:about="http://erlangen-crm.org/efrbroo/F2_Expression"/>
                    <rdf:Description rdf:about="http://www.semanticweb.org/oberreb4/ontologies/2018/9/INTRO#INT3_Architextual_Entity"/>
                    <rdf:Description rdf:about="http://www.semanticweb.org/oberreb4/ontologies/2018/9/INTRO#INT5_Actualization_of_Feature"/>
                </owl:unionOf>
            </owl:Class>
        </rdfs:range>
    </owl:ObjectProperty>
    


    <!-- http://www.semanticweb.org/oberreb4/ontologies/2018/9/INTRO#R18_shows_actualization -->

    <owl:ObjectProperty rdf:about="http://www.semanticweb.org/oberreb4/ontologies/2018/9/INTRO#R18_shows_actualization">
        <rdfs:domain>
            <owl:Class>
                <owl:unionOf rdf:parseType="Collection">
                    <rdf:Description rdf:about="http://erlangen-crm.org/efrbroo/F1_Work"/>
                    <rdf:Description rdf:about="http://erlangen-crm.org/efrbroo/F2_Expression"/>
                    <rdf:Description rdf:about="http://www.semanticweb.org/oberreb4/ontologies/2018/9/INTRO#INT3_Architextual_Entity"/>
                    <rdf:Description rdf:about="http://www.semanticweb.org/oberreb4/ontologies/2018/9/INTRO#INT5_Actualization_of_Feature"/>
                </owl:unionOf>
            </owl:Class>
        </rdfs:domain>
        <rdfs:range rdf:resource="http://www.semanticweb.org/oberreb4/ontologies/2018/9/INTRO#INT5_Actualization_of_Feature"/>
    </owl:ObjectProperty>
    


    <!-- http://www.semanticweb.org/oberreb4/ontologies/2018/9/INTRO#R19_has_type -->

    <owl:ObjectProperty rdf:about="http://www.semanticweb.org/oberreb4/ontologies/2018/9/INTRO#R19_has_type">
        <rdfs:subPropertyOf rdf:resource="http://erlangen-crm.org/current/P2_has_type"/>
        <owl:inverseOf rdf:resource="http://www.semanticweb.org/oberreb4/ontologies/2018/9/INTRO#R19_is_type_of"/>
        <rdfs:domain rdf:resource="http://www.semanticweb.org/oberreb4/ontologies/2018/9/INTRO#INT4_Intertextual_Relationship"/>
        <rdfs:range rdf:resource="http://www.semanticweb.org/oberreb4/ontologies/2018/9/INTRO#INT22_Type_of_Intertextual_Relationship"/>
        <rdfs:comment>Links an INT4 Reference to its INT22 Type of Intertextual Relationship.</rdfs:comment>
    </owl:ObjectProperty>
    


    <!-- http://www.semanticweb.org/oberreb4/ontologies/2018/9/INTRO#R19_is_type_of -->

    <owl:ObjectProperty rdf:about="http://www.semanticweb.org/oberreb4/ontologies/2018/9/INTRO#R19_is_type_of">
        <rdfs:subPropertyOf rdf:resource="http://erlangen-crm.org/current/P2i_is_type_of"/>
        <rdfs:domain rdf:resource="http://www.semanticweb.org/oberreb4/ontologies/2018/9/INTRO#INT22_Type_of_Intertextual_Relationship"/>
        <rdfs:range rdf:resource="http://www.semanticweb.org/oberreb4/ontologies/2018/9/INTRO#INT4_Intertextual_Relationship"/>
        <rdfs:comment>Links a INT22 Type of Intertextual Relationship to the INT4 Reference of that type.</rdfs:comment>
    </owl:ObjectProperty>
    


    <!-- http://www.semanticweb.org/oberreb4/ontologies/2018/9/INTRO#R1_affiliation_supported_by -->

    <owl:ObjectProperty rdf:about="http://www.semanticweb.org/oberreb4/ontologies/2018/9/INTRO#R1_affiliation_supported_by">
        <owl:inverseOf rdf:resource="http://www.semanticweb.org/oberreb4/ontologies/2018/9/INTRO#R1_supports_affiliation_to"/>
        <rdfs:domain rdf:resource="http://www.semanticweb.org/oberreb4/ontologies/2018/9/INTRO#INT3_Architextual_Entity"/>
        <rdfs:range rdf:resource="http://www.semanticweb.org/oberreb4/ontologies/2018/9/INTRO#INT6_Characteristic"/>
        <rdfs:comment>Links an INT3 Architextual Entity to a INT6 Characteristic that, found on a text, is a reason to consider the text an element of the INT3 Architextual Entity. For example: The appearance of a ghost is a reason to consider a text a representative of the &apos;Gothic novel&apos;.</rdfs:comment>
    </owl:ObjectProperty>
    


    <!-- http://www.semanticweb.org/oberreb4/ontologies/2018/9/INTRO#R1_supports_affiliation_to -->

    <owl:ObjectProperty rdf:about="http://www.semanticweb.org/oberreb4/ontologies/2018/9/INTRO#R1_supports_affiliation_to">
        <rdfs:domain rdf:resource="http://www.semanticweb.org/oberreb4/ontologies/2018/9/INTRO#INT6_Characteristic"/>
        <rdfs:range rdf:resource="http://www.semanticweb.org/oberreb4/ontologies/2018/9/INTRO#INT3_Architextual_Entity"/>
        <rdfs:comment>Links to an INT3 Architextual Entity a INT6 Characteristic that, if found on a text, is a reason to consider the text an element of the INT3 Architextual Entity. For example: The appearance of a ghost is a reason to consider a text a representative of the &apos;Gothic novel&apos;.</rdfs:comment>
    </owl:ObjectProperty>
    


    <!-- http://www.semanticweb.org/oberreb4/ontologies/2018/9/INTRO#R20_discusses -->

    <owl:ObjectProperty rdf:about="http://www.semanticweb.org/oberreb4/ontologies/2018/9/INTRO#R20_discusses">
        <rdfs:subPropertyOf rdf:resource="http://erlangen-crm.org/current/P67_refers_to"/>
        <owl:inverseOf rdf:resource="http://www.semanticweb.org/oberreb4/ontologies/2018/9/INTRO#R20_is_discussed_in"/>
        <rdfs:domain rdf:resource="http://www.semanticweb.org/oberreb4/ontologies/2018/9/INTRO#INT44_Interpretament"/>
        <rdfs:range>
            <owl:Class>
                <owl:unionOf rdf:parseType="Collection">
                    <rdf:Description rdf:about="http://erlangen-crm.org/efrbroo/F1_Work"/>
                    <rdf:Description rdf:about="http://erlangen-crm.org/efrbroo/F2_Expression"/>
                    <rdf:Description rdf:about="http://www.semanticweb.org/oberreb4/ontologies/2018/9/INTRO#INT3_Architextual_Entity"/>
                </owl:unionOf>
            </owl:Class>
        </rdfs:range>
        <rdfs:comment>Links an INT44 Interpretament to the textual instance (on any ontological level) it discusses.</rdfs:comment>
    </owl:ObjectProperty>
    


    <!-- http://www.semanticweb.org/oberreb4/ontologies/2018/9/INTRO#R20_is_discussed_in -->

    <owl:ObjectProperty rdf:about="http://www.semanticweb.org/oberreb4/ontologies/2018/9/INTRO#R20_is_discussed_in">
        <rdfs:subPropertyOf rdf:resource="http://erlangen-crm.org/current/P67i_is_referred_to_by"/>
        <rdfs:domain>
            <owl:Class>
                <owl:unionOf rdf:parseType="Collection">
                    <rdf:Description rdf:about="http://erlangen-crm.org/efrbroo/F1_Work"/>
                    <rdf:Description rdf:about="http://erlangen-crm.org/efrbroo/F2_Expression"/>
                    <rdf:Description rdf:about="http://www.semanticweb.org/oberreb4/ontologies/2018/9/INTRO#INT3_Architextual_Entity"/>
                </owl:unionOf>
            </owl:Class>
        </rdfs:domain>
        <rdfs:range rdf:resource="http://www.semanticweb.org/oberreb4/ontologies/2018/9/INTRO#INT44_Interpretament"/>
        <rdfs:comment>Links a textual instance (on any ontological level) to the INT44 Interpretament it is discussed in.</rdfs:comment>
    </owl:ObjectProperty>
    


    <!-- http://www.semanticweb.org/oberreb4/ontologies/2018/9/INTRO#R21_identifies -->

    <owl:ObjectProperty rdf:about="http://www.semanticweb.org/oberreb4/ontologies/2018/9/INTRO#R21_identifies">
        <rdfs:subPropertyOf rdf:resource="http://erlangen-crm.org/current/P67_refers_to"/>
        <owl:inverseOf rdf:resource="http://www.semanticweb.org/oberreb4/ontologies/2018/9/INTRO#R21_is_identified_by"/>
        <rdfs:domain rdf:resource="http://www.semanticweb.org/oberreb4/ontologies/2018/9/INTRO#INT44_Interpretament"/>
        <rdfs:range>
            <owl:Class>
                <owl:unionOf rdf:parseType="Collection">
                    <rdf:Description rdf:about="http://www.semanticweb.org/oberreb4/ontologies/2018/9/INTRO#INT4_Intertextual_Relationship"/>
                    <rdf:Description rdf:about="http://www.semanticweb.org/oberreb4/ontologies/2018/9/INTRO#INT5_Actualization_of_Feature"/>
                    <rdf:Description rdf:about="http://www.semanticweb.org/oberreb4/ontologies/2018/9/INTRO#INT6_Characteristic"/>
                </owl:unionOf>
            </owl:Class>
        </rdfs:range>
        <rdfs:comment>Links an INT44 Interpretament to the INT6 Characteristic, the INT4 Reference or the INT5 Actualization of Feature it identifies.</rdfs:comment>
    </owl:ObjectProperty>
    


    <!-- http://www.semanticweb.org/oberreb4/ontologies/2018/9/INTRO#R21_is_identified_by -->

    <owl:ObjectProperty rdf:about="http://www.semanticweb.org/oberreb4/ontologies/2018/9/INTRO#R21_is_identified_by">
        <rdfs:subPropertyOf rdf:resource="http://erlangen-crm.org/current/P67i_is_referred_to_by"/>
        <rdfs:domain>
            <owl:Class>
                <owl:unionOf rdf:parseType="Collection">
                    <rdf:Description rdf:about="http://www.semanticweb.org/oberreb4/ontologies/2018/9/INTRO#INT4_Intertextual_Relationship"/>
                    <rdf:Description rdf:about="http://www.semanticweb.org/oberreb4/ontologies/2018/9/INTRO#INT5_Actualization_of_Feature"/>
                    <rdf:Description rdf:about="http://www.semanticweb.org/oberreb4/ontologies/2018/9/INTRO#INT6_Characteristic"/>
                </owl:unionOf>
            </owl:Class>
        </rdfs:domain>
        <rdfs:range rdf:resource="http://www.semanticweb.org/oberreb4/ontologies/2018/9/INTRO#INT44_Interpretament"/>
        <rdfs:comment>Links an INT6 Characteristic, an INT4 Reference or an INT5 Actualization of Featurea to the INT44 Interpretament it is identified in.</rdfs:comment>
    </owl:ObjectProperty>
    


    <!-- http://www.semanticweb.org/oberreb4/ontologies/2018/9/INTRO#R22_provides_similarity_for_reference -->

    <owl:ObjectProperty rdf:about="http://www.semanticweb.org/oberreb4/ontologies/2018/9/INTRO#R22_provides_similarity_for_reference">
        <owl:inverseOf rdf:resource="http://www.semanticweb.org/oberreb4/ontologies/2018/9/INTRO#R22_reference_is_based_on_similarity"/>
        <rdfs:domain rdf:resource="http://www.semanticweb.org/oberreb4/ontologies/2018/9/INTRO#INT2_Receptional_Entity"/>
        <rdfs:range rdf:resource="http://www.semanticweb.org/oberreb4/ontologies/2018/9/INTRO#INT4_Intertextual_Relationship"/>
        <rdfs:comment>Links a INT2 Receptional Entity to a INT4 Reference it provides the similarity for, the similarity being necessary for the detection of the INT4 Reference. States that an INT4 Reference is based on a similarity, i.e. the occurrence of the same INT2 Receptional Entity in two different texts.</rdfs:comment>
    </owl:ObjectProperty>
    


    <!-- http://www.semanticweb.org/oberreb4/ontologies/2018/9/INTRO#R22_reference_is_based_on_similarity -->

    <owl:ObjectProperty rdf:about="http://www.semanticweb.org/oberreb4/ontologies/2018/9/INTRO#R22_reference_is_based_on_similarity">
        <rdfs:domain rdf:resource="http://www.semanticweb.org/oberreb4/ontologies/2018/9/INTRO#INT4_Intertextual_Relationship"/>
        <rdfs:range rdf:resource="http://www.semanticweb.org/oberreb4/ontologies/2018/9/INTRO#INT2_Receptional_Entity"/>
        <rdfs:comment>Links an INT4 Reference to an INT2 Receptional Entity that provides the similarity necessary for the detection of the INT4 Reference. States that an INT4 Reference is based on a similarity, i.e. the occurrence of the same receptional entity in two different texts.</rdfs:comment>
    </owl:ObjectProperty>
    


    <!-- http://www.semanticweb.org/oberreb4/ontologies/2018/9/INTRO#R23_provides_support_for -->

    <owl:ObjectProperty rdf:about="http://www.semanticweb.org/oberreb4/ontologies/2018/9/INTRO#R23_provides_support_for">
        <owl:inverseOf rdf:resource="http://www.semanticweb.org/oberreb4/ontologies/2018/9/INTRO#R23_support_provided_by"/>
        <rdfs:domain>
            <owl:Class>
                <owl:unionOf rdf:parseType="Collection">
                    <rdf:Description rdf:about="http://erlangen-crm.org/efrbroo/F1_Work"/>
                    <rdf:Description rdf:about="http://erlangen-crm.org/efrbroo/F2_Expression"/>
                    <rdf:Description rdf:about="http://www.semanticweb.org/oberreb4/ontologies/2018/9/INTRO#INT3_Architextual_Entity"/>
                    <rdf:Description rdf:about="http://www.semanticweb.org/oberreb4/ontologies/2018/9/INTRO#INT5_Actualization_of_Feature"/>
                </owl:unionOf>
            </owl:Class>
        </rdfs:domain>
        <rdfs:range>
            <owl:Class>
                <owl:unionOf rdf:parseType="Collection">
                    <rdf:Description rdf:about="http://www.semanticweb.org/oberreb4/ontologies/2018/9/INTRO#INT2_Receptional_Entity"/>
                    <rdf:Description rdf:about="http://www.semanticweb.org/oberreb4/ontologies/2018/9/INTRO#INT44_Interpretament"/>
                    <rdf:Description rdf:about="http://www.semanticweb.org/oberreb4/ontologies/2018/9/INTRO#INT4_Intertextual_Relationship"/>
                    <rdf:Description rdf:about="http://www.semanticweb.org/oberreb4/ontologies/2018/9/INTRO#INT5_Actualization_of_Feature"/>
                    <rdf:Description rdf:about="http://www.semanticweb.org/oberreb4/ontologies/2018/9/INTRO#INT6_Characteristic"/>
                </owl:unionOf>
            </owl:Class>
        </rdfs:range>
        <rdfs:comment>Relates a source (a text on any ontological level) to the outcome of a receptional or interpretative act (an INT6 Characteristic, an INT5 Actualization of Feature, a INT2 Receptional Entity, an INT4 Reference, an INT44 Interpretament) to support it.</rdfs:comment>
    </owl:ObjectProperty>
    


    <!-- http://www.semanticweb.org/oberreb4/ontologies/2018/9/INTRO#R23_support_provided_by -->

    <owl:ObjectProperty rdf:about="http://www.semanticweb.org/oberreb4/ontologies/2018/9/INTRO#R23_support_provided_by">
        <rdfs:domain>
            <owl:Class>
                <owl:unionOf rdf:parseType="Collection">
                    <rdf:Description rdf:about="http://www.semanticweb.org/oberreb4/ontologies/2018/9/INTRO#INT2_Receptional_Entity"/>
                    <rdf:Description rdf:about="http://www.semanticweb.org/oberreb4/ontologies/2018/9/INTRO#INT44_Interpretament"/>
                    <rdf:Description rdf:about="http://www.semanticweb.org/oberreb4/ontologies/2018/9/INTRO#INT4_Intertextual_Relationship"/>
                    <rdf:Description rdf:about="http://www.semanticweb.org/oberreb4/ontologies/2018/9/INTRO#INT5_Actualization_of_Feature"/>
                    <rdf:Description rdf:about="http://www.semanticweb.org/oberreb4/ontologies/2018/9/INTRO#INT6_Characteristic"/>
                </owl:unionOf>
            </owl:Class>
        </rdfs:domain>
        <rdfs:range>
            <owl:Class>
                <owl:unionOf rdf:parseType="Collection">
                    <rdf:Description rdf:about="http://erlangen-crm.org/efrbroo/F1_Work"/>
                    <rdf:Description rdf:about="http://erlangen-crm.org/efrbroo/F2_Expression"/>
                    <rdf:Description rdf:about="http://www.semanticweb.org/oberreb4/ontologies/2018/9/INTRO#INT3_Architextual_Entity"/>
                    <rdf:Description rdf:about="http://www.semanticweb.org/oberreb4/ontologies/2018/9/INTRO#INT5_Actualization_of_Feature"/>
                </owl:unionOf>
            </owl:Class>
        </rdfs:range>
        <rdfs:comment>Relates the decision made in any receptional or interpretative act - the determination of an INT6 Characteristic, an INT5 Actualization of Feature, a INT2 Receptional Entity, an INT4 Reference, an INT44 Interpretament - to a source that can support this decision (a text on any ontological level).</rdfs:comment>
    </owl:ObjectProperty>
    


    <!-- http://www.semanticweb.org/oberreb4/ontologies/2018/9/INTRO#R24_has_related_entity -->

    <owl:ObjectProperty rdf:about="http://www.semanticweb.org/oberreb4/ontologies/2018/9/INTRO#R24_has_related_entity">
        <owl:inverseOf rdf:resource="http://www.semanticweb.org/oberreb4/ontologies/2018/9/INTRO#R24_is_related_entity"/>
        <rdfs:domain rdf:resource="http://www.semanticweb.org/oberreb4/ontologies/2018/9/INTRO#INT4_Intertextual_Relationship"/>
        <rdfs:range>
            <owl:Class>
                <owl:unionOf rdf:parseType="Collection">
                    <rdf:Description rdf:about="http://erlangen-crm.org/efrbroo/F1_Work"/>
                    <rdf:Description rdf:about="http://erlangen-crm.org/efrbroo/F2_Expression"/>
                    <rdf:Description rdf:about="http://www.semanticweb.org/oberreb4/ontologies/2018/9/INTRO#INT3_Architextual_Entity"/>
                    <rdf:Description rdf:about="http://www.semanticweb.org/oberreb4/ontologies/2018/9/INTRO#INT5_Actualization_of_Feature"/>
                </owl:unionOf>
            </owl:Class>
        </rdfs:range>
        <rdfs:comment>Links any INT4 Intertextual Relationship to a text (on any ontological level) or INT5 Actualization of Feature that is part of the INT4 Intertextual Relationship.</rdfs:comment>
    </owl:ObjectProperty>
    


    <!-- http://www.semanticweb.org/oberreb4/ontologies/2018/9/INTRO#R24_is_related_entity -->

    <owl:ObjectProperty rdf:about="http://www.semanticweb.org/oberreb4/ontologies/2018/9/INTRO#R24_is_related_entity">
        <rdfs:domain>
            <owl:Class>
                <owl:unionOf rdf:parseType="Collection">
                    <rdf:Description rdf:about="http://erlangen-crm.org/efrbroo/F1_Work"/>
                    <rdf:Description rdf:about="http://erlangen-crm.org/efrbroo/F2_Expression"/>
                    <rdf:Description rdf:about="http://www.semanticweb.org/oberreb4/ontologies/2018/9/INTRO#INT3_Architextual_Entity"/>
                    <rdf:Description rdf:about="http://www.semanticweb.org/oberreb4/ontologies/2018/9/INTRO#INT5_Actualization_of_Feature"/>
                </owl:unionOf>
            </owl:Class>
        </rdfs:domain>
        <rdfs:range rdf:resource="http://www.semanticweb.org/oberreb4/ontologies/2018/9/INTRO#INT4_Intertextual_Relationship"/>
        <rdfs:comment>Links any text (on any ontological level) or INT5 Actualization of Feature to the INT4 Intertextual Relationship it is a part of.</rdfs:comment>
    </owl:ObjectProperty>
    


    <!-- http://www.semanticweb.org/oberreb4/ontologies/2018/9/INTRO#R2_consists_in -->

    <owl:ObjectProperty rdf:about="http://www.semanticweb.org/oberreb4/ontologies/2018/9/INTRO#R2_consists_in">
        <owl:inverseOf rdf:resource="http://www.semanticweb.org/oberreb4/ontologies/2018/9/INTRO#R2_constitutes"/>
        <rdfs:domain>
            <owl:Class>
                <owl:unionOf rdf:parseType="Collection">
                    <rdf:Description rdf:about="http://www.semanticweb.org/oberreb4/ontologies/2018/9/INTRO#INT44_Interpretament"/>
                    <rdf:Description rdf:about="http://www.semanticweb.org/oberreb4/ontologies/2018/9/INTRO#INT6_Characteristic"/>
                </owl:unionOf>
            </owl:Class>
        </rdfs:domain>
        <rdfs:range rdf:resource="http://www.semanticweb.org/oberreb4/ontologies/2018/9/INTRO#INT5_Actualization_of_Feature"/>
        <rdfs:comment>Links a INT6 Characteristic of a text to the INT5 Actualization of Feature in order to state that the Feature is &apos;characteristic&apos;, meaning: it affiliates the text with an INT3 Architextual Entity.
Also used to link an INT44_Interpretament to the INT5 Actualization of feature, in this case: of the semantic feature INT31_Interpretation.</rdfs:comment>
    </owl:ObjectProperty>
    


    <!-- http://www.semanticweb.org/oberreb4/ontologies/2018/9/INTRO#R2_constitutes -->

    <owl:ObjectProperty rdf:about="http://www.semanticweb.org/oberreb4/ontologies/2018/9/INTRO#R2_constitutes">
        <rdfs:domain rdf:resource="http://www.semanticweb.org/oberreb4/ontologies/2018/9/INTRO#INT5_Actualization_of_Feature"/>
        <rdfs:range>
            <owl:Class>
                <owl:unionOf rdf:parseType="Collection">
                    <rdf:Description rdf:about="http://www.semanticweb.org/oberreb4/ontologies/2018/9/INTRO#INT44_Interpretament"/>
                    <rdf:Description rdf:about="http://www.semanticweb.org/oberreb4/ontologies/2018/9/INTRO#INT6_Characteristic"/>
                </owl:unionOf>
            </owl:Class>
        </rdfs:range>
        <rdfs:comment>States that a feature as actualized in a specific text can be seen as a characteristic and thus affiliating the text with an INT3 Architextual Entity.
Also used to state that the actualization of the semantic feature INT31_Interpretation can be seen as an INT44 Interpretament and thus identify INT4_References, INT6_Characteristics and so on.</rdfs:comment>
    </owl:ObjectProperty>
    


    <!-- http://www.semanticweb.org/oberreb4/ontologies/2018/9/INTRO#R3_constellates -->

    <owl:ObjectProperty rdf:about="http://www.semanticweb.org/oberreb4/ontologies/2018/9/INTRO#R3_constellates">
        <owl:inverseOf rdf:resource="http://www.semanticweb.org/oberreb4/ontologies/2018/9/INTRO#R3_is_constellated_by"/>
        <rdfs:domain rdf:resource="http://www.semanticweb.org/oberreb4/ontologies/2018/9/INTRO#INT29_Constellation"/>
        <rdfs:range rdf:resource="http://www.semanticweb.org/oberreb4/ontologies/2018/9/INTRO#INT5_Actualization_of_Feature"/>
        <rdfs:comment>Links an INT29 Constellation to the elements (INT5 Actualizations of Feature) that together form that INT29 Constellation.</rdfs:comment>
    </owl:ObjectProperty>
    


    <!-- http://www.semanticweb.org/oberreb4/ontologies/2018/9/INTRO#R3_is_constellated_by -->

    <owl:ObjectProperty rdf:about="http://www.semanticweb.org/oberreb4/ontologies/2018/9/INTRO#R3_is_constellated_by">
        <rdfs:domain rdf:resource="http://www.semanticweb.org/oberreb4/ontologies/2018/9/INTRO#INT5_Actualization_of_Feature"/>
        <rdfs:range rdf:resource="http://www.semanticweb.org/oberreb4/ontologies/2018/9/INTRO#INT29_Constellation"/>
        <rdfs:comment>Links INT5 Actualizations of Feature of at least two INT2_Receptional_Entitiess with the INT29 Constellation they form (i.e. stating that they do so).</rdfs:comment>
    </owl:ObjectProperty>
    


    <!-- http://www.semanticweb.org/oberreb4/ontologies/2018/9/INTRO#R4_defines -->

    <owl:ObjectProperty rdf:about="http://www.semanticweb.org/oberreb4/ontologies/2018/9/INTRO#R4_defines">
        <owl:inverseOf rdf:resource="http://www.semanticweb.org/oberreb4/ontologies/2018/9/INTRO#R4_is_defined_in"/>
        <rdfs:domain rdf:resource="http://www.semanticweb.org/oberreb4/ontologies/2018/9/INTRO#INT5_Actualization_of_Feature"/>
        <rdfs:range>
            <owl:Class>
                <owl:unionOf rdf:parseType="Collection">
                    <rdf:Description rdf:about="http://www.semanticweb.org/oberreb4/ontologies/2018/9/INTRO#INT22_Type_of_Intertextual_Relationship"/>
                    <rdf:Description rdf:about="http://www.semanticweb.org/oberreb4/ontologies/2018/9/INTRO#INT2_Receptional_Entity"/>
                    <rdf:Description rdf:about="http://www.semanticweb.org/oberreb4/ontologies/2018/9/INTRO#INT3_Architextual_Entity"/>
                </owl:unionOf>
            </owl:Class>
        </rdfs:range>
        <rdfs:comment>Relates the actualization (usually: of the semantic feature &apos;definition&apos;) to a type of intertextual relationship and to receptional, transtextual and supratextual entities and thereby links a concept - e.g. &apos;discourse&apos; - to a definition - e.g. in Foucault&apos;s writings.</rdfs:comment>
    </owl:ObjectProperty>
    


    <!-- http://www.semanticweb.org/oberreb4/ontologies/2018/9/INTRO#R4_is_defined_in -->

    <owl:ObjectProperty rdf:about="http://www.semanticweb.org/oberreb4/ontologies/2018/9/INTRO#R4_is_defined_in">
        <rdfs:domain>
            <owl:Class>
                <owl:unionOf rdf:parseType="Collection">
                    <rdf:Description rdf:about="http://www.semanticweb.org/oberreb4/ontologies/2018/9/INTRO#INT22_Type_of_Intertextual_Relationship"/>
                    <rdf:Description rdf:about="http://www.semanticweb.org/oberreb4/ontologies/2018/9/INTRO#INT2_Receptional_Entity"/>
                    <rdf:Description rdf:about="http://www.semanticweb.org/oberreb4/ontologies/2018/9/INTRO#INT3_Architextual_Entity"/>
                </owl:unionOf>
            </owl:Class>
        </rdfs:domain>
        <rdfs:range rdf:resource="http://www.semanticweb.org/oberreb4/ontologies/2018/9/INTRO#INT5_Actualization_of_Feature"/>
        <rdfs:comment>Relates a type of intertextual relationship or a receptional, transtextual and supratextual entity to the actualization of a feature (usually: of the semantic feature &apos;definition&apos;) in order to link a definition - e.g. in Foucault&apos;s writings - to the concept it defines - e.g. &apos;discourse&apos;.</rdfs:comment>
    </owl:ObjectProperty>
    


    <!-- http://www.semanticweb.org/oberreb4/ontologies/2018/9/INTRO#R5_has_appurtenant_element -->

    <owl:ObjectProperty rdf:about="http://www.semanticweb.org/oberreb4/ontologies/2018/9/INTRO#R5_has_appurtenant_element">
        <owl:inverseOf rdf:resource="http://www.semanticweb.org/oberreb4/ontologies/2018/9/INTRO#R5_is_appurtenant_element"/>
        <rdfs:domain rdf:resource="http://www.semanticweb.org/oberreb4/ontologies/2018/9/INTRO#INT3_Architextual_Entity"/>
        <rdfs:range>
            <owl:Class>
                <owl:unionOf rdf:parseType="Collection">
                    <rdf:Description rdf:about="http://erlangen-crm.org/efrbroo/F1_Work"/>
                    <rdf:Description rdf:about="http://erlangen-crm.org/efrbroo/F2_Expression"/>
                    <rdf:Description rdf:about="http://www.semanticweb.org/oberreb4/ontologies/2018/9/INTRO#INT3_Architextual_Entity"/>
                </owl:unionOf>
            </owl:Class>
        </rdfs:range>
        <rdfs:comment>Links a transtextual entity to a text (on any ontological level) that is an element of the transtextual entity.</rdfs:comment>
    </owl:ObjectProperty>
    


    <!-- http://www.semanticweb.org/oberreb4/ontologies/2018/9/INTRO#R5_is_appurtenant_element -->

    <owl:ObjectProperty rdf:about="http://www.semanticweb.org/oberreb4/ontologies/2018/9/INTRO#R5_is_appurtenant_element">
        <rdfs:domain>
            <owl:Class>
                <owl:unionOf rdf:parseType="Collection">
                    <rdf:Description rdf:about="http://erlangen-crm.org/efrbroo/F1_Work"/>
                    <rdf:Description rdf:about="http://erlangen-crm.org/efrbroo/F2_Expression"/>
                    <rdf:Description rdf:about="http://www.semanticweb.org/oberreb4/ontologies/2018/9/INTRO#INT3_Architextual_Entity"/>
                </owl:unionOf>
            </owl:Class>
        </rdfs:domain>
        <rdfs:range rdf:resource="http://www.semanticweb.org/oberreb4/ontologies/2018/9/INTRO#INT3_Architextual_Entity"/>
        <rdfs:comment>Links a text (on any ontological level) to a transtextual entity that it is an element of.</rdfs:comment>
    </owl:ObjectProperty>
    


    <!-- http://www.semanticweb.org/oberreb4/ontologies/2018/9/INTRO#R6_has_initial_element -->

    <owl:ObjectProperty rdf:about="http://www.semanticweb.org/oberreb4/ontologies/2018/9/INTRO#R6_has_initial_element">
        <rdfs:subPropertyOf rdf:resource="http://www.semanticweb.org/oberreb4/ontologies/2018/9/INTRO#R5_has_appurtenant_element"/>
        <owl:inverseOf rdf:resource="http://www.semanticweb.org/oberreb4/ontologies/2018/9/INTRO#R7_is_initial_element"/>
    </owl:ObjectProperty>
    


    <!-- http://www.semanticweb.org/oberreb4/ontologies/2018/9/INTRO#R6_has_representative_element -->

    <owl:ObjectProperty rdf:about="http://www.semanticweb.org/oberreb4/ontologies/2018/9/INTRO#R6_has_representative_element">
        <rdfs:subPropertyOf rdf:resource="http://www.semanticweb.org/oberreb4/ontologies/2018/9/INTRO#R5_has_appurtenant_element"/>
        <owl:inverseOf rdf:resource="http://www.semanticweb.org/oberreb4/ontologies/2018/9/INTRO#R7_is_representative_element"/>
    </owl:ObjectProperty>
    


    <!-- http://www.semanticweb.org/oberreb4/ontologies/2018/9/INTRO#R7_is_initial_element -->

    <owl:ObjectProperty rdf:about="http://www.semanticweb.org/oberreb4/ontologies/2018/9/INTRO#R7_is_initial_element">
        <rdfs:subPropertyOf rdf:resource="http://www.semanticweb.org/oberreb4/ontologies/2018/9/INTRO#R5_is_appurtenant_element"/>
    </owl:ObjectProperty>
    


    <!-- http://www.semanticweb.org/oberreb4/ontologies/2018/9/INTRO#R7_is_representative_element -->

    <owl:ObjectProperty rdf:about="http://www.semanticweb.org/oberreb4/ontologies/2018/9/INTRO#R7_is_representative_element">
        <rdfs:subPropertyOf rdf:resource="http://www.semanticweb.org/oberreb4/ontologies/2018/9/INTRO#R5_is_appurtenant_element"/>
    </owl:ObjectProperty>
    


    <!-- http://www.semanticweb.org/oberreb4/ontologies/2018/9/INTRO#R8_has_opinion_object -->

    <owl:ObjectProperty rdf:about="http://www.semanticweb.org/oberreb4/ontologies/2018/9/INTRO#R8_has_opinion_object">
        <owl:inverseOf rdf:resource="http://www.semanticweb.org/oberreb4/ontologies/2018/9/INTRO#R8_is_opinion_object_of"/>
        <rdfs:domain rdf:resource="http://www.semanticweb.org/oberreb4/ontologies/2018/9/INTRO#INT34_Opinion"/>
        <rdfs:range rdf:resource="http://www.w3.org/2002/07/owl#Thing"/>
        <rdfs:comment>Links an opinion with its object - for example an opinion with the theme fashion (to make it an opinion about fashion).</rdfs:comment>
    </owl:ObjectProperty>
    


    <!-- http://www.semanticweb.org/oberreb4/ontologies/2018/9/INTRO#R8_is_opinion_object_of -->

    <owl:ObjectProperty rdf:about="http://www.semanticweb.org/oberreb4/ontologies/2018/9/INTRO#R8_is_opinion_object_of">
        <rdfs:domain rdf:resource="http://www.w3.org/2002/07/owl#Thing"/>
        <rdfs:range rdf:resource="http://www.semanticweb.org/oberreb4/ontologies/2018/9/INTRO#INT34_Opinion"/>
        <rdfs:comment>Links an object with an opinion about it.</rdfs:comment>
    </owl:ObjectProperty>
    


    <!-- http://www.semanticweb.org/oberreb4/ontologies/2018/9/INTRO#R9_has_preceding_interpretament -->

    <owl:ObjectProperty rdf:about="http://www.semanticweb.org/oberreb4/ontologies/2018/9/INTRO#R9_has_preceding_interpretament">
        <owl:inverseOf rdf:resource="http://www.semanticweb.org/oberreb4/ontologies/2018/9/INTRO#R9_has_subsequent_interpretament"/>
        <rdf:type rdf:resource="http://www.w3.org/2002/07/owl#TransitiveProperty"/>
        <rdfs:domain rdf:resource="http://www.semanticweb.org/oberreb4/ontologies/2018/9/INTRO#INT44_Interpretament"/>
        <rdfs:range rdf:resource="http://www.semanticweb.org/oberreb4/ontologies/2018/9/INTRO#INT44_Interpretament"/>
        <rdfs:comment>Links two interpretamets who have a linear (logical or chronological) order.</rdfs:comment>
    </owl:ObjectProperty>
    


    <!-- http://www.semanticweb.org/oberreb4/ontologies/2018/9/INTRO#R9_has_subsequent_interpretament -->

    <owl:ObjectProperty rdf:about="http://www.semanticweb.org/oberreb4/ontologies/2018/9/INTRO#R9_has_subsequent_interpretament">
        <rdf:type rdf:resource="http://www.w3.org/2002/07/owl#TransitiveProperty"/>
        <rdfs:domain rdf:resource="http://www.semanticweb.org/oberreb4/ontologies/2018/9/INTRO#INT44_Interpretament"/>
        <rdfs:range rdf:resource="http://www.semanticweb.org/oberreb4/ontologies/2018/9/INTRO#INT44_Interpretament"/>
        <rdfs:comment>Links two interpretamets who have a linear (logical or chronological) order.</rdfs:comment>
    </owl:ObjectProperty>
    


    <!-- 
    ///////////////////////////////////////////////////////////////////////////////////////
    //
    // Data properties
    //
    ///////////////////////////////////////////////////////////////////////////////////////
     -->

    


    <!-- http://www.semanticweb.org/oberreb4/ontologies/2018/9/INTRO#R40_has_bibliographical_data -->

    <owl:DatatypeProperty rdf:about="http://www.semanticweb.org/oberreb4/ontologies/2018/9/INTRO#R40_has_bibliographical_data">
        <rdfs:domain>
            <owl:Class>
                <owl:unionOf rdf:parseType="Collection">
                    <rdf:Description rdf:about="http://erlangen-crm.org/efrbroo/F1_Work"/>
                    <rdf:Description rdf:about="http://erlangen-crm.org/efrbroo/F2_Expression"/>
                </owl:unionOf>
            </owl:Class>
        </rdfs:domain>
        <rdfs:range rdf:resource="http://www.w3.org/2001/XMLSchema#string"/>
    </owl:DatatypeProperty>
    


    <!-- http://www.semanticweb.org/oberreb4/ontologies/2018/9/INTRO#R41_has_location -->

    <owl:DatatypeProperty rdf:about="http://www.semanticweb.org/oberreb4/ontologies/2018/9/INTRO#R41_has_location">
        <rdfs:domain rdf:resource="http://www.semanticweb.org/oberreb4/ontologies/2018/9/INTRO#INT1_Text_Passage"/>
        <rdfs:range rdf:resource="http://www.w3.org/2001/XMLSchema#string"/>
        <rdfs:comment>Defines the exact location of an INT1 Text Passage in a Publication Expression.</rdfs:comment>
    </owl:DatatypeProperty>
    


    <!-- http://www.semanticweb.org/oberreb4/ontologies/2018/9/INTRO#R42_has_paraphrase_or_definition -->

    <owl:DatatypeProperty rdf:about="http://www.semanticweb.org/oberreb4/ontologies/2018/9/INTRO#R42_has_paraphrase_or_definition">
        <rdfs:domain>
            <owl:Class>
                <owl:unionOf rdf:parseType="Collection">
                    <rdf:Description rdf:about="http://www.semanticweb.org/oberreb4/ontologies/2018/9/INTRO#INT22_Type_of_Intertextual_Relationship"/>
                    <rdf:Description rdf:about="http://www.semanticweb.org/oberreb4/ontologies/2018/9/INTRO#INT2_Receptional_Entity"/>
                    <rdf:Description rdf:about="http://www.semanticweb.org/oberreb4/ontologies/2018/9/INTRO#INT3_Architextual_Entity"/>
                    <rdf:Description rdf:about="http://www.semanticweb.org/oberreb4/ontologies/2018/9/INTRO#INT44_Interpretament"/>
                    <rdf:Description rdf:about="http://www.semanticweb.org/oberreb4/ontologies/2018/9/INTRO#INT5_Actualization_of_Feature"/>
                    <rdf:Description rdf:about="http://www.semanticweb.org/oberreb4/ontologies/2018/9/INTRO#INT6_Characteristic"/>
                </owl:unionOf>
            </owl:Class>
        </rdfs:domain>
        <rdfs:range rdf:resource="http://www.w3.org/2001/XMLSchema#string"/>
    </owl:DatatypeProperty>
    


    <!-- http://www.semanticweb.org/oberreb4/ontologies/2018/9/INTRO#R43_has_specification -->

    <owl:DatatypeProperty rdf:about="http://www.semanticweb.org/oberreb4/ontologies/2018/9/INTRO#R43_has_specification">
        <rdfs:domain rdf:resource="http://www.semanticweb.org/oberreb4/ontologies/2018/9/INTRO#INT29_Constellation"/>
        <rdfs:range rdf:resource="http://www.w3.org/2001/XMLSchema#string"/>
    </owl:DatatypeProperty>
    


    <!-- http://www.semanticweb.org/oberreb4/ontologies/2018/9/INTRO#R44_has_wording -->

    <owl:DatatypeProperty rdf:about="http://www.semanticweb.org/oberreb4/ontologies/2018/9/INTRO#R44_has_wording">
        <rdfs:domain rdf:resource="http://www.semanticweb.org/oberreb4/ontologies/2018/9/INTRO#INT1_Text_Passage"/>
    </owl:DatatypeProperty>
    


    <!-- 
    ///////////////////////////////////////////////////////////////////////////////////////
    //
    // Classes
    //
    ///////////////////////////////////////////////////////////////////////////////////////
     -->

    


    <!-- http://erlangen-crm.org/efrbroo/F2_Expression -->

    <rdf:Description rdf:about="http://erlangen-crm.org/efrbroo/F2_Expression">
        <rdfs:subClassOf rdf:resource="http://www.semanticweb.org/oberreb4/ontologies/2018/9/INTRO#INT21_Text"/>
    </rdf:Description>
    


    <!-- http://www.semanticweb.org/oberreb4/ontologies/2018/9/INTRO#INT10_Discourse -->

    <owl:Class rdf:about="http://www.semanticweb.org/oberreb4/ontologies/2018/9/INTRO#INT10_Discourse">
        <rdfs:subClassOf rdf:resource="http://www.semanticweb.org/oberreb4/ontologies/2018/9/INTRO#INT3_Architextual_Entity"/>
    </owl:Class>
    


    <!-- http://www.semanticweb.org/oberreb4/ontologies/2018/9/INTRO#INT11_Discipline -->

    <owl:Class rdf:about="http://www.semanticweb.org/oberreb4/ontologies/2018/9/INTRO#INT11_Discipline">
        <rdfs:subClassOf rdf:resource="http://www.semanticweb.org/oberreb4/ontologies/2018/9/INTRO#INT3_Architextual_Entity"/>
    </owl:Class>
    


    <!-- http://www.semanticweb.org/oberreb4/ontologies/2018/9/INTRO#INT12_Epoch -->

    <owl:Class rdf:about="http://www.semanticweb.org/oberreb4/ontologies/2018/9/INTRO#INT12_Epoch">
        <rdfs:subClassOf rdf:resource="http://www.semanticweb.org/oberreb4/ontologies/2018/9/INTRO#INT3_Architextual_Entity"/>
    </owl:Class>
    


    <!-- http://www.semanticweb.org/oberreb4/ontologies/2018/9/INTRO#INT13_Genre_Trias -->

    <owl:Class rdf:about="http://www.semanticweb.org/oberreb4/ontologies/2018/9/INTRO#INT13_Genre_Trias">
        <rdfs:subClassOf rdf:resource="http://www.semanticweb.org/oberreb4/ontologies/2018/9/INTRO#INT3_Architextual_Entity"/>
    </owl:Class>
    


    <!-- http://www.semanticweb.org/oberreb4/ontologies/2018/9/INTRO#INT14_Genre_sub_Trias -->

    <owl:Class rdf:about="http://www.semanticweb.org/oberreb4/ontologies/2018/9/INTRO#INT14_Genre_sub_Trias">
        <rdfs:subClassOf rdf:resource="http://www.semanticweb.org/oberreb4/ontologies/2018/9/INTRO#INT3_Architextual_Entity"/>
    </owl:Class>
    


    <!-- http://www.semanticweb.org/oberreb4/ontologies/2018/9/INTRO#INT15_Movement -->

    <owl:Class rdf:about="http://www.semanticweb.org/oberreb4/ontologies/2018/9/INTRO#INT15_Movement">
        <rdfs:subClassOf rdf:resource="http://www.semanticweb.org/oberreb4/ontologies/2018/9/INTRO#INT3_Architextual_Entity"/>
    </owl:Class>
    


    <!-- http://www.semanticweb.org/oberreb4/ontologies/2018/9/INTRO#INT16_Oeuvre -->

    <owl:Class rdf:about="http://www.semanticweb.org/oberreb4/ontologies/2018/9/INTRO#INT16_Oeuvre">
        <rdfs:subClassOf rdf:resource="http://www.semanticweb.org/oberreb4/ontologies/2018/9/INTRO#INT3_Architextual_Entity"/>
    </owl:Class>
    


    <!-- http://www.semanticweb.org/oberreb4/ontologies/2018/9/INTRO#INT17_School -->

    <owl:Class rdf:about="http://www.semanticweb.org/oberreb4/ontologies/2018/9/INTRO#INT17_School">
        <rdfs:subClassOf rdf:resource="http://www.semanticweb.org/oberreb4/ontologies/2018/9/INTRO#INT3_Architextual_Entity"/>
    </owl:Class>
    


    <!-- http://www.semanticweb.org/oberreb4/ontologies/2018/9/INTRO#INT18_Spacially_defined_Architext -->

    <owl:Class rdf:about="http://www.semanticweb.org/oberreb4/ontologies/2018/9/INTRO#INT18_Spacially_defined_Architext">
        <rdfs:subClassOf rdf:resource="http://www.semanticweb.org/oberreb4/ontologies/2018/9/INTRO#INT3_Architextual_Entity"/>
    </owl:Class>
    


    <!-- http://www.semanticweb.org/oberreb4/ontologies/2018/9/INTRO#INT19_Temporally_defined_Architext -->

    <owl:Class rdf:about="http://www.semanticweb.org/oberreb4/ontologies/2018/9/INTRO#INT19_Temporally_defined_Architext">
        <rdfs:subClassOf rdf:resource="http://www.semanticweb.org/oberreb4/ontologies/2018/9/INTRO#INT3_Architextual_Entity"/>
    </owl:Class>
    


    <!-- http://www.semanticweb.org/oberreb4/ontologies/2018/9/INTRO#INT1_Text_Passage -->

    <owl:Class rdf:about="http://www.semanticweb.org/oberreb4/ontologies/2018/9/INTRO#INT1_Text_Passage">
        <rdfs:subClassOf rdf:resource="http://erlangen-crm.org/efrbroo/F24_Publication_Expression"/>
        <rdfs:comment>An addition to FRBRoo due to the focus of this ontology.
FRBRoo&apos;s &apos;Expression Fragment&apos; is by definition a fragment of an expression, which is the immaterial realisation of a work - and for this reason cannot be object of a citation or a detailed bibliographical record (an expression has no page numbers). The FRBRoo &apos;Publication Expression&apos; is itself an immaterial (ideal) version of a text. However it adds concreteness to the &apos;Expression&apos;, it has a publisher, a publishing date, page numbers, an ISBN and so on.
The &apos;INT1 Text Passage&apos; is an identifiable part (a paragraph, a couple of lines, and so forth) of the &apos;Publication Expression&apos; - a &apos;Üublication Expression Fragment&apos;, so to speak.

For Example:
- the words &apos;Abandon all hope ye who enter here&apos; from page 3 of the publication with the ISBN 978-0307278630.</rdfs:comment>
    </owl:Class>
    


    <!-- http://www.semanticweb.org/oberreb4/ontologies/2018/9/INTRO#INT20_Variety_of_Text -->

    <owl:Class rdf:about="http://www.semanticweb.org/oberreb4/ontologies/2018/9/INTRO#INT20_Variety_of_Text">
        <rdfs:subClassOf rdf:resource="http://www.semanticweb.org/oberreb4/ontologies/2018/9/INTRO#INT3_Architextual_Entity"/>
    </owl:Class>
    


    <!-- http://www.semanticweb.org/oberreb4/ontologies/2018/9/INTRO#INT21_Text -->

    <owl:Class rdf:about="http://www.semanticweb.org/oberreb4/ontologies/2018/9/INTRO#INT21_Text">
        <rdfs:subClassOf rdf:resource="http://erlangen-crm.org/current/E71_Man-Made_Thing"/>
    </owl:Class>
    


    <!-- http://www.semanticweb.org/oberreb4/ontologies/2018/9/INTRO#INT22_Type_of_Intertextual_Relationship -->

    <owl:Class rdf:about="http://www.semanticweb.org/oberreb4/ontologies/2018/9/INTRO#INT22_Type_of_Intertextual_Relationship">
        <rdfs:subClassOf rdf:resource="http://erlangen-crm.org/current/E55_Type"/>
        <rdfs:comment>This class comprises (as subclasses) the many classifications of intertextual relationships that can be found, for example, in research literature, but also in greek rhetoric, in genre theory and so on.</rdfs:comment>
    </owl:Class>
    


    <!-- http://www.semanticweb.org/oberreb4/ontologies/2018/9/INTRO#INT23_Common_Concepts_of_Intertextuality -->

    <owl:Class rdf:about="http://www.semanticweb.org/oberreb4/ontologies/2018/9/INTRO#INT23_Common_Concepts_of_Intertextuality">
        <rdfs:subClassOf rdf:resource="http://www.semanticweb.org/oberreb4/ontologies/2018/9/INTRO#INT22_Type_of_Intertextual_Relationship"/>
    </owl:Class>
    


    <!-- http://www.semanticweb.org/oberreb4/ontologies/2018/9/INTRO#INT24_Intertextuality_in_Genre_Theory -->

    <owl:Class rdf:about="http://www.semanticweb.org/oberreb4/ontologies/2018/9/INTRO#INT24_Intertextuality_in_Genre_Theory">
        <rdfs:subClassOf rdf:resource="http://www.semanticweb.org/oberreb4/ontologies/2018/9/INTRO#INT22_Type_of_Intertextual_Relationship"/>
    </owl:Class>
    


    <!-- http://www.semanticweb.org/oberreb4/ontologies/2018/9/INTRO#INT25_Intertextuailty_in_Rhetoric -->

    <owl:Class rdf:about="http://www.semanticweb.org/oberreb4/ontologies/2018/9/INTRO#INT25_Intertextuailty_in_Rhetoric">
        <rdfs:subClassOf rdf:resource="http://www.semanticweb.org/oberreb4/ontologies/2018/9/INTRO#INT22_Type_of_Intertextual_Relationship"/>
    </owl:Class>
    


    <!-- http://www.semanticweb.org/oberreb4/ontologies/2018/9/INTRO#INT26_Intertextuality_Theories -->

    <owl:Class rdf:about="http://www.semanticweb.org/oberreb4/ontologies/2018/9/INTRO#INT26_Intertextuality_Theories">
        <rdfs:subClassOf rdf:resource="http://www.semanticweb.org/oberreb4/ontologies/2018/9/INTRO#INT22_Type_of_Intertextual_Relationship"/>
    </owl:Class>
    


    <!-- http://www.semanticweb.org/oberreb4/ontologies/2018/9/INTRO#INT27_Atmosphere -->

    <owl:Class rdf:about="http://www.semanticweb.org/oberreb4/ontologies/2018/9/INTRO#INT27_Atmosphere">
        <rdfs:subClassOf rdf:resource="http://www.semanticweb.org/oberreb4/ontologies/2018/9/INTRO#INT9_Semantic_Feature"/>
    </owl:Class>
    


    <!-- http://www.semanticweb.org/oberreb4/ontologies/2018/9/INTRO#INT28_Individual_Character -->

    <owl:Class rdf:about="http://www.semanticweb.org/oberreb4/ontologies/2018/9/INTRO#INT28_Individual_Character">
        <rdfs:subClassOf rdf:resource="http://www.semanticweb.org/oberreb4/ontologies/2018/9/INTRO#INT_Character"/>
    </owl:Class>
    


    <!-- http://www.semanticweb.org/oberreb4/ontologies/2018/9/INTRO#INT29_Constellation -->

    <owl:Class rdf:about="http://www.semanticweb.org/oberreb4/ontologies/2018/9/INTRO#INT29_Constellation">
        <rdfs:subClassOf rdf:resource="http://www.semanticweb.org/oberreb4/ontologies/2018/9/INTRO#INT9_Semantic_Feature"/>
    </owl:Class>
    


    <!-- http://www.semanticweb.org/oberreb4/ontologies/2018/9/INTRO#INT29_Definition -->

    <owl:Class rdf:about="http://www.semanticweb.org/oberreb4/ontologies/2018/9/INTRO#INT29_Definition">
        <rdfs:subClassOf rdf:resource="http://www.semanticweb.org/oberreb4/ontologies/2018/9/INTRO#INT9_Semantic_Feature"/>
    </owl:Class>
    


    <!-- http://www.semanticweb.org/oberreb4/ontologies/2018/9/INTRO#INT2_Receptional_Entity -->

    <owl:Class rdf:about="http://www.semanticweb.org/oberreb4/ontologies/2018/9/INTRO#INT2_Receptional_Entity">
        <rdfs:subClassOf rdf:resource="http://erlangen-crm.org/current/E28_Conceptual_Object"/>
        <rdfs:comment>Whatever &apos;is in&apos; or &apos;can be found in&apos; or &apos;can be read out of&apos; a text, apart from the wording itself. Strictly speaking: the result of a mental process that is applied to a text and that made out distinct abstract concepts which take a specific (yet identifiable and probably individual) form in the text.
This class therefore has an extremely wide scope, its subclasses are open to additions and are to be populated from relevant reference works (e.g. the subclass &apos;Rhetorical Entity&apos; could contain concepts based on Lausberg&apos;s &apos;Handbook of Literary Rhetoric&apos;, many lemmata from the &apos;Princeton Handbook of Poetic Terms&apos; could populate the subclass &quot;Formal Entity&quot; and so on).
It is highly likely (and welcome) that the instances of subclasses or sub-subclasses of the class &apos;receptional Entity&apos; are instances or sub-subclasses of more than one subclass (e.g. that a rhetorical entity is at the same time a semantic entity as in the case of an &apos;argument&apos; or &apos;rhyme&apos;).</rdfs:comment>
    </owl:Class>
    


    <!-- http://www.semanticweb.org/oberreb4/ontologies/2018/9/INTRO#INT30_Description -->

    <owl:Class rdf:about="http://www.semanticweb.org/oberreb4/ontologies/2018/9/INTRO#INT30_Description">
        <rdfs:subClassOf rdf:resource="http://www.semanticweb.org/oberreb4/ontologies/2018/9/INTRO#INT9_Semantic_Feature"/>
    </owl:Class>
    


    <!-- http://www.semanticweb.org/oberreb4/ontologies/2018/9/INTRO#INT31_Interpretation -->

    <owl:Class rdf:about="http://www.semanticweb.org/oberreb4/ontologies/2018/9/INTRO#INT31_Interpretation">
        <rdfs:subClassOf rdf:resource="http://www.semanticweb.org/oberreb4/ontologies/2018/9/INTRO#INT9_Semantic_Feature"/>
    </owl:Class>
    


    <!-- http://www.semanticweb.org/oberreb4/ontologies/2018/9/INTRO#INT32_Mood -->

    <owl:Class rdf:about="http://www.semanticweb.org/oberreb4/ontologies/2018/9/INTRO#INT32_Mood">
        <rdfs:subClassOf rdf:resource="http://www.semanticweb.org/oberreb4/ontologies/2018/9/INTRO#INT9_Semantic_Feature"/>
    </owl:Class>
    


    <!-- http://www.semanticweb.org/oberreb4/ontologies/2018/9/INTRO#INT33_Motif -->

    <owl:Class rdf:about="http://www.semanticweb.org/oberreb4/ontologies/2018/9/INTRO#INT33_Motif">
        <rdfs:subClassOf rdf:resource="http://www.semanticweb.org/oberreb4/ontologies/2018/9/INTRO#INT9_Semantic_Feature"/>
    </owl:Class>
    


    <!-- http://www.semanticweb.org/oberreb4/ontologies/2018/9/INTRO#INT34_Opinion -->

    <owl:Class rdf:about="http://www.semanticweb.org/oberreb4/ontologies/2018/9/INTRO#INT34_Opinion">
        <rdfs:subClassOf rdf:resource="http://www.semanticweb.org/oberreb4/ontologies/2018/9/INTRO#INT9_Semantic_Feature"/>
    </owl:Class>
    


    <!-- http://www.semanticweb.org/oberreb4/ontologies/2018/9/INTRO#INT35_Plot -->

    <owl:Class rdf:about="http://www.semanticweb.org/oberreb4/ontologies/2018/9/INTRO#INT35_Plot">
        <rdfs:subClassOf rdf:resource="http://www.semanticweb.org/oberreb4/ontologies/2018/9/INTRO#INT9_Semantic_Feature"/>
    </owl:Class>
    


    <!-- http://www.semanticweb.org/oberreb4/ontologies/2018/9/INTRO#INT36_Subject -->

    <owl:Class rdf:about="http://www.semanticweb.org/oberreb4/ontologies/2018/9/INTRO#INT36_Subject">
        <rdfs:subClassOf rdf:resource="http://www.semanticweb.org/oberreb4/ontologies/2018/9/INTRO#INT9_Semantic_Feature"/>
    </owl:Class>
    


    <!-- http://www.semanticweb.org/oberreb4/ontologies/2018/9/INTRO#INT37_Subtext -->

    <owl:Class rdf:about="http://www.semanticweb.org/oberreb4/ontologies/2018/9/INTRO#INT37_Subtext">
        <rdfs:subClassOf rdf:resource="http://www.semanticweb.org/oberreb4/ontologies/2018/9/INTRO#INT9_Semantic_Feature"/>
    </owl:Class>
    


    <!-- http://www.semanticweb.org/oberreb4/ontologies/2018/9/INTRO#INT38_Theme -->

    <owl:Class rdf:about="http://www.semanticweb.org/oberreb4/ontologies/2018/9/INTRO#INT38_Theme">
        <rdfs:subClassOf rdf:resource="http://www.semanticweb.org/oberreb4/ontologies/2018/9/INTRO#INT9_Semantic_Feature"/>
    </owl:Class>
    


    <!-- http://www.semanticweb.org/oberreb4/ontologies/2018/9/INTRO#INT39_Leitmotiv -->

    <owl:Class rdf:about="http://www.semanticweb.org/oberreb4/ontologies/2018/9/INTRO#INT39_Leitmotiv">
        <rdfs:subClassOf rdf:resource="http://www.semanticweb.org/oberreb4/ontologies/2018/9/INTRO#INT33_Motif"/>
    </owl:Class>
    


    <!-- http://www.semanticweb.org/oberreb4/ontologies/2018/9/INTRO#INT39_Topic -->

    <owl:Class rdf:about="http://www.semanticweb.org/oberreb4/ontologies/2018/9/INTRO#INT39_Topic">
        <rdfs:subClassOf rdf:resource="http://www.semanticweb.org/oberreb4/ontologies/2018/9/INTRO#INT9_Semantic_Feature"/>
    </owl:Class>
    


    <!-- http://www.semanticweb.org/oberreb4/ontologies/2018/9/INTRO#INT3_Architextual_Entity -->

    <owl:Class rdf:about="http://www.semanticweb.org/oberreb4/ontologies/2018/9/INTRO#INT3_Architextual_Entity">
        <rdfs:subClassOf rdf:resource="http://erlangen-crm.org/current/E28_Conceptual_Object"/>
        <rdfs:subClassOf rdf:resource="http://www.semanticweb.org/oberreb4/ontologies/2018/9/INTRO#INT21_Text"/>
        <rdfs:comment>A transtextual entity consists in a number of texts which in some way give reason to see them as connected, related, sharing a common feature.
Examples for transtextual entities can be disourses (texts sharing a discousive element, a topic etc.), genres (texts sharing genre conventions), a discipline (texts deriving from the same disciplinary background), an oeuvre (texts written by the same person), national literatures (texts whose authors share a nationality) etc.</rdfs:comment>
    </owl:Class>
    


    <!-- http://www.semanticweb.org/oberreb4/ontologies/2018/9/INTRO#INT40_Situational_Motif -->

    <owl:Class rdf:about="http://www.semanticweb.org/oberreb4/ontologies/2018/9/INTRO#INT40_Situational_Motif">
        <rdfs:subClassOf rdf:resource="http://www.semanticweb.org/oberreb4/ontologies/2018/9/INTRO#INT33_Motif"/>
    </owl:Class>
    


    <!-- http://www.semanticweb.org/oberreb4/ontologies/2018/9/INTRO#INT40_Theory -->

    <owl:Class rdf:about="http://www.semanticweb.org/oberreb4/ontologies/2018/9/INTRO#INT40_Theory">
        <rdfs:subClassOf rdf:resource="http://www.semanticweb.org/oberreb4/ontologies/2018/9/INTRO#INT9_Semantic_Feature"/>
    </owl:Class>
    


    <!-- http://www.semanticweb.org/oberreb4/ontologies/2018/9/INTRO#INT41_Spatial_Motif -->

    <owl:Class rdf:about="http://www.semanticweb.org/oberreb4/ontologies/2018/9/INTRO#INT41_Spatial_Motif">
        <rdfs:subClassOf rdf:resource="http://www.semanticweb.org/oberreb4/ontologies/2018/9/INTRO#INT33_Motif"/>
    </owl:Class>
    


    <!-- http://www.semanticweb.org/oberreb4/ontologies/2018/9/INTRO#INT41_Topos -->

    <owl:Class rdf:about="http://www.semanticweb.org/oberreb4/ontologies/2018/9/INTRO#INT41_Topos">
        <rdfs:subClassOf rdf:resource="http://www.semanticweb.org/oberreb4/ontologies/2018/9/INTRO#INT9_Semantic_Feature"/>
    </owl:Class>
    


    <!-- http://www.semanticweb.org/oberreb4/ontologies/2018/9/INTRO#INT42_Temporal_Motif -->

    <owl:Class rdf:about="http://www.semanticweb.org/oberreb4/ontologies/2018/9/INTRO#INT42_Temporal_Motif">
        <rdfs:subClassOf rdf:resource="http://www.semanticweb.org/oberreb4/ontologies/2018/9/INTRO#INT33_Motif"/>
    </owl:Class>
    


    <!-- http://www.semanticweb.org/oberreb4/ontologies/2018/9/INTRO#INT42_Type_of_Character -->

    <owl:Class rdf:about="http://www.semanticweb.org/oberreb4/ontologies/2018/9/INTRO#INT42_Type_of_Character">
        <rdfs:subClassOf rdf:resource="http://www.semanticweb.org/oberreb4/ontologies/2018/9/INTRO#INT_Character"/>
    </owl:Class>
    


    <!-- http://www.semanticweb.org/oberreb4/ontologies/2018/9/INTRO#INT43_Type_Motif -->

    <owl:Class rdf:about="http://www.semanticweb.org/oberreb4/ontologies/2018/9/INTRO#INT43_Type_Motif">
        <rdfs:subClassOf rdf:resource="http://www.semanticweb.org/oberreb4/ontologies/2018/9/INTRO#INT33_Motif"/>
    </owl:Class>
    


    <!-- http://www.semanticweb.org/oberreb4/ontologies/2018/9/INTRO#INT44_Interpretament -->

    <owl:Class rdf:about="http://www.semanticweb.org/oberreb4/ontologies/2018/9/INTRO#INT44_Interpretament">
        <rdfs:subClassOf rdf:resource="http://erlangen-crm.org/current/E89_Propositional_Object"/>
        <rdfs:comment>The abstract content of a interpretative act.
An interpretament identifies references, actualizations of features or characteristics that assign texts to a transtextual entity.
Interpretaments themselves can originate in texts and thus be actualizations of the semantic feature &apos;Interpretation&apos;.

Examples:
- the statement that Umberto Eco&apos;s &apos;The Name of the Rose&apos; features a detective character.
- the statement that Umberto Eco&apos;s &apos;The Name of the Rose&apos; contains references to Arthur Conan Doyle&apos;s &apos;Sherlock Holmes&apos;.
- the statement that Umberto Exo&apos;s &apos;The Name of the Rose&apos; is set in the 14th century.
- the conclusion that Umberto Eco&apos;s &apos;The Name of the Rose&apos; belongs to the genre &apos;postmodern crime novel&apos;.</rdfs:comment>
    </owl:Class>
    


    <!-- http://www.semanticweb.org/oberreb4/ontologies/2018/9/INTRO#INT46_Punned_CiTO_Properties -->

    <owl:Class rdf:about="http://www.semanticweb.org/oberreb4/ontologies/2018/9/INTRO#INT46_Punned_CiTO_Properties">
        <rdfs:subClassOf rdf:resource="http://www.semanticweb.org/oberreb4/ontologies/2018/9/INTRO#INT23_Common_Concepts_of_Intertextuality"/>
        <rdfs:comment>All Instances in this class are derived from CiTO - the Citation Typing Ontology. CiTO IRIs originally identifying object properties are used as IRIs for the instances in this class. Annotations (comments, descriptions) are from the original source: http://purl.org/spar/cito.xml.

Reference: Peroni, S., Shotton, D. (2012). FaBiO and CiTO: ontologies for describing bibliographic resources and citations. In Journal of Web Semantics: Science, Services and Agents on the World Wide Web, 17 (December 2012): 33-43. Amsterdam, The Netherlands: Elsevier. https://doi.org/10.1016/j.websem.2012.08.001
Open Access at: http://speroni.web.cs.unibo.it/publications/peroni-2012-fabio-cito-ontologies.pdf</rdfs:comment>
    </owl:Class>
    


    <!-- http://www.semanticweb.org/oberreb4/ontologies/2018/9/INTRO#INT49_Act_Drama -->

    <owl:Class rdf:about="http://www.semanticweb.org/oberreb4/ontologies/2018/9/INTRO#INT49_Act_Drama">
        <rdfs:subClassOf rdf:resource="http://www.semanticweb.org/oberreb4/ontologies/2018/9/INTRO#INT7_Formal_Feature"/>
    </owl:Class>
    


    <!-- http://www.semanticweb.org/oberreb4/ontologies/2018/9/INTRO#INT4_Intertextual_Relationship -->

    <owl:Class rdf:about="http://www.semanticweb.org/oberreb4/ontologies/2018/9/INTRO#INT4_Intertextual_Relationship">
        <rdfs:subClassOf rdf:resource="http://erlangen-crm.org/current/E28_Conceptual_Object"/>
        <rdfs:subClassOf rdf:resource="http://www.semanticweb.org/oberreb4/ontologies/2018/9/INTRO#INT2_Receptional_Entity"/>
        <rdfs:comment>This class is meant for the abstract notion of an intertextual relationship as it is identified by a reader (and is not to be confused with the rhetorical entity &apos;quotation&apos;). Every INT4 Intertextual Relationship has at least 2 related entities, which are texts (on any ontological level) or INT3 Actualizations of Features.
An INT4 Intertextual Relationship is possibly identified in an interpretative.</rdfs:comment>
    </owl:Class>
    


    <!-- http://www.semanticweb.org/oberreb4/ontologies/2018/9/INTRO#INT50_Scene_Drama -->

    <owl:Class rdf:about="http://www.semanticweb.org/oberreb4/ontologies/2018/9/INTRO#INT50_Scene_Drama">
        <rdfs:subClassOf rdf:resource="http://www.semanticweb.org/oberreb4/ontologies/2018/9/INTRO#INT7_Formal_Feature"/>
    </owl:Class>
    


    <!-- http://www.semanticweb.org/oberreb4/ontologies/2018/9/INTRO#INT5_Actualization_of_Feature -->

    <owl:Class rdf:about="http://www.semanticweb.org/oberreb4/ontologies/2018/9/INTRO#INT5_Actualization_of_Feature">
        <rdfs:subClassOf rdf:resource="http://erlangen-crm.org/current/E28_Conceptual_Object"/>
        <rdfs:comment>The fact that a certain text shows - in its own specific way - a certain feature (which itself is an abstract concept and takes form in many texts), e.g. a motif, an atmosphere, a theme, a figure of speech.

Examples:
- the specific actualization of the motif of patricide in Sophokles&apos; &apos;Ödipus Rex&apos;.
- the specific actualization of the Faust-subject in Goethe&apos;s &apos;Faust&apos;.
- the specific actualization of the iambic pentameter in Rilke&apos;s &apos;Archaischer Torso Apollos&quot;.</rdfs:comment>
    </owl:Class>
    


    <!-- http://www.semanticweb.org/oberreb4/ontologies/2018/9/INTRO#INT60_Tableau_Drama -->

    <owl:Class rdf:about="http://www.semanticweb.org/oberreb4/ontologies/2018/9/INTRO#INT60_Tableau_Drama">
        <rdfs:subClassOf rdf:resource="http://www.semanticweb.org/oberreb4/ontologies/2018/9/INTRO#INT7_Formal_Feature"/>
    </owl:Class>
    


    <!-- http://www.semanticweb.org/oberreb4/ontologies/2018/9/INTRO#INT6_Characteristic -->

    <owl:Class rdf:about="http://www.semanticweb.org/oberreb4/ontologies/2018/9/INTRO#INT6_Characteristic">
        <rdfs:subClassOf rdf:resource="http://erlangen-crm.org/current/E28_Conceptual_Object"/>
        <rdfs:comment>The concept that (the actualization of) a certain feature can indicate to a text&apos;s affiliation or likeness to an architextual entity. A Characteristic is identified in an interpretative and is thus itself based on text.

Examples:
- how (the actualization of) the theme &apos;fashion&apos; in many german novels from 1995 to 2001 supports their affiliation to the movement (or school, or epoch) &apos;German Pop Literature&apos;.
- how (the actualization of) the underdog detective in Wolf Haas&apos; &apos;Silentium&apos; supports the novel&apos;s affiliation to the genre &apos;hardboiled crime fiction&apos;.</rdfs:comment>
    </owl:Class>
    


    <!-- http://www.semanticweb.org/oberreb4/ontologies/2018/9/INTRO#INT7_Formal_Feature -->

    <owl:Class rdf:about="http://www.semanticweb.org/oberreb4/ontologies/2018/9/INTRO#INT7_Formal_Feature">
        <rdfs:subClassOf rdf:resource="http://www.semanticweb.org/oberreb4/ontologies/2018/9/INTRO#INT2_Receptional_Entity"/>
        <rdfs:comment>This class comprises subclasses for every formal aspect of a text: Subclasses will provide the general terms (e.g. &apos;stanza&apos;), instances are meant to be specific types (e.g. &apos;Sapphic stanza&apos;).</rdfs:comment>
    </owl:Class>
    


    <!-- http://www.semanticweb.org/oberreb4/ontologies/2018/9/INTRO#INT8_Rhetorical_Feature -->

    <owl:Class rdf:about="http://www.semanticweb.org/oberreb4/ontologies/2018/9/INTRO#INT8_Rhetorical_Feature">
        <rdfs:subClassOf rdf:resource="http://www.semanticweb.org/oberreb4/ontologies/2018/9/INTRO#INT2_Receptional_Entity"/>
        <rdfs:comment>This class comprises every aspect of a text that can be described in terms of rhetorics - ranging from the occurrence of rhetorical tropes (figures of speech) to parts of a e.g. research paper like &apos;introduction&apos; or &apos;quotation&apos; (pragmatic entities) to aspects of the narrative act such as &apos;voice&apos; or &apos;narrating time&apos; (narratological entities).</rdfs:comment>
    </owl:Class>
    


    <!-- http://www.semanticweb.org/oberreb4/ontologies/2018/9/INTRO#INT9_Semantic_Feature -->

    <owl:Class rdf:about="http://www.semanticweb.org/oberreb4/ontologies/2018/9/INTRO#INT9_Semantic_Feature">
        <rdfs:subClassOf rdf:resource="http://www.semanticweb.org/oberreb4/ontologies/2018/9/INTRO#INT2_Receptional_Entity"/>
        <rdfs:comment>This class comprises every semantic aspect of a text: from the common notions of &apos;plot&apos; or &apos;character&apos; up to the specific classification of forms such as &apos;situational motif&apos;.</rdfs:comment>
    </owl:Class>
    


    <!-- http://www.semanticweb.org/oberreb4/ontologies/2018/9/INTRO#INT_Character -->

    <owl:Class rdf:about="http://www.semanticweb.org/oberreb4/ontologies/2018/9/INTRO#INT_Character">
        <rdfs:subClassOf rdf:resource="http://www.semanticweb.org/oberreb4/ontologies/2018/9/INTRO#INT9_Semantic_Feature"/>
    </owl:Class>
    


    <!-- 
    ///////////////////////////////////////////////////////////////////////////////////////
    //
    // Individuals
    //
    ///////////////////////////////////////////////////////////////////////////////////////
     -->

    


    <!-- http://purl.org/spar/cito/agreesWith -->

    <owl:NamedIndividual rdf:about="http://purl.org/spar/cito/agreesWith">
        <rdf:type rdf:resource="http://www.semanticweb.org/oberreb4/ontologies/2018/9/INTRO#INT46_Punned_CiTO_Properties"/>
        <dc:description xml:lang="en">Example: We share Galileo&apos;s opinion: the Earth moves [X].</dc:description>
        <rdfs:comment xml:lang="en">The citing entity agrees with statements, ideas or conclusions presented in the cited entity.</rdfs:comment>
        <rdfs:label xml:lang="en">agrees with</rdfs:label>
    </owl:NamedIndividual>
    


    <!-- http://purl.org/spar/cito/citesAsAuthority -->

    <owl:NamedIndividual rdf:about="http://purl.org/spar/cito/citesAsAuthority">
        <rdf:type rdf:resource="http://www.semanticweb.org/oberreb4/ontologies/2018/9/INTRO#INT46_Punned_CiTO_Properties"/>
        <dc:description xml:lang="en">Example: Newton asserted that we are like dwarfs standing on the shoulders of giants [X].</dc:description>
        <rdfs:comment xml:lang="en">The citing entity cites the cited entity as one that provides an authoritative description or definition of the subject under discussion.</rdfs:comment>
        <rdfs:label xml:lang="en">cites as authority</rdfs:label>
    </owl:NamedIndividual>
    


    <!-- http://purl.org/spar/cito/citesAsDataSource -->

    <owl:NamedIndividual rdf:about="http://purl.org/spar/cito/citesAsDataSource">
        <rdf:type rdf:resource="http://www.semanticweb.org/oberreb4/ontologies/2018/9/INTRO#INT46_Punned_CiTO_Properties"/>
        <dc:description xml:lang="en">Example: Italy has more than ten thousand kilometers of shoreline: see [X].</dc:description>
        <rdfs:comment xml:lang="en">The citing entity cites the cited entity as source of data.</rdfs:comment>
        <rdfs:label xml:lang="en">cites as data source</rdfs:label>
    </owl:NamedIndividual>
    


    <!-- http://purl.org/spar/cito/citesAsEvidence -->

    <owl:NamedIndividual rdf:about="http://purl.org/spar/cito/citesAsEvidence">
        <rdf:type rdf:resource="http://www.semanticweb.org/oberreb4/ontologies/2018/9/INTRO#INT46_Punned_CiTO_Properties"/>
        <dc:description xml:lang="en">Example: We found an unquestionable demonstration of our hypothesis in [X].</dc:description>
        <rdfs:comment xml:lang="en">The citing entity cites the cited entity as source of factual evidence for statements it contains.</rdfs:comment>
        <rdfs:label xml:lang="en">cites as evidence</rdfs:label>
    </owl:NamedIndividual>
    


    <!-- http://purl.org/spar/cito/citesAsMetadataDocument -->

    <owl:NamedIndividual rdf:about="http://purl.org/spar/cito/citesAsMetadataDocument">
        <rdf:type rdf:resource="http://www.semanticweb.org/oberreb4/ontologies/2018/9/INTRO#INT46_Punned_CiTO_Properties"/>
        <dc:description xml:lang="en">Example: Basic bibliographic, entity and project metadata relating to this article, recorded in a structured machine-readable form, is available as an additional file [X] accompanying this paper.</dc:description>
        <rdfs:comment xml:lang="en">The citing entity cites the cited entity as being the container of metadata describing the citing entity.</rdfs:comment>
        <rdfs:label xml:lang="en">cites as metadata document</rdfs:label>
    </owl:NamedIndividual>
    


    <!-- http://purl.org/spar/cito/citesAsPotentialSolution -->

    <owl:NamedIndividual rdf:about="http://purl.org/spar/cito/citesAsPotentialSolution">
        <rdf:type rdf:resource="http://www.semanticweb.org/oberreb4/ontologies/2018/9/INTRO#INT46_Punned_CiTO_Properties"/>
        <dc:description xml:lang="en">Example: This risk could be avoided using the approach shown in [X].</dc:description>
        <rdfs:comment xml:lang="en">The citing entity cites the cited entity as providing or containing a possible solution to the issues being discussed.</rdfs:comment>
        <rdfs:label xml:lang="en">cites as potential solution</rdfs:label>
    </owl:NamedIndividual>
    


    <!-- http://purl.org/spar/cito/citesAsRecommendedReading -->

    <owl:NamedIndividual rdf:about="http://purl.org/spar/cito/citesAsRecommendedReading">
        <rdf:type rdf:resource="http://www.semanticweb.org/oberreb4/ontologies/2018/9/INTRO#INT46_Punned_CiTO_Properties"/>
        <dc:description xml:lang="en">Example: To our knowledge, [X] is the best source of exercises about UML, making it a valuable proposal for beginners.</dc:description>
        <rdfs:comment xml:lang="en">The citing entity cites the cited entity as an item of recommended reading.  This property can be used, for example, to describe references in a lecture reading list, where the cited references are relevant to the general topic of the lecture, but might not be individually cited within the text of the lecture.  Similarly, it could be used to describe items in a &apos;Suggested further reading&apos; list at the end of a book chapter.</rdfs:comment>
        <rdfs:label xml:lang="en">cites as recommended reading</rdfs:label>
    </owl:NamedIndividual>
    


    <!-- http://purl.org/spar/cito/citesAsRelated -->

    <owl:NamedIndividual rdf:about="http://purl.org/spar/cito/citesAsRelated">
        <rdf:type rdf:resource="http://www.semanticweb.org/oberreb4/ontologies/2018/9/INTRO#INT46_Punned_CiTO_Properties"/>
        <dc:description xml:lang="en">Example: An analysis similar to what we proposed here is presented in [X].</dc:description>
        <rdfs:comment xml:lang="en">The citing entity cites the cited entity as one that is related.</rdfs:comment>
        <rdfs:label xml:lang="en">cites as related</rdfs:label>
    </owl:NamedIndividual>
    


    <!-- http://purl.org/spar/cito/citesAsSourceDocument -->

    <owl:NamedIndividual rdf:about="http://purl.org/spar/cito/citesAsSourceDocument">
        <rdf:type rdf:resource="http://www.semanticweb.org/oberreb4/ontologies/2018/9/INTRO#INT46_Punned_CiTO_Properties"/>
        <dc:description xml:lang="en">Example: Several sections of this work are based on our literature review of the topic published as journal article [X].</dc:description>
        <rdfs:comment xml:lang="en">The citing entity cites the cited entity as being the entity from which the citing entity is derived, or about which the citing entity contains metadata.</rdfs:comment>
        <rdfs:label xml:lang="en">cites as source document</rdfs:label>
    </owl:NamedIndividual>
    


    <!-- http://purl.org/spar/cito/citesForInformation -->

    <owl:NamedIndividual rdf:about="http://purl.org/spar/cito/citesForInformation">
        <rdf:type rdf:resource="http://www.semanticweb.org/oberreb4/ontologies/2018/9/INTRO#INT46_Punned_CiTO_Properties"/>
        <dc:description xml:lang="en">Example: The grammar of Pascal was introduced in [X].</dc:description>
        <rdfs:comment xml:lang="en">The citing entity cites the cited entity as a source of information on the subject under discussion.</rdfs:comment>
        <rdfs:label xml:lang="en">cites for information</rdfs:label>
    </owl:NamedIndividual>
    


    <!-- http://purl.org/spar/cito/compiles -->

    <owl:NamedIndividual rdf:about="http://purl.org/spar/cito/compiles">
        <rdf:type rdf:resource="http://www.semanticweb.org/oberreb4/ontologies/2018/9/INTRO#INT46_Punned_CiTO_Properties"/>
        <dc:description xml:lang="en">Example: This book gathers interviews with academic researchers of several disciplines [X].</dc:description>
        <dc:description xml:lang="en">Note: This property has been imported from the CiTO4Data ontology, usage of which has been deprecated.</dc:description>
        <rdfs:comment xml:lang="en">The citing entity is used to create or compile the cited entity.</rdfs:comment>
        <rdfs:label xml:lang="en">compiles</rdfs:label>
    </owl:NamedIndividual>
    


    <!-- http://purl.org/spar/cito/confirms -->

    <owl:NamedIndividual rdf:about="http://purl.org/spar/cito/confirms">
        <rdf:type rdf:resource="http://www.semanticweb.org/oberreb4/ontologies/2018/9/INTRO#INT46_Punned_CiTO_Properties"/>
        <dc:description xml:lang="en">Example: Our findings are similar to those published in [X].</dc:description>
        <rdfs:comment xml:lang="en">The citing entity confirms facts, ideas or statements presented in the cited entity.</rdfs:comment>
        <rdfs:label xml:lang="en">confirms</rdfs:label>
    </owl:NamedIndividual>
    


    <!-- http://purl.org/spar/cito/containsAssertionFrom -->

    <owl:NamedIndividual rdf:about="http://purl.org/spar/cito/containsAssertionFrom">
        <rdf:type rdf:resource="http://www.semanticweb.org/oberreb4/ontologies/2018/9/INTRO#INT46_Punned_CiTO_Properties"/>
        <dc:description xml:lang="en">Example: We think that to stand on the top of giants [X] is a valuable principle to follow for our own research.</dc:description>
        <rdfs:comment xml:lang="en">The citing entity contains a statement of fact or a logical assertion (or a collection of such facts and/or assertions) originally present in the cited entity.   This object property is designed to be used to relate a separate abstract, summary or nanopublication to the cited entity upon which it is based.</rdfs:comment>
        <rdfs:label xml:lang="en">contains assertion from</rdfs:label>
    </owl:NamedIndividual>
    


    <!-- http://purl.org/spar/cito/corrects -->

    <owl:NamedIndividual rdf:about="http://purl.org/spar/cito/corrects">
        <rdf:type rdf:resource="http://www.semanticweb.org/oberreb4/ontologies/2018/9/INTRO#INT46_Punned_CiTO_Properties"/>
        <dc:description xml:lang="en">Example: The result published in [X] is partially wrong, the correct result is 42.</dc:description>
        <rdfs:comment xml:lang="en">The citing entity corrects statements, ideas or conclusions presented in the cited entity.</rdfs:comment>
        <rdfs:label xml:lang="en">corrects</rdfs:label>
    </owl:NamedIndividual>
    


    <!-- http://purl.org/spar/cito/credits -->

    <owl:NamedIndividual rdf:about="http://purl.org/spar/cito/credits">
        <rdf:type rdf:resource="http://www.semanticweb.org/oberreb4/ontologies/2018/9/INTRO#INT46_Punned_CiTO_Properties"/>
        <dc:description xml:lang="en">Example: Galileo was the first to observe Jupiter&apos;s satellites [X].</dc:description>
        <rdfs:comment xml:lang="en">The citing entity acknowledges contributions made by the cited entity.</rdfs:comment>
        <rdfs:label xml:lang="en">credits</rdfs:label>
    </owl:NamedIndividual>
    


    <!-- http://purl.org/spar/cito/critiques -->

    <owl:NamedIndividual rdf:about="http://purl.org/spar/cito/critiques">
        <rdf:type rdf:resource="http://www.semanticweb.org/oberreb4/ontologies/2018/9/INTRO#INT46_Punned_CiTO_Properties"/>
        <dc:description xml:lang="en">Example: The ideas presented in [X] are badly substantantiated.</dc:description>
        <rdfs:comment xml:lang="en">The citing entity critiques statements, ideas or conclusions presented in the cited entity.</rdfs:comment>
        <rdfs:label xml:lang="en">critiques</rdfs:label>
    </owl:NamedIndividual>
    


    <!-- http://purl.org/spar/cito/derides -->

    <owl:NamedIndividual rdf:about="http://purl.org/spar/cito/derides">
        <rdf:type rdf:resource="http://www.semanticweb.org/oberreb4/ontologies/2018/9/INTRO#INT46_Punned_CiTO_Properties"/>
        <dc:description xml:lang="en">Example: The ideas published in [X] are incredibly stupid.</dc:description>
        <rdfs:comment xml:lang="en">The citing entity express derision for the cited entity, or for ideas or conclusions contained within it.</rdfs:comment>
        <rdfs:label xml:lang="en">derides</rdfs:label>
    </owl:NamedIndividual>
    


    <!-- http://purl.org/spar/cito/describes -->

    <owl:NamedIndividual rdf:about="http://purl.org/spar/cito/describes">
        <rdf:type rdf:resource="http://www.semanticweb.org/oberreb4/ontologies/2018/9/INTRO#INT46_Punned_CiTO_Properties"/>
        <dc:description xml:lang="en">Example: Galileo&apos;s book [X] is a dialog among three scientists about Copernicus&apos; eliocentric theory.</dc:description>
        <rdfs:comment xml:lang="en">The citing entity describes the cited entity.</rdfs:comment>
        <rdfs:label xml:lang="en">describes</rdfs:label>
    </owl:NamedIndividual>
    


    <!-- http://purl.org/spar/cito/disagreesWith -->

    <owl:NamedIndividual rdf:about="http://purl.org/spar/cito/disagreesWith">
        <rdf:type rdf:resource="http://www.semanticweb.org/oberreb4/ontologies/2018/9/INTRO#INT46_Punned_CiTO_Properties"/>
        <dc:description xml:lang="en">Example: We do not share Galileo&apos;s opinion [X]: the Earth does not move.</dc:description>
        <rdfs:comment xml:lang="en">The citing entity disagrees with statements, ideas or conclusions presented in the cited entity.</rdfs:comment>
        <rdfs:label xml:lang="en">disagrees with</rdfs:label>
    </owl:NamedIndividual>
    


    <!-- http://purl.org/spar/cito/discusses -->

    <owl:NamedIndividual rdf:about="http://purl.org/spar/cito/discusses">
        <rdf:type rdf:resource="http://www.semanticweb.org/oberreb4/ontologies/2018/9/INTRO#INT46_Punned_CiTO_Properties"/>
        <dc:description xml:lang="en">Example: We now examine if Galileo is right when he writes [X] that the Earth moves.</dc:description>
        <rdfs:comment xml:lang="en">The citing entity discusses statements, ideas or conclusions presented in the cited entity.</rdfs:comment>
        <rdfs:label xml:lang="en">discusses</rdfs:label>
    </owl:NamedIndividual>
    


    <!-- http://purl.org/spar/cito/disputes -->

    <owl:NamedIndividual rdf:about="http://purl.org/spar/cito/disputes">
        <rdf:type rdf:resource="http://www.semanticweb.org/oberreb4/ontologies/2018/9/INTRO#INT46_Punned_CiTO_Properties"/>
        <dc:description xml:lang="en">Example: We doubt that Galileo is right when he writes [X] that the Earth moves.</dc:description>
        <rdfs:comment xml:lang="en">The citing entity disputes statements, ideas or conclusions presented in the cited entity.</rdfs:comment>
        <rdfs:label xml:lang="en">disputes</rdfs:label>
    </owl:NamedIndividual>
    


    <!-- http://purl.org/spar/cito/documents -->

    <owl:NamedIndividual rdf:about="http://purl.org/spar/cito/documents">
        <rdf:type rdf:resource="http://www.semanticweb.org/oberreb4/ontologies/2018/9/INTRO#INT46_Punned_CiTO_Properties"/>
        <dc:description xml:lang="en">Example: Herein we report in detail the complete set of ontological rules defined in the Overlapping Ontology [X].</dc:description>
        <rdfs:comment>The citing entity documents information about the cited entity.</rdfs:comment>
        <rdfs:label xml:lang="en">documents</rdfs:label>
    </owl:NamedIndividual>
    


    <!-- http://purl.org/spar/cito/extends -->

    <owl:NamedIndividual rdf:about="http://purl.org/spar/cito/extends">
        <rdf:type rdf:resource="http://www.semanticweb.org/oberreb4/ontologies/2018/9/INTRO#INT46_Punned_CiTO_Properties"/>
        <dc:description xml:lang="en">Example: We add to Galileo&apos;s findings concerning the Earth [X] that also the Moon moves.</dc:description>
        <rdfs:comment xml:lang="en">The citing entity extends facts, ideas or understandings presented in the cited entity.</rdfs:comment>
        <rdfs:label xml:lang="en">extends</rdfs:label>
    </owl:NamedIndividual>
    


    <!-- http://purl.org/spar/cito/givesSupportTo -->

    <owl:NamedIndividual rdf:about="http://purl.org/spar/cito/givesSupportTo">
        <rdf:type rdf:resource="http://www.semanticweb.org/oberreb4/ontologies/2018/9/INTRO#INT46_Punned_CiTO_Properties"/>
        <rdfs:comment xml:lang="en">The cited entity provides intellectual or factual support for the citing entity.</rdfs:comment>
        <rdfs:label xml:lang="en">gives support to</rdfs:label>
    </owl:NamedIndividual>
    


    <!-- http://purl.org/spar/cito/includesExcerptFrom -->

    <owl:NamedIndividual rdf:about="http://purl.org/spar/cito/includesExcerptFrom">
        <rdf:type rdf:resource="http://www.semanticweb.org/oberreb4/ontologies/2018/9/INTRO#INT46_Punned_CiTO_Properties"/>
        <dc:description xml:lang="en">An excerpt is more general than a quotation. It is generally used to indicate a re-published extract from a book, instruction manual, film, radio programme, etc, that need not be what someone said.  For example:

    Oxford 01865
    Oxshott 01372
    Oxted 01883
    Oxton 01578

    is an excerpt from the UK Dialling Codes section of the Oxford Telephone Directory.</dc:description>
        <dc:description xml:lang="en">Example: In her work, the author states that even though most Human Information Behaviour researchers are familiar with the literature related to their studies, it is not uncommon for investigators to fail to see the benefits they may gain from previous mistakes [X].</dc:description>
        <rdfs:comment xml:lang="en">The citing entity includes one or more excerpts from the cited entity.</rdfs:comment>
        <rdfs:label xml:lang="en">includes excerpt from</rdfs:label>
    </owl:NamedIndividual>
    


    <!-- http://purl.org/spar/cito/includesQuotationFrom -->

    <owl:NamedIndividual rdf:about="http://purl.org/spar/cito/includesQuotationFrom">
        <rdf:type rdf:resource="http://www.semanticweb.org/oberreb4/ontologies/2018/9/INTRO#INT46_Punned_CiTO_Properties"/>
        <dc:description xml:lang="en">A quotation is a repetition of what someone has said, and is presented &quot;within quotation marks&quot;, for example:

    On June 4th 1940, Winston Churchill made a speech on the radio that has since become famous, that included the words: &quot; . . . we shall fight on the beaches, we shall fight on the landing grounds, we shall fight in the fields and in the streets, we shall fight in the hills; we shall never surrender . . .&quot;</dc:description>
        <dc:description xml:lang="en">Example: As Newton wrote in [X]: &quot;We are like dwarfs standing on the shoulders of giants&quot;.</dc:description>
        <rdfs:comment xml:lang="en">The citing entity includes one or more quotations from the cited entity.</rdfs:comment>
        <rdfs:label xml:lang="en">includes quotation from</rdfs:label>
    </owl:NamedIndividual>
    


    <!-- http://purl.org/spar/cito/isCitedForInformationBy -->

    <owl:NamedIndividual rdf:about="http://purl.org/spar/cito/isCitedForInformationBy">
        <rdf:type rdf:resource="http://www.semanticweb.org/oberreb4/ontologies/2018/9/INTRO#INT46_Punned_CiTO_Properties"/>
        <rdfs:comment xml:lang="en">The cited entity is cited as a source of information on the subject under discussion in the citing entity.</rdfs:comment>
        <rdfs:label xml:lang="en">is cited for information by</rdfs:label>
    </owl:NamedIndividual>
    


    <!-- http://purl.org/spar/cito/likes -->

    <owl:NamedIndividual rdf:about="http://purl.org/spar/cito/likes">
        <rdf:type rdf:resource="http://www.semanticweb.org/oberreb4/ontologies/2018/9/INTRO#INT46_Punned_CiTO_Properties"/>
        <rdfs:comment xml:lang="en">A property that permits you to express appreciation of or interest in something that is the object of the RDF triple, or to express that it is worth thinking about even if you do not agree with its content, enabling social media &apos;likes&apos; statements to be encoded in RDF.  Use of this property does NOT imply the existence of a formal citation of the entity that is &apos;liked&apos;.</rdfs:comment>
        <rdfs:label xml:lang="en">likes</rdfs:label>
    </owl:NamedIndividual>
    


    <!-- http://purl.org/spar/cito/linksTo -->

    <owl:NamedIndividual rdf:about="http://purl.org/spar/cito/linksTo">
        <rdf:type rdf:resource="http://www.semanticweb.org/oberreb4/ontologies/2018/9/INTRO#INT46_Punned_CiTO_Properties"/>
        <dc:description xml:lang="en">Example: The BioSharing registry (https://biosharing.org) can be of use as it describes the standards in detail, including versions where applicable.</dc:description>
        <rdfs:comment xml:lang="en">The citing entity provides a link, in the form of an HTTP Uniform Resource Locator (URL), to the cited entity.</rdfs:comment>
        <rdfs:label xml:lang="en">links to</rdfs:label>
    </owl:NamedIndividual>
    


    <!-- http://purl.org/spar/cito/obtainsBackgroundFrom -->

    <owl:NamedIndividual rdf:about="http://purl.org/spar/cito/obtainsBackgroundFrom">
        <rdf:type rdf:resource="http://www.semanticweb.org/oberreb4/ontologies/2018/9/INTRO#INT46_Punned_CiTO_Properties"/>
        <dc:description xml:lang="en">Example: There is a need for more observational studies and studies using narrative causation to describe the potential contribution of information in problem-solving and decision-making [X]; our work addresses these needs.</dc:description>
        <rdfs:comment xml:lang="en">The citing entity obtains background information from the cited entity.</rdfs:comment>
        <rdfs:label xml:lang="en">obtains background from</rdfs:label>
    </owl:NamedIndividual>
    


    <!-- http://purl.org/spar/cito/obtainsSupportFrom -->

    <owl:NamedIndividual rdf:about="http://purl.org/spar/cito/obtainsSupportFrom">
        <rdf:type rdf:resource="http://www.semanticweb.org/oberreb4/ontologies/2018/9/INTRO#INT46_Punned_CiTO_Properties"/>
        <dc:description xml:lang="en">Example: Our ideas were also shared by Doe et al. [X].</dc:description>
        <rdfs:comment xml:lang="en">The citing entity obtains intellectual or factual support from the cited entity.</rdfs:comment>
        <rdfs:label xml:lang="en">obtains support from</rdfs:label>
    </owl:NamedIndividual>
    


    <!-- http://purl.org/spar/cito/parodies -->

    <owl:NamedIndividual rdf:about="http://purl.org/spar/cito/parodies">
        <rdf:type rdf:resource="http://www.semanticweb.org/oberreb4/ontologies/2018/9/INTRO#INT46_Punned_CiTO_Properties"/>
        <dc:description xml:lang="en">Example: We act as giants on the shoulders of dwarfs [X]!</dc:description>
        <rdfs:comment xml:lang="en">The citing entity imitates the characteristic style or content of the cited entity for comic effect, usually without explicit citation.</rdfs:comment>
        <rdfs:label xml:lang="en">parodies</rdfs:label>
    </owl:NamedIndividual>
    


    <!-- http://purl.org/spar/cito/plagiarizes -->

    <owl:NamedIndividual rdf:about="http://purl.org/spar/cito/plagiarizes">
        <rdf:type rdf:resource="http://www.semanticweb.org/oberreb4/ontologies/2018/9/INTRO#INT46_Punned_CiTO_Properties"/>
        <dc:description xml:lang="en">Example: The conclusion of our dissertation can be summarised by the following motto, we created specifically for this purpose: we are like dwarfs standing on the shoulders of giants.</dc:description>
        <rdfs:comment xml:lang="en">A property indicating that the author of the citing entity plagiarizes the cited entity, by including textual or other elements from the cited entity without formal acknowledgement of their source.  The citing entity thus contains no explicit citation of the cited entity, according to the norms of scholarly practice, but cites it implicitly.</rdfs:comment>
        <rdfs:label xml:lang="en">plagiarizes</rdfs:label>
    </owl:NamedIndividual>
    


    <!-- http://purl.org/spar/cito/qualifies -->

    <owl:NamedIndividual rdf:about="http://purl.org/spar/cito/qualifies">
        <rdf:type rdf:resource="http://www.semanticweb.org/oberreb4/ontologies/2018/9/INTRO#INT46_Punned_CiTO_Properties"/>
        <dc:description xml:lang="en">Example: Galileo&apos;s masterpiece &apos;Dialogo sopra i due massimi sistemi del mondo&apos; [X] is formally a dialog and substantially a scientific pamphlet.</dc:description>
        <rdfs:comment xml:lang="en">The citing entity qualifies or places conditions or restrictions upon statements, ideas or conclusions presented in the cited entity.</rdfs:comment>
        <rdfs:label xml:lang="en">qualifies</rdfs:label>
    </owl:NamedIndividual>
    


    <!-- http://purl.org/spar/cito/refutes -->

    <owl:NamedIndividual rdf:about="http://purl.org/spar/cito/refutes">
        <rdf:type rdf:resource="http://www.semanticweb.org/oberreb4/ontologies/2018/9/INTRO#INT46_Punned_CiTO_Properties"/>
        <dc:description xml:lang="en">Example: We do not think that all their arguments in favour of their own and against the other strategies are equally convincing [X].</dc:description>
        <rdfs:comment xml:lang="en">The citing entity refutes statements, ideas or conclusions presented in the cited entity.</rdfs:comment>
        <rdfs:label xml:lang="en">refutes</rdfs:label>
    </owl:NamedIndividual>
    


    <!-- http://purl.org/spar/cito/repliesTo -->

    <owl:NamedIndividual rdf:about="http://purl.org/spar/cito/repliesTo">
        <rdf:type rdf:resource="http://www.semanticweb.org/oberreb4/ontologies/2018/9/INTRO#INT46_Punned_CiTO_Properties"/>
        <dc:description xml:lang="en">Example: We will not investigate the issues of the approach proposed in [X] here, but rather we introduce yet another alternative.</dc:description>
        <rdfs:comment xml:lang="en">The citing entity replies to statements, ideas or criticisms presented in the cited entity.</rdfs:comment>
        <rdfs:label xml:lang="en">replies to</rdfs:label>
    </owl:NamedIndividual>
    


    <!-- http://purl.org/spar/cito/retracts -->

    <owl:NamedIndividual rdf:about="http://purl.org/spar/cito/retracts">
        <rdf:type rdf:resource="http://www.semanticweb.org/oberreb4/ontologies/2018/9/INTRO#INT46_Punned_CiTO_Properties"/>
        <dc:description xml:lang="en">Example: We wrote that the Earth moves in [X]; we now retire such statement.</dc:description>
        <rdfs:comment xml:lang="en">The citing entity constitutes a formal retraction of the cited entity.</rdfs:comment>
        <rdfs:label xml:lang="en">retracts</rdfs:label>
    </owl:NamedIndividual>
    


    <!-- http://purl.org/spar/cito/reviews -->

    <owl:NamedIndividual rdf:about="http://purl.org/spar/cito/reviews">
        <rdf:type rdf:resource="http://www.semanticweb.org/oberreb4/ontologies/2018/9/INTRO#INT46_Punned_CiTO_Properties"/>
        <dc:description xml:lang="en">Example: This paper discusses Toulmin&apos;s methodology in modelling argumentation [X], focussing on highlighting advantages and drawbacks of the application of such a methodology in the Social Web.</dc:description>
        <rdfs:comment xml:lang="en">The citing entity reviews statements, ideas or conclusions presented in the cited entity.</rdfs:comment>
        <rdfs:label xml:lang="en">reviews</rdfs:label>
    </owl:NamedIndividual>
    


    <!-- http://purl.org/spar/cito/ridicules -->

    <owl:NamedIndividual rdf:about="http://purl.org/spar/cito/ridicules">
        <rdf:type rdf:resource="http://www.semanticweb.org/oberreb4/ontologies/2018/9/INTRO#INT46_Punned_CiTO_Properties"/>
        <dc:description xml:lang="en">Example: Galileo said that the Earth &quot;moves&quot; [X]; really? And where is it going?</dc:description>
        <rdfs:comment xml:lang="en">The citing entity ridicules the cited entity or aspects of its contents.</rdfs:comment>
        <rdfs:label xml:lang="en">ridicules</rdfs:label>
    </owl:NamedIndividual>
    


    <!-- http://purl.org/spar/cito/speculatesOn -->

    <owl:NamedIndividual rdf:about="http://purl.org/spar/cito/speculatesOn">
        <rdf:type rdf:resource="http://www.semanticweb.org/oberreb4/ontologies/2018/9/INTRO#INT46_Punned_CiTO_Properties"/>
        <dc:description xml:lang="en">Example: We believe that if Galileo believed that Earth goes around the Sun [X], he also should believe that Moon goes around Earth.</dc:description>
        <rdfs:comment xml:lang="en">The citing entity speculates on something within or related to the cited entity, without firm evidence.</rdfs:comment>
        <rdfs:label xml:lang="en">speculates on</rdfs:label>
    </owl:NamedIndividual>
    


    <!-- http://purl.org/spar/cito/supports -->

    <owl:NamedIndividual rdf:about="http://purl.org/spar/cito/supports">
        <rdf:type rdf:resource="http://www.semanticweb.org/oberreb4/ontologies/2018/9/INTRO#INT46_Punned_CiTO_Properties"/>
        <dc:description xml:lang="en">Example: We support Galileo&apos;s statement [X], that Earth moves.</dc:description>
        <rdfs:comment xml:lang="en">The citing entity provides intellectual or factual support for statements, ideas or conclusions presented in the cited entity.</rdfs:comment>
        <rdfs:label xml:lang="en">supports</rdfs:label>
    </owl:NamedIndividual>
    


    <!-- http://purl.org/spar/cito/updates -->

    <owl:NamedIndividual rdf:about="http://purl.org/spar/cito/updates">
        <rdf:type rdf:resource="http://www.semanticweb.org/oberreb4/ontologies/2018/9/INTRO#INT46_Punned_CiTO_Properties"/>
        <dc:description xml:lang="en">Example: Earth moves, said Galileo [X]; in addition, we can say now it moves very fast.</dc:description>
        <rdfs:comment xml:lang="en">The citing entity updates statements, ideas, hypotheses or understanding presented in the cited entity.</rdfs:comment>
        <rdfs:label xml:lang="en">updates</rdfs:label>
    </owl:NamedIndividual>
    


    <!-- http://purl.org/spar/cito/usesConclusionsFrom -->

    <owl:NamedIndividual rdf:about="http://purl.org/spar/cito/usesConclusionsFrom">
        <rdf:type rdf:resource="http://www.semanticweb.org/oberreb4/ontologies/2018/9/INTRO#INT46_Punned_CiTO_Properties"/>
        <dc:description xml:lang="en">Example: Building upon Galileo&apos;s findings [X], we discovered that all the planets move.</dc:description>
        <rdfs:comment xml:lang="en">The citing entity describes work that uses conclusions presented in the cited entity.</rdfs:comment>
        <rdfs:label xml:lang="en">uses conclusions from</rdfs:label>
    </owl:NamedIndividual>
    


    <!-- http://purl.org/spar/cito/usesDataFrom -->

    <owl:NamedIndividual rdf:about="http://purl.org/spar/cito/usesDataFrom">
        <rdf:type rdf:resource="http://www.semanticweb.org/oberreb4/ontologies/2018/9/INTRO#INT46_Punned_CiTO_Properties"/>
        <dc:description xml:lang="en">Example: Using the information collected from our recent study [X], we can estimate that there are tens of millions of HTML forms with potentially useful deep-web content.</dc:description>
        <rdfs:comment xml:lang="en">The citing entity describes work that uses data presented in the cited entity.</rdfs:comment>
        <rdfs:label xml:lang="en">uses data from</rdfs:label>
    </owl:NamedIndividual>
    


    <!-- http://purl.org/spar/cito/usesMethodIn -->

    <owl:NamedIndividual rdf:about="http://purl.org/spar/cito/usesMethodIn">
        <rdf:type rdf:resource="http://www.semanticweb.org/oberreb4/ontologies/2018/9/INTRO#INT46_Punned_CiTO_Properties"/>
        <dc:description xml:lang="en">Example: We follow [X] in using design patterns for testing.</dc:description>
        <rdfs:comment xml:lang="en">The citing entity describes work that uses a method detailed in the cited entity.</rdfs:comment>
        <rdfs:label xml:lang="en">uses method in</rdfs:label>
    </owl:NamedIndividual>
    


    <!-- http://www.semanticweb.org/oberreb4/ontologies/2018/9/INTRO#Act_Character_Alice -->

    <owl:NamedIndividual rdf:about="http://www.semanticweb.org/oberreb4/ontologies/2018/9/INTRO#Act_Character_Alice">
        <rdf:type rdf:resource="http://www.semanticweb.org/oberreb4/ontologies/2018/9/INTRO#INT5_Actualization_of_Feature"/>
        <R17_actualizes_feature rdf:resource="http://www.semanticweb.org/oberreb4/ontologies/2018/9/INTRO#Alice"/>
        <R18_actualization_found_on rdf:resource="http://www.semanticweb.org/oberreb4/ontologies/2018/9/INTRO#Kubrick,_Eyes"/>
    </owl:NamedIndividual>
    


    <!-- http://www.semanticweb.org/oberreb4/ontologies/2018/9/INTRO#Act_Character_Beatrice -->

    <owl:NamedIndividual rdf:about="http://www.semanticweb.org/oberreb4/ontologies/2018/9/INTRO#Act_Character_Beatrice">
        <rdf:type rdf:resource="http://www.semanticweb.org/oberreb4/ontologies/2018/9/INTRO#INT5_Actualization_of_Feature"/>
        <R17_actualizes_feature rdf:resource="http://www.semanticweb.org/oberreb4/ontologies/2018/9/INTRO#Beatrice"/>
    </owl:NamedIndividual>
    


    <!-- http://www.semanticweb.org/oberreb4/ontologies/2018/9/INTRO#Act_Character_Brangäne -->

    <owl:NamedIndividual rdf:about="http://www.semanticweb.org/oberreb4/ontologies/2018/9/INTRO#Act_Character_Brangäne">
        <rdf:type rdf:resource="http://www.semanticweb.org/oberreb4/ontologies/2018/9/INTRO#INT5_Actualization_of_Feature"/>
        <R17_actualizes_feature rdf:resource="http://www.semanticweb.org/oberreb4/ontologies/2018/9/INTRO#Brangäne"/>
        <R18_actualization_found_on rdf:resource="http://www.semanticweb.org/oberreb4/ontologies/2018/9/INTRO#Wagner,_Tristan"/>
    </owl:NamedIndividual>
    


    <!-- http://www.semanticweb.org/oberreb4/ontologies/2018/9/INTRO#Act_Character_Hippolyta -->

    <owl:NamedIndividual rdf:about="http://www.semanticweb.org/oberreb4/ontologies/2018/9/INTRO#Act_Character_Hippolyta">
        <rdf:type rdf:resource="http://www.semanticweb.org/oberreb4/ontologies/2018/9/INTRO#INT5_Actualization_of_Feature"/>
        <R17_actualizes_feature rdf:resource="http://www.semanticweb.org/oberreb4/ontologies/2018/9/INTRO#Hippolyta"/>
    </owl:NamedIndividual>
    


    <!-- http://www.semanticweb.org/oberreb4/ontologies/2018/9/INTRO#Act_Character_Klara -->

    <owl:NamedIndividual rdf:about="http://www.semanticweb.org/oberreb4/ontologies/2018/9/INTRO#Act_Character_Klara">
        <rdf:type rdf:resource="http://www.semanticweb.org/oberreb4/ontologies/2018/9/INTRO#INT5_Actualization_of_Feature"/>
        <R17_actualizes_feature rdf:resource="http://www.semanticweb.org/oberreb4/ontologies/2018/9/INTRO#Klara"/>
        <R18_actualization_found_on rdf:resource="http://www.semanticweb.org/oberreb4/ontologies/2018/9/INTRO#Hoffmann,_Sandmann"/>
    </owl:NamedIndividual>
    


    <!-- http://www.semanticweb.org/oberreb4/ontologies/2018/9/INTRO#Act_Character_Marla -->

    <owl:NamedIndividual rdf:about="http://www.semanticweb.org/oberreb4/ontologies/2018/9/INTRO#Act_Character_Marla">
        <rdf:type rdf:resource="http://www.semanticweb.org/oberreb4/ontologies/2018/9/INTRO#INT5_Actualization_of_Feature"/>
        <R17_actualizes_feature rdf:resource="http://www.semanticweb.org/oberreb4/ontologies/2018/9/INTRO#Marla"/>
        <R18_actualization_found_on rdf:resource="http://www.semanticweb.org/oberreb4/ontologies/2018/9/INTRO#Fincher,_Fight_Club"/>
    </owl:NamedIndividual>
    


    <!-- http://www.semanticweb.org/oberreb4/ontologies/2018/9/INTRO#Act_Clara -->

    <owl:NamedIndividual rdf:about="http://www.semanticweb.org/oberreb4/ontologies/2018/9/INTRO#Act_Clara">
        <rdf:type rdf:resource="http://www.semanticweb.org/oberreb4/ontologies/2018/9/INTRO#INT5_Actualization_of_Feature"/>
        <R17_actualizes_feature rdf:resource="http://www.semanticweb.org/oberreb4/ontologies/2018/9/INTRO#Clara"/>
        <R18_actualization_found_on rdf:resource="http://www.semanticweb.org/oberreb4/ontologies/2018/9/INTRO#Brown,_Wieland"/>
    </owl:NamedIndividual>
    


    <!-- http://www.semanticweb.org/oberreb4/ontologies/2018/9/INTRO#Act_CrossMapping_IntRels -->

    <owl:NamedIndividual rdf:about="http://www.semanticweb.org/oberreb4/ontologies/2018/9/INTRO#Act_CrossMapping_IntRels">
        <rdf:type rdf:resource="http://www.semanticweb.org/oberreb4/ontologies/2018/9/INTRO#INT5_Actualization_of_Feature"/>
        <R17_actualizes_feature rdf:resource="http://www.semanticweb.org/oberreb4/ontologies/2018/9/INTRO#Feat_CrossMapping_IntRels"/>
    </owl:NamedIndividual>
    


    <!-- http://www.semanticweb.org/oberreb4/ontologies/2018/9/INTRO#Act_CrossMapping_References -->

    <owl:NamedIndividual rdf:about="http://www.semanticweb.org/oberreb4/ontologies/2018/9/INTRO#Act_CrossMapping_References">
        <rdf:type rdf:resource="http://www.semanticweb.org/oberreb4/ontologies/2018/9/INTRO#INT5_Actualization_of_Feature"/>
        <R17_actualizes_feature rdf:resource="http://www.semanticweb.org/oberreb4/ontologies/2018/9/INTRO#Feat_CrossMapping_Ref"/>
        <R18_actualization_found_on rdf:resource="http://www.semanticweb.org/oberreb4/ontologies/2018/9/INTRO#Bronfen,_Cross-Mapping"/>
    </owl:NamedIndividual>
    


    <!-- http://www.semanticweb.org/oberreb4/ontologies/2018/9/INTRO#Act_CrossMapping_Sources -->

    <owl:NamedIndividual rdf:about="http://www.semanticweb.org/oberreb4/ontologies/2018/9/INTRO#Act_CrossMapping_Sources">
        <rdf:type rdf:resource="http://www.semanticweb.org/oberreb4/ontologies/2018/9/INTRO#INT5_Actualization_of_Feature"/>
        <R18_actualization_found_on rdf:resource="http://www.semanticweb.org/oberreb4/ontologies/2018/9/INTRO#Bronfen,_Cross-Mapping"/>
    </owl:NamedIndividual>
    


    <!-- http://www.semanticweb.org/oberreb4/ontologies/2018/9/INTRO#Act_Interpretation_CrossMapping -->

    <owl:NamedIndividual rdf:about="http://www.semanticweb.org/oberreb4/ontologies/2018/9/INTRO#Act_Interpretation_CrossMapping">
        <rdf:type rdf:resource="http://www.semanticweb.org/oberreb4/ontologies/2018/9/INTRO#INT5_Actualization_of_Feature"/>
        <R17_actualizes_feature rdf:resource="http://www.semanticweb.org/oberreb4/ontologies/2018/9/INTRO#Feat_Interpretation_CrossMapping"/>
    </owl:NamedIndividual>
    


    <!-- http://www.semanticweb.org/oberreb4/ontologies/2018/9/INTRO#Alice -->

    <owl:NamedIndividual rdf:about="http://www.semanticweb.org/oberreb4/ontologies/2018/9/INTRO#Alice">
        <rdf:type rdf:resource="http://www.semanticweb.org/oberreb4/ontologies/2018/9/INTRO#INT28_Individual_Character"/>
    </owl:NamedIndividual>
    


    <!-- http://www.semanticweb.org/oberreb4/ontologies/2018/9/INTRO#Beatrice -->

    <owl:NamedIndividual rdf:about="http://www.semanticweb.org/oberreb4/ontologies/2018/9/INTRO#Beatrice">
        <rdf:type rdf:resource="http://www.semanticweb.org/oberreb4/ontologies/2018/9/INTRO#INT28_Individual_Character"/>
    </owl:NamedIndividual>
    


    <!-- http://www.semanticweb.org/oberreb4/ontologies/2018/9/INTRO#Brangäne -->

    <owl:NamedIndividual rdf:about="http://www.semanticweb.org/oberreb4/ontologies/2018/9/INTRO#Brangäne">
        <rdf:type rdf:resource="http://www.semanticweb.org/oberreb4/ontologies/2018/9/INTRO#INT28_Individual_Character"/>
    </owl:NamedIndividual>
    


    <!-- http://www.semanticweb.org/oberreb4/ontologies/2018/9/INTRO#Clara -->

    <owl:NamedIndividual rdf:about="http://www.semanticweb.org/oberreb4/ontologies/2018/9/INTRO#Clara">
        <rdf:type rdf:resource="http://www.semanticweb.org/oberreb4/ontologies/2018/9/INTRO#INT28_Individual_Character"/>
    </owl:NamedIndividual>
    


    <!-- http://www.semanticweb.org/oberreb4/ontologies/2018/9/INTRO#Clear_Sighted_Daughter -->

    <owl:NamedIndividual rdf:about="http://www.semanticweb.org/oberreb4/ontologies/2018/9/INTRO#Clear_Sighted_Daughter">
        <rdf:type rdf:resource="http://www.semanticweb.org/oberreb4/ontologies/2018/9/INTRO#INT42_Type_of_Character"/>
        <R17_feature_actualized_in rdf:resource="http://www.semanticweb.org/oberreb4/ontologies/2018/9/INTRO#Act_Character_Alice"/>
        <R17_feature_actualized_in rdf:resource="http://www.semanticweb.org/oberreb4/ontologies/2018/9/INTRO#Act_Character_Beatrice"/>
        <R17_feature_actualized_in rdf:resource="http://www.semanticweb.org/oberreb4/ontologies/2018/9/INTRO#Act_Character_Brangäne"/>
        <R17_feature_actualized_in rdf:resource="http://www.semanticweb.org/oberreb4/ontologies/2018/9/INTRO#Act_Character_Hippolyta"/>
        <R17_feature_actualized_in rdf:resource="http://www.semanticweb.org/oberreb4/ontologies/2018/9/INTRO#Act_Character_Klara"/>
        <R17_feature_actualized_in rdf:resource="http://www.semanticweb.org/oberreb4/ontologies/2018/9/INTRO#Act_Character_Marla"/>
        <R17_feature_actualized_in rdf:resource="http://www.semanticweb.org/oberreb4/ontologies/2018/9/INTRO#Act_Clara"/>
    </owl:NamedIndividual>
    


    <!-- http://www.semanticweb.org/oberreb4/ontologies/2018/9/INTRO#Def_Clear_Sigthed_Daughter -->

    <owl:NamedIndividual rdf:about="http://www.semanticweb.org/oberreb4/ontologies/2018/9/INTRO#Def_Clear_Sigthed_Daughter">
        <rdf:type rdf:resource="http://www.semanticweb.org/oberreb4/ontologies/2018/9/INTRO#INT1_Text_Passage"/>
        <R44_has_wording>die klugen Heldinnen der Komödien, die in dem Sinne ein Gegengewicht zu den Hexen und schönen Toten der Tragödien darstellen, insofern sie für ein Aushandeln des sie beschränkenden und kränkenden Gesetzes einstehen, anstatt dieses radikal zu überschreiten: Portia in Merchant of Venice, die Prinzessin in Love’s Labour’s Lost, Beatrice in Much Ado about Nothing.
Vornehmlich seit dem epistemischen Bruch, den der Historiker Michel Foucault um 1800 ansetzt, um den Anfang der Moderne festzulegen, flackern mit neuer Brisanz spezifische Figurierungen des weiblichen Subjekts wieder auf. Sie fungieren als Stellvertreterinnen genau jenes kulturellen Kodes, der der Frau eigentlich seit der Renaissance eine dominante Position innerhalb der symbolischen Ordnung absprach […].
Die vernünftige und überlebensfähige Tochter.</R44_has_wording>
    </owl:NamedIndividual>
    


    <!-- http://www.semanticweb.org/oberreb4/ontologies/2018/9/INTRO#Def_Cross-Mapping -->

    <owl:NamedIndividual rdf:about="http://www.semanticweb.org/oberreb4/ontologies/2018/9/INTRO#Def_Cross-Mapping">
        <rdf:type rdf:resource="http://www.semanticweb.org/oberreb4/ontologies/2018/9/INTRO#INT29_Definition"/>
    </owl:NamedIndividual>
    


    <!-- http://www.semanticweb.org/oberreb4/ontologies/2018/9/INTRO#Def_Rewriting -->

    <owl:NamedIndividual rdf:about="http://www.semanticweb.org/oberreb4/ontologies/2018/9/INTRO#Def_Rewriting">
        <rdf:type rdf:resource="http://www.semanticweb.org/oberreb4/ontologies/2018/9/INTRO#INT29_Definition"/>
    </owl:NamedIndividual>
    


    <!-- http://www.semanticweb.org/oberreb4/ontologies/2018/9/INTRO#Feat_CrossMapping_IntRels -->

    <owl:NamedIndividual rdf:about="http://www.semanticweb.org/oberreb4/ontologies/2018/9/INTRO#Feat_CrossMapping_IntRels">
        <rdf:type rdf:resource="http://www.semanticweb.org/oberreb4/ontologies/2018/9/INTRO#INT4_Intertextual_Relationship"/>
        <R12_has_referred_to_entity rdf:resource="http://www.semanticweb.org/oberreb4/ontologies/2018/9/INTRO#Brown,_Wieland"/>
        <R12_has_referred_to_entity rdf:resource="http://www.semanticweb.org/oberreb4/ontologies/2018/9/INTRO#Fincher,_Fight_Club"/>
        <R12_has_referred_to_entity rdf:resource="http://www.semanticweb.org/oberreb4/ontologies/2018/9/INTRO#Freud,_Hysterie"/>
        <R12_has_referred_to_entity rdf:resource="http://www.semanticweb.org/oberreb4/ontologies/2018/9/INTRO#Hoffmann,_Sandmann"/>
        <R12_has_referred_to_entity rdf:resource="http://www.semanticweb.org/oberreb4/ontologies/2018/9/INTRO#Kubrick,_Eyes"/>
        <R12_has_referred_to_entity rdf:resource="http://www.semanticweb.org/oberreb4/ontologies/2018/9/INTRO#Shakespeare,_Merchant"/>
        <R12_has_referred_to_entity rdf:resource="http://www.semanticweb.org/oberreb4/ontologies/2018/9/INTRO#Shakespeare,_Midsummer"/>
        <R12_has_referred_to_entity rdf:resource="http://www.semanticweb.org/oberreb4/ontologies/2018/9/INTRO#Shakespeare,_Much_Ado"/>
        <R12_has_referred_to_entity rdf:resource="http://www.semanticweb.org/oberreb4/ontologies/2018/9/INTRO#Shakespeare,_Love&apos;s_Labours"/>
        <R12_has_referred_to_entity rdf:resource="http://www.semanticweb.org/oberreb4/ontologies/2018/9/INTRO#Wagner,_Tristan"/>
        <R13_has_referring_entity rdf:resource="http://www.semanticweb.org/oberreb4/ontologies/2018/9/INTRO#Bronfen,_Cross-Mapping"/>
        <R19_has_type rdf:resource="http://purl.org/spar/cito/discusses"/>
    </owl:NamedIndividual>
    


    <!-- http://www.semanticweb.org/oberreb4/ontologies/2018/9/INTRO#Feat_CrossMapping_Ref -->

    <owl:NamedIndividual rdf:about="http://www.semanticweb.org/oberreb4/ontologies/2018/9/INTRO#Feat_CrossMapping_Ref">
        <rdf:type rdf:resource="http://www.semanticweb.org/oberreb4/ontologies/2018/9/INTRO#INT4_Intertextual_Relationship"/>
        <R12_has_referred_to_entity rdf:resource="http://www.semanticweb.org/oberreb4/ontologies/2018/9/INTRO#Cavell,_Pursuit"/>
        <R12_has_referred_to_entity rdf:resource="http://www.semanticweb.org/oberreb4/ontologies/2018/9/INTRO#Greenblatt,_Circulation"/>
        <R12_has_referred_to_entity rdf:resource="http://www.semanticweb.org/oberreb4/ontologies/2018/9/INTRO#Stafford,_Visual_Analogy"/>
        <R13_has_referring_entity rdf:resource="http://www.semanticweb.org/oberreb4/ontologies/2018/9/INTRO#Bronfen,_Cross-Mapping"/>
        <R17_feature_actualized_in rdf:resource="http://www.semanticweb.org/oberreb4/ontologies/2018/9/INTRO#Act_CrossMapping_References"/>
        <R19_has_type rdf:resource="http://purl.org/spar/cito/usesMethodIn"/>
    </owl:NamedIndividual>
    


    <!-- http://www.semanticweb.org/oberreb4/ontologies/2018/9/INTRO#Feat_CrossMapping_Sources -->

    <owl:NamedIndividual rdf:about="http://www.semanticweb.org/oberreb4/ontologies/2018/9/INTRO#Feat_CrossMapping_Sources">
        <rdf:type rdf:resource="http://www.semanticweb.org/oberreb4/ontologies/2018/9/INTRO#INT4_Intertextual_Relationship"/>
        <R12_has_referred_to_entity rdf:resource="http://www.semanticweb.org/oberreb4/ontologies/2018/9/INTRO#Butler,_Bodies"/>
        <R12_has_referred_to_entity rdf:resource="http://www.semanticweb.org/oberreb4/ontologies/2018/9/INTRO#Butler,_Gender_Trouble"/>
        <R12_has_referred_to_entity rdf:resource="http://www.semanticweb.org/oberreb4/ontologies/2018/9/INTRO#Foucault,_Savoir"/>
        <R12_has_referred_to_entity rdf:resource="http://www.semanticweb.org/oberreb4/ontologies/2018/9/INTRO#Freud,_Hysterie"/>
        <R13_has_referring_entity rdf:resource="http://www.semanticweb.org/oberreb4/ontologies/2018/9/INTRO#Bronfen,_Cross-Mapping"/>
        <R17_feature_actualized_in rdf:resource="http://www.semanticweb.org/oberreb4/ontologies/2018/9/INTRO#Act_CrossMapping_Sources"/>
    </owl:NamedIndividual>
    


    <!-- http://www.semanticweb.org/oberreb4/ontologies/2018/9/INTRO#Feat_Interpretation_CrossMapping -->

    <owl:NamedIndividual rdf:about="http://www.semanticweb.org/oberreb4/ontologies/2018/9/INTRO#Feat_Interpretation_CrossMapping">
        <rdf:type rdf:resource="http://www.semanticweb.org/oberreb4/ontologies/2018/9/INTRO#INT31_Interpretation"/>
    </owl:NamedIndividual>
    


    <!-- http://www.semanticweb.org/oberreb4/ontologies/2018/9/INTRO#Hippolyta -->

    <owl:NamedIndividual rdf:about="http://www.semanticweb.org/oberreb4/ontologies/2018/9/INTRO#Hippolyta">
        <rdf:type rdf:resource="http://www.semanticweb.org/oberreb4/ontologies/2018/9/INTRO#INT28_Individual_Character"/>
    </owl:NamedIndividual>
    


    <!-- http://www.semanticweb.org/oberreb4/ontologies/2018/9/INTRO#Interpretament_CrossMapping -->

    <owl:NamedIndividual rdf:about="http://www.semanticweb.org/oberreb4/ontologies/2018/9/INTRO#Interpretament_CrossMapping">
        <rdf:type rdf:resource="http://www.semanticweb.org/oberreb4/ontologies/2018/9/INTRO#INT44_Interpretament"/>
        <R21_identifies rdf:resource="http://www.semanticweb.org/oberreb4/ontologies/2018/9/INTRO#Clear_Sighted_Daughter"/>
        <R2_consists_in rdf:resource="http://www.semanticweb.org/oberreb4/ontologies/2018/9/INTRO#Act_Interpretation_CrossMapping"/>
    </owl:NamedIndividual>
    


    <!-- http://www.semanticweb.org/oberreb4/ontologies/2018/9/INTRO#Klara -->

    <owl:NamedIndividual rdf:about="http://www.semanticweb.org/oberreb4/ontologies/2018/9/INTRO#Klara">
        <rdf:type rdf:resource="http://www.semanticweb.org/oberreb4/ontologies/2018/9/INTRO#INT28_Individual_Character"/>
    </owl:NamedIndividual>
    


    <!-- http://www.semanticweb.org/oberreb4/ontologies/2018/9/INTRO#Marla -->

    <owl:NamedIndividual rdf:about="http://www.semanticweb.org/oberreb4/ontologies/2018/9/INTRO#Marla">
        <rdf:type rdf:resource="http://www.semanticweb.org/oberreb4/ontologies/2018/9/INTRO#INT28_Individual_Character"/>
    </owl:NamedIndividual>
    


    <!-- http://www.semanticweb.org/oberreb4/ontologies/2018/9/INTRO#Pass._Def._Cross-Mapping -->

    <owl:NamedIndividual rdf:about="http://www.semanticweb.org/oberreb4/ontologies/2018/9/INTRO#Pass._Def._Cross-Mapping">
        <rdf:type rdf:resource="http://www.semanticweb.org/oberreb4/ontologies/2018/9/INTRO#INT1_Text_Passage"/>
        <R44_has_wording>Beim Verfahren des cross-mapping geht es um das Feststellen und Festhalten von Ähnlichkeiten, die sich zwischen ästhetischen Werken ergeben, für die keine eindeutigen intertextuellen Beziehungen im Sinne von explizit thematisierten Einflüssen festgemacht werden können. Es geht darum, die Transformation, die sich durch die Bewegung von einer historischen Zeit in die andere ergibt, hervorzuheben oder die Bewegung von einem medialen Diskurs in einen anderen nachzuzeichnen.</R44_has_wording>
    </owl:NamedIndividual>
    


    <!-- http://www.semanticweb.org/oberreb4/ontologies/2018/9/INTRO#Portia -->

    <owl:NamedIndividual rdf:about="http://www.semanticweb.org/oberreb4/ontologies/2018/9/INTRO#Portia">
        <rdf:type rdf:resource="http://www.semanticweb.org/oberreb4/ontologies/2018/9/INTRO#INT28_Individual_Character"/>
    </owl:NamedIndividual>
    


    <!-- http://www.semanticweb.org/oberreb4/ontologies/2018/9/INTRO#Princess -->

    <owl:NamedIndividual rdf:about="http://www.semanticweb.org/oberreb4/ontologies/2018/9/INTRO#Princess">
        <rdf:type rdf:resource="http://www.semanticweb.org/oberreb4/ontologies/2018/9/INTRO#INT28_Individual_Character"/>
    </owl:NamedIndividual>
    


    <!-- http://www.semanticweb.org/oberreb4/ontologies/2018/9/INTRO#Rewriting_Clear_Sighted_Daughter -->

    <owl:NamedIndividual rdf:about="http://www.semanticweb.org/oberreb4/ontologies/2018/9/INTRO#Rewriting_Clear_Sighted_Daughter">
        <rdf:type rdf:resource="http://www.semanticweb.org/oberreb4/ontologies/2018/9/INTRO#INT4_Intertextual_Relationship"/>
    </owl:NamedIndividual>
    


    <!-- http://www.semanticweb.org/oberreb4/ontologies/2018/9/INTRO#rewriting -->

    <owl:NamedIndividual rdf:about="http://www.semanticweb.org/oberreb4/ontologies/2018/9/INTRO#rewriting">
        <rdf:type rdf:resource="http://www.semanticweb.org/oberreb4/ontologies/2018/9/INTRO#INT22_Type_of_Intertextual_Relationship"/>
    </owl:NamedIndividual>
    


    <!-- http://www.semanticweb.org/oberreb4/ontologies/2018/9/INTRO#Bronfen,_Cross-Mapping -->

    <owl:NamedIndividual rdf:about="http://www.semanticweb.org/oberreb4/ontologies/2018/9/INTRO#Bronfen,_Cross-Mapping">
        <rdf:type rdf:resource="http://erlangen-crm.org/efrbroo/F24_Publication_Expression"/>
        <R10_has_Text_Passage rdf:resource="http://www.semanticweb.org/oberreb4/ontologies/2018/9/INTRO#Pass._Def._Cross-Mapping"/>
        <R18_shows_actualization rdf:resource="http://www.semanticweb.org/oberreb4/ontologies/2018/9/INTRO#Act_CrossMapping_IntRels"/>
    </owl:NamedIndividual>
    


    <!-- http://www.semanticweb.org/oberreb4/ontologies/2018/9/INTRO#Brown,_Wieland -->

    <owl:NamedIndividual rdf:about="http://www.semanticweb.org/oberreb4/ontologies/2018/9/INTRO#Brown,_Wieland">
        <rdf:type rdf:resource="http://erlangen-crm.org/efrbroo/F24_Publication_Expression"/>
    </owl:NamedIndividual>
    


    <!-- http://www.semanticweb.org/oberreb4/ontologies/2018/9/INTRO#Butler,_Bodies -->

    <owl:NamedIndividual rdf:about="http://www.semanticweb.org/oberreb4/ontologies/2018/9/INTRO#Butler,_Bodies">
        <rdf:type rdf:resource="http://erlangen-crm.org/efrbroo/F24_Publication_Expression"/>
    </owl:NamedIndividual>
    


    <!-- http://www.semanticweb.org/oberreb4/ontologies/2018/9/INTRO#Butler,_Gender_Trouble -->

    <owl:NamedIndividual rdf:about="http://www.semanticweb.org/oberreb4/ontologies/2018/9/INTRO#Butler,_Gender_Trouble">
        <rdf:type rdf:resource="http://erlangen-crm.org/efrbroo/F24_Publication_Expression"/>
    </owl:NamedIndividual>
    


    <!-- http://www.semanticweb.org/oberreb4/ontologies/2018/9/INTRO#Cavell,_Pursuit -->

    <owl:NamedIndividual rdf:about="http://www.semanticweb.org/oberreb4/ontologies/2018/9/INTRO#Cavell,_Pursuit">
        <rdf:type rdf:resource="http://erlangen-crm.org/efrbroo/F24_Publication_Expression"/>
    </owl:NamedIndividual>
    


    <!-- http://www.semanticweb.org/oberreb4/ontologies/2018/9/INTRO#Fincher,_Fight_Club -->

    <owl:NamedIndividual rdf:about="http://www.semanticweb.org/oberreb4/ontologies/2018/9/INTRO#Fincher,_Fight_Club">
        <rdf:type rdf:resource="http://erlangen-crm.org/efrbroo/F24_Publication_Expression"/>
    </owl:NamedIndividual>
    


    <!-- http://www.semanticweb.org/oberreb4/ontologies/2018/9/INTRO#Foucault,_Savoir -->

    <owl:NamedIndividual rdf:about="http://www.semanticweb.org/oberreb4/ontologies/2018/9/INTRO#Foucault,_Savoir">
        <rdf:type rdf:resource="http://erlangen-crm.org/efrbroo/F24_Publication_Expression"/>
    </owl:NamedIndividual>
    


    <!-- http://www.semanticweb.org/oberreb4/ontologies/2018/9/INTRO#Freud,_Brief -->

    <owl:NamedIndividual rdf:about="http://www.semanticweb.org/oberreb4/ontologies/2018/9/INTRO#Freud,_Brief">
        <rdf:type rdf:resource="http://erlangen-crm.org/efrbroo/F24_Publication_Expression"/>
    </owl:NamedIndividual>
    


    <!-- http://www.semanticweb.org/oberreb4/ontologies/2018/9/INTRO#Freud,_Hysterie -->

    <owl:NamedIndividual rdf:about="http://www.semanticweb.org/oberreb4/ontologies/2018/9/INTRO#Freud,_Hysterie">
        <rdf:type rdf:resource="http://erlangen-crm.org/efrbroo/F24_Publication_Expression"/>
    </owl:NamedIndividual>
    


    <!-- http://www.semanticweb.org/oberreb4/ontologies/2018/9/INTRO#Freud,_Penis_Normalis -->

    <owl:NamedIndividual rdf:about="http://www.semanticweb.org/oberreb4/ontologies/2018/9/INTRO#Freud,_Penis_Normalis">
        <rdf:type rdf:resource="http://erlangen-crm.org/efrbroo/F23_Expression_Fragment"/>
    </owl:NamedIndividual>
    


    <!-- http://www.semanticweb.org/oberreb4/ontologies/2018/9/INTRO#Greenblatt,_Circulation -->

    <owl:NamedIndividual rdf:about="http://www.semanticweb.org/oberreb4/ontologies/2018/9/INTRO#Greenblatt,_Circulation">
        <rdf:type rdf:resource="http://erlangen-crm.org/efrbroo/F24_Publication_Expression"/>
    </owl:NamedIndividual>
    


    <!-- http://www.semanticweb.org/oberreb4/ontologies/2018/9/INTRO#Hoffmann,_Sandmann -->

    <owl:NamedIndividual rdf:about="http://www.semanticweb.org/oberreb4/ontologies/2018/9/INTRO#Hoffmann,_Sandmann">
        <rdf:type rdf:resource="http://erlangen-crm.org/efrbroo/F24_Publication_Expression"/>
    </owl:NamedIndividual>
    


    <!-- http://www.semanticweb.org/oberreb4/ontologies/2018/9/INTRO#Kubrick,_Eyes -->

    <owl:NamedIndividual rdf:about="http://www.semanticweb.org/oberreb4/ontologies/2018/9/INTRO#Kubrick,_Eyes">
        <rdf:type rdf:resource="http://erlangen-crm.org/efrbroo/F24_Publication_Expression"/>
    </owl:NamedIndividual>
    


    <!-- http://www.semanticweb.org/oberreb4/ontologies/2018/9/INTRO#Shakespeare,_Merchant -->

    <owl:NamedIndividual rdf:about="http://www.semanticweb.org/oberreb4/ontologies/2018/9/INTRO#Shakespeare,_Merchant">
        <rdf:type rdf:resource="http://erlangen-crm.org/efrbroo/F2_Expression"/>
    </owl:NamedIndividual>
    


    <!-- http://www.semanticweb.org/oberreb4/ontologies/2018/9/INTRO#Shakespeare,_Midsummer -->

    <owl:NamedIndividual rdf:about="http://www.semanticweb.org/oberreb4/ontologies/2018/9/INTRO#Shakespeare,_Midsummer">
        <rdf:type rdf:resource="http://erlangen-crm.org/efrbroo/F2_Expression"/>
    </owl:NamedIndividual>
    


    <!-- http://www.semanticweb.org/oberreb4/ontologies/2018/9/INTRO#Shakespeare,_Much_Ado -->

    <owl:NamedIndividual rdf:about="http://www.semanticweb.org/oberreb4/ontologies/2018/9/INTRO#Shakespeare,_Much_Ado">
        <rdf:type rdf:resource="http://erlangen-crm.org/efrbroo/F2_Expression"/>
    </owl:NamedIndividual>
    


    <!-- http://www.semanticweb.org/oberreb4/ontologies/2018/9/INTRO#Shakespeare,_Love&apos;s_Labours -->

    <owl:NamedIndividual rdf:about="http://www.semanticweb.org/oberreb4/ontologies/2018/9/INTRO#Shakespeare,_Love&apos;s_Labours">
        <rdf:type rdf:resource="http://erlangen-crm.org/efrbroo/F2_Expression"/>
    </owl:NamedIndividual>
    


    <!-- http://www.semanticweb.org/oberreb4/ontologies/2018/9/INTRO#Stafford,_Visual_Analogy -->

    <owl:NamedIndividual rdf:about="http://www.semanticweb.org/oberreb4/ontologies/2018/9/INTRO#Stafford,_Visual_Analogy">
        <rdf:type rdf:resource="http://erlangen-crm.org/efrbroo/F24_Publication_Expression"/>
    </owl:NamedIndividual>
    


    <!-- http://www.semanticweb.org/oberreb4/ontologies/2018/9/INTRO#Summ_&apos;Cross-Mapping&apos; -->

    <owl:NamedIndividual rdf:about="http://www.semanticweb.org/oberreb4/ontologies/2018/9/INTRO#Summ_&apos;Cross-Mapping&apos;">
        <rdf:type rdf:resource="http://www.semanticweb.org/oberreb4/ontologies/2018/9/INTRO#INT1_Text_Passage"/>
        <R44_has_wording>eine Lektüre zweier zeitgenössischer Filme im Rückbezug auf literarische Texte [...], die um die Frage kreisen, wie das weibliche Subjekt sich in Bezug auf die symbolischen Kodes und Gesetze, die es definieren, entwirft bzw. wie es durch diese symbolische Ordnung konzipiert wird.</R44_has_wording>
    </owl:NamedIndividual>
    


    <!-- http://www.semanticweb.org/oberreb4/ontologies/2018/9/INTRO#Wagner,_Tristan -->

    <owl:NamedIndividual rdf:about="http://www.semanticweb.org/oberreb4/ontologies/2018/9/INTRO#Wagner,_Tristan">
        <rdf:type rdf:resource="http://erlangen-crm.org/efrbroo/F24_Publication_Expression"/>
    </owl:NamedIndividual>
</rdf:RDF>



<!-- Generated by the OWL API (version 4.2.8.20170104-2310) https://github.com/owlcs/owlapi -->

