<?xml version="1.0"?>
<rdf:RDF xmlns="https://raw.githubusercontent.com/BOberreither/INTRO/master/INTRO_outdated.owl#"
     xml:base="https://raw.githubusercontent.com/BOberreither/INTRO/master/INTRO_outdated.owl"
     xmlns:rdf="http://www.w3.org/1999/02/22-rdf-syntax-ns#"
     xmlns:owl="http://www.w3.org/2002/07/owl#"
     xmlns:xml="http://www.w3.org/XML/1998/namespace"
     xmlns:xsd="http://www.w3.org/2001/XMLSchema#"
     xmlns:skos="http://www.w3.org/2004/02/skos/core#"
     xmlns:rdfs="http://www.w3.org/2000/01/rdf-schema#"
     xmlns:dc="http://purl.org/dc/elements/1.1/"
     xmlns:frbroo="http://iflastandards.info/ns/fr/frbr/frbroo/">
    <owl:Ontology rdf:about="https://raw.githubusercontent.com/BOberreither/INTRO/master/INTRO_outdated.owl">
        <owl:versionInfo rdf:datatype="http://www.w3.org/2001/XMLSchema#string">BETA, outdated - Demo</owl:versionInfo>
        <rdfs:label rdf:datatype="http://www.w3.org/2001/XMLSchema#string">INTRO</rdfs:label>
        <dc:creator rdf:datatype="http://www.w3.org/2001/XMLSchema#string">Bernhard Oberreither</dc:creator>
        <rdfs:comment rdf:datatype="http://www.w3.org/2001/XMLSchema#string"></rdfs:comment>
    </owl:Ontology>
    


    <!-- 
    ///////////////////////////////////////////////////////////////////////////////////////
    //
    // Annotation properties
    //
    ///////////////////////////////////////////////////////////////////////////////////////
     -->

    


    <!-- http://purl.org/dc/elements/1.1/creator -->

    <owl:AnnotationProperty rdf:about="http://purl.org/dc/elements/1.1/creator"/>
    


    <!-- http://purl.org/dc/elements/1.1/description -->

    <owl:AnnotationProperty rdf:about="http://purl.org/dc/elements/1.1/description"/>
    


    <!-- http://www.w3.org/2004/02/skos/core#closeMatch -->

    <owl:AnnotationProperty rdf:about="http://www.w3.org/2004/02/skos/core#closeMatch"/>
    


    <!-- http://www.w3.org/2004/02/skos/core#notation -->

    <owl:AnnotationProperty rdf:about="http://www.w3.org/2004/02/skos/core#notation"/>
    


    <!-- 
    ///////////////////////////////////////////////////////////////////////////////////////
    //
    // Object Properties
    //
    ///////////////////////////////////////////////////////////////////////////////////////
     -->

    


    <!-- http://iflastandards.info/ns/fr/frbr/frbroo/R15_has_fragment -->

    <owl:ObjectProperty rdf:about="http://iflastandards.info/ns/fr/frbr/frbroo/R15_has_fragment">
        <rdfs:subPropertyOf rdf:resource="http://www.cidoc-crm.org/cidoc-crm/P106_is_composed_of"/>
        <owl:inverseOf rdf:resource="http://iflastandards.info/ns/fr/frbr/frbroo/R15i_is_fragment_of"/>
        <rdfs:domain rdf:resource="http://iflastandards.info/ns/fr/frbr/frbroo/F2_Expression"/>
        <rdfs:range rdf:resource="http://iflastandards.info/ns/fr/frbr/frbroo/F23_Expression_Fragment"/>
        <rdfs:comment xml:lang="en">This property associates the fragment of an expression and the expression of which it is a fragment.
</rdfs:comment>
        <rdfs:label xml:lang="en">has fragment</rdfs:label>
    </owl:ObjectProperty>
    


    <!-- http://iflastandards.info/ns/fr/frbr/frbroo/R15i_is_fragment_of -->

    <owl:ObjectProperty rdf:about="http://iflastandards.info/ns/fr/frbr/frbroo/R15i_is_fragment_of">
        <rdfs:subPropertyOf rdf:resource="http://www.cidoc-crm.org/cidoc-crm/P106i_forms_part_of"/>
        <rdfs:domain rdf:resource="http://iflastandards.info/ns/fr/frbr/frbroo/F23_Expression_Fragment"/>
        <rdfs:range rdf:resource="http://iflastandards.info/ns/fr/frbr/frbroo/F2_Expression"/>
        <rdfs:comment xml:lang="en">
</rdfs:comment>
        <rdfs:label xml:lang="en">is fragment of</rdfs:label>
    </owl:ObjectProperty>
    


    <!-- http://iflastandards.info/ns/fr/frbr/frbroo/R3_is_realised_in -->

    <owl:ObjectProperty rdf:about="http://iflastandards.info/ns/fr/frbr/frbroo/R3_is_realised_in">
        <rdfs:subPropertyOf rdf:resource="http://www.cidoc-crm.org/cidoc-crm/P130_shows_features_of"/>
        <owl:inverseOf rdf:resource="http://iflastandards.info/ns/fr/frbr/frbroo/R3i_realises"/>
        <rdfs:domain rdf:resource="http://iflastandards.info/ns/fr/frbr/frbroo/F1_Work"/>
        <rdfs:range rdf:resource="http://iflastandards.info/ns/fr/frbr/frbroo/F22_Self-Contained_Expression"/>
        <rdfs:comment xml:lang="en">This property associates an instance of F22 Self-Contained Expression with an instance of F1 Work.
This property expresses the association that exists between an expression (F22) and the work that this expression conveys. The semantics of the association will be different depending on what specific subtype of F1 Work the work is an instance of. If the work is an instance of F14 Individual Work, the F22 Self-Contained Expression completely conveys the individual work. If the work is an instance of F15 Complex Work, the F22 Self-Contained Expression conveys an alternative member of the complex work.
Our factual knowledge of how a given work is realised into an expression is often limited and this property makes it possible to express the association between instances of F22 Self-Contained Expression and the work it conveys without using the more developed paths.
The property R3.1 has type: E55 Type allows for specifying the role played by the referred to expression in the overall bibliographic history of the work (e.g., ‘progenitor expression’, on which all other expressions of the same work are based; ‘reference for canonical citations’, in the sense of the HuCit ontology developed by Matteo Romanello and Michele Pasin; ‘earliest draft’, ‘intermediate draft’, ‘final clean draft’, ‘princeps edition’, etc.).
</rdfs:comment>
        <rdfs:label xml:lang="en">is realised in</rdfs:label>
    </owl:ObjectProperty>
    


    <!-- http://iflastandards.info/ns/fr/frbr/frbroo/R3i_realises -->

    <owl:ObjectProperty rdf:about="http://iflastandards.info/ns/fr/frbr/frbroo/R3i_realises">
        <rdfs:subPropertyOf rdf:resource="http://www.cidoc-crm.org/cidoc-crm/P130i_features_are_also_found_on"/>
        <rdfs:domain rdf:resource="http://iflastandards.info/ns/fr/frbr/frbroo/F22_Self-Contained_Expression"/>
        <rdfs:range rdf:resource="http://iflastandards.info/ns/fr/frbr/frbroo/F1_Work"/>
        <rdfs:comment xml:lang="en">
</rdfs:comment>
        <rdfs:label xml:lang="en">realises</rdfs:label>
    </owl:ObjectProperty>
    


    <!-- http://iflastandards.info/ns/fr/frbr/frbroo/R40_has_representative_expression -->

    <owl:ObjectProperty rdf:about="http://iflastandards.info/ns/fr/frbr/frbroo/R40_has_representative_expression">
        <rdfs:subPropertyOf rdf:resource="http://iflastandards.info/ns/fr/frbr/frbroo/R3_is_realised_in"/>
        <owl:inverseOf rdf:resource="http://iflastandards.info/ns/fr/frbr/frbroo/R40i_is_representative_expression_for"/>
        <rdfs:domain rdf:resource="http://iflastandards.info/ns/fr/frbr/frbroo/F1_Work"/>
        <rdfs:range rdf:resource="http://iflastandards.info/ns/fr/frbr/frbroo/F22_Self-Contained_Expression"/>
        <rdfs:comment xml:lang="en">This property identifies an instance of F22 Self-Contained Expression that has been chosen as the most characteristic expression of the instance of F1 Work of which it is an expression. There is no other semantic implication to this notion of being characteristic than to be an adequate candidate to uniquely identify the Work realized by it. Prototypically, this is the instance of F22 Self-Contained Expression that is deemed characteristic of an instance of F15 Complex Work.
Typically, any expression that is not regarded as “representative” for the work it expresses, would require a controlled access point, with qualifiers specifying the differences between that expression and a representative expression, although this may not always be done in practice. The title of a Work may not be one taken from a representative expression.
A given work can have more than one representative expression, provided the differences between these expressions are not deemed “substantial.” If the anticipated needs of users are not considered to call for bibliographic distinctions between variant expressions of a work, then even expressions that differ significantly from each other can be regarded as equally representative for the work. (See FRBR: Final Report, p. 19-20).
A given expression can be deemed representative for a work with regard to some of its aspects (e.g., the text contained in an edition the title proper of which reads ‘The tragicall historie of HAMLET Prince of Denmarke’, and the language of that text), and not representative for it with regard to some other aspects (e.g., the title proper ‘The tragicall historie of HAMLET Prince of Denmarke’ itself, which, being different from the title that is regarded as “representative” for Shakespeare’s work, will require the use of a controlled access point).
R40 has representative expression is a shortcut of the more developed path F1 Work R50i was assigned by F42 Representative Expression Assignment R51 assigned F2 Expression.

</rdfs:comment>
        <rdfs:label xml:lang="en">has representative expression</rdfs:label>
    </owl:ObjectProperty>
    


    <!-- http://iflastandards.info/ns/fr/frbr/frbroo/R40i_is_representative_expression_for -->

    <owl:ObjectProperty rdf:about="http://iflastandards.info/ns/fr/frbr/frbroo/R40i_is_representative_expression_for">
        <rdfs:subPropertyOf rdf:resource="http://iflastandards.info/ns/fr/frbr/frbroo/R3i_realises"/>
        <rdfs:domain rdf:resource="http://iflastandards.info/ns/fr/frbr/frbroo/F22_Self-Contained_Expression"/>
        <rdfs:range rdf:resource="http://iflastandards.info/ns/fr/frbr/frbroo/F1_Work"/>
        <rdfs:comment xml:lang="en">
</rdfs:comment>
        <rdfs:label xml:lang="en">is representative expression for</rdfs:label>
    </owl:ObjectProperty>
    


    <!-- http://iflastandards.info/ns/fr/frbr/frbroo/R41_has_rep_manifestation_product_type -->

    <owl:ObjectProperty rdf:about="http://iflastandards.info/ns/fr/frbr/frbroo/R41_has_rep_manifestation_product_type">
        <rdfs:subPropertyOf rdf:resource="http://iflastandards.info/ns/fr/frbr/frbroo/R4_carriers_provided_by"/>
        <owl:inverseOf rdf:resource="http://iflastandards.info/ns/fr/frbr/frbroo/R41i_is_rep_manifestation_product_type_for"/>
        <rdfs:domain rdf:resource="http://iflastandards.info/ns/fr/frbr/frbroo/F2_Expression"/>
        <rdfs:range rdf:resource="http://iflastandards.info/ns/fr/frbr/frbroo/F3_Manifestation_Product_Type"/>
        <rdfs:comment xml:lang="en">This property identifies an instance of F3 Manifestation Product Type that has been chosen as the most characteristic Manifestation Product Type of the instance of F2 Expression of which it is a manifestation.
Identifying an instance of F3 Manifestation Product Type that is representative for an instance of F2 Expression makes it possible in turn to identify an instance of F2 Expression that is representative for an instance of F1 Work, and to decide what should be regarded as the title of the work.
The title of an Expression may not be one taken from a representative Manifestation Product Type or Manifestation Singleton.
A given expression can have more than one Representative Manifestation Product Type.
R41 has representative manifestation product type is a shortcut of the more developed path F2 Expression R48i was assigned by F41 Representative Manifestation Assignment R49 assigned F3 Manifestation Product Type.

</rdfs:comment>
        <rdfs:label xml:lang="en">has rep manifestation product type</rdfs:label>
    </owl:ObjectProperty>
    


    <!-- http://iflastandards.info/ns/fr/frbr/frbroo/R41i_is_rep_manifestation_product_type_for -->

    <owl:ObjectProperty rdf:about="http://iflastandards.info/ns/fr/frbr/frbroo/R41i_is_rep_manifestation_product_type_for">
        <rdfs:subPropertyOf rdf:resource="http://iflastandards.info/ns/fr/frbr/frbroo/R4i_comprises_carriers_of"/>
        <rdfs:domain rdf:resource="http://iflastandards.info/ns/fr/frbr/frbroo/F3_Manifestation_Product_Type"/>
        <rdfs:range rdf:resource="http://iflastandards.info/ns/fr/frbr/frbroo/F2_Expression"/>
        <rdfs:comment xml:lang="en">
</rdfs:comment>
        <rdfs:label xml:lang="en">is rep manifestation product type for</rdfs:label>
    </owl:ObjectProperty>
    


    <!-- http://iflastandards.info/ns/fr/frbr/frbroo/R4_carriers_provided_by -->

    <owl:ObjectProperty rdf:about="http://iflastandards.info/ns/fr/frbr/frbroo/R4_carriers_provided_by">
        <rdfs:subPropertyOf rdf:resource="http://www.cidoc-crm.org/cidoc-crm/P128i_is_carried_by"/>
        <owl:inverseOf rdf:resource="http://iflastandards.info/ns/fr/frbr/frbroo/R4i_comprises_carriers_of"/>
        <rdfs:domain rdf:resource="http://iflastandards.info/ns/fr/frbr/frbroo/F2_Expression"/>
        <rdfs:range rdf:resource="http://iflastandards.info/ns/fr/frbr/frbroo/F3_Manifestation_Product_Type"/>
        <rdfs:comment xml:lang="en">This property associates a publication, i.e. an instance of F3 Manifestation Product Type, with an instance of F2 Expression, which all exemplars of that publication should carry, as long as they are recognised as complete exemplars of that publication. Typically, this property is observed on one exemplar of a publication, and extrapolated to all other exemplars of the same publication.
This property is a shortcut of: F2 Expression P165i is incorporated in F24 Publication Expression CLR6i should be carried by F3 Manifestation Product Type.
</rdfs:comment>
        <rdfs:label xml:lang="en">carriers provided by</rdfs:label>
    </owl:ObjectProperty>
    


    <!-- http://iflastandards.info/ns/fr/frbr/frbroo/R4i_comprises_carriers_of -->

    <owl:ObjectProperty rdf:about="http://iflastandards.info/ns/fr/frbr/frbroo/R4i_comprises_carriers_of">
        <rdfs:subPropertyOf rdf:resource="http://www.cidoc-crm.org/cidoc-crm/P128_carries"/>
        <rdfs:domain rdf:resource="http://iflastandards.info/ns/fr/frbr/frbroo/F3_Manifestation_Product_Type"/>
        <rdfs:range rdf:resource="http://iflastandards.info/ns/fr/frbr/frbroo/F2_Expression"/>
        <rdfs:comment xml:lang="en">
</rdfs:comment>
        <rdfs:label xml:lang="en">comprises carriers of</rdfs:label>
    </owl:ObjectProperty>
    


    <!-- http://purl.org/dc/terms/hasPart -->

    <owl:ObjectProperty rdf:about="http://purl.org/dc/terms/hasPart"/>
    


    <!-- http://purl.org/dc/terms/isPartOf -->

    <owl:ObjectProperty rdf:about="http://purl.org/dc/terms/isPartOf"/>
    


    <!-- http://purl.org/dc/terms/relation -->

    <owl:ObjectProperty rdf:about="http://purl.org/dc/terms/relation"/>
    


    <!-- http://purl.org/spar/cito/agreesWith -->

    <owl:ObjectProperty rdf:about="http://purl.org/spar/cito/agreesWith">
        <rdfs:subPropertyOf rdf:resource="http://purl.org/spar/cito/cites"/>
        <owl:inverseOf rdf:resource="http://purl.org/spar/cito/isAgreedWithBy"/>
        <dc:description xml:lang="en">Example: We share Galileo&apos;s opinion: the Earth moves [X].</dc:description>
        <rdfs:comment xml:lang="en">The citing entity agrees with statements, ideas or conclusions presented in the cited entity.</rdfs:comment>
        <rdfs:label xml:lang="en">agrees with</rdfs:label>
    </owl:ObjectProperty>
    


    <!-- http://purl.org/spar/cito/cites -->

    <owl:ObjectProperty rdf:about="http://purl.org/spar/cito/cites">
        <rdfs:subPropertyOf rdf:resource="http://www.w3.org/2002/07/owl#topObjectProperty"/>
        <owl:inverseOf rdf:resource="http://purl.org/spar/cito/isCitedBy"/>
        <rdfs:comment xml:lang="en">The citing entity cites the cited entity, either directly and explicitly (as in the reference list of a journal article), indirectly (e.g. by citing a more recent paper by the same group on the same topic), or implicitly (e.g. as in artistic quotations or parodies, or in cases of plagiarism).</rdfs:comment>
        <rdfs:label xml:lang="en">cites</rdfs:label>
    </owl:ObjectProperty>
    


    <!-- http://purl.org/spar/cito/citesAsAuthority -->

    <owl:ObjectProperty rdf:about="http://purl.org/spar/cito/citesAsAuthority">
        <rdfs:subPropertyOf rdf:resource="http://purl.org/spar/cito/cites"/>
        <owl:inverseOf rdf:resource="http://purl.org/spar/cito/isCitedAsAuthorityBy"/>
        <dc:description xml:lang="en">Example: Newton asserted that we are like dwarfs standing on the shoulders of giants [X].</dc:description>
        <rdfs:comment xml:lang="en">The citing entity cites the cited entity as one that provides an authoritative description or definition of the subject under discussion.</rdfs:comment>
        <rdfs:label xml:lang="en">cites as authority</rdfs:label>
    </owl:ObjectProperty>
    


    <!-- http://purl.org/spar/cito/citesAsDataSource -->

    <owl:ObjectProperty rdf:about="http://purl.org/spar/cito/citesAsDataSource">
        <rdfs:subPropertyOf rdf:resource="http://purl.org/spar/cito/cites"/>
        <owl:inverseOf rdf:resource="http://purl.org/spar/cito/isCitedAsDataSourceBy"/>
        <dc:description xml:lang="en">Example: Italy has more than ten thousand kilometers of shoreline: see [X].</dc:description>
        <rdfs:comment xml:lang="en">The citing entity cites the cited entity as source of data.</rdfs:comment>
        <rdfs:label xml:lang="en">cites as data source</rdfs:label>
    </owl:ObjectProperty>
    


    <!-- http://purl.org/spar/cito/citesAsEvidence -->

    <owl:ObjectProperty rdf:about="http://purl.org/spar/cito/citesAsEvidence">
        <rdfs:subPropertyOf rdf:resource="http://purl.org/spar/cito/cites"/>
        <owl:inverseOf rdf:resource="http://purl.org/spar/cito/isCitedAsEvidenceBy"/>
        <dc:description xml:lang="en">Example: We found an unquestionable demonstration of our hypothesis in [X].</dc:description>
        <rdfs:comment xml:lang="en">The citing entity cites the cited entity as source of factual evidence for statements it contains.</rdfs:comment>
        <rdfs:label xml:lang="en">cites as evidence</rdfs:label>
    </owl:ObjectProperty>
    


    <!-- http://purl.org/spar/cito/citesAsMetadataDocument -->

    <owl:ObjectProperty rdf:about="http://purl.org/spar/cito/citesAsMetadataDocument">
        <rdfs:subPropertyOf rdf:resource="http://purl.org/spar/cito/cites"/>
        <owl:inverseOf rdf:resource="http://purl.org/spar/cito/isCitedAsMetadataDocumentBy"/>
        <dc:description xml:lang="en">Example: Basic bibliographic, entity and project metadata relating to this article, recorded in a structured machine-readable form, is available as an additional file [X] accompanying this paper.</dc:description>
        <rdfs:comment xml:lang="en">The citing entity cites the cited entity as being the container of metadata describing the citing entity.</rdfs:comment>
        <rdfs:label xml:lang="en">cites as metadata document</rdfs:label>
    </owl:ObjectProperty>
    


    <!-- http://purl.org/spar/cito/citesAsPotentialSolution -->

    <owl:ObjectProperty rdf:about="http://purl.org/spar/cito/citesAsPotentialSolution">
        <rdfs:subPropertyOf rdf:resource="http://purl.org/spar/cito/cites"/>
        <owl:inverseOf rdf:resource="http://purl.org/spar/cito/isCitedAsPontentialSolutionBy"/>
        <dc:description xml:lang="en">Example: This risk could be avoided using the approach shown in [X].</dc:description>
        <rdfs:comment xml:lang="en">The citing entity cites the cited entity as providing or containing a possible solution to the issues being discussed.</rdfs:comment>
        <rdfs:label xml:lang="en">cites as potential solution</rdfs:label>
    </owl:ObjectProperty>
    


    <!-- http://purl.org/spar/cito/citesAsRecommendedReading -->

    <owl:ObjectProperty rdf:about="http://purl.org/spar/cito/citesAsRecommendedReading">
        <rdfs:subPropertyOf rdf:resource="http://purl.org/spar/cito/cites"/>
        <owl:inverseOf rdf:resource="http://purl.org/spar/cito/isCitedAsRecommendedReadingBy"/>
        <dc:description xml:lang="en">Example: To our knowledge, [X] is the best source of exercises about UML, making it a valuable proposal for beginners.</dc:description>
        <rdfs:comment xml:lang="en">The citing entity cites the cited entity as an item of recommended reading.  This property can be used, for example, to describe references in a lecture reading list, where the cited references are relevant to the general topic of the lecture, but might not be individually cited within the text of the lecture.  Similarly, it could be used to describe items in a &apos;Suggested further reading&apos; list at the end of a book chapter.</rdfs:comment>
        <rdfs:label xml:lang="en">cites as recommended reading</rdfs:label>
    </owl:ObjectProperty>
    


    <!-- http://purl.org/spar/cito/citesAsRelated -->

    <owl:ObjectProperty rdf:about="http://purl.org/spar/cito/citesAsRelated">
        <rdfs:subPropertyOf rdf:resource="http://purl.org/spar/cito/cites"/>
        <owl:inverseOf rdf:resource="http://purl.org/spar/cito/isCitedAsRelatedBy"/>
        <dc:description xml:lang="en">Example: An analysis similar to what we proposed here is presented in [X].</dc:description>
        <rdfs:comment xml:lang="en">The citing entity cites the cited entity as one that is related.</rdfs:comment>
        <rdfs:label xml:lang="en">cites as related</rdfs:label>
    </owl:ObjectProperty>
    


    <!-- http://purl.org/spar/cito/citesAsSourceDocument -->

    <owl:ObjectProperty rdf:about="http://purl.org/spar/cito/citesAsSourceDocument">
        <rdfs:subPropertyOf rdf:resource="http://purl.org/spar/cito/cites"/>
        <owl:inverseOf rdf:resource="http://purl.org/spar/cito/isCitedAsSourceDocumentBy"/>
        <dc:description xml:lang="en">Example: Several sections of this work are based on our literature review of the topic published as journal article [X].</dc:description>
        <rdfs:comment xml:lang="en">The citing entity cites the cited entity as being the entity from which the citing entity is derived, or about which the citing entity contains metadata.</rdfs:comment>
        <rdfs:label xml:lang="en">cites as source document</rdfs:label>
    </owl:ObjectProperty>
    


    <!-- http://purl.org/spar/cito/citesForInformation -->

    <owl:ObjectProperty rdf:about="http://purl.org/spar/cito/citesForInformation">
        <rdfs:subPropertyOf rdf:resource="http://purl.org/spar/cito/cites"/>
        <owl:inverseOf rdf:resource="http://purl.org/spar/cito/isCitedForInformationBy"/>
        <dc:description xml:lang="en">Example: The grammar of Pascal was introduced in [X].</dc:description>
        <rdfs:comment xml:lang="en">The citing entity cites the cited entity as a source of information on the subject under discussion.</rdfs:comment>
        <rdfs:label xml:lang="en">cites for information</rdfs:label>
    </owl:ObjectProperty>
    


    <!-- http://purl.org/spar/cito/compiles -->

    <owl:ObjectProperty rdf:about="http://purl.org/spar/cito/compiles">
        <rdfs:subPropertyOf rdf:resource="http://purl.org/spar/cito/cites"/>
        <owl:inverseOf rdf:resource="http://purl.org/spar/cito/isCompiledBy"/>
        <dc:description xml:lang="en">Example: This book gathers interviews with academic researchers of several disciplines [X].</dc:description>
        <dc:description xml:lang="en">Note: This property has been imported from the CiTO4Data ontology, usage of which has been deprecated.</dc:description>
        <rdfs:comment xml:lang="en">The citing entity is used to create or compile the cited entity.</rdfs:comment>
        <rdfs:label xml:lang="en">compiles</rdfs:label>
    </owl:ObjectProperty>
    


    <!-- http://purl.org/spar/cito/confirms -->

    <owl:ObjectProperty rdf:about="http://purl.org/spar/cito/confirms">
        <rdfs:subPropertyOf rdf:resource="http://purl.org/spar/cito/cites"/>
        <owl:inverseOf rdf:resource="http://purl.org/spar/cito/isConfirmedBy"/>
        <dc:description xml:lang="en">Example: Our findings are similar to those published in [X].</dc:description>
        <rdfs:comment xml:lang="en">The citing entity confirms facts, ideas or statements presented in the cited entity.</rdfs:comment>
        <rdfs:label xml:lang="en">confirms</rdfs:label>
    </owl:ObjectProperty>
    


    <!-- http://purl.org/spar/cito/containsAssertionFrom -->

    <owl:ObjectProperty rdf:about="http://purl.org/spar/cito/containsAssertionFrom">
        <rdfs:subPropertyOf rdf:resource="http://purl.org/spar/cito/cites"/>
        <owl:inverseOf rdf:resource="http://purl.org/spar/cito/providesAssertionFor"/>
        <dc:description xml:lang="en">Example: We think that to stand on the top of giants [X] is a valuable principle to follow for our own research.</dc:description>
        <rdfs:comment xml:lang="en">The citing entity contains a statement of fact or a logical assertion (or a collection of such facts and/or assertions) originally present in the cited entity.   This object property is designed to be used to relate a separate abstract, summary or nanopublication to the cited entity upon which it is based.</rdfs:comment>
        <rdfs:label xml:lang="en">contains assertion from</rdfs:label>
    </owl:ObjectProperty>
    


    <!-- http://purl.org/spar/cito/corrects -->

    <owl:ObjectProperty rdf:about="http://purl.org/spar/cito/corrects">
        <rdfs:subPropertyOf rdf:resource="http://purl.org/spar/cito/cites"/>
        <owl:inverseOf rdf:resource="http://purl.org/spar/cito/isCorrectedBy"/>
        <dc:description xml:lang="en">Example: The result published in [X] is partially wrong, the correct result is 42.</dc:description>
        <rdfs:comment xml:lang="en">The citing entity corrects statements, ideas or conclusions presented in the cited entity.</rdfs:comment>
        <rdfs:label xml:lang="en">corrects</rdfs:label>
    </owl:ObjectProperty>
    


    <!-- http://purl.org/spar/cito/credits -->

    <owl:ObjectProperty rdf:about="http://purl.org/spar/cito/credits">
        <rdfs:subPropertyOf rdf:resource="http://purl.org/spar/cito/cites"/>
        <owl:inverseOf rdf:resource="http://purl.org/spar/cito/isCreditedBy"/>
        <dc:description xml:lang="en">Example: Galileo was the first to observe Jupiter&apos;s satellites [X].</dc:description>
        <rdfs:comment xml:lang="en">The citing entity acknowledges contributions made by the cited entity.</rdfs:comment>
        <rdfs:label xml:lang="en">credits</rdfs:label>
    </owl:ObjectProperty>
    


    <!-- http://purl.org/spar/cito/critiques -->

    <owl:ObjectProperty rdf:about="http://purl.org/spar/cito/critiques">
        <rdfs:subPropertyOf rdf:resource="http://purl.org/spar/cito/cites"/>
        <owl:inverseOf rdf:resource="http://purl.org/spar/cito/isCritiquedBy"/>
        <dc:description xml:lang="en">Example: The ideas presented in [X] are badly substantantiated.</dc:description>
        <rdfs:comment xml:lang="en">The citing entity critiques statements, ideas or conclusions presented in the cited entity.</rdfs:comment>
        <rdfs:label xml:lang="en">critiques</rdfs:label>
    </owl:ObjectProperty>
    


    <!-- http://purl.org/spar/cito/derides -->

    <owl:ObjectProperty rdf:about="http://purl.org/spar/cito/derides">
        <rdfs:subPropertyOf rdf:resource="http://purl.org/spar/cito/cites"/>
        <owl:inverseOf rdf:resource="http://purl.org/spar/cito/isDeridedBy"/>
        <dc:description xml:lang="en">Example: The ideas published in [X] are incredibly stupid.</dc:description>
        <rdfs:comment xml:lang="en">The citing entity express derision for the cited entity, or for ideas or conclusions contained within it.</rdfs:comment>
        <rdfs:label xml:lang="en">derides</rdfs:label>
    </owl:ObjectProperty>
    


    <!-- http://purl.org/spar/cito/describes -->

    <owl:ObjectProperty rdf:about="http://purl.org/spar/cito/describes">
        <rdfs:subPropertyOf rdf:resource="http://purl.org/spar/cito/cites"/>
        <owl:inverseOf rdf:resource="http://purl.org/spar/cito/isDescribedBy"/>
        <dc:description xml:lang="en">Example: Galileo&apos;s book [X] is a dialog among three scientists about Copernicus&apos; eliocentric theory.</dc:description>
        <rdfs:comment xml:lang="en">The citing entity describes the cited entity.</rdfs:comment>
        <rdfs:label xml:lang="en">describes</rdfs:label>
    </owl:ObjectProperty>
    


    <!-- http://purl.org/spar/cito/disagreesWith -->

    <owl:ObjectProperty rdf:about="http://purl.org/spar/cito/disagreesWith">
        <rdfs:subPropertyOf rdf:resource="http://purl.org/spar/cito/cites"/>
        <owl:inverseOf rdf:resource="http://purl.org/spar/cito/isDisagreedWithBy"/>
        <dc:description xml:lang="en">Example: We do not share Galileo&apos;s opinion [X]: the Earth does not move.</dc:description>
        <rdfs:comment xml:lang="en">The citing entity disagrees with statements, ideas or conclusions presented in the cited entity.</rdfs:comment>
        <rdfs:label xml:lang="en">disagrees with</rdfs:label>
    </owl:ObjectProperty>
    


    <!-- http://purl.org/spar/cito/discusses -->

    <owl:ObjectProperty rdf:about="http://purl.org/spar/cito/discusses">
        <rdfs:subPropertyOf rdf:resource="http://purl.org/spar/cito/cites"/>
        <owl:inverseOf rdf:resource="http://purl.org/spar/cito/isDiscussedBy"/>
        <dc:description xml:lang="en">Example: We now examine if Galileo is right when he writes [X] that the Earth moves.</dc:description>
        <rdfs:comment xml:lang="en">The citing entity discusses statements, ideas or conclusions presented in the cited entity.</rdfs:comment>
        <rdfs:label xml:lang="en">discusses</rdfs:label>
    </owl:ObjectProperty>
    


    <!-- http://purl.org/spar/cito/disputes -->

    <owl:ObjectProperty rdf:about="http://purl.org/spar/cito/disputes">
        <rdfs:subPropertyOf rdf:resource="http://purl.org/spar/cito/cites"/>
        <owl:inverseOf rdf:resource="http://purl.org/spar/cito/isDisputedBy"/>
        <dc:description xml:lang="en">Example: We doubt that Galileo is right when he writes [X] that the Earth moves.</dc:description>
        <rdfs:comment xml:lang="en">The citing entity disputes statements, ideas or conclusions presented in the cited entity.</rdfs:comment>
        <rdfs:label xml:lang="en">disputes</rdfs:label>
    </owl:ObjectProperty>
    


    <!-- http://purl.org/spar/cito/documents -->

    <owl:ObjectProperty rdf:about="http://purl.org/spar/cito/documents">
        <rdfs:subPropertyOf rdf:resource="http://purl.org/spar/cito/cites"/>
        <owl:inverseOf rdf:resource="http://purl.org/spar/cito/isDocumentedBy"/>
        <dc:description xml:lang="en">Example: Herein we report in detail the complete set of ontological rules defined in the Overlapping Ontology [X].</dc:description>
        <rdfs:comment>The citing entity documents information about the cited entity.</rdfs:comment>
        <rdfs:label xml:lang="en">documents</rdfs:label>
    </owl:ObjectProperty>
    


    <!-- http://purl.org/spar/cito/extends -->

    <owl:ObjectProperty rdf:about="http://purl.org/spar/cito/extends">
        <rdfs:subPropertyOf rdf:resource="http://purl.org/spar/cito/cites"/>
        <owl:inverseOf rdf:resource="http://purl.org/spar/cito/isExtendedBy"/>
        <dc:description xml:lang="en">Example: We add to Galileo&apos;s findings concerning the Earth [X] that also the Moon moves.</dc:description>
        <rdfs:comment xml:lang="en">The citing entity extends facts, ideas or understandings presented in the cited entity.</rdfs:comment>
        <rdfs:label xml:lang="en">extends</rdfs:label>
    </owl:ObjectProperty>
    


    <!-- http://purl.org/spar/cito/givesBackgroundTo -->

    <owl:ObjectProperty rdf:about="http://purl.org/spar/cito/givesBackgroundTo">
        <rdfs:subPropertyOf rdf:resource="http://purl.org/spar/cito/isCitedBy"/>
        <owl:inverseOf rdf:resource="http://purl.org/spar/cito/obtainsBackgroundFrom"/>
        <rdfs:comment xml:lang="en">The cited entity provides background information for the citing entity.</rdfs:comment>
        <rdfs:label xml:lang="en">gives background to</rdfs:label>
    </owl:ObjectProperty>
    


    <!-- http://purl.org/spar/cito/givesSupportTo -->

    <owl:ObjectProperty rdf:about="http://purl.org/spar/cito/givesSupportTo">
        <rdfs:subPropertyOf rdf:resource="http://purl.org/spar/cito/isCitedBy"/>
        <owl:inverseOf rdf:resource="http://purl.org/spar/cito/obtainsSupportFrom"/>
        <rdfs:comment xml:lang="en">The cited entity provides intellectual or factual support for the citing entity.</rdfs:comment>
        <rdfs:label xml:lang="en">gives support to</rdfs:label>
    </owl:ObjectProperty>
    


    <!-- http://purl.org/spar/cito/hasReplyFrom -->

    <owl:ObjectProperty rdf:about="http://purl.org/spar/cito/hasReplyFrom">
        <rdfs:subPropertyOf rdf:resource="http://purl.org/spar/cito/isCitedBy"/>
        <owl:inverseOf rdf:resource="http://purl.org/spar/cito/repliesTo"/>
        <rdfs:comment xml:lang="en">The cited entity evokes a reply from the citing entity.</rdfs:comment>
        <rdfs:label xml:lang="en">has reply from</rdfs:label>
    </owl:ObjectProperty>
    


    <!-- http://purl.org/spar/cito/includesExcerptFrom -->

    <owl:ObjectProperty rdf:about="http://purl.org/spar/cito/includesExcerptFrom">
        <rdfs:subPropertyOf rdf:resource="http://purl.org/spar/cito/cites"/>
        <owl:inverseOf rdf:resource="http://purl.org/spar/cito/providesExcerptFor"/>
        <dc:description xml:lang="en">An excerpt is more general than a quotation. It is generally used to indicate a re-published extract from a book, instruction manual, film, radio programme, etc, that need not be what someone said.  For example:

Oxford 01865
Oxshott 01372
Oxted 01883
Oxton 01578

is an excerpt from the UK Dialling Codes section of the Oxford Telephone Directory.</dc:description>
        <dc:description xml:lang="en">Example: In her work, the author states that even though most Human Information Behaviour researchers are familiar with the literature related to their studies, it is not uncommon for investigators to fail to see the benefits they may gain from previous mistakes [X].</dc:description>
        <rdfs:comment xml:lang="en">The citing entity includes one or more excerpts from the cited entity.</rdfs:comment>
        <rdfs:label xml:lang="en">includes excerpt from</rdfs:label>
    </owl:ObjectProperty>
    


    <!-- http://purl.org/spar/cito/includesQuotationFrom -->

    <owl:ObjectProperty rdf:about="http://purl.org/spar/cito/includesQuotationFrom">
        <rdfs:subPropertyOf rdf:resource="http://purl.org/spar/cito/cites"/>
        <owl:inverseOf rdf:resource="http://purl.org/spar/cito/providesQuotationFor"/>
        <dc:description xml:lang="en">A quotation is a repetition of what someone has said, and is presented &quot;within quotation marks&quot;, for example:

On June 4th 1940, Winston Churchill made a speech on the radio that has since become famous, that included the words: &quot; . . . we shall fight on the beaches, we shall fight on the landing grounds, we shall fight in the fields and in the streets, we shall fight in the hills; we shall never surrender . . .&quot;</dc:description>
        <dc:description xml:lang="en">Example: As Newton wrote in [X]: &quot;We are like dwarfs standing on the shoulders of giants&quot;.</dc:description>
        <rdfs:comment xml:lang="en">The citing entity includes one or more quotations from the cited entity.</rdfs:comment>
        <rdfs:label xml:lang="en">includes quotation from</rdfs:label>
    </owl:ObjectProperty>
    


    <!-- http://purl.org/spar/cito/isAgreedWithBy -->

    <owl:ObjectProperty rdf:about="http://purl.org/spar/cito/isAgreedWithBy">
        <rdfs:subPropertyOf rdf:resource="http://purl.org/spar/cito/isCitedBy"/>
        <rdfs:comment xml:lang="en">The cited entity contains statements, ideas or conclusions with which the citing entity agrees.</rdfs:comment>
        <rdfs:label xml:lang="en">is agreed with by</rdfs:label>
    </owl:ObjectProperty>
    


    <!-- http://purl.org/spar/cito/isCitedAsAuthorityBy -->

    <owl:ObjectProperty rdf:about="http://purl.org/spar/cito/isCitedAsAuthorityBy">
        <rdfs:subPropertyOf rdf:resource="http://purl.org/spar/cito/isCitedBy"/>
        <rdfs:comment xml:lang="en">The cited entity is cited as providing an authoritative description or definition of the subject under discussion in the citing entity.</rdfs:comment>
        <rdfs:label xml:lang="en">is cited as authority by</rdfs:label>
    </owl:ObjectProperty>
    


    <!-- http://purl.org/spar/cito/isCitedAsDataSourceBy -->

    <owl:ObjectProperty rdf:about="http://purl.org/spar/cito/isCitedAsDataSourceBy">
        <rdfs:subPropertyOf rdf:resource="http://purl.org/spar/cito/isCitedBy"/>
        <rdfs:comment xml:lang="en">The cited entity is cited as a data source by the citing entity.</rdfs:comment>
        <rdfs:label xml:lang="en">is cited as data source by</rdfs:label>
    </owl:ObjectProperty>
    


    <!-- http://purl.org/spar/cito/isCitedAsEvidenceBy -->

    <owl:ObjectProperty rdf:about="http://purl.org/spar/cito/isCitedAsEvidenceBy">
        <rdfs:subPropertyOf rdf:resource="http://purl.org/spar/cito/isCitedBy"/>
        <rdfs:comment xml:lang="en">The cited entity is cited for providing factual evidence to the citing entity.</rdfs:comment>
        <rdfs:label xml:lang="en">is cited as evidence by</rdfs:label>
    </owl:ObjectProperty>
    


    <!-- http://purl.org/spar/cito/isCitedAsMetadataDocumentBy -->

    <owl:ObjectProperty rdf:about="http://purl.org/spar/cito/isCitedAsMetadataDocumentBy">
        <rdfs:subPropertyOf rdf:resource="http://purl.org/spar/cito/isCitedBy"/>
        <rdfs:comment xml:lang="en">The cited entity is cited as being the container of metadata relating to the citing entity.</rdfs:comment>
        <rdfs:label xml:lang="en">is cited as metadata document by</rdfs:label>
    </owl:ObjectProperty>
    


    <!-- http://purl.org/spar/cito/isCitedAsPontentialSolutionBy -->

    <owl:ObjectProperty rdf:about="http://purl.org/spar/cito/isCitedAsPontentialSolutionBy">
        <rdfs:subPropertyOf rdf:resource="http://purl.org/spar/cito/isCitedBy"/>
        <rdfs:comment xml:lang="en">The cited entity is cited as providing or containing a possible solution to the issues being discussed in the citing entity.</rdfs:comment>
        <rdfs:label xml:lang="en">is cited as potential solution by</rdfs:label>
    </owl:ObjectProperty>
    


    <!-- http://purl.org/spar/cito/isCitedAsRecommendedReadingBy -->

    <owl:ObjectProperty rdf:about="http://purl.org/spar/cito/isCitedAsRecommendedReadingBy">
        <rdfs:subPropertyOf rdf:resource="http://purl.org/spar/cito/isCitedBy"/>
        <rdfs:comment xml:lang="en">The cited entity is cited by the citing entity as an item of recommended reading.  This property can be used, for example, to describe references in a lecture reading list, where the cited references are relevant to the general topic of the lecture, but might not be individually cited within the text of the lecture.  Similarly, it could be used to describe items in a &apos;Suggested further reading&apos; list at the end of a book chapter.</rdfs:comment>
        <rdfs:label xml:lang="en">is cited as recommended reading by</rdfs:label>
    </owl:ObjectProperty>
    


    <!-- http://purl.org/spar/cito/isCitedAsRelatedBy -->

    <owl:ObjectProperty rdf:about="http://purl.org/spar/cito/isCitedAsRelatedBy">
        <rdfs:subPropertyOf rdf:resource="http://purl.org/spar/cito/isCitedBy"/>
        <rdfs:comment xml:lang="en">The cited entity is cited as being related to the citing entity.</rdfs:comment>
        <rdfs:label xml:lang="en">is cited as related by</rdfs:label>
    </owl:ObjectProperty>
    


    <!-- http://purl.org/spar/cito/isCitedAsSourceDocumentBy -->

    <owl:ObjectProperty rdf:about="http://purl.org/spar/cito/isCitedAsSourceDocumentBy">
        <rdfs:subPropertyOf rdf:resource="http://purl.org/spar/cito/isCitedBy"/>
        <rdfs:comment xml:lang="en">The cited entity is cited as being the entity from which the citing entity is derived, or about which the citing entity contains metadata.</rdfs:comment>
        <rdfs:label xml:lang="en">is cited as source document by</rdfs:label>
    </owl:ObjectProperty>
    


    <!-- http://purl.org/spar/cito/isCitedBy -->

    <owl:ObjectProperty rdf:about="http://purl.org/spar/cito/isCitedBy">
        <rdfs:subPropertyOf rdf:resource="http://www.w3.org/2002/07/owl#topObjectProperty"/>
        <rdfs:comment xml:lang="en">The cited entity (the subject of the RDF triple) is cited by the citing entity (the object of the triple).</rdfs:comment>
        <rdfs:label xml:lang="en">is cited by</rdfs:label>
    </owl:ObjectProperty>
    


    <!-- http://purl.org/spar/cito/isCitedForInformationBy -->

    <owl:ObjectProperty rdf:about="http://purl.org/spar/cito/isCitedForInformationBy">
        <rdfs:subPropertyOf rdf:resource="http://purl.org/spar/cito/isCitedBy"/>
        <rdfs:comment xml:lang="en">The cited entity is cited as a source of information on the subject under discussion in the citing entity.</rdfs:comment>
        <rdfs:label xml:lang="en">is cited for information by</rdfs:label>
    </owl:ObjectProperty>
    


    <!-- http://purl.org/spar/cito/isCompiledBy -->

    <owl:ObjectProperty rdf:about="http://purl.org/spar/cito/isCompiledBy">
        <rdfs:subPropertyOf rdf:resource="http://purl.org/spar/cito/isCitedBy"/>
        <dc:description xml:lang="en">Note: This property has been imported from the CiTO4Data ontology, usage of which has been deprecated.</dc:description>
        <rdfs:comment xml:lang="en">The cited entity is the result of a compile or creation event using the citing entity.</rdfs:comment>
        <rdfs:label xml:lang="en">is compiled by</rdfs:label>
    </owl:ObjectProperty>
    


    <!-- http://purl.org/spar/cito/isConfirmedBy -->

    <owl:ObjectProperty rdf:about="http://purl.org/spar/cito/isConfirmedBy">
        <rdfs:subPropertyOf rdf:resource="http://purl.org/spar/cito/isCitedBy"/>
        <rdfs:comment xml:lang="en">The cited entity presents facts, ideas or statements that are confirmed by the citing entity.</rdfs:comment>
        <rdfs:label xml:lang="en">is confirmed by</rdfs:label>
    </owl:ObjectProperty>
    


    <!-- http://purl.org/spar/cito/isCorrectedBy -->

    <owl:ObjectProperty rdf:about="http://purl.org/spar/cito/isCorrectedBy">
        <rdfs:subPropertyOf rdf:resource="http://purl.org/spar/cito/isCitedBy"/>
        <rdfs:comment xml:lang="en">The cited entity presents statements, ideas or conclusions that are corrected by the citing entity.</rdfs:comment>
        <rdfs:label xml:lang="en">is corrected by</rdfs:label>
    </owl:ObjectProperty>
    


    <!-- http://purl.org/spar/cito/isCreditedBy -->

    <owl:ObjectProperty rdf:about="http://purl.org/spar/cito/isCreditedBy">
        <rdfs:subPropertyOf rdf:resource="http://purl.org/spar/cito/isCitedBy"/>
        <rdfs:comment xml:lang="en">The cited entity makes contributions that are acknowledged by the citing entity.</rdfs:comment>
        <rdfs:label xml:lang="en">is credited by</rdfs:label>
    </owl:ObjectProperty>
    


    <!-- http://purl.org/spar/cito/isCritiquedBy -->

    <owl:ObjectProperty rdf:about="http://purl.org/spar/cito/isCritiquedBy">
        <rdfs:subPropertyOf rdf:resource="http://purl.org/spar/cito/isCitedBy"/>
        <rdfs:comment xml:lang="en">The cited entity presents statements, ideas or conclusions that are critiqued by the citing entity.</rdfs:comment>
        <rdfs:label xml:lang="en">is critiqued by</rdfs:label>
    </owl:ObjectProperty>
    


    <!-- http://purl.org/spar/cito/isDeridedBy -->

    <owl:ObjectProperty rdf:about="http://purl.org/spar/cito/isDeridedBy">
        <rdfs:subPropertyOf rdf:resource="http://purl.org/spar/cito/isCitedBy"/>
        <rdfs:comment xml:lang="en">The cited entity contains ideas or conclusions for which the citing entity express derision.</rdfs:comment>
        <rdfs:label xml:lang="en">is derided by</rdfs:label>
    </owl:ObjectProperty>
    


    <!-- http://purl.org/spar/cito/isDescribedBy -->

    <owl:ObjectProperty rdf:about="http://purl.org/spar/cito/isDescribedBy">
        <rdfs:subPropertyOf rdf:resource="http://purl.org/spar/cito/isCitedBy"/>
        <rdfs:comment xml:lang="en">The cited entity is described by the citing entity.</rdfs:comment>
        <rdfs:label xml:lang="en">is described by</rdfs:label>
    </owl:ObjectProperty>
    


    <!-- http://purl.org/spar/cito/isDisagreedWithBy -->

    <owl:ObjectProperty rdf:about="http://purl.org/spar/cito/isDisagreedWithBy">
        <rdfs:subPropertyOf rdf:resource="http://purl.org/spar/cito/isCitedBy"/>
        <rdfs:comment xml:lang="en">The cited entity presents statements, ideas or conclusions that are disagreed with by the citing entity.</rdfs:comment>
        <rdfs:label xml:lang="en">is disagreed with by</rdfs:label>
    </owl:ObjectProperty>
    


    <!-- http://purl.org/spar/cito/isDiscussedBy -->

    <owl:ObjectProperty rdf:about="http://purl.org/spar/cito/isDiscussedBy">
        <rdfs:subPropertyOf rdf:resource="http://purl.org/spar/cito/isCitedBy"/>
        <rdfs:comment xml:lang="en">The cited entity presents statements, ideas or conclusions that are discussed by the citing entity.</rdfs:comment>
        <rdfs:label xml:lang="en">is discussed by</rdfs:label>
    </owl:ObjectProperty>
    


    <!-- http://purl.org/spar/cito/isDisputedBy -->

    <owl:ObjectProperty rdf:about="http://purl.org/spar/cito/isDisputedBy">
        <rdfs:subPropertyOf rdf:resource="http://purl.org/spar/cito/isCitedBy"/>
        <rdfs:comment xml:lang="en">The cited entity presents statements, ideas or conclusions that are disputed by the citing entity.</rdfs:comment>
        <rdfs:label xml:lang="en">is disputed by</rdfs:label>
    </owl:ObjectProperty>
    


    <!-- http://purl.org/spar/cito/isDocumentedBy -->

    <owl:ObjectProperty rdf:about="http://purl.org/spar/cito/isDocumentedBy">
        <rdfs:subPropertyOf rdf:resource="http://purl.org/spar/cito/isCitedBy"/>
        <rdfs:comment xml:lang="en">Information about the cited entity is documented by the citing entity.</rdfs:comment>
        <rdfs:label xml:lang="en">is documented by</rdfs:label>
    </owl:ObjectProperty>
    


    <!-- http://purl.org/spar/cito/isExtendedBy -->

    <owl:ObjectProperty rdf:about="http://purl.org/spar/cito/isExtendedBy">
        <rdfs:subPropertyOf rdf:resource="http://purl.org/spar/cito/isCitedBy"/>
        <rdfs:comment xml:lang="en">The cited entity presents facts, ideas or understandings that are extended by the citing entity.</rdfs:comment>
        <rdfs:label xml:lang="en">is extended by</rdfs:label>
    </owl:ObjectProperty>
    


    <!-- http://purl.org/spar/cito/isLinkedToBy -->

    <owl:ObjectProperty rdf:about="http://purl.org/spar/cito/isLinkedToBy">
        <rdfs:subPropertyOf rdf:resource="http://purl.org/spar/cito/isCitedBy"/>
        <owl:inverseOf rdf:resource="http://purl.org/spar/cito/linksTo"/>
        <rdfs:comment xml:lang="en">The cited entity is the target for an HTTP Uniform Resource Locator (URL) link within the citing entity.</rdfs:comment>
        <rdfs:label xml:lang="en">is linked to by</rdfs:label>
    </owl:ObjectProperty>
    


    <!-- http://purl.org/spar/cito/isParodiedBy -->

    <owl:ObjectProperty rdf:about="http://purl.org/spar/cito/isParodiedBy">
        <rdfs:subPropertyOf rdf:resource="http://purl.org/spar/cito/isCitedBy"/>
        <owl:inverseOf rdf:resource="http://purl.org/spar/cito/parodies"/>
        <rdfs:comment xml:lang="en">The characteristic style or content of the cited entity is imitated by the citing entity for comic effect, usually without explicit citation.</rdfs:comment>
        <rdfs:label xml:lang="en">is parodied by</rdfs:label>
    </owl:ObjectProperty>
    


    <!-- http://purl.org/spar/cito/isPlagiarizedBy -->

    <owl:ObjectProperty rdf:about="http://purl.org/spar/cito/isPlagiarizedBy">
        <rdfs:subPropertyOf rdf:resource="http://purl.org/spar/cito/isCitedBy"/>
        <owl:inverseOf rdf:resource="http://purl.org/spar/cito/plagiarizes"/>
        <rdfs:comment xml:lang="en">The cited entity is plagiarized by the author of the citing entity, who includes within the citing entity textual or other elements from the cited entity without formal acknowledgement of their source. The cited entity is thus not explicitly cited from within the citing entity, according to the norms of scholarly practice, but is cited implicitly.</rdfs:comment>
        <rdfs:label xml:lang="en">is plagiarized by</rdfs:label>
    </owl:ObjectProperty>
    


    <!-- http://purl.org/spar/cito/isQualifiedBy -->

    <owl:ObjectProperty rdf:about="http://purl.org/spar/cito/isQualifiedBy">
        <rdfs:subPropertyOf rdf:resource="http://purl.org/spar/cito/isCitedBy"/>
        <owl:inverseOf rdf:resource="http://purl.org/spar/cito/qualifies"/>
        <rdfs:comment xml:lang="en">The cited entity presents statements, ideas or conclusions that are qualified or have conditions placed upon them by the citing entity.</rdfs:comment>
        <rdfs:label xml:lang="en">is qualified by</rdfs:label>
    </owl:ObjectProperty>
    


    <!-- http://purl.org/spar/cito/isRefutedBy -->

    <owl:ObjectProperty rdf:about="http://purl.org/spar/cito/isRefutedBy">
        <rdfs:subPropertyOf rdf:resource="http://purl.org/spar/cito/isCitedBy"/>
        <owl:inverseOf rdf:resource="http://purl.org/spar/cito/refutes"/>
        <rdfs:comment xml:lang="en">The cited entity presents statements, ideas or conclusions that are refuted by the citing entity.</rdfs:comment>
        <rdfs:label xml:lang="en">is refuted by</rdfs:label>
    </owl:ObjectProperty>
    


    <!-- http://purl.org/spar/cito/isRetractedBy -->

    <owl:ObjectProperty rdf:about="http://purl.org/spar/cito/isRetractedBy">
        <rdfs:subPropertyOf rdf:resource="http://purl.org/spar/cito/isCitedBy"/>
        <owl:inverseOf rdf:resource="http://purl.org/spar/cito/retracts"/>
        <rdfs:comment xml:lang="en">The cited entity is formally retracted by the citing entity.</rdfs:comment>
        <rdfs:label xml:lang="en">is retracted by</rdfs:label>
    </owl:ObjectProperty>
    


    <!-- http://purl.org/spar/cito/isReviewedBy -->

    <owl:ObjectProperty rdf:about="http://purl.org/spar/cito/isReviewedBy">
        <rdfs:subPropertyOf rdf:resource="http://purl.org/spar/cito/isCitedBy"/>
        <owl:inverseOf rdf:resource="http://purl.org/spar/cito/reviews"/>
        <rdfs:comment xml:lang="en">The cited entity presents statements, ideas or conclusions that are reviewed by the citing entity.</rdfs:comment>
        <rdfs:label xml:lang="en">is reviewed by</rdfs:label>
    </owl:ObjectProperty>
    


    <!-- http://purl.org/spar/cito/isRidiculedBy -->

    <owl:ObjectProperty rdf:about="http://purl.org/spar/cito/isRidiculedBy">
        <rdfs:subPropertyOf rdf:resource="http://purl.org/spar/cito/isCitedBy"/>
        <owl:inverseOf rdf:resource="http://purl.org/spar/cito/ridicules"/>
        <rdfs:comment xml:lang="en">The cited entity or aspects of its contents are ridiculed by the citing entity.</rdfs:comment>
        <rdfs:label xml:lang="en">is ridiculed by</rdfs:label>
    </owl:ObjectProperty>
    


    <!-- http://purl.org/spar/cito/isSpeculatedOnBy -->

    <owl:ObjectProperty rdf:about="http://purl.org/spar/cito/isSpeculatedOnBy">
        <rdfs:subPropertyOf rdf:resource="http://purl.org/spar/cito/isCitedBy"/>
        <owl:inverseOf rdf:resource="http://purl.org/spar/cito/speculatesOn"/>
        <rdfs:comment xml:lang="en">The cited entity is cited because the citing article contains speculations on its content or ideas.</rdfs:comment>
        <rdfs:label xml:lang="en">is speculated on by</rdfs:label>
    </owl:ObjectProperty>
    


    <!-- http://purl.org/spar/cito/isSupportedBy -->

    <owl:ObjectProperty rdf:about="http://purl.org/spar/cito/isSupportedBy">
        <rdfs:subPropertyOf rdf:resource="http://purl.org/spar/cito/isCitedBy"/>
        <owl:inverseOf rdf:resource="http://purl.org/spar/cito/supports"/>
        <rdfs:comment xml:lang="en">The cited entity receives intellectual or factual support from the citing entity.</rdfs:comment>
        <rdfs:label xml:lang="en">is supported by</rdfs:label>
    </owl:ObjectProperty>
    


    <!-- http://purl.org/spar/cito/isUpdatedBy -->

    <owl:ObjectProperty rdf:about="http://purl.org/spar/cito/isUpdatedBy">
        <rdfs:subPropertyOf rdf:resource="http://purl.org/spar/cito/isCitedBy"/>
        <owl:inverseOf rdf:resource="http://purl.org/spar/cito/updates"/>
        <rdfs:comment xml:lang="en">The cited entity presents statements, ideas, hypotheses or understanding that are updated by the cited entity.</rdfs:comment>
        <rdfs:label xml:lang="en">is updated by</rdfs:label>
    </owl:ObjectProperty>
    


    <!-- http://purl.org/spar/cito/linksTo -->

    <owl:ObjectProperty rdf:about="http://purl.org/spar/cito/linksTo">
        <rdfs:subPropertyOf rdf:resource="http://purl.org/spar/cito/cites"/>
        <dc:description xml:lang="en">Example: The BioSharing registry (https://biosharing.org) can be of use as it describes the standards in detail, including versions where applicable.</dc:description>
        <rdfs:comment xml:lang="en">The citing entity provides a link, in the form of an HTTP Uniform Resource Locator (URL), to the cited entity.</rdfs:comment>
        <rdfs:label xml:lang="en">links to</rdfs:label>
    </owl:ObjectProperty>
    


    <!-- http://purl.org/spar/cito/obtainsBackgroundFrom -->

    <owl:ObjectProperty rdf:about="http://purl.org/spar/cito/obtainsBackgroundFrom">
        <rdfs:subPropertyOf rdf:resource="http://purl.org/spar/cito/cites"/>
        <dc:description xml:lang="en">Example: There is a need for more observational studies and studies using narrative causation to describe the potential contribution of information in problem-solving and decision-making [X]; our work addresses these needs.</dc:description>
        <rdfs:comment xml:lang="en">The citing entity obtains background information from the cited entity.</rdfs:comment>
        <rdfs:label xml:lang="en">obtains background from</rdfs:label>
    </owl:ObjectProperty>
    


    <!-- http://purl.org/spar/cito/obtainsSupportFrom -->

    <owl:ObjectProperty rdf:about="http://purl.org/spar/cito/obtainsSupportFrom">
        <rdfs:subPropertyOf rdf:resource="http://purl.org/spar/cito/cites"/>
        <dc:description xml:lang="en">Example: Our ideas were also shared by Doe et al. [X].</dc:description>
        <rdfs:comment xml:lang="en">The citing entity obtains intellectual or factual support from the cited entity.</rdfs:comment>
        <rdfs:label xml:lang="en">obtains support from</rdfs:label>
    </owl:ObjectProperty>
    


    <!-- http://purl.org/spar/cito/parodies -->

    <owl:ObjectProperty rdf:about="http://purl.org/spar/cito/parodies">
        <rdfs:subPropertyOf rdf:resource="http://purl.org/spar/cito/cites"/>
        <dc:description xml:lang="en">Example: We act as giants on the shoulders of dwarfs [X]!</dc:description>
        <rdfs:comment xml:lang="en">The citing entity imitates the characteristic style or content of the cited entity for comic effect, usually without explicit citation.</rdfs:comment>
        <rdfs:label xml:lang="en">parodies</rdfs:label>
    </owl:ObjectProperty>
    


    <!-- http://purl.org/spar/cito/plagiarizes -->

    <owl:ObjectProperty rdf:about="http://purl.org/spar/cito/plagiarizes">
        <rdfs:subPropertyOf rdf:resource="http://purl.org/spar/cito/cites"/>
        <dc:description xml:lang="en">Example: The conclusion of our dissertation can be summarised by the following motto, we created specifically for this purpose: we are like dwarfs standing on the shoulders of giants.</dc:description>
        <rdfs:comment xml:lang="en">A property indicating that the author of the citing entity plagiarizes the cited entity, by including textual or other elements from the cited entity without formal acknowledgement of their source.  The citing entity thus contains no explicit citation of the cited entity, according to the norms of scholarly practice, but cites it implicitly.</rdfs:comment>
        <rdfs:label xml:lang="en">plagiarizes</rdfs:label>
    </owl:ObjectProperty>
    


    <!-- http://purl.org/spar/cito/providesAssertionFor -->

    <owl:ObjectProperty rdf:about="http://purl.org/spar/cito/providesAssertionFor">
        <rdfs:subPropertyOf rdf:resource="http://purl.org/spar/cito/isCitedBy"/>
        <rdfs:comment xml:lang="en">The cited entity contains and is the original source of a statement of fact or a logical assertion (or a collection of such facts and/or assertions) that is to be found in the citing entity.   This inverse object property is designed to be used to relate a cited entity to a separate abstract, summary or nanopublication based upon it.</rdfs:comment>
        <rdfs:label xml:lang="en">provides assertion for</rdfs:label>
    </owl:ObjectProperty>
    


    <!-- http://purl.org/spar/cito/providesConclusionsFor -->

    <owl:ObjectProperty rdf:about="http://purl.org/spar/cito/providesConclusionsFor">
        <rdfs:subPropertyOf rdf:resource="http://purl.org/spar/cito/isCitedBy"/>
        <owl:inverseOf rdf:resource="http://purl.org/spar/cito/usesConclusionsFrom"/>
        <rdfs:comment xml:lang="en">The cited entity presents conclusions that are used in work described in the citing entity.</rdfs:comment>
        <rdfs:label xml:lang="en">provides conclusions for</rdfs:label>
    </owl:ObjectProperty>
    


    <!-- http://purl.org/spar/cito/providesDataFor -->

    <owl:ObjectProperty rdf:about="http://purl.org/spar/cito/providesDataFor">
        <rdfs:subPropertyOf rdf:resource="http://purl.org/spar/cito/isCitedBy"/>
        <owl:inverseOf rdf:resource="http://purl.org/spar/cito/usesDataFrom"/>
        <rdfs:comment xml:lang="en">The cited entity presents data that are used in work described in the citing entity.</rdfs:comment>
        <rdfs:label xml:lang="en">provides data for</rdfs:label>
    </owl:ObjectProperty>
    


    <!-- http://purl.org/spar/cito/providesExcerptFor -->

    <owl:ObjectProperty rdf:about="http://purl.org/spar/cito/providesExcerptFor">
        <rdfs:subPropertyOf rdf:resource="http://purl.org/spar/cito/isCitedBy"/>
        <rdfs:comment xml:lang="en">The cited entity contains information, usually of a textual nature, that is excerpted by (used as an excerpt within) the citing entity.</rdfs:comment>
        <rdfs:label xml:lang="en">provides excerpt for</rdfs:label>
    </owl:ObjectProperty>
    


    <!-- http://purl.org/spar/cito/providesMethodFor -->

    <owl:ObjectProperty rdf:about="http://purl.org/spar/cito/providesMethodFor">
        <rdfs:subPropertyOf rdf:resource="http://purl.org/spar/cito/isCitedBy"/>
        <owl:inverseOf rdf:resource="http://purl.org/spar/cito/usesMethodIn"/>
        <rdfs:comment xml:lang="en">The cited entity details a method that is used in work described by the citing entity.</rdfs:comment>
        <rdfs:label xml:lang="en">provides method for</rdfs:label>
    </owl:ObjectProperty>
    


    <!-- http://purl.org/spar/cito/providesQuotationFor -->

    <owl:ObjectProperty rdf:about="http://purl.org/spar/cito/providesQuotationFor">
        <rdfs:subPropertyOf rdf:resource="http://purl.org/spar/cito/isCitedBy"/>
        <rdfs:comment xml:lang="en">The cited entity contains information, usually of a textual nature, that is quoted by (used as a quotation within) the citing entity.</rdfs:comment>
        <rdfs:label xml:lang="en">provides quotation for</rdfs:label>
    </owl:ObjectProperty>
    


    <!-- http://purl.org/spar/cito/qualifies -->

    <owl:ObjectProperty rdf:about="http://purl.org/spar/cito/qualifies">
        <rdfs:subPropertyOf rdf:resource="http://purl.org/spar/cito/cites"/>
        <dc:description xml:lang="en">Example: Galileo&apos;s masterpiece &apos;Dialogo sopra i due massimi sistemi del mondo&apos; [X] is formally a dialog and substantially a scientific pamphlet.</dc:description>
        <rdfs:comment xml:lang="en">The citing entity qualifies or places conditions or restrictions upon statements, ideas or conclusions presented in the cited entity.</rdfs:comment>
        <rdfs:label xml:lang="en">qualifies</rdfs:label>
    </owl:ObjectProperty>
    


    <!-- http://purl.org/spar/cito/refutes -->

    <owl:ObjectProperty rdf:about="http://purl.org/spar/cito/refutes">
        <rdfs:subPropertyOf rdf:resource="http://purl.org/spar/cito/cites"/>
        <dc:description xml:lang="en">Example: We do not think that all their arguments in favour of their own and against the other strategies are equally convincing [X].</dc:description>
        <rdfs:comment xml:lang="en">The citing entity refutes statements, ideas or conclusions presented in the cited entity.</rdfs:comment>
        <rdfs:label xml:lang="en">refutes</rdfs:label>
    </owl:ObjectProperty>
    


    <!-- http://purl.org/spar/cito/repliesTo -->

    <owl:ObjectProperty rdf:about="http://purl.org/spar/cito/repliesTo">
        <rdfs:subPropertyOf rdf:resource="http://purl.org/spar/cito/cites"/>
        <dc:description xml:lang="en">Example: We will not investigate the issues of the approach proposed in [X] here, but rather we introduce yet another alternative.</dc:description>
        <rdfs:comment xml:lang="en">The citing entity replies to statements, ideas or criticisms presented in the cited entity.</rdfs:comment>
        <rdfs:label xml:lang="en">replies to</rdfs:label>
    </owl:ObjectProperty>
    


    <!-- http://purl.org/spar/cito/retracts -->

    <owl:ObjectProperty rdf:about="http://purl.org/spar/cito/retracts">
        <rdfs:subPropertyOf rdf:resource="http://purl.org/spar/cito/cites"/>
        <dc:description xml:lang="en">Example: We wrote that the Earth moves in [X]; we now retire such statement.</dc:description>
        <rdfs:comment xml:lang="en">The citing entity constitutes a formal retraction of the cited entity.</rdfs:comment>
        <rdfs:label xml:lang="en">retracts</rdfs:label>
    </owl:ObjectProperty>
    


    <!-- http://purl.org/spar/cito/reviews -->

    <owl:ObjectProperty rdf:about="http://purl.org/spar/cito/reviews">
        <rdfs:subPropertyOf rdf:resource="http://purl.org/spar/cito/cites"/>
        <dc:description xml:lang="en">Example: This paper discusses Toulmin&apos;s methodology in modelling argumentation [X], focussing on highlighting advantages and drawbacks of the application of such a methodology in the Social Web.</dc:description>
        <rdfs:comment xml:lang="en">The citing entity reviews statements, ideas or conclusions presented in the cited entity.</rdfs:comment>
        <rdfs:label xml:lang="en">reviews</rdfs:label>
    </owl:ObjectProperty>
    


    <!-- http://purl.org/spar/cito/ridicules -->

    <owl:ObjectProperty rdf:about="http://purl.org/spar/cito/ridicules">
        <rdfs:subPropertyOf rdf:resource="http://purl.org/spar/cito/cites"/>
        <dc:description xml:lang="en">Example: Galileo said that the Earth &quot;moves&quot; [X]; really? And where is it going?</dc:description>
        <rdfs:comment xml:lang="en">The citing entity ridicules the cited entity or aspects of its contents.</rdfs:comment>
        <rdfs:label xml:lang="en">ridicules</rdfs:label>
    </owl:ObjectProperty>
    


    <!-- http://purl.org/spar/cito/speculatesOn -->

    <owl:ObjectProperty rdf:about="http://purl.org/spar/cito/speculatesOn">
        <rdfs:subPropertyOf rdf:resource="http://purl.org/spar/cito/cites"/>
        <dc:description xml:lang="en">Example: We believe that if Galileo believed that Earth goes around the Sun [X], he also should believe that Moon goes around Earth.</dc:description>
        <rdfs:comment xml:lang="en">The citing entity speculates on something within or related to the cited entity, without firm evidence.</rdfs:comment>
        <rdfs:label xml:lang="en">speculates on</rdfs:label>
    </owl:ObjectProperty>
    


    <!-- http://purl.org/spar/cito/supports -->

    <owl:ObjectProperty rdf:about="http://purl.org/spar/cito/supports">
        <rdfs:subPropertyOf rdf:resource="http://purl.org/spar/cito/cites"/>
        <dc:description xml:lang="en">Example: We support Galileo&apos;s statement [X], that Earth moves.</dc:description>
        <rdfs:comment xml:lang="en">The citing entity provides intellectual or factual support for statements, ideas or conclusions presented in the cited entity.</rdfs:comment>
        <rdfs:label xml:lang="en">supports</rdfs:label>
    </owl:ObjectProperty>
    


    <!-- http://purl.org/spar/cito/updates -->

    <owl:ObjectProperty rdf:about="http://purl.org/spar/cito/updates">
        <rdfs:subPropertyOf rdf:resource="http://purl.org/spar/cito/cites"/>
        <dc:description xml:lang="en">Example: Earth moves, said Galileo [X]; in addition, we can say now it moves very fast.</dc:description>
        <rdfs:comment xml:lang="en">The citing entity updates statements, ideas, hypotheses or understanding presented in the cited entity.</rdfs:comment>
        <rdfs:label xml:lang="en">updates</rdfs:label>
    </owl:ObjectProperty>
    


    <!-- http://purl.org/spar/cito/usesConclusionsFrom -->

    <owl:ObjectProperty rdf:about="http://purl.org/spar/cito/usesConclusionsFrom">
        <rdfs:subPropertyOf rdf:resource="http://purl.org/spar/cito/cites"/>
        <dc:description xml:lang="en">Example: Building upon Galileo&apos;s findings [X], we discovered that all the planets move.</dc:description>
        <rdfs:comment xml:lang="en">The citing entity describes work that uses conclusions presented in the cited entity.</rdfs:comment>
        <rdfs:label xml:lang="en">uses conclusions from</rdfs:label>
    </owl:ObjectProperty>
    


    <!-- http://purl.org/spar/cito/usesDataFrom -->

    <owl:ObjectProperty rdf:about="http://purl.org/spar/cito/usesDataFrom">
        <rdfs:subPropertyOf rdf:resource="http://purl.org/spar/cito/cites"/>
        <dc:description xml:lang="en">Example: Using the information collected from our recent study [X], we can estimate that there are tens of millions of HTML forms with potentially useful deep-web content.</dc:description>
        <rdfs:comment xml:lang="en">The citing entity describes work that uses data presented in the cited entity.</rdfs:comment>
        <rdfs:label xml:lang="en">uses data from</rdfs:label>
    </owl:ObjectProperty>
    


    <!-- http://purl.org/spar/cito/usesMethodIn -->

    <owl:ObjectProperty rdf:about="http://purl.org/spar/cito/usesMethodIn">
        <rdfs:subPropertyOf rdf:resource="http://purl.org/spar/cito/cites"/>
        <dc:description xml:lang="en">Example: We follow [X] in using design patterns for testing.</dc:description>
        <rdfs:comment xml:lang="en">The citing entity describes work that uses a method detailed in the cited entity.</rdfs:comment>
        <rdfs:label xml:lang="en">uses method in</rdfs:label>
    </owl:ObjectProperty>
    


    <!-- http://schema.org/citation -->

    <owl:ObjectProperty rdf:about="http://schema.org/citation">
        <rdfs:subPropertyOf rdf:resource="http://purl.org/spar/cito/cites"/>
        <rdfs:comment xml:lang="en">This property is defined in schema.org and has been added here to align schema.org with CiTO. The object property schema:citation expresses similar semantics to cito:cites except for the explicit definition of domain and range classes, that are schema:CreativeWork according to schema.org. For that reason, it is here defined as a subproperty of cito:cites.</rdfs:comment>
        <rdfs:label>citation</rdfs:label>
    </owl:ObjectProperty>
    


    <!-- http://www.cidoc-crm.org/cidoc-crm/P106_is_composed_of -->

    <owl:ObjectProperty rdf:about="http://www.cidoc-crm.org/cidoc-crm/P106_is_composed_of">
        <owl:inverseOf rdf:resource="http://www.cidoc-crm.org/cidoc-crm/P106i_forms_part_of"/>
        <rdf:type rdf:resource="http://www.w3.org/2002/07/owl#TransitiveProperty"/>
        <rdfs:domain rdf:resource="http://www.cidoc-crm.org/cidoc-crm/E90_Symbolic_Object"/>
        <rdfs:range rdf:resource="http://www.cidoc-crm.org/cidoc-crm/E90_Symbolic_Object"/>
        <rdfs:comment xml:lang="en">Scope note:
This property associates an instance of E90 Symbolic Object with a part of it that is by itself an instance of E90 Symbolic Object, such as fragments of texts or clippings from an image.

Examples:
- This Scope note P106 (E33) is composed of fragments of texts (E33)
- &apos;recognizable&apos; P106 (E90) is composed of &apos;ecognizabl&apos; (E90)

In First Order Logic:
P106(x,y) ⊃ E90(x)
P106(x,y) ⊃ E90(y)</rdfs:comment>
        <rdfs:label xml:lang="en">P106 is composed of</rdfs:label>
        <skos:notation rdf:datatype="http://www.w3.org/2001/XMLSchema#string">P106</skos:notation>
    </owl:ObjectProperty>
    


    <!-- http://www.cidoc-crm.org/cidoc-crm/P106i_forms_part_of -->

    <owl:ObjectProperty rdf:about="http://www.cidoc-crm.org/cidoc-crm/P106i_forms_part_of">
        <rdf:type rdf:resource="http://www.w3.org/2002/07/owl#TransitiveProperty"/>
        <rdfs:domain rdf:resource="http://www.cidoc-crm.org/cidoc-crm/E90_Symbolic_Object"/>
        <rdfs:range rdf:resource="http://www.cidoc-crm.org/cidoc-crm/E90_Symbolic_Object"/>
        <rdfs:label xml:lang="en">P106 forms part of</rdfs:label>
        <skos:notation rdf:datatype="http://www.w3.org/2001/XMLSchema#string">P106i</skos:notation>
    </owl:ObjectProperty>
    


    <!-- http://www.cidoc-crm.org/cidoc-crm/P128_carries -->

    <owl:ObjectProperty rdf:about="http://www.cidoc-crm.org/cidoc-crm/P128_carries">
        <rdfs:subPropertyOf rdf:resource="http://www.cidoc-crm.org/cidoc-crm/P130_shows_features_of"/>
        <owl:inverseOf rdf:resource="http://www.cidoc-crm.org/cidoc-crm/P128i_is_carried_by"/>
        <rdfs:domain rdf:resource="http://www.cidoc-crm.org/cidoc-crm/E24_Physical_Man-Made_Thing"/>
        <rdfs:range rdf:resource="http://www.cidoc-crm.org/cidoc-crm/E90_Symbolic_Object"/>
        <rdfs:comment xml:lang="en">Scope note:
This property identifies an E90 Symbolic Object carried by an instance of E18 Physical Thing.


Examples:
- Matthew&apos;s paperback copy of Reach for the Sky (E84) carries the text of Reach for the Sky (E73)

In First Order Logic:
P128(x,y) ⊃ E18(x)
P128(x,y) ⊃ E90(y)
P128(x,y) ⊃ P130(x,y)</rdfs:comment>
        <rdfs:label xml:lang="en">P128 carries</rdfs:label>
        <skos:notation rdf:datatype="http://www.w3.org/2001/XMLSchema#string">P128</skos:notation>
    </owl:ObjectProperty>
    


    <!-- http://www.cidoc-crm.org/cidoc-crm/P128i_is_carried_by -->

    <owl:ObjectProperty rdf:about="http://www.cidoc-crm.org/cidoc-crm/P128i_is_carried_by">
        <rdfs:subPropertyOf rdf:resource="http://www.cidoc-crm.org/cidoc-crm/P130i_features_are_also_found_on"/>
        <rdfs:domain rdf:resource="http://www.cidoc-crm.org/cidoc-crm/E90_Symbolic_Object"/>
        <rdfs:range rdf:resource="http://www.cidoc-crm.org/cidoc-crm/E24_Physical_Man-Made_Thing"/>
        <rdfs:label xml:lang="en">P128 is carried by</rdfs:label>
        <skos:notation rdf:datatype="http://www.w3.org/2001/XMLSchema#string">P128i</skos:notation>
    </owl:ObjectProperty>
    


    <!-- http://www.cidoc-crm.org/cidoc-crm/P130_shows_features_of -->

    <owl:ObjectProperty rdf:about="http://www.cidoc-crm.org/cidoc-crm/P130_shows_features_of">
        <owl:inverseOf rdf:resource="http://www.cidoc-crm.org/cidoc-crm/P130i_features_are_also_found_on"/>
        <rdfs:domain rdf:resource="http://www.cidoc-crm.org/cidoc-crm/E70_Thing"/>
        <rdfs:range rdf:resource="http://www.cidoc-crm.org/cidoc-crm/E70_Thing"/>
        <rdfs:comment xml:lang="en">Scope note:
This property generalises the notions of &quot;copy of&quot; and &quot;similar to&quot; into a dynamic, asymmetric relationship, where the domain expresses the derivative, if such a direction can be established.
Otherwise, the relationship is symmetric. It is a shortcut of P15 was influenced by (influenced) in a creation or production, if such a reason for the similarity can be verified. Moreover it expresses similarity in cases that can be stated between two objects only, without historical knowledge about its reasons.

Examples:
- the Parthenon Frieze on the Acropolis in Athens (E22) shows features of the Original Parthenon Frieze in the British museum (E22). Kind of similarity: Copy (E55)

In First Order Logic:
P130 (x,y) ⊃ E70(x)
P130 (x,y) ⊃ E70(y)
P130(x,y,z) ⊃ [P130(x,y) ∧ E55(z)]
P130(x,y) ⊃ P130(y,x)

Properties: P130.1 kind of similarity: E55 Type</rdfs:comment>
        <rdfs:label xml:lang="en">P130 shows features of</rdfs:label>
        <skos:notation rdf:datatype="http://www.w3.org/2001/XMLSchema#string">P130</skos:notation>
    </owl:ObjectProperty>
    


    <!-- http://www.cidoc-crm.org/cidoc-crm/P130i_features_are_also_found_on -->

    <owl:ObjectProperty rdf:about="http://www.cidoc-crm.org/cidoc-crm/P130i_features_are_also_found_on">
        <rdfs:domain rdf:resource="http://www.cidoc-crm.org/cidoc-crm/E70_Thing"/>
        <rdfs:range rdf:resource="http://www.cidoc-crm.org/cidoc-crm/E70_Thing"/>
        <rdfs:label xml:lang="en">P130 features are also found on</rdfs:label>
        <skos:notation rdf:datatype="http://www.w3.org/2001/XMLSchema#string">P130i</skos:notation>
    </owl:ObjectProperty>
    


    <!-- http://www.cidoc-crm.org/cidoc-crm/P2_has_type -->

    <owl:ObjectProperty rdf:about="http://www.cidoc-crm.org/cidoc-crm/P2_has_type">
        <owl:inverseOf rdf:resource="http://www.cidoc-crm.org/cidoc-crm/P2i_is_type_of"/>
        <rdfs:range rdf:resource="http://www.cidoc-crm.org/cidoc-crm/E55_Type"/>
        <rdfs:comment xml:lang="en">Scope note:
This property allows sub typing of CRM entities - a form of specialisation – through the use of a terminological hierarchy, or thesaurus.

The CRM is intended to focus on the high-level entities and relationships needed to describe data structures. Consequently, it does not specialise entities any further than is required for this immediate purpose. However, entities in the isA hierarchy of the CRM may by specialised into any number of sub entities, which can be defined in the E55 Type hierarchy. E51 Contact Point, for example, may be specialised into &quot;e-mail address&quot;, &quot;telephone number&quot;, &quot;post office box&quot;, &quot;URL&quot; etc. none of which figures explicitly in the CRM hierarchy. Sub typing obviously requires consistency between the meaning of the terms assigned and the more general intent of the CRM entity in question.

Examples:
- &quot;enquiries@cidoc-crm.org&quot; (E51) has type e-mail address (E55)

In First Order Logic:
P2(x,y) ⊃ E1(x)
P2(x,y) ⊃ E55(y)</rdfs:comment>
        <rdfs:label xml:lang="en">P2 has type</rdfs:label>
        <skos:notation rdf:datatype="http://www.w3.org/2001/XMLSchema#string">P2</skos:notation>
    </owl:ObjectProperty>
    


    <!-- http://www.cidoc-crm.org/cidoc-crm/P2i_is_type_of -->

    <owl:ObjectProperty rdf:about="http://www.cidoc-crm.org/cidoc-crm/P2i_is_type_of">
        <rdfs:domain rdf:resource="http://www.cidoc-crm.org/cidoc-crm/E55_Type"/>
        <rdfs:label xml:lang="en">P2 is type of</rdfs:label>
        <skos:notation rdf:datatype="http://www.w3.org/2001/XMLSchema#string">P2i</skos:notation>
    </owl:ObjectProperty>
    


    <!-- http://www.cidoc-crm.org/cidoc-crm/P67_refers_to -->

    <owl:ObjectProperty rdf:about="http://www.cidoc-crm.org/cidoc-crm/P67_refers_to">
        <owl:inverseOf rdf:resource="http://www.cidoc-crm.org/cidoc-crm/P67i_is_referred_to_by"/>
        <rdfs:domain rdf:resource="http://www.cidoc-crm.org/cidoc-crm/E89_Propositional_Object"/>
        <rdfs:comment xml:lang="en">Scope note:
This property documents that an E89 Propositional Object makes a statement about an instance of E1 CRM Entity. P67 refers to (is referred to by) has the P67.1 has type link to an instance of E55 Type. This is intended to allow a more detailed description of the type of reference. This differs from P129 is about (is subject of), which describes the primary subject or subjects of the E89 Propositional Object.

Examples:
- the eBay auction listing for 4 July 2002 (E73) refers to silver cup 232 (E22) has type item for sale (E55)

In First Order Logic:
P67(x,y) ⊃ E89(x)
P67(x,y) ⊃ E1(y)
P67(x,y,z) ⊃ [P67(x,y) ∧ E55(z)]

Properties: P67.1 has type: E55 Type</rdfs:comment>
        <rdfs:label xml:lang="en">P67 refers to</rdfs:label>
        <skos:notation rdf:datatype="http://www.w3.org/2001/XMLSchema#string">P67</skos:notation>
    </owl:ObjectProperty>
    


    <!-- http://www.cidoc-crm.org/cidoc-crm/P67i_is_referred_to_by -->

    <owl:ObjectProperty rdf:about="http://www.cidoc-crm.org/cidoc-crm/P67i_is_referred_to_by">
        <rdfs:range rdf:resource="http://www.cidoc-crm.org/cidoc-crm/E89_Propositional_Object"/>
        <rdfs:label xml:lang="en">P67 is referred to by</rdfs:label>
        <skos:notation rdf:datatype="http://www.w3.org/2001/XMLSchema#string">P67i</skos:notation>
    </owl:ObjectProperty>
    


    <!-- http://www.essepuntato.it/2008/12/pattern#contains -->

    <owl:ObjectProperty rdf:about="http://www.essepuntato.it/2008/12/pattern#contains"/>
    


    <!-- http://www.essepuntato.it/2008/12/pattern#isContainedBy -->

    <owl:ObjectProperty rdf:about="http://www.essepuntato.it/2008/12/pattern#isContainedBy"/>
    


    <!-- http://www.essepuntato.it/2008/12/pattern#isContainedByAsHeader -->

    <owl:ObjectProperty rdf:about="http://www.essepuntato.it/2008/12/pattern#isContainedByAsHeader"/>
    


    <!-- https://raw.githubusercontent.com/BOberreither/INTRO/master/INTRO_outdated.owl#actualizationFoundOn -->

    <owl:ObjectProperty rdf:about="https://raw.githubusercontent.com/BOberreither/INTRO/master/INTRO_outdated.owl#actualizationFoundOn">
        <rdfs:subPropertyOf rdf:resource="http://www.cidoc-crm.org/cidoc-crm/P130i_features_are_also_found_on"/>
        <owl:inverseOf rdf:resource="https://raw.githubusercontent.com/BOberreither/INTRO/master/INTRO_outdated.owl#showsActualization"/>
        <rdfs:comment>Links the actualization of a feature, a receptional entity, to the text that shows said feature.</rdfs:comment>
        <rdfs:label>actualization found on</rdfs:label>
    </owl:ObjectProperty>
    


    <!-- https://raw.githubusercontent.com/BOberreither/INTRO/master/INTRO_outdated.owl#actualizesFeature -->

    <owl:ObjectProperty rdf:about="https://raw.githubusercontent.com/BOberreither/INTRO/master/INTRO_outdated.owl#actualizesFeature">
        <rdfs:subPropertyOf rdf:resource="http://www.cidoc-crm.org/cidoc-crm/P130_shows_features_of"/>
        <owl:inverseOf rdf:resource="https://raw.githubusercontent.com/BOberreither/INTRO/master/INTRO_outdated.owl#featureActualizedIn"/>
        <rdfs:comment>Links the specific actualization of a feature to the (abstract concept of the) feature it actualizes.</rdfs:comment>
        <rdfs:label>actualizes feature</rdfs:label>
    </owl:ObjectProperty>
    


    <!-- https://raw.githubusercontent.com/BOberreither/INTRO/master/INTRO_outdated.owl#actualizesFormalFeature -->

    <owl:ObjectProperty rdf:about="https://raw.githubusercontent.com/BOberreither/INTRO/master/INTRO_outdated.owl#actualizesFormalFeature">
        <rdfs:subPropertyOf rdf:resource="https://raw.githubusercontent.com/BOberreither/INTRO/master/INTRO_outdated.owl#actualizesFeature"/>
        <owl:inverseOf rdf:resource="https://raw.githubusercontent.com/BOberreither/INTRO/master/INTRO_outdated.owl#formalFeatureActualizedIn"/>
    </owl:ObjectProperty>
    


    <!-- https://raw.githubusercontent.com/BOberreither/INTRO/master/INTRO_outdated.owl#actualizesRhetoricalFeature -->

    <owl:ObjectProperty rdf:about="https://raw.githubusercontent.com/BOberreither/INTRO/master/INTRO_outdated.owl#actualizesRhetoricalFeature">
        <rdfs:subPropertyOf rdf:resource="https://raw.githubusercontent.com/BOberreither/INTRO/master/INTRO_outdated.owl#actualizesFeature"/>
        <owl:inverseOf rdf:resource="https://raw.githubusercontent.com/BOberreither/INTRO/master/INTRO_outdated.owl#rhetoricalFeatureActualizedIn"/>
    </owl:ObjectProperty>
    


    <!-- https://raw.githubusercontent.com/BOberreither/INTRO/master/INTRO_outdated.owl#actualizesSemanticFeature -->

    <owl:ObjectProperty rdf:about="https://raw.githubusercontent.com/BOberreither/INTRO/master/INTRO_outdated.owl#actualizesSemanticFeature">
        <rdfs:subPropertyOf rdf:resource="https://raw.githubusercontent.com/BOberreither/INTRO/master/INTRO_outdated.owl#actualizesFeature"/>
        <owl:inverseOf rdf:resource="https://raw.githubusercontent.com/BOberreither/INTRO/master/INTRO_outdated.owl#semanticFeatureActualizedIn"/>
    </owl:ObjectProperty>
    


    <!-- https://raw.githubusercontent.com/BOberreither/INTRO/master/INTRO_outdated.owl#affiliationSupportedBy -->

    <owl:ObjectProperty rdf:about="https://raw.githubusercontent.com/BOberreither/INTRO/master/INTRO_outdated.owl#affiliationSupportedBy">
        <owl:inverseOf rdf:resource="https://raw.githubusercontent.com/BOberreither/INTRO/master/INTRO_outdated.owl#supportsAffiliationTo"/>
        <rdfs:comment>Links a transtextual entity to a characteristic that, found on a text, is a reason to consider the text an element of the transtextual entity. For example: The appearance of a ghost is a reason to consider a text a representative of the &apos;Gothic novel&apos;.</rdfs:comment>
        <rdfs:label>affiliation supported by</rdfs:label>
    </owl:ObjectProperty>
    


    <!-- https://raw.githubusercontent.com/BOberreither/INTRO/master/INTRO_outdated.owl#characteristicShownBy -->

    <owl:ObjectProperty rdf:about="https://raw.githubusercontent.com/BOberreither/INTRO/master/INTRO_outdated.owl#characteristicShownBy">
        <rdfs:subPropertyOf rdf:resource="http://www.cidoc-crm.org/cidoc-crm/P130i_features_are_also_found_on"/>
        <owl:inverseOf rdf:resource="https://raw.githubusercontent.com/BOberreither/INTRO/master/INTRO_outdated.owl#showsCharacteristics"/>
        <rdfs:comment>Links a characteristic to the text (on any ontologic level) that shows it.</rdfs:comment>
        <rdfs:label>characteristics shown by</rdfs:label>
    </owl:ObjectProperty>
    


    <!-- https://raw.githubusercontent.com/BOberreither/INTRO/master/INTRO_outdated.owl#comprisesFragmentCarriersOf -->

    <owl:ObjectProperty rdf:about="https://raw.githubusercontent.com/BOberreither/INTRO/master/INTRO_outdated.owl#comprisesFragmentCarriersOf">
        <rdfs:subPropertyOf rdf:resource="http://www.cidoc-crm.org/cidoc-crm/P128_carries"/>
        <owl:inverseOf rdf:resource="https://raw.githubusercontent.com/BOberreither/INTRO/master/INTRO_outdated.owl#fragmentCarriersProvidedBy"/>
        <rdfs:domain rdf:resource="https://raw.githubusercontent.com/BOberreither/INTRO/master/INTRO_outdated.owl#ManifestationProductTypeFragment"/>
        <rdfs:range rdf:resource="http://iflastandards.info/ns/fr/frbr/frbroo/F23_Expression_Fragment"/>
    </owl:ObjectProperty>
    


    <!-- https://raw.githubusercontent.com/BOberreither/INTRO/master/INTRO_outdated.owl#consistsIn -->

    <owl:ObjectProperty rdf:about="https://raw.githubusercontent.com/BOberreither/INTRO/master/INTRO_outdated.owl#consistsIn">
        <owl:inverseOf rdf:resource="https://raw.githubusercontent.com/BOberreither/INTRO/master/INTRO_outdated.owl#constitutes"/>
        <rdfs:comment>Links a Characteristic of a text to the Actualization of a certain Feature in order to state that the Feature is &apos;characteristic&apos;, meaning: it affiliates the text with a Transtextual Entity.
Also used to link an Interpretament to the Actualization of a certain feature, in this case: of the semantic feature &apos;Interpretation&apos;.</rdfs:comment>
        <rdfs:label>consists in</rdfs:label>
    </owl:ObjectProperty>
    


    <!-- https://raw.githubusercontent.com/BOberreither/INTRO/master/INTRO_outdated.owl#constellates -->

    <owl:ObjectProperty rdf:about="https://raw.githubusercontent.com/BOberreither/INTRO/master/INTRO_outdated.owl#constellates">
        <owl:inverseOf rdf:resource="https://raw.githubusercontent.com/BOberreither/INTRO/master/INTRO_outdated.owl#isConstellatedBy"/>
        <rdfs:comment>Links a constellation to the elements (actualized features) that together form that constellation.</rdfs:comment>
        <rdfs:label>constellates</rdfs:label>
    </owl:ObjectProperty>
    


    <!-- https://raw.githubusercontent.com/BOberreither/INTRO/master/INTRO_outdated.owl#constitutes -->

    <owl:ObjectProperty rdf:about="https://raw.githubusercontent.com/BOberreither/INTRO/master/INTRO_outdated.owl#constitutes">
        <rdfs:comment>States that a feature as actualized in a specific text can be seen as a characteristic and thus affiliating the text with a Transtextual Entity.
Also used to state that the actualization of the semantic feature &apos;interpretation&apos; can be seen as an &apos;interpretament&apos; and thus identify references, characteristics and so on.</rdfs:comment>
        <rdfs:label>constitutes</rdfs:label>
    </owl:ObjectProperty>
    


    <!-- https://raw.githubusercontent.com/BOberreither/INTRO/master/INTRO_outdated.owl#definitionProvidedBy -->

    <owl:ObjectProperty rdf:about="https://raw.githubusercontent.com/BOberreither/INTRO/master/INTRO_outdated.owl#definitionProvidedBy">
        <owl:inverseOf rdf:resource="https://raw.githubusercontent.com/BOberreither/INTRO/master/INTRO_outdated.owl#providesDefinitionFor"/>
        <rdfs:comment>Relates a type of intertextual relationship or a receptional, transtextual and supratextual entity to the actualization of a feature (usually: of the semantic feature &apos;definition&apos;) in order to link a definition - e.g. in Foucault&apos;s writings - to the concept it defines - e.g. &apos;discourse&apos;.</rdfs:comment>
        <rdfs:label>definition provided by</rdfs:label>
    </owl:ObjectProperty>
    


    <!-- https://raw.githubusercontent.com/BOberreither/INTRO/master/INTRO_outdated.owl#discusses -->

    <owl:ObjectProperty rdf:about="https://raw.githubusercontent.com/BOberreither/INTRO/master/INTRO_outdated.owl#discusses">
        <rdfs:subPropertyOf rdf:resource="http://www.cidoc-crm.org/cidoc-crm/P67_refers_to"/>
        <owl:inverseOf rdf:resource="https://raw.githubusercontent.com/BOberreither/INTRO/master/INTRO_outdated.owl#isDiscussedIn"/>
        <rdfs:comment>Links an interpretament to the textual instance (on any ontological level) it discusses.</rdfs:comment>
    </owl:ObjectProperty>
    


    <!-- https://raw.githubusercontent.com/BOberreither/INTRO/master/INTRO_outdated.owl#featureActualizedIn -->

    <owl:ObjectProperty rdf:about="https://raw.githubusercontent.com/BOberreither/INTRO/master/INTRO_outdated.owl#featureActualizedIn">
        <rdfs:subPropertyOf rdf:resource="http://www.cidoc-crm.org/cidoc-crm/P130i_features_are_also_found_on"/>
        <rdfs:comment>Links the receptional entity, the feature, to an actualization that is itself linked to a specific text.</rdfs:comment>
        <rdfs:label>feature actualized in</rdfs:label>
    </owl:ObjectProperty>
    


    <!-- https://raw.githubusercontent.com/BOberreither/INTRO/master/INTRO_outdated.owl#formalFeatureActualizedIn -->

    <owl:ObjectProperty rdf:about="https://raw.githubusercontent.com/BOberreither/INTRO/master/INTRO_outdated.owl#formalFeatureActualizedIn">
        <rdfs:subPropertyOf rdf:resource="https://raw.githubusercontent.com/BOberreither/INTRO/master/INTRO_outdated.owl#featureActualizedIn"/>
    </owl:ObjectProperty>
    


    <!-- https://raw.githubusercontent.com/BOberreither/INTRO/master/INTRO_outdated.owl#fragmentCarriersProvidedBy -->

    <owl:ObjectProperty rdf:about="https://raw.githubusercontent.com/BOberreither/INTRO/master/INTRO_outdated.owl#fragmentCarriersProvidedBy">
        <rdfs:subPropertyOf rdf:resource="http://www.cidoc-crm.org/cidoc-crm/P128i_is_carried_by"/>
        <rdfs:domain rdf:resource="http://iflastandards.info/ns/fr/frbr/frbroo/F23_Expression_Fragment"/>
        <rdfs:range rdf:resource="https://raw.githubusercontent.com/BOberreither/INTRO/master/INTRO_outdated.owl#ManifestationProductTypeFragment"/>
    </owl:ObjectProperty>
    


    <!-- https://raw.githubusercontent.com/BOberreither/INTRO/master/INTRO_outdated.owl#hasAppurtenantElement -->

    <owl:ObjectProperty rdf:about="https://raw.githubusercontent.com/BOberreither/INTRO/master/INTRO_outdated.owl#hasAppurtenantElement">
        <rdfs:subPropertyOf rdf:resource="http://www.w3.org/2002/07/owl#topObjectProperty"/>
        <owl:inverseOf rdf:resource="https://raw.githubusercontent.com/BOberreither/INTRO/master/INTRO_outdated.owl#isAppurtenantElement"/>
        <rdfs:comment>Links a transtextual entity to a text (on any ontological level) that is an element of the transtextual entity.</rdfs:comment>
        <rdfs:label>has appurtenant element</rdfs:label>
    </owl:ObjectProperty>
    


    <!-- https://raw.githubusercontent.com/BOberreither/INTRO/master/INTRO_outdated.owl#hasInitialElement -->

    <owl:ObjectProperty rdf:about="https://raw.githubusercontent.com/BOberreither/INTRO/master/INTRO_outdated.owl#hasInitialElement">
        <rdfs:subPropertyOf rdf:resource="https://raw.githubusercontent.com/BOberreither/INTRO/master/INTRO_outdated.owl#hasAppurtenantElement"/>
        <owl:inverseOf rdf:resource="https://raw.githubusercontent.com/BOberreither/INTRO/master/INTRO_outdated.owl#isInitialElement"/>
    </owl:ObjectProperty>
    


    <!-- https://raw.githubusercontent.com/BOberreither/INTRO/master/INTRO_outdated.owl#hasOpinionObject -->

    <owl:ObjectProperty rdf:about="https://raw.githubusercontent.com/BOberreither/INTRO/master/INTRO_outdated.owl#hasOpinionObject">
        <owl:inverseOf rdf:resource="https://raw.githubusercontent.com/BOberreither/INTRO/master/INTRO_outdated.owl#isOpinionObjectOf"/>
        <rdfs:comment>Links an opinion with its object - for example an opinion with the theme fashion (to make it an opinion about fashion).</rdfs:comment>
        <rdfs:label>has opinion object</rdfs:label>
    </owl:ObjectProperty>
    


    <!-- https://raw.githubusercontent.com/BOberreither/INTRO/master/INTRO_outdated.owl#hasPrecedingInterpretament -->

    <owl:ObjectProperty rdf:about="https://raw.githubusercontent.com/BOberreither/INTRO/master/INTRO_outdated.owl#hasPrecedingInterpretament">
        <owl:inverseOf rdf:resource="https://raw.githubusercontent.com/BOberreither/INTRO/master/INTRO_outdated.owl#hasSubsequentInterpretament"/>
        <rdfs:comment>Links two interpretamets who have a linear, logical or chronological order.</rdfs:comment>
        <rdfs:label>has preceding interpretament</rdfs:label>
    </owl:ObjectProperty>
    


    <!-- https://raw.githubusercontent.com/BOberreither/INTRO/master/INTRO_outdated.owl#hasProductTypeFragment -->

    <owl:ObjectProperty rdf:about="https://raw.githubusercontent.com/BOberreither/INTRO/master/INTRO_outdated.owl#hasProductTypeFragment">
        <rdfs:subPropertyOf rdf:resource="http://www.w3.org/2002/07/owl#topObjectProperty"/>
        <owl:inverseOf rdf:resource="https://raw.githubusercontent.com/BOberreither/INTRO/master/INTRO_outdated.owl#isProductTypeFragmentOf"/>
        <rdfs:domain rdf:resource="http://iflastandards.info/ns/fr/frbr/frbroo/F3_Manifestation_Product_Type"/>
        <rdfs:range rdf:resource="https://raw.githubusercontent.com/BOberreither/INTRO/master/INTRO_outdated.owl#ManifestationProductTypeFragment"/>
        <rdfs:comment>Links a product type to its fragments, e.g. the book with the ISBN 978-0307278630 to a passage on page three of this book.</rdfs:comment>
        <rdfs:label>has product type fragment</rdfs:label>
    </owl:ObjectProperty>
    


    <!-- https://raw.githubusercontent.com/BOberreither/INTRO/master/INTRO_outdated.owl#hasProductTypeFragmentFragment -->

    <owl:ObjectProperty rdf:about="https://raw.githubusercontent.com/BOberreither/INTRO/master/INTRO_outdated.owl#hasProductTypeFragmentFragment">
        <owl:inverseOf rdf:resource="https://raw.githubusercontent.com/BOberreither/INTRO/master/INTRO_outdated.owl#isProductTypeFragmentFragmentOf"/>
        <rdfs:label>has productTypefragment-fragment</rdfs:label>
    </owl:ObjectProperty>
    


    <!-- https://raw.githubusercontent.com/BOberreither/INTRO/master/INTRO_outdated.owl#hasReferredToEntity -->

    <owl:ObjectProperty rdf:about="https://raw.githubusercontent.com/BOberreither/INTRO/master/INTRO_outdated.owl#hasReferredToEntity">
        <owl:inverseOf rdf:resource="https://raw.githubusercontent.com/BOberreither/INTRO/master/INTRO_outdated.owl#isReferredToEntity"/>
        <rdfs:comment>Links a reference to a referred to entity (a text on any ontological level).</rdfs:comment>
        <rdfs:label>has referred to entity</rdfs:label>
        <skos:closeMatch>cito:hasCitedEntity</skos:closeMatch>
    </owl:ObjectProperty>
    


    <!-- https://raw.githubusercontent.com/BOberreither/INTRO/master/INTRO_outdated.owl#hasReferringEntity -->

    <owl:ObjectProperty rdf:about="https://raw.githubusercontent.com/BOberreither/INTRO/master/INTRO_outdated.owl#hasReferringEntity">
        <owl:inverseOf rdf:resource="https://raw.githubusercontent.com/BOberreither/INTRO/master/INTRO_outdated.owl#isReferringEntity"/>
        <rdfs:comment>Links a reference to a referring entity (a text on any ontological level).</rdfs:comment>
        <rdfs:label>has referring entity</rdfs:label>
        <skos:closeMatch>cito:hasCitingEntity</skos:closeMatch>
    </owl:ObjectProperty>
    


    <!-- https://raw.githubusercontent.com/BOberreither/INTRO/master/INTRO_outdated.owl#hasRepresentativeElement -->

    <owl:ObjectProperty rdf:about="https://raw.githubusercontent.com/BOberreither/INTRO/master/INTRO_outdated.owl#hasRepresentativeElement">
        <rdfs:subPropertyOf rdf:resource="https://raw.githubusercontent.com/BOberreither/INTRO/master/INTRO_outdated.owl#hasAppurtenantElement"/>
        <owl:inverseOf rdf:resource="https://raw.githubusercontent.com/BOberreither/INTRO/master/INTRO_outdated.owl#isRepresentativeElement"/>
    </owl:ObjectProperty>
    


    <!-- https://raw.githubusercontent.com/BOberreither/INTRO/master/INTRO_outdated.owl#hasSubsequentInterpretament -->

    <owl:ObjectProperty rdf:about="https://raw.githubusercontent.com/BOberreither/INTRO/master/INTRO_outdated.owl#hasSubsequentInterpretament">
        <rdfs:comment>Links two interpretamets who have a linear, logical or chronological order.</rdfs:comment>
        <rdfs:label>has subsequent interpretament</rdfs:label>
    </owl:ObjectProperty>
    


    <!-- https://raw.githubusercontent.com/BOberreither/INTRO/master/INTRO_outdated.owl#hasType -->

    <owl:ObjectProperty rdf:about="https://raw.githubusercontent.com/BOberreither/INTRO/master/INTRO_outdated.owl#hasType">
        <rdfs:subPropertyOf rdf:resource="http://www.cidoc-crm.org/cidoc-crm/P2_has_type"/>
        <owl:inverseOf rdf:resource="https://raw.githubusercontent.com/BOberreither/INTRO/master/INTRO_outdated.owl#isTypeOf"/>
        <rdfs:comment>Links a reference to its type of intertextual relationship.</rdfs:comment>
    </owl:ObjectProperty>
    


    <!-- https://raw.githubusercontent.com/BOberreither/INTRO/master/INTRO_outdated.owl#holdsInterpretament -->

    <owl:ObjectProperty rdf:about="https://raw.githubusercontent.com/BOberreither/INTRO/master/INTRO_outdated.owl#holdsInterpretament">
        <rdfs:subPropertyOf rdf:resource="http://www.cidoc-crm.org/cidoc-crm/P130_shows_features_of"/>
        <owl:inverseOf rdf:resource="https://raw.githubusercontent.com/BOberreither/INTRO/master/INTRO_outdated.owl#interpretamentOriginatingIn"/>
        <rdfs:comment>Links a text to the interpretament - i.e. to the specific mental act of which the text holds the written form.</rdfs:comment>
        <rdfs:label>holds interpretament</rdfs:label>
    </owl:ObjectProperty>
    


    <!-- https://raw.githubusercontent.com/BOberreither/INTRO/master/INTRO_outdated.owl#identifies -->

    <owl:ObjectProperty rdf:about="https://raw.githubusercontent.com/BOberreither/INTRO/master/INTRO_outdated.owl#identifies">
        <rdfs:subPropertyOf rdf:resource="http://www.cidoc-crm.org/cidoc-crm/P67_refers_to"/>
        <owl:inverseOf rdf:resource="https://raw.githubusercontent.com/BOberreither/INTRO/master/INTRO_outdated.owl#isIdentifiedBy"/>
        <rdfs:comment>Links an interpretament to the characteristic, the reference or the actualization of a feature it identifies.</rdfs:comment>
        <rdfs:label>identifies</rdfs:label>
    </owl:ObjectProperty>
    


    <!-- https://raw.githubusercontent.com/BOberreither/INTRO/master/INTRO_outdated.owl#interpretamentOriginatingIn -->

    <owl:ObjectProperty rdf:about="https://raw.githubusercontent.com/BOberreither/INTRO/master/INTRO_outdated.owl#interpretamentOriginatingIn">
        <rdfs:subPropertyOf rdf:resource="http://www.cidoc-crm.org/cidoc-crm/P130i_features_are_also_found_on"/>
        <rdfs:comment>Links an interpretament to the text that holds its written form.</rdfs:comment>
        <rdfs:label>interpretament originating in</rdfs:label>
    </owl:ObjectProperty>
    


    <!-- https://raw.githubusercontent.com/BOberreither/INTRO/master/INTRO_outdated.owl#isAppurtenantElement -->

    <owl:ObjectProperty rdf:about="https://raw.githubusercontent.com/BOberreither/INTRO/master/INTRO_outdated.owl#isAppurtenantElement">
        <rdfs:subPropertyOf rdf:resource="http://www.w3.org/2002/07/owl#topObjectProperty"/>
        <rdfs:comment>Links a text (on any ontological level) to a transtextual entity that it is an element of.</rdfs:comment>
        <rdfs:label>is appurtenant element</rdfs:label>
    </owl:ObjectProperty>
    


    <!-- https://raw.githubusercontent.com/BOberreither/INTRO/master/INTRO_outdated.owl#isConstellatedBy -->

    <owl:ObjectProperty rdf:about="https://raw.githubusercontent.com/BOberreither/INTRO/master/INTRO_outdated.owl#isConstellatedBy">
        <rdfs:comment>Links the actualizations of at least two receptional entities with the constellation they form (i.e. stating that they do so).</rdfs:comment>
        <rdfs:label>is constellated by</rdfs:label>
    </owl:ObjectProperty>
    


    <!-- https://raw.githubusercontent.com/BOberreither/INTRO/master/INTRO_outdated.owl#isDiscussedIn -->

    <owl:ObjectProperty rdf:about="https://raw.githubusercontent.com/BOberreither/INTRO/master/INTRO_outdated.owl#isDiscussedIn">
        <rdfs:subPropertyOf rdf:resource="http://www.cidoc-crm.org/cidoc-crm/P67i_is_referred_to_by"/>
        <rdfs:comment>Links a textual instance (on any ontological level) to the interpretament it is discussed in.</rdfs:comment>
        <rdfs:label>is discussed in</rdfs:label>
    </owl:ObjectProperty>
    


    <!-- https://raw.githubusercontent.com/BOberreither/INTRO/master/INTRO_outdated.owl#isIdentifiedBy -->

    <owl:ObjectProperty rdf:about="https://raw.githubusercontent.com/BOberreither/INTRO/master/INTRO_outdated.owl#isIdentifiedBy">
        <rdfs:subPropertyOf rdf:resource="http://www.cidoc-crm.org/cidoc-crm/P67i_is_referred_to_by"/>
        <rdfs:comment>Links a characteristic, a reference or an actualization of a feature to the interpretament it is identified in.</rdfs:comment>
        <rdfs:label>is identified by</rdfs:label>
    </owl:ObjectProperty>
    


    <!-- https://raw.githubusercontent.com/BOberreither/INTRO/master/INTRO_outdated.owl#isInitialElement -->

    <owl:ObjectProperty rdf:about="https://raw.githubusercontent.com/BOberreither/INTRO/master/INTRO_outdated.owl#isInitialElement">
        <rdfs:subPropertyOf rdf:resource="https://raw.githubusercontent.com/BOberreither/INTRO/master/INTRO_outdated.owl#isAppurtenantElement"/>
    </owl:ObjectProperty>
    


    <!-- https://raw.githubusercontent.com/BOberreither/INTRO/master/INTRO_outdated.owl#isOpinionObjectOf -->

    <owl:ObjectProperty rdf:about="https://raw.githubusercontent.com/BOberreither/INTRO/master/INTRO_outdated.owl#isOpinionObjectOf">
        <rdfs:label>is opinion object of</rdfs:label>
    </owl:ObjectProperty>
    


    <!-- https://raw.githubusercontent.com/BOberreither/INTRO/master/INTRO_outdated.owl#isProductTypeFragmentFragmentOf -->

    <owl:ObjectProperty rdf:about="https://raw.githubusercontent.com/BOberreither/INTRO/master/INTRO_outdated.owl#isProductTypeFragmentFragmentOf">
        <rdfs:label>is productTypeFragment-fragment of</rdfs:label>
    </owl:ObjectProperty>
    


    <!-- https://raw.githubusercontent.com/BOberreither/INTRO/master/INTRO_outdated.owl#isProductTypeFragmentOf -->

    <owl:ObjectProperty rdf:about="https://raw.githubusercontent.com/BOberreither/INTRO/master/INTRO_outdated.owl#isProductTypeFragmentOf">
        <rdfs:subPropertyOf rdf:resource="http://www.w3.org/2002/07/owl#topObjectProperty"/>
        <rdfs:domain rdf:resource="https://raw.githubusercontent.com/BOberreither/INTRO/master/INTRO_outdated.owl#ManifestationProductTypeFragment"/>
        <rdfs:range rdf:resource="http://iflastandards.info/ns/fr/frbr/frbroo/F3_Manifestation_Product_Type"/>
        <rdfs:comment>Links a manifestation product type fragment to its manifestation product type, e.g. a passage on page three of the book with the ISBN 978-0307278630 to this book.</rdfs:comment>
        <rdfs:label>is product type fragment of</rdfs:label>
    </owl:ObjectProperty>
    


    <!-- https://raw.githubusercontent.com/BOberreither/INTRO/master/INTRO_outdated.owl#isReferredToEntity -->

    <owl:ObjectProperty rdf:about="https://raw.githubusercontent.com/BOberreither/INTRO/master/INTRO_outdated.owl#isReferredToEntity">
        <rdfs:comment>Linksa referring entity - a text on any ontological level - to the reference it forms a necessary part of.</rdfs:comment>
        <rdfs:label>is referred to entity</rdfs:label>
    </owl:ObjectProperty>
    


    <!-- https://raw.githubusercontent.com/BOberreither/INTRO/master/INTRO_outdated.owl#isReferringEntity -->

    <owl:ObjectProperty rdf:about="https://raw.githubusercontent.com/BOberreither/INTRO/master/INTRO_outdated.owl#isReferringEntity">
        <rdfs:comment>Links a referred to entity - a text on any ontological level - to the reference it forms a necessary part of.</rdfs:comment>
        <rdfs:label>is referring entity</rdfs:label>
    </owl:ObjectProperty>
    


    <!-- https://raw.githubusercontent.com/BOberreither/INTRO/master/INTRO_outdated.owl#isRepresentativeElement -->

    <owl:ObjectProperty rdf:about="https://raw.githubusercontent.com/BOberreither/INTRO/master/INTRO_outdated.owl#isRepresentativeElement">
        <rdfs:subPropertyOf rdf:resource="https://raw.githubusercontent.com/BOberreither/INTRO/master/INTRO_outdated.owl#isAppurtenantElement"/>
    </owl:ObjectProperty>
    


    <!-- https://raw.githubusercontent.com/BOberreither/INTRO/master/INTRO_outdated.owl#isTypeOf -->

    <owl:ObjectProperty rdf:about="https://raw.githubusercontent.com/BOberreither/INTRO/master/INTRO_outdated.owl#isTypeOf">
        <rdfs:subPropertyOf rdf:resource="http://www.cidoc-crm.org/cidoc-crm/P2i_is_type_of"/>
        <rdfs:comment>Links a type of intertextual relationship to the reference of that type.</rdfs:comment>
    </owl:ObjectProperty>
    


    <!-- https://raw.githubusercontent.com/BOberreither/INTRO/master/INTRO_outdated.owl#likenessSupportedBy -->

    <owl:ObjectProperty rdf:about="https://raw.githubusercontent.com/BOberreither/INTRO/master/INTRO_outdated.owl#likenessSupportedBy">
        <owl:inverseOf rdf:resource="https://raw.githubusercontent.com/BOberreither/INTRO/master/INTRO_outdated.owl#supportsLikenessTo"/>
        <rdfs:comment>Links a Transtextual Entity to a Characteristic that, found on a text, establishes a likeness to the Transtextual Entity. For Example: The appearance of a ghost in a text establishes a likeness to the &apos;Gothic novel&apos;.</rdfs:comment>
        <rdfs:label>likeness supported by</rdfs:label>
    </owl:ObjectProperty>
    


    <!-- https://raw.githubusercontent.com/BOberreither/INTRO/master/INTRO_outdated.owl#nonAffiliationSupportedBy -->

    <owl:ObjectProperty rdf:about="https://raw.githubusercontent.com/BOberreither/INTRO/master/INTRO_outdated.owl#nonAffiliationSupportedBy">
        <owl:inverseOf rdf:resource="https://raw.githubusercontent.com/BOberreither/INTRO/master/INTRO_outdated.owl#supportsNonAffiliationTo"/>
        <rdfs:comment>Links a Transtextual Entity to a Characteristic that, found on a text, is a reason to consider the text not an element of the Transtextual Entity. For Example: The appearance of a teenage vampire could be a reason to consider a text not a representative of a &apos;Bildungsroman&apos;.</rdfs:comment>
        <rdfs:label>non-affiliation supported by</rdfs:label>
    </owl:ObjectProperty>
    


    <!-- https://raw.githubusercontent.com/BOberreither/INTRO/master/INTRO_outdated.owl#othernessSupportedBy -->

    <owl:ObjectProperty rdf:about="https://raw.githubusercontent.com/BOberreither/INTRO/master/INTRO_outdated.owl#othernessSupportedBy">
        <owl:inverseOf rdf:resource="https://raw.githubusercontent.com/BOberreither/INTRO/master/INTRO_outdated.owl#supportsOthernessTo"/>
        <rdfs:comment>Links a Transtextual Entity to a Characteristic that, found on a text, establishes an unlikeness to the Transtextual Entity. For Example: The appearance of a ghost in a text establishes an unlikeness to the genre &apos;detective fiction&apos;.</rdfs:comment>
        <rdfs:label>otherness supported by</rdfs:label>
    </owl:ObjectProperty>
    


    <!-- https://raw.githubusercontent.com/BOberreither/INTRO/master/INTRO_outdated.owl#providesDefinitionFor -->

    <owl:ObjectProperty rdf:about="https://raw.githubusercontent.com/BOberreither/INTRO/master/INTRO_outdated.owl#providesDefinitionFor">
        <rdfs:comment>Relates the actualization (usually: of the semantic feature &apos;definition&apos;) to a type of intertextual relationship and to receptional, transtextual and supratextual entities and thereby links a concept - e.g. &apos;discourse&apos; - to a definition - e.g. in Foucault&apos;s writings.</rdfs:comment>
        <rdfs:label>provides definition for</rdfs:label>
    </owl:ObjectProperty>
    


    <!-- https://raw.githubusercontent.com/BOberreither/INTRO/master/INTRO_outdated.owl#providesSimilarityForReference -->

    <owl:ObjectProperty rdf:about="https://raw.githubusercontent.com/BOberreither/INTRO/master/INTRO_outdated.owl#providesSimilarityForReference">
        <owl:inverseOf rdf:resource="https://raw.githubusercontent.com/BOberreither/INTRO/master/INTRO_outdated.owl#referenceIsBasedOnSimilarity"/>
        <rdfs:comment>Links a receptional entity to a reference it provides the similarity for, the similarity being necessary for the detection of the reference. States that a reference is based on a similarity, i.e. the occurrence of the same receptional entity in two different texts.</rdfs:comment>
        <rdfs:label>provides similarity for reference</rdfs:label>
    </owl:ObjectProperty>
    


    <!-- https://raw.githubusercontent.com/BOberreither/INTRO/master/INTRO_outdated.owl#providesSupportFor -->

    <owl:ObjectProperty rdf:about="https://raw.githubusercontent.com/BOberreither/INTRO/master/INTRO_outdated.owl#providesSupportFor">
        <owl:inverseOf rdf:resource="https://raw.githubusercontent.com/BOberreither/INTRO/master/INTRO_outdated.owl#supportProvidedBy"/>
        <rdfs:comment>Relates a source (a text on any ontological level) to the outcome of a receptional or interpretative act (a characteristic, an actualization of a feature, a receptional entity, a reference, an interpretament, an opinion) to support it.</rdfs:comment>
        <rdfs:label>provides support for</rdfs:label>
    </owl:ObjectProperty>
    


    <!-- https://raw.githubusercontent.com/BOberreither/INTRO/master/INTRO_outdated.owl#referenceIsBasedOnSimilarity -->

    <owl:ObjectProperty rdf:about="https://raw.githubusercontent.com/BOberreither/INTRO/master/INTRO_outdated.owl#referenceIsBasedOnSimilarity">
        <rdfs:comment>Links a reference to a receptional entity that provides the similarity necessary for the detection of the reference. States that a reference is based on a similarity, i.e. the occurrence of the same receptional entity in two different texts.</rdfs:comment>
        <rdfs:label>reference is based on similarity</rdfs:label>
    </owl:ObjectProperty>
    


    <!-- https://raw.githubusercontent.com/BOberreither/INTRO/master/INTRO_outdated.owl#rhetoricalFeatureActualizedIn -->

    <owl:ObjectProperty rdf:about="https://raw.githubusercontent.com/BOberreither/INTRO/master/INTRO_outdated.owl#rhetoricalFeatureActualizedIn">
        <rdfs:subPropertyOf rdf:resource="https://raw.githubusercontent.com/BOberreither/INTRO/master/INTRO_outdated.owl#featureActualizedIn"/>
    </owl:ObjectProperty>
    


    <!-- https://raw.githubusercontent.com/BOberreither/INTRO/master/INTRO_outdated.owl#semanticFeatureActualizedIn -->

    <owl:ObjectProperty rdf:about="https://raw.githubusercontent.com/BOberreither/INTRO/master/INTRO_outdated.owl#semanticFeatureActualizedIn">
        <rdfs:subPropertyOf rdf:resource="https://raw.githubusercontent.com/BOberreither/INTRO/master/INTRO_outdated.owl#featureActualizedIn"/>
    </owl:ObjectProperty>
    


    <!-- https://raw.githubusercontent.com/BOberreither/INTRO/master/INTRO_outdated.owl#showsActualization -->

    <owl:ObjectProperty rdf:about="https://raw.githubusercontent.com/BOberreither/INTRO/master/INTRO_outdated.owl#showsActualization">
        <rdfs:subPropertyOf rdf:resource="http://www.cidoc-crm.org/cidoc-crm/P130_shows_features_of"/>
        <rdfs:comment>Links a text to the actualization of a feature found on said text.</rdfs:comment>
        <rdfs:label>shows actualization</rdfs:label>
    </owl:ObjectProperty>
    


    <!-- https://raw.githubusercontent.com/BOberreither/INTRO/master/INTRO_outdated.owl#showsCharacteristics -->

    <owl:ObjectProperty rdf:about="https://raw.githubusercontent.com/BOberreither/INTRO/master/INTRO_outdated.owl#showsCharacteristics">
        <rdfs:subPropertyOf rdf:resource="http://www.cidoc-crm.org/cidoc-crm/P130_shows_features_of"/>
        <rdfs:comment>Links a text to the characteristic it holds.</rdfs:comment>
        <rdfs:label>shows characteristic</rdfs:label>
    </owl:ObjectProperty>
    


    <!-- https://raw.githubusercontent.com/BOberreither/INTRO/master/INTRO_outdated.owl#supportProvidedBy -->

    <owl:ObjectProperty rdf:about="https://raw.githubusercontent.com/BOberreither/INTRO/master/INTRO_outdated.owl#supportProvidedBy">
        <rdfs:comment>Relates the decision made in any receptional or interpretative act - the determination of a Characteristic, an Actualization of a Feature, any Receptional Entity, any Reference - to a source that can support this decision (on any ontological level, ranging from &apos;Transtextual Entity&apos; to &apos;Manifestation Product Type Fragment&apos;).</rdfs:comment>
        <rdfs:label>support provided by</rdfs:label>
        <skos:closeMatch rdf:datatype="http://www.w3.org/2001/XMLSchema#string">CiTO:obtainsSupportFrom</skos:closeMatch>
    </owl:ObjectProperty>
    


    <!-- https://raw.githubusercontent.com/BOberreither/INTRO/master/INTRO_outdated.owl#supportsAffiliationTo -->

    <owl:ObjectProperty rdf:about="https://raw.githubusercontent.com/BOberreither/INTRO/master/INTRO_outdated.owl#supportsAffiliationTo">
        <rdfs:comment>Links to a transtextual entity a characteristic that, if found on a text, is a reason to consider the text an element of the transtextual entity. For example: The appearance of a ghost is a reason to consider a text a representative of the &apos;Gothic novel&apos;.</rdfs:comment>
        <rdfs:label>supports affiliation to</rdfs:label>
    </owl:ObjectProperty>
    


    <!-- https://raw.githubusercontent.com/BOberreither/INTRO/master/INTRO_outdated.owl#supportsLikenessTo -->

    <owl:ObjectProperty rdf:about="https://raw.githubusercontent.com/BOberreither/INTRO/master/INTRO_outdated.owl#supportsLikenessTo">
        <rdfs:comment>Links to a transtextual entity a Characteristic that, found on a text, establishes a likeness to the Transtextual Entity. For example: The appearance of a ghost in a text establishes a likeness to the &apos;Gothic novel&apos;.</rdfs:comment>
        <rdfs:label>supports likeness to</rdfs:label>
    </owl:ObjectProperty>
    


    <!-- https://raw.githubusercontent.com/BOberreither/INTRO/master/INTRO_outdated.owl#supportsNonAffiliationTo -->

    <owl:ObjectProperty rdf:about="https://raw.githubusercontent.com/BOberreither/INTRO/master/INTRO_outdated.owl#supportsNonAffiliationTo">
        <rdfs:comment>Links to a transtextual entity a characteristic that, found on a text, is a reason to consider the text not an element of the transtextual Entity. For example: The appearance of a ghost is a reason not to consider a text a representative of the genre &apos;crime fiction&apos;.</rdfs:comment>
        <rdfs:label>supports non-affiliation to</rdfs:label>
    </owl:ObjectProperty>
    


    <!-- https://raw.githubusercontent.com/BOberreither/INTRO/master/INTRO_outdated.owl#supportsOthernessTo -->

    <owl:ObjectProperty rdf:about="https://raw.githubusercontent.com/BOberreither/INTRO/master/INTRO_outdated.owl#supportsOthernessTo">
        <rdfs:comment>Links to a transtextual entity a characteristic that, found on a text, establishes an unlikeness to the transtextual entity. For example: The appearance of a ghost in a text establishes an unlikeness to the genre &apos;detective fiction&apos;.</rdfs:comment>
        <rdfs:label>supports Otherness to</rdfs:label>
    </owl:ObjectProperty>
    


    <!-- 
    ///////////////////////////////////////////////////////////////////////////////////////
    //
    // Data properties
    //
    ///////////////////////////////////////////////////////////////////////////////////////
     -->

    


    <!-- https://raw.githubusercontent.com/BOberreither/INTRO/master/INTRO_outdated.owl#hasBibliographicalData -->

    <owl:DatatypeProperty rdf:about="https://raw.githubusercontent.com/BOberreither/INTRO/master/INTRO_outdated.owl#hasBibliographicalData">
        <rdfs:range rdf:resource="http://www.w3.org/2001/XMLSchema#string"/>
    </owl:DatatypeProperty>
    


    <!-- https://raw.githubusercontent.com/BOberreither/INTRO/master/INTRO_outdated.owl#hasLocation -->

    <owl:DatatypeProperty rdf:about="https://raw.githubusercontent.com/BOberreither/INTRO/master/INTRO_outdated.owl#hasLocation">
        <rdfs:subPropertyOf rdf:resource="http://www.w3.org/2002/07/owl#topDataProperty"/>
        <rdfs:range rdf:resource="http://www.w3.org/2001/XMLSchema#string"/>
    </owl:DatatypeProperty>
    


    <!-- https://raw.githubusercontent.com/BOberreither/INTRO/master/INTRO_outdated.owl#hasParaphraseOrDefinition -->

    <owl:DatatypeProperty rdf:about="https://raw.githubusercontent.com/BOberreither/INTRO/master/INTRO_outdated.owl#hasParaphraseOrDefinition"/>
    


    <!-- https://raw.githubusercontent.com/BOberreither/INTRO/master/INTRO_outdated.owl#hasSpecification -->

    <owl:DatatypeProperty rdf:about="https://raw.githubusercontent.com/BOberreither/INTRO/master/INTRO_outdated.owl#hasSpecification">
        <rdfs:range rdf:resource="http://www.w3.org/2001/XMLSchema#string"/>
    </owl:DatatypeProperty>
    


    <!-- https://raw.githubusercontent.com/BOberreither/INTRO/master/INTRO_outdated.owl#hasWording -->

    <owl:DatatypeProperty rdf:about="https://raw.githubusercontent.com/BOberreither/INTRO/master/INTRO_outdated.owl#hasWording">
        <rdfs:range rdf:resource="http://www.w3.org/2001/XMLSchema#string"/>
    </owl:DatatypeProperty>
    


    <!-- 
    ///////////////////////////////////////////////////////////////////////////////////////
    //
    // Classes
    //
    ///////////////////////////////////////////////////////////////////////////////////////
     -->

    


    <!-- http://iflastandards.info/ns/fr/frbr/frbroo/F1_Work -->

    <owl:Class rdf:about="http://iflastandards.info/ns/fr/frbr/frbroo/F1_Work">
        <rdfs:subClassOf rdf:resource="http://www.cidoc-crm.org/cidoc-crm/E89_Propositional_Object"/>
        <rdfs:subClassOf>
            <owl:Restriction>
                <owl:onProperty rdf:resource="https://raw.githubusercontent.com/BOberreither/INTRO/master/INTRO_outdated.owl#isAppurtenantElement"/>
                <owl:allValuesFrom rdf:resource="https://raw.githubusercontent.com/BOberreither/INTRO/master/INTRO_outdated.owl#ArchitextualEntity"/>
            </owl:Restriction>
        </rdfs:subClassOf>
        <rdfs:subClassOf>
            <owl:Restriction>
                <owl:onProperty rdf:resource="https://raw.githubusercontent.com/BOberreither/INTRO/master/INTRO_outdated.owl#isDiscussedIn"/>
                <owl:allValuesFrom rdf:resource="https://raw.githubusercontent.com/BOberreither/INTRO/master/INTRO_outdated.owl#Interpretament"/>
            </owl:Restriction>
        </rdfs:subClassOf>
        <rdfs:subClassOf>
            <owl:Restriction>
                <owl:onProperty rdf:resource="https://raw.githubusercontent.com/BOberreither/INTRO/master/INTRO_outdated.owl#isInitialElement"/>
                <owl:allValuesFrom rdf:resource="https://raw.githubusercontent.com/BOberreither/INTRO/master/INTRO_outdated.owl#ArchitextualEntity"/>
            </owl:Restriction>
        </rdfs:subClassOf>
        <rdfs:subClassOf>
            <owl:Restriction>
                <owl:onProperty rdf:resource="https://raw.githubusercontent.com/BOberreither/INTRO/master/INTRO_outdated.owl#isReferredToEntity"/>
                <owl:allValuesFrom rdf:resource="https://raw.githubusercontent.com/BOberreither/INTRO/master/INTRO_outdated.owl#Reference"/>
            </owl:Restriction>
        </rdfs:subClassOf>
        <rdfs:subClassOf>
            <owl:Restriction>
                <owl:onProperty rdf:resource="https://raw.githubusercontent.com/BOberreither/INTRO/master/INTRO_outdated.owl#isReferringEntity"/>
                <owl:allValuesFrom rdf:resource="https://raw.githubusercontent.com/BOberreither/INTRO/master/INTRO_outdated.owl#Reference"/>
            </owl:Restriction>
        </rdfs:subClassOf>
        <rdfs:subClassOf>
            <owl:Restriction>
                <owl:onProperty rdf:resource="https://raw.githubusercontent.com/BOberreither/INTRO/master/INTRO_outdated.owl#isRepresentativeElement"/>
                <owl:allValuesFrom rdf:resource="https://raw.githubusercontent.com/BOberreither/INTRO/master/INTRO_outdated.owl#ArchitextualEntity"/>
            </owl:Restriction>
        </rdfs:subClassOf>
        <rdfs:subClassOf>
            <owl:Restriction>
                <owl:onProperty rdf:resource="https://raw.githubusercontent.com/BOberreither/INTRO/master/INTRO_outdated.owl#providesSupportFor"/>
                <owl:allValuesFrom>
                    <owl:Class>
                        <owl:unionOf rdf:parseType="Collection">
                            <rdf:Description rdf:about="https://raw.githubusercontent.com/BOberreither/INTRO/master/INTRO_outdated.owl#ActualizationOfFeature"/>
                            <rdf:Description rdf:about="https://raw.githubusercontent.com/BOberreither/INTRO/master/INTRO_outdated.owl#Characteristic"/>
                            <rdf:Description rdf:about="https://raw.githubusercontent.com/BOberreither/INTRO/master/INTRO_outdated.owl#Interpretament"/>
                            <rdf:Description rdf:about="https://raw.githubusercontent.com/BOberreither/INTRO/master/INTRO_outdated.owl#Opinion"/>
                            <rdf:Description rdf:about="https://raw.githubusercontent.com/BOberreither/INTRO/master/INTRO_outdated.owl#Reference"/>
                            <rdf:Description rdf:about="https://raw.githubusercontent.com/BOberreither/INTRO/master/INTRO_outdated.owl#TypeOfIntertextualRelationship"/>
                        </owl:unionOf>
                    </owl:Class>
                </owl:allValuesFrom>
            </owl:Restriction>
        </rdfs:subClassOf>
        <rdfs:subClassOf>
            <owl:Restriction>
                <owl:onProperty rdf:resource="https://raw.githubusercontent.com/BOberreither/INTRO/master/INTRO_outdated.owl#showsActualization"/>
                <owl:allValuesFrom rdf:resource="https://raw.githubusercontent.com/BOberreither/INTRO/master/INTRO_outdated.owl#ActualizationOfFeature"/>
            </owl:Restriction>
        </rdfs:subClassOf>
        <rdfs:subClassOf>
            <owl:Restriction>
                <owl:onProperty rdf:resource="https://raw.githubusercontent.com/BOberreither/INTRO/master/INTRO_outdated.owl#showsCharacteristics"/>
                <owl:allValuesFrom rdf:resource="https://raw.githubusercontent.com/BOberreither/INTRO/master/INTRO_outdated.owl#Characteristic"/>
            </owl:Restriction>
        </rdfs:subClassOf>
        <rdfs:subClassOf>
            <owl:Restriction>
                <owl:onProperty rdf:resource="https://raw.githubusercontent.com/BOberreither/INTRO/master/INTRO_outdated.owl#hasBibliographicalData"/>
                <owl:someValuesFrom rdf:resource="http://www.w3.org/2001/XMLSchema#string"/>
            </owl:Restriction>
        </rdfs:subClassOf>
        <rdfs:comment xml:lang="en">This class comprises distinct concepts or combinations of concepts identified in artistic and intellectual expressions, such as poems, stories or musical compositions. Such concepts may appear in the course of the coherent evolution of an original idea into one or more expressions that are dominated by the original idea. A Work may be elaborated by one or more Actors simultaneously or over time. The substance of Work is ideas. A Work may have members that are works in their own right.
A Work can be either individual or complex. If it is individual its concept is completely realised in a single F22 Self-Contained Expression. If it is complex its concept is embedded in an F15 Complex Work. An F15 Complex Work consists of alternative members that are either F15 Complex Works themselves or F14 Individual Works.
A Work is the product of an intellectual process of one or more persons, yet only indirect evidence about it is at our hands. This can be contextual information such as the existence of an order for a work, reflections of the creators themselves that are documented somewhere, and finally the expressions of the work created. As ideas normally take shape during discussion, elaboration and implementation, it is not reasonable to assume that a work starts with a complete concept. In some cases, it can be very difficult or impossible to define the whole of the concept of a work at a particular time. The objective evidence for such a notion can only be based on a stage of expressions at a given time. In this sense, the sets of ideas that constitute  particular self-contained expressions may be regarded as a kind of “snap-shot” of a work.
A Work may include the concept of aggregating expressions of other works into a new expression. For instance, an anthology of poems is regarded as a work in its own right that makes use of expressions of the individual poems that have been selected and ordered as part of an intellectual process. This does not make the contents of the aggregated expressions part of this work, but only parts of the resulting expression.
</rdfs:comment>
        <rdfs:label xml:lang="en">Work</rdfs:label>
    </owl:Class>
    


    <!-- http://iflastandards.info/ns/fr/frbr/frbroo/F22_Self-Contained_Expression -->

    <owl:Class rdf:about="http://iflastandards.info/ns/fr/frbr/frbroo/F22_Self-Contained_Expression">
        <rdfs:subClassOf rdf:resource="http://iflastandards.info/ns/fr/frbr/frbroo/F2_Expression"/>
        <rdfs:subClassOf>
            <owl:Restriction>
                <owl:onProperty rdf:resource="https://raw.githubusercontent.com/BOberreither/INTRO/master/INTRO_outdated.owl#isAppurtenantElement"/>
                <owl:allValuesFrom rdf:resource="https://raw.githubusercontent.com/BOberreither/INTRO/master/INTRO_outdated.owl#ArchitextualEntity"/>
            </owl:Restriction>
        </rdfs:subClassOf>
        <rdfs:subClassOf>
            <owl:Restriction>
                <owl:onProperty rdf:resource="https://raw.githubusercontent.com/BOberreither/INTRO/master/INTRO_outdated.owl#isReferredToEntity"/>
                <owl:allValuesFrom rdf:resource="https://raw.githubusercontent.com/BOberreither/INTRO/master/INTRO_outdated.owl#Reference"/>
            </owl:Restriction>
        </rdfs:subClassOf>
        <rdfs:subClassOf>
            <owl:Restriction>
                <owl:onProperty rdf:resource="https://raw.githubusercontent.com/BOberreither/INTRO/master/INTRO_outdated.owl#isReferringEntity"/>
                <owl:allValuesFrom rdf:resource="https://raw.githubusercontent.com/BOberreither/INTRO/master/INTRO_outdated.owl#Reference"/>
            </owl:Restriction>
        </rdfs:subClassOf>
        <rdfs:subClassOf>
            <owl:Restriction>
                <owl:onProperty rdf:resource="https://raw.githubusercontent.com/BOberreither/INTRO/master/INTRO_outdated.owl#showsActualization"/>
                <owl:allValuesFrom rdf:resource="https://raw.githubusercontent.com/BOberreither/INTRO/master/INTRO_outdated.owl#ActualizationOfFeature"/>
            </owl:Restriction>
        </rdfs:subClassOf>
        <rdfs:comment xml:lang="en">This class comprises the immaterial realisations of individual works at a particular time that are regarded as a complete whole. The quality of wholeness reflects the intention of its creator that this expression should convey the concept of the work. Such a whole can in turn be part of a larger whole.
Inherent to the notion of work is the completion of recognisable outcomes of the work. These outcomes, i.e. the Self-Contained Expressions, are regarded as the symbolic equivalents of Individual Works, which form the atoms of a complex work. A Self-Contained Expression may contain expressions or parts of expressions from other work, such as citations or items collected in anthologies. Even though they are incorporated in the Self-Contained Expression, they are not regarded as becoming members of the expressed container work by their inclusion in the expression, but are rather regarded as foreign or referred to elements.
F22 Self-Contained Expression can be distinguished from F23 Expression Fragment in that an F23 Expression Fragment was not intended by its creator to make sense by itself. Normally creators would characterise an outcome of a work as finished. In other cases, one could recognise an outcome of a work as complete from the elaboration or logical coherence of its content, or if there is any historical knowledge about the creator deliberately or accidentally never finishing (completing) that particular expression. In all those cases, one would regard an expression as self-contained.
</rdfs:comment>
        <rdfs:label xml:lang="en">Self-Contained Expression</rdfs:label>
    </owl:Class>
    


    <!-- http://iflastandards.info/ns/fr/frbr/frbroo/F23_Expression_Fragment -->

    <owl:Class rdf:about="http://iflastandards.info/ns/fr/frbr/frbroo/F23_Expression_Fragment">
        <rdfs:subClassOf rdf:resource="http://iflastandards.info/ns/fr/frbr/frbroo/F2_Expression"/>
        <rdfs:subClassOf>
            <owl:Restriction>
                <owl:onProperty rdf:resource="https://raw.githubusercontent.com/BOberreither/INTRO/master/INTRO_outdated.owl#fragmentCarriersProvidedBy"/>
                <owl:allValuesFrom rdf:resource="https://raw.githubusercontent.com/BOberreither/INTRO/master/INTRO_outdated.owl#ManifestationProductTypeFragment"/>
            </owl:Restriction>
        </rdfs:subClassOf>
        <rdfs:subClassOf>
            <owl:Restriction>
                <owl:onProperty rdf:resource="https://raw.githubusercontent.com/BOberreither/INTRO/master/INTRO_outdated.owl#isAppurtenantElement"/>
                <owl:allValuesFrom rdf:resource="https://raw.githubusercontent.com/BOberreither/INTRO/master/INTRO_outdated.owl#ArchitextualEntity"/>
            </owl:Restriction>
        </rdfs:subClassOf>
        <rdfs:subClassOf>
            <owl:Restriction>
                <owl:onProperty rdf:resource="https://raw.githubusercontent.com/BOberreither/INTRO/master/INTRO_outdated.owl#isReferredToEntity"/>
                <owl:allValuesFrom rdf:resource="https://raw.githubusercontent.com/BOberreither/INTRO/master/INTRO_outdated.owl#Reference"/>
            </owl:Restriction>
        </rdfs:subClassOf>
        <rdfs:subClassOf>
            <owl:Restriction>
                <owl:onProperty rdf:resource="https://raw.githubusercontent.com/BOberreither/INTRO/master/INTRO_outdated.owl#isReferringEntity"/>
                <owl:allValuesFrom rdf:resource="https://raw.githubusercontent.com/BOberreither/INTRO/master/INTRO_outdated.owl#Reference"/>
            </owl:Restriction>
        </rdfs:subClassOf>
        <rdfs:subClassOf>
            <owl:Restriction>
                <owl:onProperty rdf:resource="https://raw.githubusercontent.com/BOberreither/INTRO/master/INTRO_outdated.owl#showsActualization"/>
                <owl:allValuesFrom rdf:resource="https://raw.githubusercontent.com/BOberreither/INTRO/master/INTRO_outdated.owl#ActualizationOfFeature"/>
            </owl:Restriction>
        </rdfs:subClassOf>
        <rdfs:comment xml:lang="en">This class comprises parts of Expressions and these parts are not Self-Contained Expressions themselves.
The existence of an instance of F23 Expression Fragment can be due to accident, such as loss of material over time, e.g. the only remaining manuscript of an antique text being partially eaten by worms, or due to deliberate isolation, such as excerpts taken from a text by the compiler of a collection of excerpts.
An F23 Expression Fragment is only identified with respect to its occurrence in a known or assumed whole. The size of an instance of F23 Expression Fragment ranges from more than 99% of an instance of F22 Self-Contained Expression to tiny bits (a few words from a text, one bar from a musical composition, one detail from a still image, a two-second clip from a movie, etc.).
</rdfs:comment>
        <rdfs:label xml:lang="en">Expression Fragment</rdfs:label>
    </owl:Class>
    


    <!-- http://iflastandards.info/ns/fr/frbr/frbroo/F2_Expression -->

    <owl:Class rdf:about="http://iflastandards.info/ns/fr/frbr/frbroo/F2_Expression">
        <rdfs:subClassOf rdf:resource="http://www.cidoc-crm.org/cidoc-crm/E73_Information_Object"/>
        <rdfs:subClassOf>
            <owl:Restriction>
                <owl:onProperty rdf:resource="https://raw.githubusercontent.com/BOberreither/INTRO/master/INTRO_outdated.owl#isAppurtenantElement"/>
                <owl:allValuesFrom rdf:resource="https://raw.githubusercontent.com/BOberreither/INTRO/master/INTRO_outdated.owl#ArchitextualEntity"/>
            </owl:Restriction>
        </rdfs:subClassOf>
        <rdfs:subClassOf>
            <owl:Restriction>
                <owl:onProperty rdf:resource="https://raw.githubusercontent.com/BOberreither/INTRO/master/INTRO_outdated.owl#isDiscussedIn"/>
                <owl:allValuesFrom rdf:resource="https://raw.githubusercontent.com/BOberreither/INTRO/master/INTRO_outdated.owl#Interpretament"/>
            </owl:Restriction>
        </rdfs:subClassOf>
        <rdfs:subClassOf>
            <owl:Restriction>
                <owl:onProperty rdf:resource="https://raw.githubusercontent.com/BOberreither/INTRO/master/INTRO_outdated.owl#isInitialElement"/>
                <owl:allValuesFrom rdf:resource="https://raw.githubusercontent.com/BOberreither/INTRO/master/INTRO_outdated.owl#ArchitextualEntity"/>
            </owl:Restriction>
        </rdfs:subClassOf>
        <rdfs:subClassOf>
            <owl:Restriction>
                <owl:onProperty rdf:resource="https://raw.githubusercontent.com/BOberreither/INTRO/master/INTRO_outdated.owl#isReferredToEntity"/>
                <owl:allValuesFrom rdf:resource="https://raw.githubusercontent.com/BOberreither/INTRO/master/INTRO_outdated.owl#Reference"/>
            </owl:Restriction>
        </rdfs:subClassOf>
        <rdfs:subClassOf>
            <owl:Restriction>
                <owl:onProperty rdf:resource="https://raw.githubusercontent.com/BOberreither/INTRO/master/INTRO_outdated.owl#isReferringEntity"/>
                <owl:allValuesFrom rdf:resource="https://raw.githubusercontent.com/BOberreither/INTRO/master/INTRO_outdated.owl#Reference"/>
            </owl:Restriction>
        </rdfs:subClassOf>
        <rdfs:subClassOf>
            <owl:Restriction>
                <owl:onProperty rdf:resource="https://raw.githubusercontent.com/BOberreither/INTRO/master/INTRO_outdated.owl#isRepresentativeElement"/>
                <owl:allValuesFrom rdf:resource="https://raw.githubusercontent.com/BOberreither/INTRO/master/INTRO_outdated.owl#ArchitextualEntity"/>
            </owl:Restriction>
        </rdfs:subClassOf>
        <rdfs:subClassOf>
            <owl:Restriction>
                <owl:onProperty rdf:resource="https://raw.githubusercontent.com/BOberreither/INTRO/master/INTRO_outdated.owl#providesSupportFor"/>
                <owl:allValuesFrom>
                    <owl:Class>
                        <owl:unionOf rdf:parseType="Collection">
                            <rdf:Description rdf:about="https://raw.githubusercontent.com/BOberreither/INTRO/master/INTRO_outdated.owl#ActualizationOfFeature"/>
                            <rdf:Description rdf:about="https://raw.githubusercontent.com/BOberreither/INTRO/master/INTRO_outdated.owl#Characteristic"/>
                            <rdf:Description rdf:about="https://raw.githubusercontent.com/BOberreither/INTRO/master/INTRO_outdated.owl#Interpretament"/>
                            <rdf:Description rdf:about="https://raw.githubusercontent.com/BOberreither/INTRO/master/INTRO_outdated.owl#Opinion"/>
                            <rdf:Description rdf:about="https://raw.githubusercontent.com/BOberreither/INTRO/master/INTRO_outdated.owl#Reference"/>
                            <rdf:Description rdf:about="https://raw.githubusercontent.com/BOberreither/INTRO/master/INTRO_outdated.owl#TypeOfIntertextualRelationship"/>
                        </owl:unionOf>
                    </owl:Class>
                </owl:allValuesFrom>
            </owl:Restriction>
        </rdfs:subClassOf>
        <rdfs:subClassOf>
            <owl:Restriction>
                <owl:onProperty rdf:resource="https://raw.githubusercontent.com/BOberreither/INTRO/master/INTRO_outdated.owl#showsActualization"/>
                <owl:allValuesFrom rdf:resource="https://raw.githubusercontent.com/BOberreither/INTRO/master/INTRO_outdated.owl#ActualizationOfFeature"/>
            </owl:Restriction>
        </rdfs:subClassOf>
        <rdfs:subClassOf>
            <owl:Restriction>
                <owl:onProperty rdf:resource="https://raw.githubusercontent.com/BOberreither/INTRO/master/INTRO_outdated.owl#showsCharacteristics"/>
                <owl:allValuesFrom rdf:resource="https://raw.githubusercontent.com/BOberreither/INTRO/master/INTRO_outdated.owl#Characteristic"/>
            </owl:Restriction>
        </rdfs:subClassOf>
        <rdfs:subClassOf>
            <owl:Restriction>
                <owl:onProperty rdf:resource="https://raw.githubusercontent.com/BOberreither/INTRO/master/INTRO_outdated.owl#hasBibliographicalData"/>
                <owl:someValuesFrom rdf:resource="http://www.w3.org/2001/XMLSchema#string"/>
            </owl:Restriction>
        </rdfs:subClassOf>
        <rdfs:comment xml:lang="en">This class comprises the intellectual or artistic realisations of works in the form of identifiable immaterial objects, such as texts, poems, jokes, musical or choreographic notations, movement pattern, sound pattern, images, multimedia objects, or any combination of such forms that have objectively recognisable structures. The substance of F2 Expression is signs.
Expressions cannot exist without a physical carrier, but do not depend on a specific physical carrier and can exist on one or more carriers simultaneously. Carriers may include human memory.
Inasmuch as the form of F2 Expression is an inherent characteristic of the F2 Expression, any change in form (e.g., from alpha-numeric notation to spoken word, a poem created in capitals and rendered in lower case) is a new F2 Expression. Similarly, changes in the intellectual conventions or instruments that are employed to express a work (e.g., translation from one language to another) result in the creation of a new F2 Expression. Thus, if a text is revised or modified, the resulting F2 Expression is considered to be a new F2 Expression. Minor changes, such as corrections of spelling and punctuation, etc., are normally considered variations within the same F2 Expression. On a practical level, the degree to which distinctions are made between variant expressions of a work will depend to some extent on the nature of the F1 Work itself, and on the anticipated needs of users.
The genre of the work may provide an indication of which features are essential to the expression. In some cases, aspects of physical form, such as typeface and page layout, are not integral to the intellectual or artistic realisation of the work as such, and therefore are not distinctive criteria for the respective expressions. For another work, features such as layout may be essential. For instance, the author or a graphic designer may wrap a poem around an image.
An expression of a work may include expressions of other works within it. For instance, an anthology of poems is regarded as a work in its own right that makes use of expressions of the individual poems that have been selected and ordered as part of an intellectual process. This does not make the contents of the aggregated expressions part of this work, but only parts of the resulting expression.
If an instance of F2 Expression is of a specific form, such as text, image, etc., it may be simultaneously instantiated in the specific classes representing these forms in CIDOC CRM. Thereby one can make use of the more specific properties of these classes, such as language (which is applicable to instances of E33 Linguistic Object only).
</rdfs:comment>
        <rdfs:label xml:lang="en">Expression</rdfs:label>
    </owl:Class>
    


    <!-- http://iflastandards.info/ns/fr/frbr/frbroo/F3_Manifestation_Product_Type -->

    <owl:Class rdf:about="http://iflastandards.info/ns/fr/frbr/frbroo/F3_Manifestation_Product_Type">
        <rdfs:subClassOf rdf:resource="http://www.cidoc-crm.org/cidoc-crm/E55_Type"/>
        <rdfs:subClassOf rdf:resource="http://www.cidoc-crm.org/cidoc-crm/E72_Legal_Object"/>
        <rdfs:subClassOf>
            <owl:Restriction>
                <owl:onProperty rdf:resource="https://raw.githubusercontent.com/BOberreither/INTRO/master/INTRO_outdated.owl#hasProductTypeFragment"/>
                <owl:allValuesFrom rdf:resource="https://raw.githubusercontent.com/BOberreither/INTRO/master/INTRO_outdated.owl#ManifestationProductTypeFragment"/>
            </owl:Restriction>
        </rdfs:subClassOf>
        <rdfs:subClassOf>
            <owl:Restriction>
                <owl:onProperty rdf:resource="https://raw.githubusercontent.com/BOberreither/INTRO/master/INTRO_outdated.owl#isAppurtenantElement"/>
                <owl:allValuesFrom rdf:resource="https://raw.githubusercontent.com/BOberreither/INTRO/master/INTRO_outdated.owl#ArchitextualEntity"/>
            </owl:Restriction>
        </rdfs:subClassOf>
        <rdfs:subClassOf>
            <owl:Restriction>
                <owl:onProperty rdf:resource="https://raw.githubusercontent.com/BOberreither/INTRO/master/INTRO_outdated.owl#isDiscussedIn"/>
                <owl:allValuesFrom rdf:resource="https://raw.githubusercontent.com/BOberreither/INTRO/master/INTRO_outdated.owl#Interpretament"/>
            </owl:Restriction>
        </rdfs:subClassOf>
        <rdfs:subClassOf>
            <owl:Restriction>
                <owl:onProperty rdf:resource="https://raw.githubusercontent.com/BOberreither/INTRO/master/INTRO_outdated.owl#isInitialElement"/>
                <owl:allValuesFrom rdf:resource="https://raw.githubusercontent.com/BOberreither/INTRO/master/INTRO_outdated.owl#ArchitextualEntity"/>
            </owl:Restriction>
        </rdfs:subClassOf>
        <rdfs:subClassOf>
            <owl:Restriction>
                <owl:onProperty rdf:resource="https://raw.githubusercontent.com/BOberreither/INTRO/master/INTRO_outdated.owl#isReferredToEntity"/>
                <owl:allValuesFrom rdf:resource="https://raw.githubusercontent.com/BOberreither/INTRO/master/INTRO_outdated.owl#Reference"/>
            </owl:Restriction>
        </rdfs:subClassOf>
        <rdfs:subClassOf>
            <owl:Restriction>
                <owl:onProperty rdf:resource="https://raw.githubusercontent.com/BOberreither/INTRO/master/INTRO_outdated.owl#isReferringEntity"/>
                <owl:allValuesFrom rdf:resource="https://raw.githubusercontent.com/BOberreither/INTRO/master/INTRO_outdated.owl#Reference"/>
            </owl:Restriction>
        </rdfs:subClassOf>
        <rdfs:subClassOf>
            <owl:Restriction>
                <owl:onProperty rdf:resource="https://raw.githubusercontent.com/BOberreither/INTRO/master/INTRO_outdated.owl#isRepresentativeElement"/>
                <owl:allValuesFrom rdf:resource="https://raw.githubusercontent.com/BOberreither/INTRO/master/INTRO_outdated.owl#ArchitextualEntity"/>
            </owl:Restriction>
        </rdfs:subClassOf>
        <rdfs:subClassOf>
            <owl:Restriction>
                <owl:onProperty rdf:resource="https://raw.githubusercontent.com/BOberreither/INTRO/master/INTRO_outdated.owl#providesSupportFor"/>
                <owl:allValuesFrom>
                    <owl:Class>
                        <owl:unionOf rdf:parseType="Collection">
                            <rdf:Description rdf:about="https://raw.githubusercontent.com/BOberreither/INTRO/master/INTRO_outdated.owl#ActualizationOfFeature"/>
                            <rdf:Description rdf:about="https://raw.githubusercontent.com/BOberreither/INTRO/master/INTRO_outdated.owl#Characteristic"/>
                            <rdf:Description rdf:about="https://raw.githubusercontent.com/BOberreither/INTRO/master/INTRO_outdated.owl#Interpretament"/>
                            <rdf:Description rdf:about="https://raw.githubusercontent.com/BOberreither/INTRO/master/INTRO_outdated.owl#Opinion"/>
                            <rdf:Description rdf:about="https://raw.githubusercontent.com/BOberreither/INTRO/master/INTRO_outdated.owl#Reference"/>
                            <rdf:Description rdf:about="https://raw.githubusercontent.com/BOberreither/INTRO/master/INTRO_outdated.owl#TypeOfIntertextualRelationship"/>
                        </owl:unionOf>
                    </owl:Class>
                </owl:allValuesFrom>
            </owl:Restriction>
        </rdfs:subClassOf>
        <rdfs:subClassOf>
            <owl:Restriction>
                <owl:onProperty rdf:resource="https://raw.githubusercontent.com/BOberreither/INTRO/master/INTRO_outdated.owl#showsActualization"/>
                <owl:allValuesFrom rdf:resource="https://raw.githubusercontent.com/BOberreither/INTRO/master/INTRO_outdated.owl#ActualizationOfFeature"/>
            </owl:Restriction>
        </rdfs:subClassOf>
        <rdfs:subClassOf>
            <owl:Restriction>
                <owl:onProperty rdf:resource="https://raw.githubusercontent.com/BOberreither/INTRO/master/INTRO_outdated.owl#showsCharacteristics"/>
                <owl:allValuesFrom rdf:resource="https://raw.githubusercontent.com/BOberreither/INTRO/master/INTRO_outdated.owl#Characteristic"/>
            </owl:Restriction>
        </rdfs:subClassOf>
        <rdfs:subClassOf>
            <owl:Restriction>
                <owl:onProperty rdf:resource="https://raw.githubusercontent.com/BOberreither/INTRO/master/INTRO_outdated.owl#hasBibliographicalData"/>
                <owl:someValuesFrom rdf:resource="http://www.w3.org/2001/XMLSchema#string"/>
            </owl:Restriction>
        </rdfs:subClassOf>
        <rdfs:comment xml:lang="en">This class comprises the definitions of publication products.
An instance of F3 Manifestation Product Type is the “species”, and all copies of a given object are “specimens” of it. An instance of F3 Manifestation Product Type defines all of the features or traits that instances of F5 Item normally display in order that they may be recognised as copies of a particular publication. However, due to production problems or subsequent events, one or more instances of F5 Item may not exhibit all these features or traits; yet such instances still retain their relationship to the same instance of F3 Manifestation Product Type.
The features that characterise a given instance of F3 Manifestation Product Type include: one instance of F24 Publication Expression, containing one or more than one instance of F2 Expression, reflecting the authors’ content of the manifestation and all additional input by the publisher; and the appropriate types of physical features for that form of the object. For example, hardcover and paperback are two distinct publications (i.e. two distinct instances of F3 Manifestation Product Type) even though authorial and editorial content are otherwise identical in both publications. The activity of cataloguing aims at the most accurate listing of features or traits of an instance of F3 Manifestation Product Type that are sufficient to distinguish it from another instance of F3 Manifestation Product Type.
</rdfs:comment>
        <rdfs:label xml:lang="en">Manifestation Product Type</rdfs:label>
    </owl:Class>
    


    <!-- http://purl.org/orb/1.0/Acknowledgements -->

    <owl:Class rdf:about="http://purl.org/orb/1.0/Acknowledgements">
        <owl:equivalentClass rdf:resource="http://purl.org/spar/deo/Acknowledgements"/>
        <rdfs:subClassOf rdf:resource="https://raw.githubusercontent.com/BOberreither/INTRO/master/INTRO_outdated.owl#PragmaticEntity"/>
    </owl:Class>
    


    <!-- http://purl.org/orb/1.0/Conclusion -->

    <owl:Class rdf:about="http://purl.org/orb/1.0/Conclusion">
        <owl:equivalentClass rdf:resource="http://purl.org/spar/deo/Conclusion"/>
        <rdfs:subClassOf rdf:resource="https://raw.githubusercontent.com/BOberreither/INTRO/master/INTRO_outdated.owl#PragmaticEntity"/>
    </owl:Class>
    


    <!-- http://purl.org/orb/1.0/Discussion -->

    <owl:Class rdf:about="http://purl.org/orb/1.0/Discussion">
        <owl:equivalentClass rdf:resource="http://purl.org/spar/deo/Discussion"/>
        <rdfs:subClassOf rdf:resource="https://raw.githubusercontent.com/BOberreither/INTRO/master/INTRO_outdated.owl#PragmaticEntity"/>
    </owl:Class>
    


    <!-- http://purl.org/orb/1.0/Header -->

    <owl:Class rdf:about="http://purl.org/orb/1.0/Header">
        <owl:equivalentClass rdf:resource="http://purl.org/spar/doco/FrontMatter"/>
        <rdfs:subClassOf rdf:resource="https://raw.githubusercontent.com/BOberreither/INTRO/master/INTRO_outdated.owl#PragmaticEntity"/>
    </owl:Class>
    


    <!-- http://purl.org/orb/1.0/Introduction -->

    <owl:Class rdf:about="http://purl.org/orb/1.0/Introduction">
        <owl:equivalentClass rdf:resource="http://purl.org/spar/deo/Introduction"/>
        <rdfs:subClassOf rdf:resource="https://raw.githubusercontent.com/BOberreither/INTRO/master/INTRO_outdated.owl#PragmaticEntity"/>
    </owl:Class>
    


    <!-- http://purl.org/orb/1.0/Methods -->

    <owl:Class rdf:about="http://purl.org/orb/1.0/Methods">
        <owl:equivalentClass rdf:resource="http://purl.org/spar/deo/Methods"/>
        <rdfs:subClassOf rdf:resource="https://raw.githubusercontent.com/BOberreither/INTRO/master/INTRO_outdated.owl#PragmaticEntity"/>
    </owl:Class>
    


    <!-- http://purl.org/orb/1.0/References -->

    <owl:Class rdf:about="http://purl.org/orb/1.0/References">
        <rdfs:subClassOf rdf:resource="https://raw.githubusercontent.com/BOberreither/INTRO/master/INTRO_outdated.owl#PragmaticEntity"/>
    </owl:Class>
    


    <!-- http://purl.org/orb/1.0/Results -->

    <owl:Class rdf:about="http://purl.org/orb/1.0/Results">
        <owl:equivalentClass rdf:resource="http://purl.org/spar/deo/Results"/>
        <rdfs:subClassOf rdf:resource="https://raw.githubusercontent.com/BOberreither/INTRO/master/INTRO_outdated.owl#PragmaticEntity"/>
    </owl:Class>
    


    <!-- http://purl.org/spar/deo/Acknowledgements -->

    <owl:Class rdf:about="http://purl.org/spar/deo/Acknowledgements">
        <rdfs:subClassOf rdf:resource="http://purl.org/spar/deo/DiscourseElement"/>
        <rdfs:comment xml:lang="en">Usually part of the preface, or a separate section in its own right, often as part of the back matter, it acknowledges those, including funding agencies, who contributed to the undertaking of a research project described in a publication, or to the creation of the work in some way. In scientific articles, the acknowledgements are usually placed as a separated section immediately following the Discussion or Conclusions.</rdfs:comment>
        <rdfs:label xml:lang="en">acknowledgements</rdfs:label>
    </owl:Class>
    


    <!-- http://purl.org/spar/deo/BibliographicReference -->

    <owl:Class rdf:about="http://purl.org/spar/deo/BibliographicReference">
        <rdfs:subClassOf rdf:resource="http://purl.org/orb/1.0/References"/>
        <rdfs:subClassOf rdf:resource="http://purl.org/spar/deo/Reference"/>
        <rdfs:comment xml:lang="en">A reference, usually contained in a footnote or a bibliographic reference list, that refer to another publication, such as a journal article, a book, a book chapter or a Web site. The inclusion of the bibliographic reference in a publication constitutes the performative act of bibliographic citation.</rdfs:comment>
        <rdfs:label xml:lang="en">bibliographic reference</rdfs:label>
    </owl:Class>
    


    <!-- http://purl.org/spar/deo/Biography -->

    <owl:Class rdf:about="http://purl.org/spar/deo/Biography">
        <rdfs:subClassOf rdf:resource="http://purl.org/spar/deo/DiscourseElement"/>
        <rdfs:comment xml:lang="en">Information describing a person and his or her life history and contributions.</rdfs:comment>
        <rdfs:label xml:lang="en">biography</rdfs:label>
    </owl:Class>
    


    <!-- http://purl.org/spar/deo/Caption -->

    <owl:Class rdf:about="http://purl.org/spar/deo/Caption">
        <rdfs:subClassOf rdf:resource="http://purl.org/spar/deo/DiscourseElement"/>
        <rdfs:comment xml:lang="en">Text accompanying another item, such as a picture.</rdfs:comment>
        <rdfs:label xml:lang="en">caption</rdfs:label>
    </owl:Class>
    


    <!-- http://purl.org/spar/deo/Conclusion -->

    <owl:Class rdf:about="http://purl.org/spar/deo/Conclusion">
        <owl:equivalentClass rdf:resource="http://salt.semanticauthoring.org/ontologies/sro#Conclusion"/>
        <rdfs:subClassOf rdf:resource="http://purl.org/spar/deo/DiscourseElement"/>
        <rdfs:comment>A reflection on the preceding text, summarizing the evidence, arguments or premises presented in the document and their logical outcomes. Conclusions are a fundamental feature in academic research publications, and may be included in the Discussion section.</rdfs:comment>
        <rdfs:label>conclusion</rdfs:label>
    </owl:Class>
    


    <!-- http://purl.org/spar/deo/Contribution -->

    <owl:Class rdf:about="http://purl.org/spar/deo/Contribution">
        <owl:equivalentClass rdf:resource="http://salt.semanticauthoring.org/ontologies/sro#Contribution"/>
        <rdfs:subClassOf rdf:resource="http://purl.org/spar/deo/DiscourseElement"/>
        <rdfs:comment>A description of the part that this publication plays in the overall field.</rdfs:comment>
        <rdfs:label>contribution</rdfs:label>
    </owl:Class>
    


    <!-- http://purl.org/spar/deo/Data -->

    <owl:Class rdf:about="http://purl.org/spar/deo/Data">
        <rdfs:subClassOf rdf:resource="http://purl.org/spar/deo/DiscourseElement"/>
        <rdfs:comment xml:lang="en">A textual description of data used or produced in the work which the document describes, or the data themselves.</rdfs:comment>
        <rdfs:label xml:lang="en">data</rdfs:label>
    </owl:Class>
    


    <!-- http://purl.org/spar/deo/Dedication -->

    <owl:Class rdf:about="http://purl.org/spar/deo/Dedication">
        <rdfs:subClassOf rdf:resource="http://purl.org/spar/deo/DiscourseElement"/>
        <rdfs:comment xml:lang="en">Text in which the author names the person or people for whom he/she has written the document, or to whose memory it is dedicated.</rdfs:comment>
        <rdfs:label xml:lang="en">dedication</rdfs:label>
    </owl:Class>
    


    <!-- http://purl.org/spar/deo/DiscourseElement -->

    <owl:Class rdf:about="http://purl.org/spar/deo/DiscourseElement">
        <rdfs:subClassOf rdf:resource="https://raw.githubusercontent.com/BOberreither/INTRO/master/INTRO_outdated.owl#PragmaticEntity"/>
    </owl:Class>
    


    <!-- http://purl.org/spar/deo/Discussion -->

    <owl:Class rdf:about="http://purl.org/spar/deo/Discussion">
        <owl:equivalentClass rdf:resource="http://salt.semanticauthoring.org/ontologies/sro#Discussion"/>
        <rdfs:subClassOf rdf:resource="http://purl.org/spar/deo/DiscourseElement"/>
        <rdfs:comment>An interpretation and discussion of the results obtained and an analysis of their significance, in support of conclusions. These conclusions may be part of this discussion or may be included in a separate section of the document.</rdfs:comment>
        <rdfs:label>discussion</rdfs:label>
    </owl:Class>
    


    <!-- http://purl.org/spar/deo/Epilogue -->

    <owl:Class rdf:about="http://purl.org/spar/deo/Epilogue">
        <rdfs:subClassOf rdf:resource="http://purl.org/spar/deo/DiscourseElement"/>
        <rdfs:comment xml:lang="en">A piece of writing at the end of a work of literature or drama, usually used to bring closure to the work.</rdfs:comment>
        <rdfs:label xml:lang="en">epilogue</rdfs:label>
    </owl:Class>
    


    <!-- http://purl.org/spar/deo/Evaluation -->

    <owl:Class rdf:about="http://purl.org/spar/deo/Evaluation">
        <owl:equivalentClass rdf:resource="http://salt.semanticauthoring.org/ontologies/sro#Evaluation"/>
        <rdfs:subClassOf rdf:resource="http://purl.org/spar/deo/DiscourseElement"/>
        <rdfs:comment>A consideration of the value, meaning and significance of the results obtained.</rdfs:comment>
        <rdfs:label>evaluation</rdfs:label>
    </owl:Class>
    


    <!-- http://purl.org/spar/deo/FutureWork -->

    <owl:Class rdf:about="http://purl.org/spar/deo/FutureWork">
        <rdfs:subClassOf rdf:resource="http://purl.org/spar/deo/DiscourseElement"/>
        <rdfs:comment xml:lang="en">A proposal for new investigation to be undertaken in order to continue and advance the work described in the publication.</rdfs:comment>
        <rdfs:label xml:lang="en">future work</rdfs:label>
    </owl:Class>
    


    <!-- http://purl.org/spar/deo/Introduction -->

    <owl:Class rdf:about="http://purl.org/spar/deo/Introduction">
        <rdfs:subClassOf rdf:resource="http://purl.org/spar/deo/DiscourseElement"/>
        <rdfs:comment xml:lang="en">An initial description which states the purpose and goals of the following writing, and, in the case of journal articles, typically includes background information on the research topic and a review of related work in the area.</rdfs:comment>
        <rdfs:label xml:lang="en">introduction</rdfs:label>
    </owl:Class>
    


    <!-- http://purl.org/spar/deo/Legend -->

    <owl:Class rdf:about="http://purl.org/spar/deo/Legend">
        <rdfs:subClassOf rdf:resource="http://purl.org/spar/deo/Caption"/>
        <rdfs:comment xml:lang="en">Informative text that explicitly explains another item, such as a figure or a table.</rdfs:comment>
        <rdfs:label xml:lang="en">legend</rdfs:label>
    </owl:Class>
    


    <!-- http://purl.org/spar/deo/Materials -->

    <owl:Class rdf:about="http://purl.org/spar/deo/Materials">
        <rdfs:subClassOf rdf:resource="http://purl.org/spar/deo/DiscourseElement"/>
        <rdfs:comment xml:lang="en">A description in a research paper documenting the specialized materials used in the work described. This description is often combined with a description of the methods used, in a section entitled &apos;Methods and Materials&apos;, &apos;Experimental&apos; or a related term.</rdfs:comment>
        <rdfs:label xml:lang="en">materials</rdfs:label>
    </owl:Class>
    


    <!-- http://purl.org/spar/deo/Methods -->

    <owl:Class rdf:about="http://purl.org/spar/deo/Methods">
        <rdfs:subClassOf rdf:resource="http://purl.org/spar/deo/DiscourseElement"/>
        <rdfs:comment xml:lang="en">A description in a research paper documenting the specialized methods used in the work described. This description is often combined with a description of the materials used, in a section entitled &apos;Methods and Materials&apos;, &apos;Experimental&apos; or a related term.</rdfs:comment>
        <rdfs:label xml:lang="en">methods</rdfs:label>
    </owl:Class>
    


    <!-- http://purl.org/spar/deo/Model -->

    <owl:Class rdf:about="http://purl.org/spar/deo/Model">
        <rdfs:subClassOf rdf:resource="http://purl.org/spar/deo/DiscourseElement"/>
        <rdfs:comment xml:lang="en">A description of a model used or produced by the work described in the publication.</rdfs:comment>
        <rdfs:label xml:lang="en">model</rdfs:label>
    </owl:Class>
    


    <!-- http://purl.org/spar/deo/Motivation -->

    <owl:Class rdf:about="http://purl.org/spar/deo/Motivation">
        <owl:equivalentClass rdf:resource="http://salt.semanticauthoring.org/ontologies/sro#Motivation"/>
        <rdfs:subClassOf rdf:resource="http://purl.org/spar/deo/DiscourseElement"/>
        <rdfs:comment>A description of the justification for undertaking the work described in the publication.</rdfs:comment>
        <rdfs:label>motivation</rdfs:label>
    </owl:Class>
    


    <!-- http://purl.org/spar/deo/Postscript -->

    <owl:Class rdf:about="http://purl.org/spar/deo/Postscript">
        <rdfs:subClassOf rdf:resource="http://purl.org/spar/deo/DiscourseElement"/>
        <rdfs:comment xml:lang="en">Text added after the signature of a letter, or sometimes after the main body of an essay or book.</rdfs:comment>
        <rdfs:label xml:lang="en">postscript</rdfs:label>
    </owl:Class>
    


    <!-- http://purl.org/spar/deo/ProblemStatement -->

    <owl:Class rdf:about="http://purl.org/spar/deo/ProblemStatement">
        <rdfs:subClassOf rdf:resource="http://purl.org/spar/deo/DiscourseElement"/>
        <dc:description xml:lang="en">A concise description of the issues that needed to be addressed by a work described in the document.</dc:description>
        <rdfs:label xml:lang="en">problem statement</rdfs:label>
    </owl:Class>
    


    <!-- http://purl.org/spar/deo/Prologue -->

    <owl:Class rdf:about="http://purl.org/spar/deo/Prologue">
        <rdfs:subClassOf rdf:resource="http://purl.org/spar/deo/DiscourseElement"/>
        <rdfs:comment xml:lang="en">A piece of writing at the beginning of a work of literature or drama, usually used to set the scene or to introduce the work.</rdfs:comment>
        <rdfs:label xml:lang="en">prologue</rdfs:label>
    </owl:Class>
    


    <!-- http://purl.org/spar/deo/Reference -->

    <owl:Class rdf:about="http://purl.org/spar/deo/Reference">
        <rdfs:subClassOf rdf:resource="http://purl.org/spar/deo/DiscourseElement"/>
        <rdfs:comment xml:lang="en">A reference to a specific part of the document, or to another publication.</rdfs:comment>
        <rdfs:label xml:lang="en">reference</rdfs:label>
    </owl:Class>
    


    <!-- http://purl.org/spar/deo/RelatedWork -->

    <owl:Class rdf:about="http://purl.org/spar/deo/RelatedWork">
        <rdfs:subClassOf rdf:resource="http://purl.org/spar/deo/DiscourseElement"/>
        <rdfs:comment xml:lang="en">The authors&apos; critical review of current knowledge by specific reference to others&apos; work, both in terms of substantive findings and theoretical and methodological contributions to a particular topic. This description is often included within the introduction section.</rdfs:comment>
        <rdfs:label xml:lang="en">related work</rdfs:label>
    </owl:Class>
    


    <!-- http://purl.org/spar/deo/Results -->

    <owl:Class rdf:about="http://purl.org/spar/deo/Results">
        <rdfs:subClassOf rdf:resource="http://purl.org/spar/deo/DiscourseElement"/>
        <rdfs:comment xml:lang="en">The report of the specific findings of an investigation, given without discussion or conclusion being drawn.</rdfs:comment>
        <rdfs:label xml:lang="en">results</rdfs:label>
    </owl:Class>
    


    <!-- http://purl.org/spar/deo/Scenario -->

    <owl:Class rdf:about="http://purl.org/spar/deo/Scenario">
        <owl:equivalentClass rdf:resource="http://salt.semanticauthoring.org/ontologies/sro#Scenario"/>
        <rdfs:subClassOf rdf:resource="http://purl.org/spar/deo/DiscourseElement"/>
        <rdfs:comment>A presentation of a use case or test, based on a real or hypothetical situation, used to help someone think through a complex problem or system.</rdfs:comment>
        <rdfs:label>scenario</rdfs:label>
    </owl:Class>
    


    <!-- http://purl.org/spar/doco/Abstract -->

    <owl:Class rdf:about="http://purl.org/spar/doco/Abstract">
        <rdfs:subClassOf rdf:resource="https://raw.githubusercontent.com/BOberreither/INTRO/master/INTRO_outdated.owl#PragmaticEntity"/>
    </owl:Class>
    


    <!-- http://purl.org/spar/doco/Afterword -->

    <owl:Class rdf:about="http://purl.org/spar/doco/Afterword">
        <rdfs:subClassOf>
            <owl:Class>
                <owl:intersectionOf rdf:parseType="Collection">
                    <rdf:Description rdf:about="http://purl.org/spar/doco/Section"/>
                    <owl:Restriction>
                        <owl:onProperty rdf:resource="http://purl.org/dc/terms/isPartOf"/>
                        <owl:someValuesFrom rdf:resource="http://purl.org/spar/doco/BackMatter"/>
                    </owl:Restriction>
                </owl:intersectionOf>
            </owl:Class>
        </rdfs:subClassOf>
        <rdfs:comment xml:lang="en">A literary device that is often found at the end of a piece of literature. It generally covers the story of how the book came into being, or how the idea for the book was developed. Alternatively, it may be written by someone other than the author of the book, and may discuss the work&apos;s historical or cultural context, if the work is being reissued many years after its original publication.</rdfs:comment>
        <rdfs:label xml:lang="en">afterword</rdfs:label>
    </owl:Class>
    


    <!-- http://purl.org/spar/doco/Appendix -->

    <owl:Class rdf:about="http://purl.org/spar/doco/Appendix">
        <rdfs:subClassOf>
            <owl:Class>
                <owl:intersectionOf rdf:parseType="Collection">
                    <owl:Class>
                        <owl:intersectionOf rdf:parseType="Collection">
                            <rdf:Description rdf:about="http://purl.org/spar/doco/Section"/>
                            <rdf:Description rdf:about="http://www.essepuntato.it/2008/12/pattern#HeadedContainer"/>
                        </owl:intersectionOf>
                    </owl:Class>
                    <owl:Restriction>
                        <owl:onProperty rdf:resource="http://purl.org/dc/terms/isPartOf"/>
                        <owl:someValuesFrom rdf:resource="http://purl.org/spar/doco/BackMatter"/>
                    </owl:Restriction>
                </owl:intersectionOf>
            </owl:Class>
        </rdfs:subClassOf>
        <rdfs:comment xml:lang="en">A supplemental addition to the main work. It may contain data, more detailed information about methods and materials, or provide additional detail concerning the information found in the main work.</rdfs:comment>
        <rdfs:label xml:lang="en">appendix</rdfs:label>
    </owl:Class>
    


    <!-- http://purl.org/spar/doco/BackMatter -->

    <owl:Class rdf:about="http://purl.org/spar/doco/BackMatter">
        <rdfs:subClassOf>
            <owl:Class>
                <owl:intersectionOf rdf:parseType="Collection">
                    <rdf:Description rdf:about="http://purl.org/spar/deo/DiscourseElement"/>
                    <rdf:Description rdf:about="http://www.essepuntato.it/2008/12/pattern#Container"/>
                </owl:intersectionOf>
            </owl:Class>
        </rdfs:subClassOf>
        <rdfs:subClassOf>
            <owl:Restriction>
                <owl:onProperty rdf:resource="http://www.essepuntato.it/2008/12/pattern#isContainedBy"/>
                <owl:allValuesFrom>
                    <owl:Class>
                        <owl:complementOf>
                            <owl:Class>
                                <owl:unionOf rdf:parseType="Collection">
                                    <rdf:Description rdf:about="http://purl.org/spar/doco/BackMatter"/>
                                    <rdf:Description rdf:about="http://purl.org/spar/doco/BodyMatter"/>
                                    <rdf:Description rdf:about="http://purl.org/spar/doco/FrontMatter"/>
                                </owl:unionOf>
                            </owl:Class>
                        </owl:complementOf>
                    </owl:Class>
                </owl:allValuesFrom>
            </owl:Restriction>
        </rdfs:subClassOf>
        <rdfs:comment xml:lang="en">The final principle part of a document, in which is usually found the bibliography, index, appendixes, etc.</rdfs:comment>
        <rdfs:label xml:lang="en">back matter</rdfs:label>
    </owl:Class>
    


    <!-- http://purl.org/spar/doco/BibliographicReferenceList -->

    <owl:Class rdf:about="http://purl.org/spar/doco/BibliographicReferenceList">
        <rdfs:subClassOf>
            <owl:Class>
                <owl:intersectionOf rdf:parseType="Collection">
                    <rdf:Description rdf:about="http://purl.org/spar/doco/ListOfReferences"/>
                    <owl:Restriction>
                        <owl:onProperty rdf:resource="http://www.essepuntato.it/2008/12/pattern#contains"/>
                        <owl:someValuesFrom rdf:resource="http://purl.org/spar/deo/BibliographicReference"/>
                    </owl:Restriction>
                </owl:intersectionOf>
            </owl:Class>
        </rdfs:subClassOf>
        <rdfs:comment xml:lang="en">A list, usually within a bibliography, of all the references within the citing document that refer to  journal articles, books, book chapters, Web sites or similar publications.</rdfs:comment>
        <rdfs:label xml:lang="en">bibliographic reference list</rdfs:label>
    </owl:Class>
    


    <!-- http://purl.org/spar/doco/BodyMatter -->

    <owl:Class rdf:about="http://purl.org/spar/doco/BodyMatter">
        <rdfs:subClassOf>
            <owl:Class>
                <owl:intersectionOf rdf:parseType="Collection">
                    <rdf:Description rdf:about="http://purl.org/spar/deo/DiscourseElement"/>
                    <rdf:Description rdf:about="http://www.essepuntato.it/2008/12/pattern#Container"/>
                </owl:intersectionOf>
            </owl:Class>
        </rdfs:subClassOf>
        <rdfs:subClassOf>
            <owl:Restriction>
                <owl:onProperty rdf:resource="http://www.essepuntato.it/2008/12/pattern#isContainedBy"/>
                <owl:allValuesFrom>
                    <owl:Class>
                        <owl:complementOf>
                            <owl:Class>
                                <owl:unionOf rdf:parseType="Collection">
                                    <rdf:Description rdf:about="http://purl.org/spar/doco/BackMatter"/>
                                    <rdf:Description rdf:about="http://purl.org/spar/doco/BodyMatter"/>
                                    <rdf:Description rdf:about="http://purl.org/spar/doco/FrontMatter"/>
                                </owl:unionOf>
                            </owl:Class>
                        </owl:complementOf>
                    </owl:Class>
                </owl:allValuesFrom>
            </owl:Restriction>
        </rdfs:subClassOf>
        <rdfs:comment xml:lang="en">The central principle part of a document, that contains the real content. It may be subdivided hierarchically by the use of chapters and sections.</rdfs:comment>
        <rdfs:label xml:lang="en">body matter</rdfs:label>
    </owl:Class>
    


    <!-- http://purl.org/spar/doco/CaptionedBox -->

    <owl:Class rdf:about="http://purl.org/spar/doco/CaptionedBox">
        <rdfs:subClassOf>
            <owl:Class>
                <owl:intersectionOf rdf:parseType="Collection">
                    <owl:Class>
                        <owl:intersectionOf rdf:parseType="Collection">
                            <rdf:Description rdf:about="http://purl.org/spar/deo/DiscourseElement"/>
                            <rdf:Description rdf:about="http://www.essepuntato.it/2008/12/pattern#Container"/>
                        </owl:intersectionOf>
                    </owl:Class>
                    <owl:Restriction>
                        <owl:onProperty rdf:resource="http://purl.org/dc/terms/hasPart"/>
                        <owl:someValuesFrom rdf:resource="http://purl.org/spar/deo/Caption"/>
                    </owl:Restriction>
                </owl:intersectionOf>
            </owl:Class>
        </rdfs:subClassOf>
        <rdfs:comment xml:lang="en">A rectangle space within a page that contains an object and its related caption.</rdfs:comment>
        <rdfs:label xml:lang="en">captioned box</rdfs:label>
    </owl:Class>
    


    <!-- http://purl.org/spar/doco/Chapter -->

    <owl:Class rdf:about="http://purl.org/spar/doco/Chapter">
        <rdfs:subClassOf rdf:resource="https://raw.githubusercontent.com/BOberreither/INTRO/master/INTRO_outdated.owl#FormalEntity"/>
        <rdfs:subClassOf>
            <owl:Class>
                <owl:intersectionOf rdf:parseType="Collection">
                    <rdf:Description rdf:about="http://purl.org/spar/deo/DiscourseElement"/>
                    <rdf:Description rdf:about="http://www.essepuntato.it/2008/12/pattern#HeadedContainer"/>
                </owl:intersectionOf>
            </owl:Class>
        </rdfs:subClassOf>
        <rdfs:subClassOf>
            <owl:Restriction>
                <owl:onProperty rdf:resource="http://www.essepuntato.it/2008/12/pattern#contains"/>
                <owl:someValuesFrom>
                    <owl:Class>
                        <owl:unionOf rdf:parseType="Collection">
                            <rdf:Description rdf:about="http://purl.org/spar/doco/Paragraph"/>
                            <rdf:Description rdf:about="http://purl.org/spar/doco/Section"/>
                        </owl:unionOf>
                    </owl:Class>
                </owl:someValuesFrom>
            </owl:Restriction>
        </rdfs:subClassOf>
        <rdfs:subClassOf>
            <owl:Restriction>
                <owl:onProperty rdf:resource="http://www.essepuntato.it/2008/12/pattern#contains"/>
                <owl:someValuesFrom>
                    <owl:Class>
                        <owl:complementOf rdf:resource="http://purl.org/spar/doco/Chapter"/>
                    </owl:Class>
                </owl:someValuesFrom>
            </owl:Restriction>
        </rdfs:subClassOf>
        <rdfs:comment xml:lang="en">A principle division of the body matter of a large document, such as a book, a report or a legislative document.</rdfs:comment>
        <rdfs:label xml:lang="en">chapter</rdfs:label>
    </owl:Class>
    


    <!-- http://purl.org/spar/doco/ChapterTitle -->

    <owl:Class rdf:about="http://purl.org/spar/doco/ChapterTitle">
        <rdfs:subClassOf rdf:resource="http://purl.org/spar/doco/Title"/>
        <rdfs:subClassOf>
            <owl:Restriction>
                <owl:onProperty rdf:resource="http://www.essepuntato.it/2008/12/pattern#isContainedByAsHeader"/>
                <owl:someValuesFrom rdf:resource="http://purl.org/spar/doco/Chapter"/>
            </owl:Restriction>
        </rdfs:subClassOf>
        <owl:disjointWith rdf:resource="http://purl.org/spar/doco/SectionTitle"/>
        <rdfs:comment xml:lang="en">The title of a chapter.</rdfs:comment>
        <rdfs:label xml:lang="en">chapter title</rdfs:label>
    </owl:Class>
    


    <!-- http://purl.org/spar/doco/Colophon -->

    <owl:Class rdf:about="http://purl.org/spar/doco/Colophon">
        <rdfs:subClassOf>
            <owl:Class>
                <owl:intersectionOf rdf:parseType="Collection">
                    <rdf:Description rdf:about="http://purl.org/spar/doco/Section"/>
                    <owl:Restriction>
                        <owl:onProperty rdf:resource="http://purl.org/dc/terms/isPartOf"/>
                        <owl:someValuesFrom>
                            <owl:Class>
                                <owl:unionOf rdf:parseType="Collection">
                                    <rdf:Description rdf:about="http://purl.org/spar/doco/BackMatter"/>
                                    <rdf:Description rdf:about="http://purl.org/spar/doco/FrontMatter"/>
                                </owl:unionOf>
                            </owl:Class>
                        </owl:someValuesFrom>
                    </owl:Restriction>
                </owl:intersectionOf>
            </owl:Class>
        </rdfs:subClassOf>
        <rdfs:comment xml:lang="en">A brief description of publication or production notes relevant to the document.</rdfs:comment>
        <rdfs:label xml:lang="en">colophon</rdfs:label>
    </owl:Class>
    


    <!-- http://purl.org/spar/doco/ComplexRunInQuotation -->

    <owl:Class rdf:about="http://purl.org/spar/doco/ComplexRunInQuotation">
        <rdfs:subClassOf rdf:resource="http://purl.org/spar/deo/DiscourseElement"/>
        <rdfs:subClassOf rdf:resource="http://www.essepuntato.it/2008/12/pattern#Popup"/>
        <rdfs:comment xml:lang="en">A quotation with a complex structure, that is included inline and is usually enclosed within quotation marks.</rdfs:comment>
        <rdfs:label xml:lang="en">complex run-in quotation</rdfs:label>
    </owl:Class>
    


    <!-- http://purl.org/spar/doco/Figure -->

    <owl:Class rdf:about="http://purl.org/spar/doco/Figure">
        <rdfs:subClassOf rdf:resource="http://purl.org/spar/deo/DiscourseElement"/>
        <rdfs:subClassOf>
            <owl:Class>
                <owl:unionOf rdf:parseType="Collection">
                    <rdf:Description rdf:about="http://www.essepuntato.it/2008/12/pattern#Meta"/>
                    <rdf:Description rdf:about="http://www.essepuntato.it/2008/12/pattern#Milestone"/>
                </owl:unionOf>
            </owl:Class>
        </rdfs:subClassOf>
        <rdfs:comment xml:lang="en">A communication object comprising one or more graphics, drawings, images, or other visual representations..</rdfs:comment>
        <rdfs:label xml:lang="en">figure</rdfs:label>
    </owl:Class>
    


    <!-- http://purl.org/spar/doco/FigureBox -->

    <owl:Class rdf:about="http://purl.org/spar/doco/FigureBox">
        <rdfs:subClassOf>
            <owl:Class>
                <owl:intersectionOf rdf:parseType="Collection">
                    <rdf:Description rdf:about="http://purl.org/spar/doco/CaptionedBox"/>
                    <owl:Restriction>
                        <owl:onProperty rdf:resource="http://purl.org/dc/terms/hasPart"/>
                        <owl:someValuesFrom rdf:resource="http://purl.org/spar/doco/Figure"/>
                    </owl:Restriction>
                </owl:intersectionOf>
            </owl:Class>
        </rdfs:subClassOf>
        <owl:disjointWith rdf:resource="http://purl.org/spar/doco/TableBox"/>
        <rdfs:comment xml:lang="en">A space within a document that contains a figure and its caption.</rdfs:comment>
        <rdfs:label xml:lang="en">figure box</rdfs:label>
    </owl:Class>
    


    <!-- http://purl.org/spar/doco/Footnote -->

    <owl:Class rdf:about="http://purl.org/spar/doco/Footnote">
        <rdfs:subClassOf rdf:resource="http://purl.org/spar/deo/DiscourseElement"/>
        <rdfs:subClassOf>
            <owl:Class>
                <owl:unionOf rdf:parseType="Collection">
                    <rdf:Description rdf:about="http://www.essepuntato.it/2008/12/pattern#Container"/>
                    <rdf:Description rdf:about="http://www.essepuntato.it/2008/12/pattern#Popup"/>
                </owl:unionOf>
            </owl:Class>
        </rdfs:subClassOf>
        <rdfs:comment xml:lang="en">A structure within a sentence that permits the author to make a comment or to cite another publication in support of the text, or both. A footnote is normally flagged by a superscript number immediately following that portion of the text to which it relates. For convenience of reading, the text of the footnote is usually printed at the bottom of the page or at the end of a text.</rdfs:comment>
        <rdfs:label xml:lang="en">footnote</rdfs:label>
    </owl:Class>
    


    <!-- http://purl.org/spar/doco/Foreword -->

    <owl:Class rdf:about="http://purl.org/spar/doco/Foreword">
        <rdfs:subClassOf>
            <owl:Class>
                <owl:intersectionOf rdf:parseType="Collection">
                    <rdf:Description rdf:about="http://purl.org/spar/doco/Section"/>
                    <owl:Restriction>
                        <owl:onProperty rdf:resource="http://purl.org/dc/terms/isPartOf"/>
                        <owl:someValuesFrom rdf:resource="http://purl.org/spar/doco/FrontMatter"/>
                    </owl:Restriction>
                </owl:intersectionOf>
            </owl:Class>
        </rdfs:subClassOf>
        <rdfs:comment xml:lang="en">A section in a book or report, usually written by someone other than the author, that introduces or commends the document to the reader. It may include description of the interaction between the writer of the foreword and the author.</rdfs:comment>
        <rdfs:label xml:lang="en">foreword</rdfs:label>
    </owl:Class>
    


    <!-- http://purl.org/spar/doco/Formula -->

    <owl:Class rdf:about="http://purl.org/spar/doco/Formula">
        <rdfs:subClassOf rdf:resource="http://purl.org/spar/deo/DiscourseElement"/>
        <rdfs:subClassOf rdf:resource="http://www.essepuntato.it/2008/12/pattern#Popup"/>
        <rdfs:comment xml:lang="en">A unit of information expressed in mathematical, chemical or logical symbols and language.</rdfs:comment>
        <rdfs:label xml:lang="en">formula</rdfs:label>
    </owl:Class>
    


    <!-- http://purl.org/spar/doco/FormulaBox -->

    <owl:Class rdf:about="http://purl.org/spar/doco/FormulaBox">
        <rdfs:subClassOf>
            <owl:Class>
                <owl:intersectionOf rdf:parseType="Collection">
                    <owl:Class>
                        <owl:intersectionOf rdf:parseType="Collection">
                            <rdf:Description rdf:about="http://purl.org/spar/deo/DiscourseElement"/>
                            <rdf:Description rdf:about="http://www.essepuntato.it/2008/12/pattern#Container"/>
                        </owl:intersectionOf>
                    </owl:Class>
                    <owl:Restriction>
                        <owl:onProperty rdf:resource="http://purl.org/dc/terms/hasPart"/>
                        <owl:someValuesFrom rdf:resource="http://purl.org/spar/doco/Formula"/>
                    </owl:Restriction>
                </owl:intersectionOf>
            </owl:Class>
        </rdfs:subClassOf>
        <rdfs:comment xml:lang="en">A space within a document that contains one or more formulae.</rdfs:comment>
        <rdfs:label xml:lang="en">formula box</rdfs:label>
    </owl:Class>
    


    <!-- http://purl.org/spar/doco/FrontMatter -->

    <owl:Class rdf:about="http://purl.org/spar/doco/FrontMatter">
        <rdfs:subClassOf>
            <owl:Class>
                <owl:intersectionOf rdf:parseType="Collection">
                    <rdf:Description rdf:about="http://purl.org/spar/deo/DiscourseElement"/>
                    <rdf:Description rdf:about="http://www.essepuntato.it/2008/12/pattern#Container"/>
                </owl:intersectionOf>
            </owl:Class>
        </rdfs:subClassOf>
        <rdfs:subClassOf>
            <owl:Restriction>
                <owl:onProperty rdf:resource="http://www.essepuntato.it/2008/12/pattern#isContainedBy"/>
                <owl:allValuesFrom>
                    <owl:Class>
                        <owl:complementOf>
                            <owl:Class>
                                <owl:unionOf rdf:parseType="Collection">
                                    <rdf:Description rdf:about="http://purl.org/spar/doco/BackMatter"/>
                                    <rdf:Description rdf:about="http://purl.org/spar/doco/BodyMatter"/>
                                    <rdf:Description rdf:about="http://purl.org/spar/doco/FrontMatter"/>
                                </owl:unionOf>
                            </owl:Class>
                        </owl:complementOf>
                    </owl:Class>
                </owl:allValuesFrom>
            </owl:Restriction>
        </rdfs:subClassOf>
        <rdfs:comment xml:lang="en">The initial principle part of a document, usually containing self-referential metadata. In a book, this typically includes its title, authors, publisher, publication date, ISBN and copyright declaration, together with the preface, foreword, table of content, etc. In a journal article, the front matter is normally restricted to the title, authors and the authors&apos; affiliation details, although the latter may alternatively be included in a footnote or the back matter. In books, the front matter pages may be numbered in lowercase Roman numerals.</rdfs:comment>
        <rdfs:label xml:lang="en">front matter</rdfs:label>
    </owl:Class>
    


    <!-- http://purl.org/spar/doco/Glossary -->

    <owl:Class rdf:about="http://purl.org/spar/doco/Glossary">
        <rdfs:subClassOf>
            <owl:Class>
                <owl:intersectionOf rdf:parseType="Collection">
                    <rdf:Description rdf:about="http://purl.org/spar/doco/Section"/>
                    <owl:Restriction>
                        <owl:onProperty rdf:resource="http://purl.org/dc/terms/isPartOf"/>
                        <owl:someValuesFrom>
                            <owl:Class>
                                <owl:unionOf rdf:parseType="Collection">
                                    <rdf:Description rdf:about="http://purl.org/spar/doco/BackMatter"/>
                                    <rdf:Description rdf:about="http://purl.org/spar/doco/FrontMatter"/>
                                </owl:unionOf>
                            </owl:Class>
                        </owl:someValuesFrom>
                    </owl:Restriction>
                </owl:intersectionOf>
            </owl:Class>
        </rdfs:subClassOf>
        <rdfs:comment xml:lang="en">A set of definitions of words or phrases of importance to the work, normally alphabetized. In longer works of fiction, the entries may contains places and characters.</rdfs:comment>
        <rdfs:label xml:lang="en">glossary</rdfs:label>
    </owl:Class>
    


    <!-- http://purl.org/spar/doco/Index -->

    <owl:Class rdf:about="http://purl.org/spar/doco/Index">
        <rdfs:subClassOf>
            <owl:Class>
                <owl:intersectionOf rdf:parseType="Collection">
                    <owl:Class>
                        <owl:intersectionOf rdf:parseType="Collection">
                            <rdf:Description rdf:about="http://purl.org/spar/doco/Section"/>
                            <rdf:Description rdf:about="http://www.essepuntato.it/2008/12/pattern#HeadedContainer"/>
                        </owl:intersectionOf>
                    </owl:Class>
                    <owl:Restriction>
                        <owl:onProperty rdf:resource="http://purl.org/dc/terms/isPartOf"/>
                        <owl:someValuesFrom rdf:resource="http://purl.org/spar/doco/BackMatter"/>
                    </owl:Restriction>
                </owl:intersectionOf>
            </owl:Class>
        </rdfs:subClassOf>
        <rdfs:comment xml:lang="en">A section containing a list of references to information on the named topic of importance to the content of the document. The references may be to page numbers, paragraph numbers, section numbers or chapter numbers within the document.</rdfs:comment>
        <rdfs:label xml:lang="en">index</rdfs:label>
    </owl:Class>
    


    <!-- http://purl.org/spar/doco/Label -->

    <owl:Class rdf:about="http://purl.org/spar/doco/Label">
        <rdfs:subClassOf rdf:resource="https://raw.githubusercontent.com/BOberreither/INTRO/master/INTRO_outdated.owl#PragmaticEntity"/>
    </owl:Class>
    


    <!-- http://purl.org/spar/doco/Line -->

    <owl:Class rdf:about="http://purl.org/spar/doco/Line">
        <rdfs:subClassOf rdf:resource="http://purl.org/spar/deo/DiscourseElement"/>
        <rdfs:comment xml:lang="en">A line in poetry is a unit of language into which a poem is divided which operates on principles which are distinct from and not necessarily coincident with grammatical structures, such as the sentence or clauses in sentences.

A distinct numbered group of lines in verse is normally called a stanza.</rdfs:comment>
        <rdfs:label xml:lang="en">line</rdfs:label>
    </owl:Class>
    


    <!-- http://purl.org/spar/doco/List -->

    <owl:Class rdf:about="http://purl.org/spar/doco/List">
        <rdfs:subClassOf rdf:resource="http://purl.org/spar/deo/DiscourseElement"/>
        <rdfs:subClassOf rdf:resource="https://raw.githubusercontent.com/BOberreither/INTRO/master/INTRO_outdated.owl#FormalEntity"/>
        <rdfs:subClassOf>
            <owl:Class>
                <owl:intersectionOf rdf:parseType="Collection">
                    <rdf:Description rdf:about="http://www.essepuntato.it/2008/12/pattern#Table"/>
                    <owl:Restriction>
                        <owl:onProperty rdf:resource="http://www.essepuntato.it/2008/12/pattern#contains"/>
                        <owl:someValuesFrom rdf:resource="http://www.essepuntato.it/2008/12/pattern#Pattern"/>
                    </owl:Restriction>
                </owl:intersectionOf>
            </owl:Class>
        </rdfs:subClassOf>
        <rdfs:comment xml:lang="en">An enumeration of items.</rdfs:comment>
        <rdfs:label xml:lang="en">list</rdfs:label>
    </owl:Class>
    


    <!-- http://purl.org/spar/doco/ListOfAgents -->

    <owl:Class rdf:about="http://purl.org/spar/doco/ListOfAgents">
        <rdfs:subClassOf rdf:resource="http://purl.org/spar/doco/List"/>
        <owl:disjointWith rdf:resource="http://purl.org/spar/doco/ListOfReferences"/>
        <rdfs:comment xml:lang="en">A list of items each denoting an agent, such as an author, a contributor or an organization, related to a particular publication.</rdfs:comment>
        <rdfs:label xml:lang="en">list of agents</rdfs:label>
    </owl:Class>
    


    <!-- http://purl.org/spar/doco/ListOfAuthors -->

    <owl:Class rdf:about="http://purl.org/spar/doco/ListOfAuthors">
        <rdfs:subClassOf rdf:resource="http://purl.org/spar/doco/ListOfAgents"/>
        <rdfs:comment xml:lang="en">A list of items each denoting an author of a particular publication.</rdfs:comment>
        <rdfs:label xml:lang="en">list of authors</rdfs:label>
    </owl:Class>
    


    <!-- http://purl.org/spar/doco/ListOfContributors -->

    <owl:Class rdf:about="http://purl.org/spar/doco/ListOfContributors">
        <rdfs:subClassOf rdf:resource="http://purl.org/spar/doco/ListOfAgents"/>
        <rdfs:comment xml:lang="en">A list of items, each denoting a contributor to a publication such as an encyclopedia or a text book, where such contributions are insufficient to warrant classification as author.</rdfs:comment>
        <rdfs:label xml:lang="en">list of contributors</rdfs:label>
    </owl:Class>
    


    <!-- http://purl.org/spar/doco/ListOfFigures -->

    <owl:Class rdf:about="http://purl.org/spar/doco/ListOfFigures">
        <rdfs:subClassOf>
            <owl:Class>
                <owl:intersectionOf rdf:parseType="Collection">
                    <owl:Class>
                        <owl:intersectionOf rdf:parseType="Collection">
                            <rdf:Description rdf:about="http://purl.org/spar/doco/Section"/>
                            <rdf:Description rdf:about="http://www.essepuntato.it/2008/12/pattern#HeadedContainer"/>
                        </owl:intersectionOf>
                    </owl:Class>
                    <owl:Restriction>
                        <owl:onProperty rdf:resource="http://purl.org/dc/terms/isPartOf"/>
                        <owl:someValuesFrom>
                            <owl:Class>
                                <owl:unionOf rdf:parseType="Collection">
                                    <rdf:Description rdf:about="http://purl.org/spar/doco/BackMatter"/>
                                    <rdf:Description rdf:about="http://purl.org/spar/doco/FrontMatter"/>
                                </owl:unionOf>
                            </owl:Class>
                        </owl:someValuesFrom>
                    </owl:Restriction>
                </owl:intersectionOf>
            </owl:Class>
        </rdfs:subClassOf>
        <rdfs:subClassOf>
            <owl:Restriction>
                <owl:onProperty rdf:resource="http://purl.org/dc/terms/hasPart"/>
                <owl:someValuesFrom>
                    <owl:Class>
                        <owl:intersectionOf rdf:parseType="Collection">
                            <rdf:Description rdf:about="http://purl.org/spar/doco/ListOfReferences"/>
                            <owl:Restriction>
                                <owl:onProperty rdf:resource="http://www.essepuntato.it/2008/12/pattern#contains"/>
                                <owl:allValuesFrom>
                                    <owl:Restriction>
                                        <owl:onProperty rdf:resource="http://purl.org/dc/terms/relation"/>
                                        <owl:someValuesFrom rdf:resource="http://purl.org/spar/doco/FigureBox"/>
                                    </owl:Restriction>
                                </owl:allValuesFrom>
                            </owl:Restriction>
                        </owl:intersectionOf>
                    </owl:Class>
                </owl:someValuesFrom>
            </owl:Restriction>
        </rdfs:subClassOf>
        <rdfs:comment xml:lang="en">A section of the document listing all the figures, identified by their titles and referenced to their locations in the document. May also be referred to as &apos;List of illustrations&apos;.</rdfs:comment>
        <rdfs:label xml:lang="en">list of figures</rdfs:label>
    </owl:Class>
    


    <!-- http://purl.org/spar/doco/ListOfOrganizations -->

    <owl:Class rdf:about="http://purl.org/spar/doco/ListOfOrganizations">
        <rdfs:subClassOf rdf:resource="http://purl.org/spar/doco/ListOfAgents"/>
        <rdfs:comment xml:lang="en">A list of items, each denoting an organization or institution related to the publication, for example the authors&apos; affiliations, or the suppliers of information, software, equipment or consumables used in the work described in the publication.</rdfs:comment>
        <rdfs:label xml:lang="en">list of organizations</rdfs:label>
    </owl:Class>
    


    <!-- http://purl.org/spar/doco/ListOfReferences -->

    <owl:Class rdf:about="http://purl.org/spar/doco/ListOfReferences">
        <rdfs:subClassOf>
            <owl:Class>
                <owl:intersectionOf rdf:parseType="Collection">
                    <rdf:Description rdf:about="http://purl.org/spar/doco/List"/>
                    <owl:Restriction>
                        <owl:onProperty rdf:resource="http://www.essepuntato.it/2008/12/pattern#contains"/>
                        <owl:allValuesFrom rdf:resource="http://purl.org/spar/deo/Reference"/>
                    </owl:Restriction>
                </owl:intersectionOf>
            </owl:Class>
        </rdfs:subClassOf>
        <rdfs:comment xml:lang="en">A list of items each representing a reference to a specific part of the same document, or to another publication.</rdfs:comment>
        <rdfs:label xml:lang="en">list of references</rdfs:label>
    </owl:Class>
    


    <!-- http://purl.org/spar/doco/ListOfTables -->

    <owl:Class rdf:about="http://purl.org/spar/doco/ListOfTables">
        <rdfs:subClassOf>
            <owl:Class>
                <owl:intersectionOf rdf:parseType="Collection">
                    <owl:Class>
                        <owl:intersectionOf rdf:parseType="Collection">
                            <rdf:Description rdf:about="http://purl.org/spar/doco/Section"/>
                            <rdf:Description rdf:about="http://www.essepuntato.it/2008/12/pattern#HeadedContainer"/>
                        </owl:intersectionOf>
                    </owl:Class>
                    <owl:Restriction>
                        <owl:onProperty rdf:resource="http://purl.org/dc/terms/isPartOf"/>
                        <owl:someValuesFrom>
                            <owl:Class>
                                <owl:unionOf rdf:parseType="Collection">
                                    <rdf:Description rdf:about="http://purl.org/spar/doco/BackMatter"/>
                                    <rdf:Description rdf:about="http://purl.org/spar/doco/FrontMatter"/>
                                </owl:unionOf>
                            </owl:Class>
                        </owl:someValuesFrom>
                    </owl:Restriction>
                </owl:intersectionOf>
            </owl:Class>
        </rdfs:subClassOf>
        <rdfs:subClassOf>
            <owl:Restriction>
                <owl:onProperty rdf:resource="http://purl.org/dc/terms/hasPart"/>
                <owl:someValuesFrom>
                    <owl:Class>
                        <owl:intersectionOf rdf:parseType="Collection">
                            <rdf:Description rdf:about="http://purl.org/spar/doco/ListOfReferences"/>
                            <owl:Restriction>
                                <owl:onProperty rdf:resource="http://www.essepuntato.it/2008/12/pattern#contains"/>
                                <owl:allValuesFrom>
                                    <owl:Restriction>
                                        <owl:onProperty rdf:resource="http://purl.org/dc/terms/relation"/>
                                        <owl:someValuesFrom rdf:resource="http://purl.org/spar/doco/TableBox"/>
                                    </owl:Restriction>
                                </owl:allValuesFrom>
                            </owl:Restriction>
                        </owl:intersectionOf>
                    </owl:Class>
                </owl:someValuesFrom>
            </owl:Restriction>
        </rdfs:subClassOf>
        <rdfs:comment xml:lang="en">A section of the document listing all the tables, identified by their titles and referenced to their locations in the document.</rdfs:comment>
        <rdfs:label xml:lang="en">list of tables</rdfs:label>
    </owl:Class>
    


    <!-- http://purl.org/spar/doco/Paragraph -->

    <owl:Class rdf:about="http://purl.org/spar/doco/Paragraph">
        <rdfs:subClassOf rdf:resource="https://raw.githubusercontent.com/BOberreither/INTRO/master/INTRO_outdated.owl#FormalEntity"/>
        <rdfs:subClassOf rdf:resource="https://raw.githubusercontent.com/BOberreither/INTRO/master/INTRO_outdated.owl#PragmaticEntity"/>
        <rdfs:comment xml:lang="en">A self-contained unit of discourse that deals with a particular point or idea. Paragraphs contains one or more sentences. The start of a paragraph is indicated by beginning on a new line, which may be indented or separated by a small vertical space by the preceding paragraph. </rdfs:comment>
        <rdfs:label xml:lang="en">paragraph</rdfs:label>
    </owl:Class>
    


    <!-- http://purl.org/spar/doco/Part -->

    <owl:Class rdf:about="http://purl.org/spar/doco/Part">
        <rdfs:subClassOf rdf:resource="https://raw.githubusercontent.com/BOberreither/INTRO/master/INTRO_outdated.owl#FormalEntity"/>
        <rdfs:subClassOf rdf:resource="https://raw.githubusercontent.com/BOberreither/INTRO/master/INTRO_outdated.owl#PragmaticEntity"/>
        <rdfs:subClassOf>
            <owl:Class>
                <owl:intersectionOf rdf:parseType="Collection">
                    <rdf:Description rdf:about="http://purl.org/spar/deo/DiscourseElement"/>
                    <rdf:Description rdf:about="http://www.essepuntato.it/2008/12/pattern#Container"/>
                </owl:intersectionOf>
            </owl:Class>
        </rdfs:subClassOf>
        <rdfs:comment xml:lang="en">A container of a semantic subdivision of a document. For example, chapters of a novel may be grouped into distinct parts that may be named &apos;Part 1&apos;, &apos;Part 2&apos;, etc., &apos;Book 1&apos;, &apos;Book 2&apos;, etc., or &apos;Genesis&apos;, &apos;Exodus&apos;, etc.</rdfs:comment>
        <rdfs:label xml:lang="en">part</rdfs:label>
    </owl:Class>
    


    <!-- http://purl.org/spar/doco/Preface -->

    <owl:Class rdf:about="http://purl.org/spar/doco/Preface">
        <rdfs:subClassOf>
            <owl:Class>
                <owl:intersectionOf rdf:parseType="Collection">
                    <rdf:Description rdf:about="http://purl.org/spar/doco/Section"/>
                    <owl:Restriction>
                        <owl:onProperty rdf:resource="http://purl.org/dc/terms/isPartOf"/>
                        <owl:someValuesFrom rdf:resource="http://purl.org/spar/doco/FrontMatter"/>
                    </owl:Restriction>
                </owl:intersectionOf>
            </owl:Class>
        </rdfs:subClassOf>
        <rdfs:comment xml:lang="en">A section describing how the document came into being, or how the idea for it was developed. The preface may contains acknowledgements. The preface to a later edition of the work often explains in what respect that edition differs from previous ones.</rdfs:comment>
        <rdfs:label xml:lang="en">preface</rdfs:label>
    </owl:Class>
    


    <!-- http://purl.org/spar/doco/Section -->

    <owl:Class rdf:about="http://purl.org/spar/doco/Section">
        <rdfs:subClassOf>
            <owl:Class>
                <owl:intersectionOf rdf:parseType="Collection">
                    <rdf:Description rdf:about="http://purl.org/spar/deo/DiscourseElement"/>
                    <rdf:Description rdf:about="http://www.essepuntato.it/2008/12/pattern#HeadedContainer"/>
                </owl:intersectionOf>
            </owl:Class>
        </rdfs:subClassOf>
        <rdfs:subClassOf>
            <owl:Restriction>
                <owl:onProperty rdf:resource="http://www.essepuntato.it/2008/12/pattern#contains"/>
                <owl:someValuesFrom>
                    <owl:Class>
                        <owl:unionOf rdf:parseType="Collection">
                            <rdf:Description rdf:about="http://purl.org/spar/doco/Paragraph"/>
                            <rdf:Description rdf:about="http://purl.org/spar/doco/Section"/>
                        </owl:unionOf>
                    </owl:Class>
                </owl:someValuesFrom>
            </owl:Restriction>
        </rdfs:subClassOf>
        <rdfs:subClassOf>
            <owl:Restriction>
                <owl:onProperty rdf:resource="http://www.essepuntato.it/2008/12/pattern#contains"/>
                <owl:someValuesFrom>
                    <owl:Class>
                        <owl:complementOf rdf:resource="http://purl.org/spar/doco/Chapter"/>
                    </owl:Class>
                </owl:someValuesFrom>
            </owl:Restriction>
        </rdfs:subClassOf>
        <rdfs:comment xml:lang="en">A logical division of the text, usually numbered and/or titled, which may contain subsections.</rdfs:comment>
        <rdfs:label xml:lang="en">section</rdfs:label>
    </owl:Class>
    


    <!-- http://purl.org/spar/doco/SectionTitle -->

    <owl:Class rdf:about="http://purl.org/spar/doco/SectionTitle">
        <rdfs:subClassOf rdf:resource="http://purl.org/spar/doco/Title"/>
        <rdfs:subClassOf>
            <owl:Restriction>
                <owl:onProperty rdf:resource="http://www.essepuntato.it/2008/12/pattern#isContainedByAsHeader"/>
                <owl:someValuesFrom rdf:resource="http://purl.org/spar/doco/Section"/>
            </owl:Restriction>
        </rdfs:subClassOf>
        <rdfs:comment xml:lang="en">The title of a section.</rdfs:comment>
        <rdfs:label xml:lang="en">section title</rdfs:label>
    </owl:Class>
    


    <!-- http://purl.org/spar/doco/Sentence -->

    <owl:Class rdf:about="http://purl.org/spar/doco/Sentence">
        <rdfs:subClassOf rdf:resource="http://purl.org/spar/deo/DiscourseElement"/>
        <rdfs:subClassOf rdf:resource="https://raw.githubusercontent.com/BOberreither/INTRO/master/INTRO_outdated.owl#FormalEntity"/>
        <rdfs:comment xml:lang="en">An expression in natural language forming a single grammatical unit. A sentence minimally consists of a subject and an intransitive verb, or a subject, a transitive verb and an object, and may include additional dependent clauses. In written text, a sentence is always terminated by a full stop. A sentence can include words grouped meaningfully to express a statement, a question, an exclamation, a request or a command.</rdfs:comment>
        <rdfs:label xml:lang="en">sentence</rdfs:label>
    </owl:Class>
    


    <!-- http://purl.org/spar/doco/Stanza -->

    <owl:Class rdf:about="http://purl.org/spar/doco/Stanza">
        <rdfs:subClassOf rdf:resource="https://raw.githubusercontent.com/BOberreither/INTRO/master/INTRO_outdated.owl#FormalEntity"/>
        <rdfs:subClassOf>
            <owl:Class>
                <owl:intersectionOf rdf:parseType="Collection">
                    <owl:Class>
                        <owl:intersectionOf rdf:parseType="Collection">
                            <rdf:Description rdf:about="http://purl.org/spar/deo/DiscourseElement"/>
                            <rdf:Description rdf:about="http://www.essepuntato.it/2008/12/pattern#Container"/>
                        </owl:intersectionOf>
                    </owl:Class>
                    <owl:Restriction>
                        <owl:onProperty rdf:resource="http://www.essepuntato.it/2008/12/pattern#contains"/>
                        <owl:allValuesFrom rdf:resource="http://purl.org/spar/doco/Line"/>
                    </owl:Restriction>
                </owl:intersectionOf>
            </owl:Class>
        </rdfs:subClassOf>
        <rdfs:comment xml:lang="en">A unit within a larger poem. A stanza consists of a grouping of lines, set off by a vertical space from other stanzas, that usually has a set pattern of meter and rhyme.</rdfs:comment>
        <rdfs:label xml:lang="en">stanza</rdfs:label>
    </owl:Class>
    


    <!-- http://purl.org/spar/doco/Table -->

    <owl:Class rdf:about="http://purl.org/spar/doco/Table">
        <rdfs:subClassOf rdf:resource="http://purl.org/spar/deo/DiscourseElement"/>
        <rdfs:subClassOf rdf:resource="http://www.essepuntato.it/2008/12/pattern#Table"/>
        <rdfs:subClassOf>
            <owl:Restriction>
                <owl:onProperty rdf:resource="http://www.essepuntato.it/2008/12/pattern#contains"/>
                <owl:someValuesFrom rdf:resource="http://www.essepuntato.it/2008/12/pattern#Container"/>
            </owl:Restriction>
        </rdfs:subClassOf>
        <rdfs:comment xml:lang="en">A set of data arranged in cells within rows and columns.</rdfs:comment>
        <rdfs:label xml:lang="en">table</rdfs:label>
    </owl:Class>
    


    <!-- http://purl.org/spar/doco/TableBox -->

    <owl:Class rdf:about="http://purl.org/spar/doco/TableBox">
        <rdfs:subClassOf>
            <owl:Class>
                <owl:intersectionOf rdf:parseType="Collection">
                    <rdf:Description rdf:about="http://purl.org/spar/doco/CaptionedBox"/>
                    <owl:Restriction>
                        <owl:onProperty rdf:resource="http://purl.org/dc/terms/hasPart"/>
                        <owl:someValuesFrom rdf:resource="http://purl.org/spar/doco/Table"/>
                    </owl:Restriction>
                </owl:intersectionOf>
            </owl:Class>
        </rdfs:subClassOf>
        <rdfs:comment xml:lang="en">A space within a document that contains a table and its caption.</rdfs:comment>
        <rdfs:label xml:lang="en">table box</rdfs:label>
    </owl:Class>
    


    <!-- http://purl.org/spar/doco/TableOfContents -->

    <owl:Class rdf:about="http://purl.org/spar/doco/TableOfContents">
        <rdfs:subClassOf>
            <owl:Class>
                <owl:intersectionOf rdf:parseType="Collection">
                    <rdf:Description rdf:about="http://purl.org/spar/doco/Section"/>
                    <owl:Restriction>
                        <owl:onProperty rdf:resource="http://purl.org/dc/terms/isPartOf"/>
                        <owl:someValuesFrom>
                            <owl:Class>
                                <owl:unionOf rdf:parseType="Collection">
                                    <rdf:Description rdf:about="http://purl.org/spar/doco/BackMatter"/>
                                    <rdf:Description rdf:about="http://purl.org/spar/doco/FrontMatter"/>
                                </owl:unionOf>
                            </owl:Class>
                        </owl:someValuesFrom>
                    </owl:Restriction>
                </owl:intersectionOf>
            </owl:Class>
        </rdfs:subClassOf>
        <rdfs:subClassOf>
            <owl:Restriction>
                <owl:onProperty rdf:resource="http://purl.org/dc/terms/hasPart"/>
                <owl:someValuesFrom>
                    <owl:Class>
                        <owl:intersectionOf rdf:parseType="Collection">
                            <rdf:Description rdf:about="http://purl.org/spar/doco/ListOfReferences"/>
                            <owl:Restriction>
                                <owl:onProperty rdf:resource="http://www.essepuntato.it/2008/12/pattern#contains"/>
                                <owl:allValuesFrom>
                                    <owl:Restriction>
                                        <owl:onProperty rdf:resource="http://purl.org/dc/terms/relation"/>
                                        <owl:someValuesFrom rdf:resource="http://purl.org/spar/doco/Section"/>
                                    </owl:Restriction>
                                </owl:allValuesFrom>
                            </owl:Restriction>
                        </owl:intersectionOf>
                    </owl:Class>
                </owl:someValuesFrom>
            </owl:Restriction>
        </rdfs:subClassOf>
        <rdfs:comment xml:lang="en">A section of the document listing all the chapters and sections, identified by their titles and referenced to their locations in the document. The table of contents may include a list of the front-matter and back-matter items, in addition to the body-matter items.  Where the document is a journal or magazine issue, the table of content lists the constituent items contained in that issue, typically by title, authors and first page number.</rdfs:comment>
        <rdfs:label xml:lang="en">table of contents</rdfs:label>
    </owl:Class>
    


    <!-- http://purl.org/spar/doco/TextBox -->

    <owl:Class rdf:about="http://purl.org/spar/doco/TextBox">
        <rdfs:subClassOf rdf:resource="http://purl.org/spar/deo/DiscourseElement"/>
        <rdfs:subClassOf rdf:resource="http://www.essepuntato.it/2008/12/pattern#Container"/>
        <rdfs:comment xml:lang="en">A space within a document that contains textual content relating to, quoting from or expanding upon the main text. Usually a textbox is delimited by a border or use of a background colour distinct from that of the main text.</rdfs:comment>
        <rdfs:label xml:lang="en">text box</rdfs:label>
    </owl:Class>
    


    <!-- http://purl.org/spar/doco/Title -->

    <owl:Class rdf:about="http://purl.org/spar/doco/Title">
        <rdfs:subClassOf rdf:resource="http://purl.org/spar/deo/DiscourseElement"/>
        <rdfs:subClassOf rdf:resource="https://raw.githubusercontent.com/BOberreither/INTRO/master/INTRO_outdated.owl#FormalEntity"/>
        <rdfs:subClassOf>
            <owl:Restriction>
                <owl:onProperty rdf:resource="http://www.essepuntato.it/2008/12/pattern#isContainedByAsHeader"/>
                <owl:someValuesFrom rdf:resource="http://www.essepuntato.it/2008/12/pattern#HeadedContainer"/>
            </owl:Restriction>
        </rdfs:subClassOf>
        <rdfs:comment xml:lang="en">A word, phrase or sentence that precedes and indicates the subject of a document or a document component - e.g., a book, a report, a news article, a chapter, a section or a table.</rdfs:comment>
        <rdfs:label xml:lang="en">title</rdfs:label>
    </owl:Class>
    


    <!-- http://salt.semanticauthoring.org/ontologies/sro#Conclusion -->

    <owl:Class rdf:about="http://salt.semanticauthoring.org/ontologies/sro#Conclusion">
        <rdfs:subClassOf rdf:resource="https://raw.githubusercontent.com/BOberreither/INTRO/master/INTRO_outdated.owl#PragmaticEntity"/>
    </owl:Class>
    


    <!-- http://salt.semanticauthoring.org/ontologies/sro#Contribution -->

    <owl:Class rdf:about="http://salt.semanticauthoring.org/ontologies/sro#Contribution">
        <rdfs:subClassOf rdf:resource="https://raw.githubusercontent.com/BOberreither/INTRO/master/INTRO_outdated.owl#PragmaticEntity"/>
    </owl:Class>
    


    <!-- http://salt.semanticauthoring.org/ontologies/sro#Discussion -->

    <owl:Class rdf:about="http://salt.semanticauthoring.org/ontologies/sro#Discussion">
        <rdfs:subClassOf rdf:resource="https://raw.githubusercontent.com/BOberreither/INTRO/master/INTRO_outdated.owl#PragmaticEntity"/>
    </owl:Class>
    


    <!-- http://salt.semanticauthoring.org/ontologies/sro#Evaluation -->

    <owl:Class rdf:about="http://salt.semanticauthoring.org/ontologies/sro#Evaluation">
        <rdfs:subClassOf rdf:resource="https://raw.githubusercontent.com/BOberreither/INTRO/master/INTRO_outdated.owl#PragmaticEntity"/>
    </owl:Class>
    


    <!-- http://salt.semanticauthoring.org/ontologies/sro#Motivation -->

    <owl:Class rdf:about="http://salt.semanticauthoring.org/ontologies/sro#Motivation">
        <rdfs:subClassOf rdf:resource="https://raw.githubusercontent.com/BOberreither/INTRO/master/INTRO_outdated.owl#PragmaticEntity"/>
    </owl:Class>
    


    <!-- http://salt.semanticauthoring.org/ontologies/sro#Scenario -->

    <owl:Class rdf:about="http://salt.semanticauthoring.org/ontologies/sro#Scenario">
        <rdfs:subClassOf rdf:resource="https://raw.githubusercontent.com/BOberreither/INTRO/master/INTRO_outdated.owl#PragmaticEntity"/>
    </owl:Class>
    


    <!-- http://www.cidoc-crm.org/cidoc-crm/E18_Physical_Thing -->

    <owl:Class rdf:about="http://www.cidoc-crm.org/cidoc-crm/E18_Physical_Thing">
        <rdfs:subClassOf rdf:resource="http://www.cidoc-crm.org/cidoc-crm/E72_Legal_Object"/>
    </owl:Class>
    


    <!-- http://www.cidoc-crm.org/cidoc-crm/E24_Physical_Man-Made_Thing -->

    <owl:Class rdf:about="http://www.cidoc-crm.org/cidoc-crm/E24_Physical_Man-Made_Thing">
        <rdfs:subClassOf rdf:resource="http://www.cidoc-crm.org/cidoc-crm/E18_Physical_Thing"/>
    </owl:Class>
    


    <!-- http://www.cidoc-crm.org/cidoc-crm/E28_Conceptual_Object -->

    <owl:Class rdf:about="http://www.cidoc-crm.org/cidoc-crm/E28_Conceptual_Object">
        <rdfs:subClassOf rdf:resource="http://www.cidoc-crm.org/cidoc-crm/E71_Man-Made_Thing"/>
    </owl:Class>
    


    <!-- http://www.cidoc-crm.org/cidoc-crm/E55_Type -->

    <owl:Class rdf:about="http://www.cidoc-crm.org/cidoc-crm/E55_Type">
        <rdfs:subClassOf rdf:resource="http://www.cidoc-crm.org/cidoc-crm/E28_Conceptual_Object"/>
    </owl:Class>
    


    <!-- http://www.cidoc-crm.org/cidoc-crm/E70_Thing -->

    <owl:Class rdf:about="http://www.cidoc-crm.org/cidoc-crm/E70_Thing">
        <rdfs:subClassOf>
            <owl:Restriction>
                <owl:onProperty rdf:resource="https://raw.githubusercontent.com/BOberreither/INTRO/master/INTRO_outdated.owl#isOpinionObjectOf"/>
                <owl:allValuesFrom rdf:resource="https://raw.githubusercontent.com/BOberreither/INTRO/master/INTRO_outdated.owl#Opinion"/>
            </owl:Restriction>
        </rdfs:subClassOf>
    </owl:Class>
    


    <!-- http://www.cidoc-crm.org/cidoc-crm/E71_Man-Made_Thing -->

    <owl:Class rdf:about="http://www.cidoc-crm.org/cidoc-crm/E71_Man-Made_Thing">
        <rdfs:subClassOf rdf:resource="http://www.cidoc-crm.org/cidoc-crm/E70_Thing"/>
    </owl:Class>
    


    <!-- http://www.cidoc-crm.org/cidoc-crm/E72_Legal_Object -->

    <owl:Class rdf:about="http://www.cidoc-crm.org/cidoc-crm/E72_Legal_Object">
        <rdfs:subClassOf rdf:resource="http://www.cidoc-crm.org/cidoc-crm/E70_Thing"/>
    </owl:Class>
    


    <!-- http://www.cidoc-crm.org/cidoc-crm/E73_Information_Object -->

    <owl:Class rdf:about="http://www.cidoc-crm.org/cidoc-crm/E73_Information_Object">
        <rdfs:subClassOf rdf:resource="http://www.cidoc-crm.org/cidoc-crm/E89_Propositional_Object"/>
        <rdfs:subClassOf rdf:resource="http://www.cidoc-crm.org/cidoc-crm/E90_Symbolic_Object"/>
    </owl:Class>
    


    <!-- http://www.cidoc-crm.org/cidoc-crm/E89_Propositional_Object -->

    <owl:Class rdf:about="http://www.cidoc-crm.org/cidoc-crm/E89_Propositional_Object">
        <rdfs:subClassOf rdf:resource="http://www.cidoc-crm.org/cidoc-crm/E28_Conceptual_Object"/>
    </owl:Class>
    


    <!-- http://www.cidoc-crm.org/cidoc-crm/E90_Symbolic_Object -->

    <owl:Class rdf:about="http://www.cidoc-crm.org/cidoc-crm/E90_Symbolic_Object">
        <rdfs:subClassOf rdf:resource="http://www.cidoc-crm.org/cidoc-crm/E28_Conceptual_Object"/>
        <rdfs:subClassOf rdf:resource="http://www.cidoc-crm.org/cidoc-crm/E72_Legal_Object"/>
    </owl:Class>
    


    <!-- http://www.essepuntato.it/2008/12/pattern#Container -->

    <owl:Class rdf:about="http://www.essepuntato.it/2008/12/pattern#Container">
        <rdfs:subClassOf rdf:resource="https://raw.githubusercontent.com/BOberreither/INTRO/master/INTRO_outdated.owl#PragmaticEntity"/>
    </owl:Class>
    


    <!-- http://www.essepuntato.it/2008/12/pattern#Field -->

    <owl:Class rdf:about="http://www.essepuntato.it/2008/12/pattern#Field">
        <rdfs:subClassOf rdf:resource="https://raw.githubusercontent.com/BOberreither/INTRO/master/INTRO_outdated.owl#PragmaticEntity"/>
    </owl:Class>
    


    <!-- http://www.essepuntato.it/2008/12/pattern#HeadedContainer -->

    <owl:Class rdf:about="http://www.essepuntato.it/2008/12/pattern#HeadedContainer">
        <rdfs:subClassOf rdf:resource="https://raw.githubusercontent.com/BOberreither/INTRO/master/INTRO_outdated.owl#PragmaticEntity"/>
    </owl:Class>
    


    <!-- http://www.essepuntato.it/2008/12/pattern#Meta -->

    <owl:Class rdf:about="http://www.essepuntato.it/2008/12/pattern#Meta">
        <rdfs:subClassOf rdf:resource="https://raw.githubusercontent.com/BOberreither/INTRO/master/INTRO_outdated.owl#PragmaticEntity"/>
    </owl:Class>
    


    <!-- http://www.essepuntato.it/2008/12/pattern#Milestone -->

    <owl:Class rdf:about="http://www.essepuntato.it/2008/12/pattern#Milestone">
        <rdfs:subClassOf rdf:resource="https://raw.githubusercontent.com/BOberreither/INTRO/master/INTRO_outdated.owl#PragmaticEntity"/>
    </owl:Class>
    


    <!-- http://www.essepuntato.it/2008/12/pattern#Pattern -->

    <owl:Class rdf:about="http://www.essepuntato.it/2008/12/pattern#Pattern">
        <rdfs:subClassOf rdf:resource="https://raw.githubusercontent.com/BOberreither/INTRO/master/INTRO_outdated.owl#PragmaticEntity"/>
    </owl:Class>
    


    <!-- http://www.essepuntato.it/2008/12/pattern#Popup -->

    <owl:Class rdf:about="http://www.essepuntato.it/2008/12/pattern#Popup">
        <rdfs:subClassOf rdf:resource="https://raw.githubusercontent.com/BOberreither/INTRO/master/INTRO_outdated.owl#PragmaticEntity"/>
    </owl:Class>
    


    <!-- http://www.essepuntato.it/2008/12/pattern#Table -->

    <owl:Class rdf:about="http://www.essepuntato.it/2008/12/pattern#Table">
        <rdfs:subClassOf rdf:resource="https://raw.githubusercontent.com/BOberreither/INTRO/master/INTRO_outdated.owl#FormalEntity"/>
        <rdfs:subClassOf rdf:resource="https://raw.githubusercontent.com/BOberreither/INTRO/master/INTRO_outdated.owl#PragmaticEntity"/>
    </owl:Class>
    


    <!-- https://raw.githubusercontent.com/BOberreither/INTRO/master/INTRO_outdated.owl#Act -->

    <owl:Class rdf:about="https://raw.githubusercontent.com/BOberreither/INTRO/master/INTRO_outdated.owl#Act">
        <rdfs:subClassOf rdf:resource="https://raw.githubusercontent.com/BOberreither/INTRO/master/INTRO_outdated.owl#FormalEntity"/>
        <rdfs:label>Act (Drama)</rdfs:label>
    </owl:Class>
    


    <!-- https://raw.githubusercontent.com/BOberreither/INTRO/master/INTRO_outdated.owl#ActualizationOfFeature -->

    <owl:Class rdf:about="https://raw.githubusercontent.com/BOberreither/INTRO/master/INTRO_outdated.owl#ActualizationOfFeature">
        <rdfs:subClassOf rdf:resource="http://www.cidoc-crm.org/cidoc-crm/E28_Conceptual_Object"/>
        <rdfs:subClassOf>
            <owl:Restriction>
                <owl:onProperty rdf:resource="https://raw.githubusercontent.com/BOberreither/INTRO/master/INTRO_outdated.owl#actualizationFoundOn"/>
                <owl:allValuesFrom>
                    <owl:Class>
                        <owl:unionOf rdf:parseType="Collection">
                            <rdf:Description rdf:about="http://iflastandards.info/ns/fr/frbr/frbroo/F1_Work"/>
                            <rdf:Description rdf:about="http://iflastandards.info/ns/fr/frbr/frbroo/F22_Self-Contained_Expression"/>
                            <rdf:Description rdf:about="http://iflastandards.info/ns/fr/frbr/frbroo/F23_Expression_Fragment"/>
                            <rdf:Description rdf:about="http://iflastandards.info/ns/fr/frbr/frbroo/F2_Expression"/>
                            <rdf:Description rdf:about="http://iflastandards.info/ns/fr/frbr/frbroo/F3_Manifestation_Product_Type"/>
                            <rdf:Description rdf:about="https://raw.githubusercontent.com/BOberreither/INTRO/master/INTRO_outdated.owl#ArchitextualEntity"/>
                            <rdf:Description rdf:about="https://raw.githubusercontent.com/BOberreither/INTRO/master/INTRO_outdated.owl#ManifestationProductTypeFragment"/>
                        </owl:unionOf>
                    </owl:Class>
                </owl:allValuesFrom>
            </owl:Restriction>
        </rdfs:subClassOf>
        <rdfs:subClassOf>
            <owl:Restriction>
                <owl:onProperty rdf:resource="https://raw.githubusercontent.com/BOberreither/INTRO/master/INTRO_outdated.owl#actualizesFeature"/>
                <owl:allValuesFrom rdf:resource="https://raw.githubusercontent.com/BOberreither/INTRO/master/INTRO_outdated.owl#ReceptionalEntity"/>
            </owl:Restriction>
        </rdfs:subClassOf>
        <rdfs:subClassOf>
            <owl:Restriction>
                <owl:onProperty rdf:resource="https://raw.githubusercontent.com/BOberreither/INTRO/master/INTRO_outdated.owl#actualizesFormalFeature"/>
                <owl:allValuesFrom rdf:resource="https://raw.githubusercontent.com/BOberreither/INTRO/master/INTRO_outdated.owl#FormalEntity"/>
            </owl:Restriction>
        </rdfs:subClassOf>
        <rdfs:subClassOf>
            <owl:Restriction>
                <owl:onProperty rdf:resource="https://raw.githubusercontent.com/BOberreither/INTRO/master/INTRO_outdated.owl#actualizesRhetoricalFeature"/>
                <owl:allValuesFrom rdf:resource="https://raw.githubusercontent.com/BOberreither/INTRO/master/INTRO_outdated.owl#RhetoricalEntity"/>
            </owl:Restriction>
        </rdfs:subClassOf>
        <rdfs:subClassOf>
            <owl:Restriction>
                <owl:onProperty rdf:resource="https://raw.githubusercontent.com/BOberreither/INTRO/master/INTRO_outdated.owl#actualizesSemanticFeature"/>
                <owl:allValuesFrom rdf:resource="https://raw.githubusercontent.com/BOberreither/INTRO/master/INTRO_outdated.owl#SemanticEntity"/>
            </owl:Restriction>
        </rdfs:subClassOf>
        <rdfs:subClassOf>
            <owl:Restriction>
                <owl:onProperty rdf:resource="https://raw.githubusercontent.com/BOberreither/INTRO/master/INTRO_outdated.owl#constitutes"/>
                <owl:allValuesFrom>
                    <owl:Class>
                        <owl:unionOf rdf:parseType="Collection">
                            <rdf:Description rdf:about="https://raw.githubusercontent.com/BOberreither/INTRO/master/INTRO_outdated.owl#Characteristic"/>
                            <rdf:Description rdf:about="https://raw.githubusercontent.com/BOberreither/INTRO/master/INTRO_outdated.owl#Interpretament"/>
                        </owl:unionOf>
                    </owl:Class>
                </owl:allValuesFrom>
            </owl:Restriction>
        </rdfs:subClassOf>
        <rdfs:subClassOf>
            <owl:Restriction>
                <owl:onProperty rdf:resource="https://raw.githubusercontent.com/BOberreither/INTRO/master/INTRO_outdated.owl#isConstellatedBy"/>
                <owl:allValuesFrom rdf:resource="https://raw.githubusercontent.com/BOberreither/INTRO/master/INTRO_outdated.owl#Constellation"/>
            </owl:Restriction>
        </rdfs:subClassOf>
        <rdfs:subClassOf>
            <owl:Restriction>
                <owl:onProperty rdf:resource="https://raw.githubusercontent.com/BOberreither/INTRO/master/INTRO_outdated.owl#isIdentifiedBy"/>
                <owl:allValuesFrom rdf:resource="https://raw.githubusercontent.com/BOberreither/INTRO/master/INTRO_outdated.owl#Interpretament"/>
            </owl:Restriction>
        </rdfs:subClassOf>
        <rdfs:subClassOf>
            <owl:Restriction>
                <owl:onProperty rdf:resource="https://raw.githubusercontent.com/BOberreither/INTRO/master/INTRO_outdated.owl#supportProvidedBy"/>
                <owl:allValuesFrom>
                    <owl:Class>
                        <owl:unionOf rdf:parseType="Collection">
                            <rdf:Description rdf:about="http://iflastandards.info/ns/fr/frbr/frbroo/F1_Work"/>
                            <rdf:Description rdf:about="http://iflastandards.info/ns/fr/frbr/frbroo/F22_Self-Contained_Expression"/>
                            <rdf:Description rdf:about="http://iflastandards.info/ns/fr/frbr/frbroo/F23_Expression_Fragment"/>
                            <rdf:Description rdf:about="http://iflastandards.info/ns/fr/frbr/frbroo/F2_Expression"/>
                            <rdf:Description rdf:about="http://iflastandards.info/ns/fr/frbr/frbroo/F3_Manifestation_Product_Type"/>
                            <rdf:Description rdf:about="https://raw.githubusercontent.com/BOberreither/INTRO/master/INTRO_outdated.owl#ArchitextualEntity"/>
                            <rdf:Description rdf:about="https://raw.githubusercontent.com/BOberreither/INTRO/master/INTRO_outdated.owl#ManifestationProductTypeFragment"/>
                        </owl:unionOf>
                    </owl:Class>
                </owl:allValuesFrom>
            </owl:Restriction>
        </rdfs:subClassOf>
        <rdfs:subClassOf>
            <owl:Restriction>
                <owl:onProperty rdf:resource="https://raw.githubusercontent.com/BOberreither/INTRO/master/INTRO_outdated.owl#hasParaphraseOrDefinition"/>
                <owl:allValuesFrom rdf:resource="http://www.w3.org/2001/XMLSchema#string"/>
            </owl:Restriction>
        </rdfs:subClassOf>
        <rdfs:comment>The fact that a certain text shows - in its own specific way - a certain feature (which itself is an abstract concept and takes form in many texts), e.g. a motif, an atmosphere, a theme, a figure of speech.

Examples:
- the specific actualization of the motif of patricide in Sophokle&apos;s &apos;Ödipus Rex&apos;.
- the specific actualization of the Faust-subject in Goethe&apos;s &apos;Faust&apos;.
- the specific actualization of the iambic pentameter in Rilke&apos;s &apos;Archaischer Torso Apollos&quot;.</rdfs:comment>
        <rdfs:label>Actualization of Feature</rdfs:label>
    </owl:Class>
    


    <!-- https://raw.githubusercontent.com/BOberreither/INTRO/master/INTRO_outdated.owl#ArchitextualEntity -->

    <owl:Class rdf:about="https://raw.githubusercontent.com/BOberreither/INTRO/master/INTRO_outdated.owl#ArchitextualEntity">
        <rdfs:subClassOf rdf:resource="http://www.cidoc-crm.org/cidoc-crm/E28_Conceptual_Object"/>
        <rdfs:subClassOf>
            <owl:Restriction>
                <owl:onProperty rdf:resource="https://raw.githubusercontent.com/BOberreither/INTRO/master/INTRO_outdated.owl#affiliationSupportedBy"/>
                <owl:allValuesFrom rdf:resource="https://raw.githubusercontent.com/BOberreither/INTRO/master/INTRO_outdated.owl#Characteristic"/>
            </owl:Restriction>
        </rdfs:subClassOf>
        <rdfs:subClassOf>
            <owl:Restriction>
                <owl:onProperty rdf:resource="https://raw.githubusercontent.com/BOberreither/INTRO/master/INTRO_outdated.owl#definitionProvidedBy"/>
                <owl:allValuesFrom rdf:resource="https://raw.githubusercontent.com/BOberreither/INTRO/master/INTRO_outdated.owl#ActualizationOfFeature"/>
            </owl:Restriction>
        </rdfs:subClassOf>
        <rdfs:subClassOf>
            <owl:Restriction>
                <owl:onProperty rdf:resource="https://raw.githubusercontent.com/BOberreither/INTRO/master/INTRO_outdated.owl#hasAppurtenantElement"/>
                <owl:allValuesFrom>
                    <owl:Class>
                        <owl:unionOf rdf:parseType="Collection">
                            <rdf:Description rdf:about="http://iflastandards.info/ns/fr/frbr/frbroo/F1_Work"/>
                            <rdf:Description rdf:about="http://iflastandards.info/ns/fr/frbr/frbroo/F22_Self-Contained_Expression"/>
                            <rdf:Description rdf:about="http://iflastandards.info/ns/fr/frbr/frbroo/F23_Expression_Fragment"/>
                            <rdf:Description rdf:about="http://iflastandards.info/ns/fr/frbr/frbroo/F2_Expression"/>
                            <rdf:Description rdf:about="http://iflastandards.info/ns/fr/frbr/frbroo/F3_Manifestation_Product_Type"/>
                            <rdf:Description rdf:about="https://raw.githubusercontent.com/BOberreither/INTRO/master/INTRO_outdated.owl#ArchitextualEntity"/>
                            <rdf:Description rdf:about="https://raw.githubusercontent.com/BOberreither/INTRO/master/INTRO_outdated.owl#ManifestationProductTypeFragment"/>
                        </owl:unionOf>
                    </owl:Class>
                </owl:allValuesFrom>
            </owl:Restriction>
        </rdfs:subClassOf>
        <rdfs:subClassOf>
            <owl:Restriction>
                <owl:onProperty rdf:resource="https://raw.githubusercontent.com/BOberreither/INTRO/master/INTRO_outdated.owl#hasInitialElement"/>
                <owl:allValuesFrom>
                    <owl:Class>
                        <owl:unionOf rdf:parseType="Collection">
                            <rdf:Description rdf:about="http://iflastandards.info/ns/fr/frbr/frbroo/F1_Work"/>
                            <rdf:Description rdf:about="http://iflastandards.info/ns/fr/frbr/frbroo/F22_Self-Contained_Expression"/>
                            <rdf:Description rdf:about="http://iflastandards.info/ns/fr/frbr/frbroo/F2_Expression"/>
                            <rdf:Description rdf:about="http://iflastandards.info/ns/fr/frbr/frbroo/F3_Manifestation_Product_Type"/>
                        </owl:unionOf>
                    </owl:Class>
                </owl:allValuesFrom>
            </owl:Restriction>
        </rdfs:subClassOf>
        <rdfs:subClassOf>
            <owl:Restriction>
                <owl:onProperty rdf:resource="https://raw.githubusercontent.com/BOberreither/INTRO/master/INTRO_outdated.owl#hasRepresentativeElement"/>
                <owl:allValuesFrom>
                    <owl:Class>
                        <owl:unionOf rdf:parseType="Collection">
                            <rdf:Description rdf:about="http://iflastandards.info/ns/fr/frbr/frbroo/F1_Work"/>
                            <rdf:Description rdf:about="http://iflastandards.info/ns/fr/frbr/frbroo/F22_Self-Contained_Expression"/>
                            <rdf:Description rdf:about="http://iflastandards.info/ns/fr/frbr/frbroo/F2_Expression"/>
                            <rdf:Description rdf:about="http://iflastandards.info/ns/fr/frbr/frbroo/F3_Manifestation_Product_Type"/>
                        </owl:unionOf>
                    </owl:Class>
                </owl:allValuesFrom>
            </owl:Restriction>
        </rdfs:subClassOf>
        <rdfs:subClassOf>
            <owl:Restriction>
                <owl:onProperty rdf:resource="https://raw.githubusercontent.com/BOberreither/INTRO/master/INTRO_outdated.owl#isAppurtenantElement"/>
                <owl:allValuesFrom rdf:resource="https://raw.githubusercontent.com/BOberreither/INTRO/master/INTRO_outdated.owl#ArchitextualEntity"/>
            </owl:Restriction>
        </rdfs:subClassOf>
        <rdfs:subClassOf>
            <owl:Restriction>
                <owl:onProperty rdf:resource="https://raw.githubusercontent.com/BOberreither/INTRO/master/INTRO_outdated.owl#isDiscussedIn"/>
                <owl:allValuesFrom rdf:resource="https://raw.githubusercontent.com/BOberreither/INTRO/master/INTRO_outdated.owl#Interpretament"/>
            </owl:Restriction>
        </rdfs:subClassOf>
        <rdfs:subClassOf>
            <owl:Restriction>
                <owl:onProperty rdf:resource="https://raw.githubusercontent.com/BOberreither/INTRO/master/INTRO_outdated.owl#isReferredToEntity"/>
                <owl:allValuesFrom rdf:resource="https://raw.githubusercontent.com/BOberreither/INTRO/master/INTRO_outdated.owl#Reference"/>
            </owl:Restriction>
        </rdfs:subClassOf>
        <rdfs:subClassOf>
            <owl:Restriction>
                <owl:onProperty rdf:resource="https://raw.githubusercontent.com/BOberreither/INTRO/master/INTRO_outdated.owl#isReferringEntity"/>
                <owl:allValuesFrom rdf:resource="https://raw.githubusercontent.com/BOberreither/INTRO/master/INTRO_outdated.owl#Reference"/>
            </owl:Restriction>
        </rdfs:subClassOf>
        <rdfs:subClassOf>
            <owl:Restriction>
                <owl:onProperty rdf:resource="https://raw.githubusercontent.com/BOberreither/INTRO/master/INTRO_outdated.owl#likenessSupportedBy"/>
                <owl:allValuesFrom rdf:resource="https://raw.githubusercontent.com/BOberreither/INTRO/master/INTRO_outdated.owl#Characteristic"/>
            </owl:Restriction>
        </rdfs:subClassOf>
        <rdfs:subClassOf>
            <owl:Restriction>
                <owl:onProperty rdf:resource="https://raw.githubusercontent.com/BOberreither/INTRO/master/INTRO_outdated.owl#nonAffiliationSupportedBy"/>
                <owl:allValuesFrom rdf:resource="https://raw.githubusercontent.com/BOberreither/INTRO/master/INTRO_outdated.owl#Characteristic"/>
            </owl:Restriction>
        </rdfs:subClassOf>
        <rdfs:subClassOf>
            <owl:Restriction>
                <owl:onProperty rdf:resource="https://raw.githubusercontent.com/BOberreither/INTRO/master/INTRO_outdated.owl#othernessSupportedBy"/>
                <owl:allValuesFrom rdf:resource="https://raw.githubusercontent.com/BOberreither/INTRO/master/INTRO_outdated.owl#Characteristic"/>
            </owl:Restriction>
        </rdfs:subClassOf>
        <rdfs:subClassOf>
            <owl:Restriction>
                <owl:onProperty rdf:resource="https://raw.githubusercontent.com/BOberreither/INTRO/master/INTRO_outdated.owl#providesSupportFor"/>
                <owl:allValuesFrom>
                    <owl:Class>
                        <owl:unionOf rdf:parseType="Collection">
                            <rdf:Description rdf:about="https://raw.githubusercontent.com/BOberreither/INTRO/master/INTRO_outdated.owl#ActualizationOfFeature"/>
                            <rdf:Description rdf:about="https://raw.githubusercontent.com/BOberreither/INTRO/master/INTRO_outdated.owl#Characteristic"/>
                            <rdf:Description rdf:about="https://raw.githubusercontent.com/BOberreither/INTRO/master/INTRO_outdated.owl#Interpretament"/>
                            <rdf:Description rdf:about="https://raw.githubusercontent.com/BOberreither/INTRO/master/INTRO_outdated.owl#Opinion"/>
                            <rdf:Description rdf:about="https://raw.githubusercontent.com/BOberreither/INTRO/master/INTRO_outdated.owl#Reference"/>
                            <rdf:Description rdf:about="https://raw.githubusercontent.com/BOberreither/INTRO/master/INTRO_outdated.owl#TypeOfIntertextualRelationship"/>
                        </owl:unionOf>
                    </owl:Class>
                </owl:allValuesFrom>
            </owl:Restriction>
        </rdfs:subClassOf>
        <rdfs:subClassOf>
            <owl:Restriction>
                <owl:onProperty rdf:resource="https://raw.githubusercontent.com/BOberreither/INTRO/master/INTRO_outdated.owl#showsActualization"/>
                <owl:allValuesFrom rdf:resource="https://raw.githubusercontent.com/BOberreither/INTRO/master/INTRO_outdated.owl#ActualizationOfFeature"/>
            </owl:Restriction>
        </rdfs:subClassOf>
        <rdfs:subClassOf>
            <owl:Restriction>
                <owl:onProperty rdf:resource="https://raw.githubusercontent.com/BOberreither/INTRO/master/INTRO_outdated.owl#showsCharacteristics"/>
                <owl:allValuesFrom rdf:resource="https://raw.githubusercontent.com/BOberreither/INTRO/master/INTRO_outdated.owl#Characteristic"/>
            </owl:Restriction>
        </rdfs:subClassOf>
        <rdfs:subClassOf>
            <owl:Restriction>
                <owl:onProperty rdf:resource="https://raw.githubusercontent.com/BOberreither/INTRO/master/INTRO_outdated.owl#hasParaphraseOrDefinition"/>
                <owl:allValuesFrom rdf:resource="http://www.w3.org/2001/XMLSchema#string"/>
            </owl:Restriction>
        </rdfs:subClassOf>
        <rdfs:comment>A transtextual entity consists in a number of texts which in some way give reason to see them as connected, related, sharing a common feature.
Examples for transtextual entities can be disourses (texts sharing a discousive element, a topic etc.), genres (texts sharing genre conventions), a discipline (texts deriving from the same disciplinary background), an oeuvre (texts written by the same person), national literatures (texts whose authors share a nationality) etc.</rdfs:comment>
        <rdfs:label>Architextual Entity</rdfs:label>
    </owl:Class>
    


    <!-- https://raw.githubusercontent.com/BOberreither/INTRO/master/INTRO_outdated.owl#Atmosphere -->

    <owl:Class rdf:about="https://raw.githubusercontent.com/BOberreither/INTRO/master/INTRO_outdated.owl#Atmosphere">
        <rdfs:subClassOf rdf:resource="https://raw.githubusercontent.com/BOberreither/INTRO/master/INTRO_outdated.owl#SemanticEntity"/>
    </owl:Class>
    


    <!-- https://raw.githubusercontent.com/BOberreither/INTRO/master/INTRO_outdated.owl#Bachtin -->

    <owl:Class rdf:about="https://raw.githubusercontent.com/BOberreither/INTRO/master/INTRO_outdated.owl#Bachtin">
        <rdfs:subClassOf rdf:resource="https://raw.githubusercontent.com/BOberreither/INTRO/master/INTRO_outdated.owl#IntertextualTheory"/>
    </owl:Class>
    


    <!-- https://raw.githubusercontent.com/BOberreither/INTRO/master/INTRO_outdated.owl#Barthes -->

    <owl:Class rdf:about="https://raw.githubusercontent.com/BOberreither/INTRO/master/INTRO_outdated.owl#Barthes">
        <rdfs:subClassOf rdf:resource="https://raw.githubusercontent.com/BOberreither/INTRO/master/INTRO_outdated.owl#IntertextualTheory"/>
    </owl:Class>
    


    <!-- https://raw.githubusercontent.com/BOberreither/INTRO/master/INTRO_outdated.owl#Bassler -->

    <owl:Class rdf:about="https://raw.githubusercontent.com/BOberreither/INTRO/master/INTRO_outdated.owl#Bassler">
        <rdfs:subClassOf rdf:resource="https://raw.githubusercontent.com/BOberreither/INTRO/master/INTRO_outdated.owl#IntertextualTheory"/>
    </owl:Class>
    


    <!-- https://raw.githubusercontent.com/BOberreither/INTRO/master/INTRO_outdated.owl#Bloom -->

    <owl:Class rdf:about="https://raw.githubusercontent.com/BOberreither/INTRO/master/INTRO_outdated.owl#Bloom">
        <rdfs:subClassOf rdf:resource="https://raw.githubusercontent.com/BOberreither/INTRO/master/INTRO_outdated.owl#IntertextualTheory"/>
    </owl:Class>
    


    <!-- https://raw.githubusercontent.com/BOberreither/INTRO/master/INTRO_outdated.owl#BroichPfister -->

    <owl:Class rdf:about="https://raw.githubusercontent.com/BOberreither/INTRO/master/INTRO_outdated.owl#BroichPfister">
        <rdfs:subClassOf rdf:resource="https://raw.githubusercontent.com/BOberreither/INTRO/master/INTRO_outdated.owl#IntertextualTheory"/>
    </owl:Class>
    


    <!-- https://raw.githubusercontent.com/BOberreither/INTRO/master/INTRO_outdated.owl#Bronfen -->

    <owl:Class rdf:about="https://raw.githubusercontent.com/BOberreither/INTRO/master/INTRO_outdated.owl#Bronfen">
        <rdfs:subClassOf rdf:resource="https://raw.githubusercontent.com/BOberreither/INTRO/master/INTRO_outdated.owl#IntertextualTheory"/>
    </owl:Class>
    


    <!-- https://raw.githubusercontent.com/BOberreither/INTRO/master/INTRO_outdated.owl#ChapterSubtitle -->

    <owl:Class rdf:about="https://raw.githubusercontent.com/BOberreither/INTRO/master/INTRO_outdated.owl#ChapterSubtitle">
        <rdfs:subClassOf rdf:resource="https://raw.githubusercontent.com/BOberreither/INTRO/master/INTRO_outdated.owl#Subtitle"/>
    </owl:Class>
    


    <!-- https://raw.githubusercontent.com/BOberreither/INTRO/master/INTRO_outdated.owl#Character -->

    <owl:Class rdf:about="https://raw.githubusercontent.com/BOberreither/INTRO/master/INTRO_outdated.owl#Character">
        <rdfs:subClassOf rdf:resource="https://raw.githubusercontent.com/BOberreither/INTRO/master/INTRO_outdated.owl#SemanticEntity"/>
    </owl:Class>
    


    <!-- https://raw.githubusercontent.com/BOberreither/INTRO/master/INTRO_outdated.owl#Characteristic -->

    <owl:Class rdf:about="https://raw.githubusercontent.com/BOberreither/INTRO/master/INTRO_outdated.owl#Characteristic">
        <rdfs:subClassOf rdf:resource="http://www.cidoc-crm.org/cidoc-crm/E28_Conceptual_Object"/>
        <rdfs:subClassOf>
            <owl:Restriction>
                <owl:onProperty rdf:resource="https://raw.githubusercontent.com/BOberreither/INTRO/master/INTRO_outdated.owl#characteristicShownBy"/>
                <owl:allValuesFrom>
                    <owl:Class>
                        <owl:unionOf rdf:parseType="Collection">
                            <rdf:Description rdf:about="http://iflastandards.info/ns/fr/frbr/frbroo/F1_Work"/>
                            <rdf:Description rdf:about="http://iflastandards.info/ns/fr/frbr/frbroo/F22_Self-Contained_Expression"/>
                            <rdf:Description rdf:about="http://iflastandards.info/ns/fr/frbr/frbroo/F23_Expression_Fragment"/>
                            <rdf:Description rdf:about="http://iflastandards.info/ns/fr/frbr/frbroo/F2_Expression"/>
                            <rdf:Description rdf:about="http://iflastandards.info/ns/fr/frbr/frbroo/F3_Manifestation_Product_Type"/>
                            <rdf:Description rdf:about="https://raw.githubusercontent.com/BOberreither/INTRO/master/INTRO_outdated.owl#ArchitextualEntity"/>
                            <rdf:Description rdf:about="https://raw.githubusercontent.com/BOberreither/INTRO/master/INTRO_outdated.owl#ManifestationProductTypeFragment"/>
                        </owl:unionOf>
                    </owl:Class>
                </owl:allValuesFrom>
            </owl:Restriction>
        </rdfs:subClassOf>
        <rdfs:subClassOf>
            <owl:Restriction>
                <owl:onProperty rdf:resource="https://raw.githubusercontent.com/BOberreither/INTRO/master/INTRO_outdated.owl#consistsIn"/>
                <owl:allValuesFrom rdf:resource="https://raw.githubusercontent.com/BOberreither/INTRO/master/INTRO_outdated.owl#ActualizationOfFeature"/>
            </owl:Restriction>
        </rdfs:subClassOf>
        <rdfs:subClassOf>
            <owl:Restriction>
                <owl:onProperty rdf:resource="https://raw.githubusercontent.com/BOberreither/INTRO/master/INTRO_outdated.owl#isIdentifiedBy"/>
                <owl:allValuesFrom rdf:resource="https://raw.githubusercontent.com/BOberreither/INTRO/master/INTRO_outdated.owl#Interpretament"/>
            </owl:Restriction>
        </rdfs:subClassOf>
        <rdfs:subClassOf>
            <owl:Restriction>
                <owl:onProperty rdf:resource="https://raw.githubusercontent.com/BOberreither/INTRO/master/INTRO_outdated.owl#supportProvidedBy"/>
                <owl:allValuesFrom>
                    <owl:Class>
                        <owl:unionOf rdf:parseType="Collection">
                            <rdf:Description rdf:about="http://iflastandards.info/ns/fr/frbr/frbroo/F1_Work"/>
                            <rdf:Description rdf:about="http://iflastandards.info/ns/fr/frbr/frbroo/F22_Self-Contained_Expression"/>
                            <rdf:Description rdf:about="http://iflastandards.info/ns/fr/frbr/frbroo/F23_Expression_Fragment"/>
                            <rdf:Description rdf:about="http://iflastandards.info/ns/fr/frbr/frbroo/F2_Expression"/>
                            <rdf:Description rdf:about="http://iflastandards.info/ns/fr/frbr/frbroo/F3_Manifestation_Product_Type"/>
                            <rdf:Description rdf:about="https://raw.githubusercontent.com/BOberreither/INTRO/master/INTRO_outdated.owl#ArchitextualEntity"/>
                            <rdf:Description rdf:about="https://raw.githubusercontent.com/BOberreither/INTRO/master/INTRO_outdated.owl#ManifestationProductTypeFragment"/>
                        </owl:unionOf>
                    </owl:Class>
                </owl:allValuesFrom>
            </owl:Restriction>
        </rdfs:subClassOf>
        <rdfs:subClassOf>
            <owl:Restriction>
                <owl:onProperty rdf:resource="https://raw.githubusercontent.com/BOberreither/INTRO/master/INTRO_outdated.owl#supportsAffiliationTo"/>
                <owl:allValuesFrom rdf:resource="https://raw.githubusercontent.com/BOberreither/INTRO/master/INTRO_outdated.owl#ArchitextualEntity"/>
            </owl:Restriction>
        </rdfs:subClassOf>
        <rdfs:subClassOf>
            <owl:Restriction>
                <owl:onProperty rdf:resource="https://raw.githubusercontent.com/BOberreither/INTRO/master/INTRO_outdated.owl#supportsLikenessTo"/>
                <owl:allValuesFrom rdf:resource="https://raw.githubusercontent.com/BOberreither/INTRO/master/INTRO_outdated.owl#ArchitextualEntity"/>
            </owl:Restriction>
        </rdfs:subClassOf>
        <rdfs:subClassOf>
            <owl:Restriction>
                <owl:onProperty rdf:resource="https://raw.githubusercontent.com/BOberreither/INTRO/master/INTRO_outdated.owl#supportsNonAffiliationTo"/>
                <owl:allValuesFrom rdf:resource="https://raw.githubusercontent.com/BOberreither/INTRO/master/INTRO_outdated.owl#ArchitextualEntity"/>
            </owl:Restriction>
        </rdfs:subClassOf>
        <rdfs:subClassOf>
            <owl:Restriction>
                <owl:onProperty rdf:resource="https://raw.githubusercontent.com/BOberreither/INTRO/master/INTRO_outdated.owl#supportsOthernessTo"/>
                <owl:allValuesFrom rdf:resource="https://raw.githubusercontent.com/BOberreither/INTRO/master/INTRO_outdated.owl#ArchitextualEntity"/>
            </owl:Restriction>
        </rdfs:subClassOf>
        <rdfs:subClassOf>
            <owl:Restriction>
                <owl:onProperty rdf:resource="https://raw.githubusercontent.com/BOberreither/INTRO/master/INTRO_outdated.owl#hasParaphraseOrDefinition"/>
                <owl:allValuesFrom rdf:resource="http://www.w3.org/2001/XMLSchema#string"/>
            </owl:Restriction>
        </rdfs:subClassOf>
        <rdfs:comment>The concept that (the actualization of) a certain feature can indicate to a text&apos;s affiliation to a transtextual entity. A Characteristic is identified in an interpretative and is thus itself based on text.

Examples:
- how (the actualization of) the theme &apos;fashion&apos; in many german novels from 1995 to 2001 supports their affiliation to the movement (or school, or epoch) &apos;German Pop Literature&apos;.
- how (the actualization of) the detective character in Wolf Haas&apos; &apos;Silentium&apos; supports the novel&apos;s affiliation to the genre &apos;hardboiled crime fiction&apos;.</rdfs:comment>
        <rdfs:label>Characteristic</rdfs:label>
    </owl:Class>
    


    <!-- https://raw.githubusercontent.com/BOberreither/INTRO/master/INTRO_outdated.owl#Citation -->

    <owl:Class rdf:about="https://raw.githubusercontent.com/BOberreither/INTRO/master/INTRO_outdated.owl#Citation">
        <rdfs:subClassOf rdf:resource="https://raw.githubusercontent.com/BOberreither/INTRO/master/INTRO_outdated.owl#PragmaticEntity"/>
    </owl:Class>
    


    <!-- https://raw.githubusercontent.com/BOberreither/INTRO/master/INTRO_outdated.owl#Constellation -->

    <owl:Class rdf:about="https://raw.githubusercontent.com/BOberreither/INTRO/master/INTRO_outdated.owl#Constellation">
        <rdfs:subClassOf rdf:resource="https://raw.githubusercontent.com/BOberreither/INTRO/master/INTRO_outdated.owl#SemanticEntity"/>
        <rdfs:subClassOf>
            <owl:Restriction>
                <owl:onProperty rdf:resource="https://raw.githubusercontent.com/BOberreither/INTRO/master/INTRO_outdated.owl#constellates"/>
                <owl:minQualifiedCardinality rdf:datatype="http://www.w3.org/2001/XMLSchema#nonNegativeInteger">2</owl:minQualifiedCardinality>
                <owl:onClass rdf:resource="https://raw.githubusercontent.com/BOberreither/INTRO/master/INTRO_outdated.owl#ActualizationOfFeature"/>
            </owl:Restriction>
        </rdfs:subClassOf>
        <rdfs:subClassOf>
            <owl:Restriction>
                <owl:onProperty rdf:resource="https://raw.githubusercontent.com/BOberreither/INTRO/master/INTRO_outdated.owl#hasSpecification"/>
                <owl:allValuesFrom rdf:resource="http://www.w3.org/2001/XMLSchema#string"/>
            </owl:Restriction>
        </rdfs:subClassOf>
    </owl:Class>
    


    <!-- https://raw.githubusercontent.com/BOberreither/INTRO/master/INTRO_outdated.owl#Culler -->

    <owl:Class rdf:about="https://raw.githubusercontent.com/BOberreither/INTRO/master/INTRO_outdated.owl#Culler">
        <rdfs:subClassOf rdf:resource="https://raw.githubusercontent.com/BOberreither/INTRO/master/INTRO_outdated.owl#IntertextualTheory"/>
    </owl:Class>
    


    <!-- https://raw.githubusercontent.com/BOberreither/INTRO/master/INTRO_outdated.owl#Definition -->

    <owl:Class rdf:about="https://raw.githubusercontent.com/BOberreither/INTRO/master/INTRO_outdated.owl#Definition">
        <rdfs:subClassOf rdf:resource="https://raw.githubusercontent.com/BOberreither/INTRO/master/INTRO_outdated.owl#PragmaticEntity"/>
        <rdfs:subClassOf rdf:resource="https://raw.githubusercontent.com/BOberreither/INTRO/master/INTRO_outdated.owl#SemanticEntity"/>
    </owl:Class>
    


    <!-- https://raw.githubusercontent.com/BOberreither/INTRO/master/INTRO_outdated.owl#Description -->

    <owl:Class rdf:about="https://raw.githubusercontent.com/BOberreither/INTRO/master/INTRO_outdated.owl#Description">
        <rdfs:subClassOf rdf:resource="https://raw.githubusercontent.com/BOberreither/INTRO/master/INTRO_outdated.owl#SemanticEntity"/>
    </owl:Class>
    


    <!-- https://raw.githubusercontent.com/BOberreither/INTRO/master/INTRO_outdated.owl#Discipline -->

    <owl:Class rdf:about="https://raw.githubusercontent.com/BOberreither/INTRO/master/INTRO_outdated.owl#Discipline">
        <rdfs:subClassOf rdf:resource="https://raw.githubusercontent.com/BOberreither/INTRO/master/INTRO_outdated.owl#ArchitextualEntity"/>
    </owl:Class>
    


    <!-- https://raw.githubusercontent.com/BOberreither/INTRO/master/INTRO_outdated.owl#Discourse -->

    <owl:Class rdf:about="https://raw.githubusercontent.com/BOberreither/INTRO/master/INTRO_outdated.owl#Discourse">
        <rdfs:subClassOf rdf:resource="https://raw.githubusercontent.com/BOberreither/INTRO/master/INTRO_outdated.owl#ArchitextualEntity"/>
    </owl:Class>
    


    <!-- https://raw.githubusercontent.com/BOberreither/INTRO/master/INTRO_outdated.owl#Epoch -->

    <owl:Class rdf:about="https://raw.githubusercontent.com/BOberreither/INTRO/master/INTRO_outdated.owl#Epoch">
        <rdfs:subClassOf rdf:resource="https://raw.githubusercontent.com/BOberreither/INTRO/master/INTRO_outdated.owl#ArchitextualEntity"/>
    </owl:Class>
    


    <!-- https://raw.githubusercontent.com/BOberreither/INTRO/master/INTRO_outdated.owl#FigureOfSpeech -->

    <owl:Class rdf:about="https://raw.githubusercontent.com/BOberreither/INTRO/master/INTRO_outdated.owl#FigureOfSpeech">
        <rdfs:subClassOf rdf:resource="https://raw.githubusercontent.com/BOberreither/INTRO/master/INTRO_outdated.owl#RhetoricalEntity"/>
        <rdfs:comment>The class comprises figures of speech. Since there are countless classification systems (the most common dividing figures into tropoi - metaphor, metonymy ... - and schemata/figurae, further dividing the latter into figures of thougth and figures of word, further dividing the latter into grammatical and rhetorical figures of word), no subclasses will be provided.</rdfs:comment>
        <rdfs:label>Figure of Speech</rdfs:label>
    </owl:Class>
    


    <!-- https://raw.githubusercontent.com/BOberreither/INTRO/master/INTRO_outdated.owl#FormalEntity -->

    <owl:Class rdf:about="https://raw.githubusercontent.com/BOberreither/INTRO/master/INTRO_outdated.owl#FormalEntity">
        <rdfs:subClassOf rdf:resource="https://raw.githubusercontent.com/BOberreither/INTRO/master/INTRO_outdated.owl#ReceptionalEntity"/>
        <rdfs:subClassOf>
            <owl:Restriction>
                <owl:onProperty rdf:resource="https://raw.githubusercontent.com/BOberreither/INTRO/master/INTRO_outdated.owl#formalFeatureActualizedIn"/>
                <owl:allValuesFrom rdf:resource="https://raw.githubusercontent.com/BOberreither/INTRO/master/INTRO_outdated.owl#ActualizationOfFeature"/>
            </owl:Restriction>
        </rdfs:subClassOf>
        <rdfs:comment>This class comprises subclasses for every formal aspect of a text: Subclasses will provide the general terms (e.g. &apos;stanza&apos;), instances are meant to be specific types (e.g. &apos;Sapphic stanza&apos;).</rdfs:comment>
        <rdfs:label>Formal Entity</rdfs:label>
    </owl:Class>
    


    <!-- https://raw.githubusercontent.com/BOberreither/INTRO/master/INTRO_outdated.owl#Genette -->

    <owl:Class rdf:about="https://raw.githubusercontent.com/BOberreither/INTRO/master/INTRO_outdated.owl#Genette">
        <rdfs:subClassOf rdf:resource="https://raw.githubusercontent.com/BOberreither/INTRO/master/INTRO_outdated.owl#IntertextualTheory"/>
    </owl:Class>
    


    <!-- https://raw.githubusercontent.com/BOberreither/INTRO/master/INTRO_outdated.owl#GenreSubTrias -->

    <owl:Class rdf:about="https://raw.githubusercontent.com/BOberreither/INTRO/master/INTRO_outdated.owl#GenreSubTrias">
        <rdfs:subClassOf rdf:resource="https://raw.githubusercontent.com/BOberreither/INTRO/master/INTRO_outdated.owl#ArchitextualEntity"/>
        <rdfs:comment>A genre, as in: comedy, tragedy, historical, biographical; or as in: novel, novella, short story. Etc.</rdfs:comment>
        <rdfs:label>Genre (sub &apos;Trias&apos;)</rdfs:label>
    </owl:Class>
    


    <!-- https://raw.githubusercontent.com/BOberreither/INTRO/master/INTRO_outdated.owl#GenreTrias -->

    <owl:Class rdf:about="https://raw.githubusercontent.com/BOberreither/INTRO/master/INTRO_outdated.owl#GenreTrias">
        <rdfs:subClassOf rdf:resource="https://raw.githubusercontent.com/BOberreither/INTRO/master/INTRO_outdated.owl#ArchitextualEntity"/>
        <rdfs:comment>A genre, as in: poetry, drama, or prose</rdfs:comment>
        <rdfs:label>Genre (the &apos;Trias&apos;)</rdfs:label>
    </owl:Class>
    


    <!-- https://raw.githubusercontent.com/BOberreither/INTRO/master/INTRO_outdated.owl#Greenblatt -->

    <owl:Class rdf:about="https://raw.githubusercontent.com/BOberreither/INTRO/master/INTRO_outdated.owl#Greenblatt">
        <rdfs:subClassOf rdf:resource="https://raw.githubusercontent.com/BOberreither/INTRO/master/INTRO_outdated.owl#IntertextualTheory"/>
    </owl:Class>
    


    <!-- https://raw.githubusercontent.com/BOberreither/INTRO/master/INTRO_outdated.owl#Interpretament -->

    <owl:Class rdf:about="https://raw.githubusercontent.com/BOberreither/INTRO/master/INTRO_outdated.owl#Interpretament">
        <rdfs:subClassOf rdf:resource="http://www.cidoc-crm.org/cidoc-crm/E89_Propositional_Object"/>
        <rdfs:subClassOf>
            <owl:Restriction>
                <owl:onProperty rdf:resource="https://raw.githubusercontent.com/BOberreither/INTRO/master/INTRO_outdated.owl#consistsIn"/>
                <owl:allValuesFrom rdf:resource="https://raw.githubusercontent.com/BOberreither/INTRO/master/INTRO_outdated.owl#ActualizationOfFeature"/>
            </owl:Restriction>
        </rdfs:subClassOf>
        <rdfs:subClassOf>
            <owl:Restriction>
                <owl:onProperty rdf:resource="https://raw.githubusercontent.com/BOberreither/INTRO/master/INTRO_outdated.owl#discusses"/>
                <owl:allValuesFrom>
                    <owl:Class>
                        <owl:unionOf rdf:parseType="Collection">
                            <rdf:Description rdf:about="http://iflastandards.info/ns/fr/frbr/frbroo/F1_Work"/>
                            <rdf:Description rdf:about="http://iflastandards.info/ns/fr/frbr/frbroo/F22_Self-Contained_Expression"/>
                            <rdf:Description rdf:about="http://iflastandards.info/ns/fr/frbr/frbroo/F23_Expression_Fragment"/>
                            <rdf:Description rdf:about="http://iflastandards.info/ns/fr/frbr/frbroo/F2_Expression"/>
                            <rdf:Description rdf:about="http://iflastandards.info/ns/fr/frbr/frbroo/F3_Manifestation_Product_Type"/>
                            <rdf:Description rdf:about="https://raw.githubusercontent.com/BOberreither/INTRO/master/INTRO_outdated.owl#ArchitextualEntity"/>
                            <rdf:Description rdf:about="https://raw.githubusercontent.com/BOberreither/INTRO/master/INTRO_outdated.owl#ManifestationProductTypeFragment"/>
                        </owl:unionOf>
                    </owl:Class>
                </owl:allValuesFrom>
            </owl:Restriction>
        </rdfs:subClassOf>
        <rdfs:subClassOf>
            <owl:Restriction>
                <owl:onProperty rdf:resource="https://raw.githubusercontent.com/BOberreither/INTRO/master/INTRO_outdated.owl#hasPrecedingInterpretament"/>
                <owl:allValuesFrom rdf:resource="https://raw.githubusercontent.com/BOberreither/INTRO/master/INTRO_outdated.owl#Interpretament"/>
            </owl:Restriction>
        </rdfs:subClassOf>
        <rdfs:subClassOf>
            <owl:Restriction>
                <owl:onProperty rdf:resource="https://raw.githubusercontent.com/BOberreither/INTRO/master/INTRO_outdated.owl#hasSubsequentInterpretament"/>
                <owl:allValuesFrom rdf:resource="https://raw.githubusercontent.com/BOberreither/INTRO/master/INTRO_outdated.owl#Interpretament"/>
            </owl:Restriction>
        </rdfs:subClassOf>
        <rdfs:subClassOf>
            <owl:Restriction>
                <owl:onProperty rdf:resource="https://raw.githubusercontent.com/BOberreither/INTRO/master/INTRO_outdated.owl#identifies"/>
                <owl:allValuesFrom>
                    <owl:Class>
                        <owl:unionOf rdf:parseType="Collection">
                            <rdf:Description rdf:about="https://raw.githubusercontent.com/BOberreither/INTRO/master/INTRO_outdated.owl#ActualizationOfFeature"/>
                            <rdf:Description rdf:about="https://raw.githubusercontent.com/BOberreither/INTRO/master/INTRO_outdated.owl#Characteristic"/>
                            <rdf:Description rdf:about="https://raw.githubusercontent.com/BOberreither/INTRO/master/INTRO_outdated.owl#ReceptionalEntity"/>
                            <rdf:Description rdf:about="https://raw.githubusercontent.com/BOberreither/INTRO/master/INTRO_outdated.owl#Reference"/>
                        </owl:unionOf>
                    </owl:Class>
                </owl:allValuesFrom>
            </owl:Restriction>
        </rdfs:subClassOf>
        <rdfs:subClassOf>
            <owl:Restriction>
                <owl:onProperty rdf:resource="https://raw.githubusercontent.com/BOberreither/INTRO/master/INTRO_outdated.owl#interpretamentOriginatingIn"/>
                <owl:allValuesFrom>
                    <owl:Class>
                        <owl:unionOf rdf:parseType="Collection">
                            <rdf:Description rdf:about="http://iflastandards.info/ns/fr/frbr/frbroo/F1_Work"/>
                            <rdf:Description rdf:about="http://iflastandards.info/ns/fr/frbr/frbroo/F22_Self-Contained_Expression"/>
                            <rdf:Description rdf:about="http://iflastandards.info/ns/fr/frbr/frbroo/F23_Expression_Fragment"/>
                            <rdf:Description rdf:about="http://iflastandards.info/ns/fr/frbr/frbroo/F2_Expression"/>
                            <rdf:Description rdf:about="http://iflastandards.info/ns/fr/frbr/frbroo/F3_Manifestation_Product_Type"/>
                            <rdf:Description rdf:about="https://raw.githubusercontent.com/BOberreither/INTRO/master/INTRO_outdated.owl#ArchitextualEntity"/>
                            <rdf:Description rdf:about="https://raw.githubusercontent.com/BOberreither/INTRO/master/INTRO_outdated.owl#ManifestationProductTypeFragment"/>
                        </owl:unionOf>
                    </owl:Class>
                </owl:allValuesFrom>
            </owl:Restriction>
        </rdfs:subClassOf>
        <rdfs:subClassOf>
            <owl:Restriction>
                <owl:onProperty rdf:resource="https://raw.githubusercontent.com/BOberreither/INTRO/master/INTRO_outdated.owl#supportProvidedBy"/>
                <owl:allValuesFrom>
                    <owl:Class>
                        <owl:unionOf rdf:parseType="Collection">
                            <rdf:Description rdf:about="http://iflastandards.info/ns/fr/frbr/frbroo/F1_Work"/>
                            <rdf:Description rdf:about="http://iflastandards.info/ns/fr/frbr/frbroo/F22_Self-Contained_Expression"/>
                            <rdf:Description rdf:about="http://iflastandards.info/ns/fr/frbr/frbroo/F23_Expression_Fragment"/>
                            <rdf:Description rdf:about="http://iflastandards.info/ns/fr/frbr/frbroo/F2_Expression"/>
                            <rdf:Description rdf:about="http://iflastandards.info/ns/fr/frbr/frbroo/F3_Manifestation_Product_Type"/>
                            <rdf:Description rdf:about="https://raw.githubusercontent.com/BOberreither/INTRO/master/INTRO_outdated.owl#ArchitextualEntity"/>
                            <rdf:Description rdf:about="https://raw.githubusercontent.com/BOberreither/INTRO/master/INTRO_outdated.owl#ManifestationProductTypeFragment"/>
                        </owl:unionOf>
                    </owl:Class>
                </owl:allValuesFrom>
            </owl:Restriction>
        </rdfs:subClassOf>
        <rdfs:subClassOf>
            <owl:Restriction>
                <owl:onProperty rdf:resource="https://raw.githubusercontent.com/BOberreither/INTRO/master/INTRO_outdated.owl#hasParaphraseOrDefinition"/>
                <owl:allValuesFrom rdf:resource="http://www.w3.org/2001/XMLSchema#string"/>
            </owl:Restriction>
        </rdfs:subClassOf>
        <rdfs:comment>The abstract content of a interpretative act that actualizes the semantic Feature &apos;Interpretation&apos; in a specific way.
An interpretative identifies references, actualizations of featores or characteristics that assign texts to a transtextual entity.
Interpretatives themselves originate in texts.

Examples:
- the statement, that Umberto Eco&apos;s &apos;The Name of the Rose&apos; features a detective character.
- the statement, that Umberto Eco&apos;s &apos;The Name of the Rose&apos; contains references to Arthur Conan Doyle&apos;s &apos;Sherlock Holmes&apos;.
- the conclusion, that Umberto Eco&apos;s &apos;The Name of the Rose&apos; belongs to the genre &apos;postmodern crime novel&apos;.</rdfs:comment>
        <rdfs:label>Interpretament</rdfs:label>
    </owl:Class>
    


    <!-- https://raw.githubusercontent.com/BOberreither/INTRO/master/INTRO_outdated.owl#Interpretation -->

    <owl:Class rdf:about="https://raw.githubusercontent.com/BOberreither/INTRO/master/INTRO_outdated.owl#Interpretation">
        <rdfs:subClassOf rdf:resource="https://raw.githubusercontent.com/BOberreither/INTRO/master/INTRO_outdated.owl#SemanticEntity"/>
    </owl:Class>
    


    <!-- https://raw.githubusercontent.com/BOberreither/INTRO/master/INTRO_outdated.owl#IntertextualCommon -->

    <owl:Class rdf:about="https://raw.githubusercontent.com/BOberreither/INTRO/master/INTRO_outdated.owl#IntertextualCommon">
        <rdfs:subClassOf rdf:resource="https://raw.githubusercontent.com/BOberreither/INTRO/master/INTRO_outdated.owl#TypeOfIntertextualRelationship"/>
        <rdfs:comment>This class comprises concepts of intertextuality, that might have a theoretic foundation in one of the other classes, but also work as &apos;colloquial&apos;, legal, moral terms for intertextuality (e.g. &apos;allusion&apos;, &apos;plagiarism&apos;, &apos;theft of ideas&apos; etc.).</rdfs:comment>
        <rdfs:label>Common Concepts of Intertextuality</rdfs:label>
    </owl:Class>
    


    <!-- https://raw.githubusercontent.com/BOberreither/INTRO/master/INTRO_outdated.owl#IntertextualGenres -->

    <owl:Class rdf:about="https://raw.githubusercontent.com/BOberreither/INTRO/master/INTRO_outdated.owl#IntertextualGenres">
        <rdfs:subClassOf rdf:resource="https://raw.githubusercontent.com/BOberreither/INTRO/master/INTRO_outdated.owl#TypeOfIntertextualRelationship"/>
        <rdfs:comment>This class comprises the many terms for intertextual relationships that originate in genre theory.</rdfs:comment>
        <rdfs:label>Intertextuality in Genre Theory</rdfs:label>
    </owl:Class>
    


    <!-- https://raw.githubusercontent.com/BOberreither/INTRO/master/INTRO_outdated.owl#IntertextualOntology -->

    <owl:Class rdf:about="https://raw.githubusercontent.com/BOberreither/INTRO/master/INTRO_outdated.owl#IntertextualOntology">
        <rdfs:subClassOf rdf:resource="https://raw.githubusercontent.com/BOberreither/INTRO/master/INTRO_outdated.owl#TypeOfIntertextualRelationship"/>
        <rdfs:comment>This class comprises types of intertextuality that have been formulated in existing ontologies on the topic.</rdfs:comment>
        <rdfs:label>Intertextuality Ontologies</rdfs:label>
    </owl:Class>
    


    <!-- https://raw.githubusercontent.com/BOberreither/INTRO/master/INTRO_outdated.owl#IntertextualRhetoric -->

    <owl:Class rdf:about="https://raw.githubusercontent.com/BOberreither/INTRO/master/INTRO_outdated.owl#IntertextualRhetoric">
        <rdfs:subClassOf rdf:resource="https://raw.githubusercontent.com/BOberreither/INTRO/master/INTRO_outdated.owl#TypeOfIntertextualRelationship"/>
        <rdfs:comment>This class comprises the many terms for intertextual relationships that originate in greek or roman rhetoric.</rdfs:comment>
        <rdfs:label>Intertextuality in Rhetoric</rdfs:label>
    </owl:Class>
    


    <!-- https://raw.githubusercontent.com/BOberreither/INTRO/master/INTRO_outdated.owl#IntertextualTheory -->

    <owl:Class rdf:about="https://raw.githubusercontent.com/BOberreither/INTRO/master/INTRO_outdated.owl#IntertextualTheory">
        <rdfs:subClassOf rdf:resource="https://raw.githubusercontent.com/BOberreither/INTRO/master/INTRO_outdated.owl#TypeOfIntertextualRelationship"/>
        <rdfs:comment>This class comprises types of intertextuality as defined within a specific theoretical context.</rdfs:comment>
        <rdfs:label>Intertextuality Theories</rdfs:label>
    </owl:Class>
    


    <!-- https://raw.githubusercontent.com/BOberreither/INTRO/master/INTRO_outdated.owl#Kristeva -->

    <owl:Class rdf:about="https://raw.githubusercontent.com/BOberreither/INTRO/master/INTRO_outdated.owl#Kristeva">
        <rdfs:subClassOf rdf:resource="https://raw.githubusercontent.com/BOberreither/INTRO/master/INTRO_outdated.owl#IntertextualTheory"/>
    </owl:Class>
    


    <!-- https://raw.githubusercontent.com/BOberreither/INTRO/master/INTRO_outdated.owl#Lachmann -->

    <owl:Class rdf:about="https://raw.githubusercontent.com/BOberreither/INTRO/master/INTRO_outdated.owl#Lachmann">
        <rdfs:subClassOf rdf:resource="https://raw.githubusercontent.com/BOberreither/INTRO/master/INTRO_outdated.owl#IntertextualTheory"/>
    </owl:Class>
    


    <!-- https://raw.githubusercontent.com/BOberreither/INTRO/master/INTRO_outdated.owl#Leitmotiv -->

    <owl:Class rdf:about="https://raw.githubusercontent.com/BOberreither/INTRO/master/INTRO_outdated.owl#Leitmotiv">
        <rdfs:subClassOf rdf:resource="https://raw.githubusercontent.com/BOberreither/INTRO/master/INTRO_outdated.owl#Motif"/>
    </owl:Class>
    


    <!-- https://raw.githubusercontent.com/BOberreither/INTRO/master/INTRO_outdated.owl#Line -->

    <owl:Class rdf:about="https://raw.githubusercontent.com/BOberreither/INTRO/master/INTRO_outdated.owl#Line">
        <rdfs:subClassOf rdf:resource="https://raw.githubusercontent.com/BOberreither/INTRO/master/INTRO_outdated.owl#FormalEntity"/>
    </owl:Class>
    


    <!-- https://raw.githubusercontent.com/BOberreither/INTRO/master/INTRO_outdated.owl#Link -->

    <owl:Class rdf:about="https://raw.githubusercontent.com/BOberreither/INTRO/master/INTRO_outdated.owl#Link">
        <rdfs:subClassOf rdf:resource="https://raw.githubusercontent.com/BOberreither/INTRO/master/INTRO_outdated.owl#IntertextualTheory"/>
    </owl:Class>
    


    <!-- https://raw.githubusercontent.com/BOberreither/INTRO/master/INTRO_outdated.owl#ManifestationProductTypeFragment -->

    <owl:Class rdf:about="https://raw.githubusercontent.com/BOberreither/INTRO/master/INTRO_outdated.owl#ManifestationProductTypeFragment">
        <rdfs:subClassOf rdf:resource="http://iflastandards.info/ns/fr/frbr/frbroo/F3_Manifestation_Product_Type"/>
        <rdfs:subClassOf rdf:resource="http://www.cidoc-crm.org/cidoc-crm/E73_Information_Object"/>
        <rdfs:subClassOf>
            <owl:Restriction>
                <owl:onProperty rdf:resource="https://raw.githubusercontent.com/BOberreither/INTRO/master/INTRO_outdated.owl#comprisesFragmentCarriersOf"/>
                <owl:allValuesFrom rdf:resource="http://iflastandards.info/ns/fr/frbr/frbroo/F23_Expression_Fragment"/>
            </owl:Restriction>
        </rdfs:subClassOf>
        <rdfs:subClassOf>
            <owl:Restriction>
                <owl:onProperty rdf:resource="https://raw.githubusercontent.com/BOberreither/INTRO/master/INTRO_outdated.owl#hasProductTypeFragmentFragment"/>
                <owl:allValuesFrom rdf:resource="https://raw.githubusercontent.com/BOberreither/INTRO/master/INTRO_outdated.owl#ManifestationProductTypeFragment"/>
            </owl:Restriction>
        </rdfs:subClassOf>
        <rdfs:subClassOf>
            <owl:Restriction>
                <owl:onProperty rdf:resource="https://raw.githubusercontent.com/BOberreither/INTRO/master/INTRO_outdated.owl#isAppurtenantElement"/>
                <owl:allValuesFrom rdf:resource="https://raw.githubusercontent.com/BOberreither/INTRO/master/INTRO_outdated.owl#ArchitextualEntity"/>
            </owl:Restriction>
        </rdfs:subClassOf>
        <rdfs:subClassOf>
            <owl:Restriction>
                <owl:onProperty rdf:resource="https://raw.githubusercontent.com/BOberreither/INTRO/master/INTRO_outdated.owl#isDiscussedIn"/>
                <owl:allValuesFrom rdf:resource="https://raw.githubusercontent.com/BOberreither/INTRO/master/INTRO_outdated.owl#Interpretament"/>
            </owl:Restriction>
        </rdfs:subClassOf>
        <rdfs:subClassOf>
            <owl:Restriction>
                <owl:onProperty rdf:resource="https://raw.githubusercontent.com/BOberreither/INTRO/master/INTRO_outdated.owl#isProductTypeFragmentFragmentOf"/>
                <owl:allValuesFrom rdf:resource="https://raw.githubusercontent.com/BOberreither/INTRO/master/INTRO_outdated.owl#ManifestationProductTypeFragment"/>
            </owl:Restriction>
        </rdfs:subClassOf>
        <rdfs:subClassOf>
            <owl:Restriction>
                <owl:onProperty rdf:resource="https://raw.githubusercontent.com/BOberreither/INTRO/master/INTRO_outdated.owl#isProductTypeFragmentOf"/>
                <owl:allValuesFrom rdf:resource="http://iflastandards.info/ns/fr/frbr/frbroo/F3_Manifestation_Product_Type"/>
            </owl:Restriction>
        </rdfs:subClassOf>
        <rdfs:subClassOf>
            <owl:Restriction>
                <owl:onProperty rdf:resource="https://raw.githubusercontent.com/BOberreither/INTRO/master/INTRO_outdated.owl#isReferredToEntity"/>
                <owl:allValuesFrom rdf:resource="https://raw.githubusercontent.com/BOberreither/INTRO/master/INTRO_outdated.owl#Reference"/>
            </owl:Restriction>
        </rdfs:subClassOf>
        <rdfs:subClassOf>
            <owl:Restriction>
                <owl:onProperty rdf:resource="https://raw.githubusercontent.com/BOberreither/INTRO/master/INTRO_outdated.owl#isReferringEntity"/>
                <owl:allValuesFrom rdf:resource="https://raw.githubusercontent.com/BOberreither/INTRO/master/INTRO_outdated.owl#Reference"/>
            </owl:Restriction>
        </rdfs:subClassOf>
        <rdfs:subClassOf>
            <owl:Restriction>
                <owl:onProperty rdf:resource="https://raw.githubusercontent.com/BOberreither/INTRO/master/INTRO_outdated.owl#providesSupportFor"/>
                <owl:allValuesFrom>
                    <owl:Class>
                        <owl:unionOf rdf:parseType="Collection">
                            <rdf:Description rdf:about="https://raw.githubusercontent.com/BOberreither/INTRO/master/INTRO_outdated.owl#ActualizationOfFeature"/>
                            <rdf:Description rdf:about="https://raw.githubusercontent.com/BOberreither/INTRO/master/INTRO_outdated.owl#Characteristic"/>
                            <rdf:Description rdf:about="https://raw.githubusercontent.com/BOberreither/INTRO/master/INTRO_outdated.owl#Interpretament"/>
                            <rdf:Description rdf:about="https://raw.githubusercontent.com/BOberreither/INTRO/master/INTRO_outdated.owl#Opinion"/>
                            <rdf:Description rdf:about="https://raw.githubusercontent.com/BOberreither/INTRO/master/INTRO_outdated.owl#Reference"/>
                            <rdf:Description rdf:about="https://raw.githubusercontent.com/BOberreither/INTRO/master/INTRO_outdated.owl#TypeOfIntertextualRelationship"/>
                        </owl:unionOf>
                    </owl:Class>
                </owl:allValuesFrom>
            </owl:Restriction>
        </rdfs:subClassOf>
        <rdfs:subClassOf>
            <owl:Restriction>
                <owl:onProperty rdf:resource="https://raw.githubusercontent.com/BOberreither/INTRO/master/INTRO_outdated.owl#showsActualization"/>
                <owl:allValuesFrom rdf:resource="https://raw.githubusercontent.com/BOberreither/INTRO/master/INTRO_outdated.owl#ActualizationOfFeature"/>
            </owl:Restriction>
        </rdfs:subClassOf>
        <rdfs:subClassOf>
            <owl:Restriction>
                <owl:onProperty rdf:resource="https://raw.githubusercontent.com/BOberreither/INTRO/master/INTRO_outdated.owl#showsCharacteristics"/>
                <owl:allValuesFrom rdf:resource="https://raw.githubusercontent.com/BOberreither/INTRO/master/INTRO_outdated.owl#Characteristic"/>
            </owl:Restriction>
        </rdfs:subClassOf>
        <rdfs:subClassOf>
            <owl:Restriction>
                <owl:onProperty rdf:resource="https://raw.githubusercontent.com/BOberreither/INTRO/master/INTRO_outdated.owl#hasBibliographicalData"/>
                <owl:someValuesFrom rdf:resource="http://www.w3.org/2001/XMLSchema#string"/>
            </owl:Restriction>
        </rdfs:subClassOf>
        <rdfs:subClassOf>
            <owl:Restriction>
                <owl:onProperty rdf:resource="https://raw.githubusercontent.com/BOberreither/INTRO/master/INTRO_outdated.owl#hasLocation"/>
                <owl:someValuesFrom rdf:resource="http://www.w3.org/2001/XMLSchema#string"/>
            </owl:Restriction>
        </rdfs:subClassOf>
        <rdfs:subClassOf>
            <owl:Restriction>
                <owl:onProperty rdf:resource="https://raw.githubusercontent.com/BOberreither/INTRO/master/INTRO_outdated.owl#hasWording"/>
                <owl:someValuesFrom rdf:resource="http://www.w3.org/2001/XMLSchema#string"/>
            </owl:Restriction>
        </rdfs:subClassOf>
        <rdfs:comment>An addition to FRBRoo, made necessary by the focus of this ontology.
FRBRoo&apos;s &apos;Expression Fragment&apos; is by definition a fragment of an expression, which is the immaterial realisation of a work - and for this reason cannot be object of a citation or a detailed bibliographical record (an expression has no page numbers). The FRBRoo &apos;Manifestation Product Type&apos; is itself an immaterial (ideal) version of a text, a &apos;species&apos; (as stated in the definition of FRBRoo), of which the numerous items are &apos;specimen&apos;. However it adds concreteness to the &apos;Expression&apos;, it has a publisher, a publishing date, page numbers, an ISBN and so on.
The &apos;Manifestation Product Type Fragment&apos; is an identifiable part (a paragraph, a couple of lines, and so forth) of the &apos;Manifestation Product Type&apos;.

(About the definition of &apos;fragment&apos;: My ontology makes use of the broad extent of the concept in FRBRoo, which one the one hand instances the remaining fragments of otherwise lost literary works or excerpts (indicating, that a fragment is a part that is by definition situated outside of its original context), but on the other hand instances statements as found on/in books (i.e. that still have their original contexts). My use of the term is based on the latter.)

For Example:
- the words &apos;Abandon all hope ye who enter here&apos; from page 3 of the publication with the ISBN 978-0307278630.</rdfs:comment>
        <rdfs:label>Manifestation Product Type Fragment</rdfs:label>
        <skos:closeMatch>http://purl.org/spar/doco/TextChunk</skos:closeMatch>
    </owl:Class>
    


    <!-- https://raw.githubusercontent.com/BOberreither/INTRO/master/INTRO_outdated.owl#Mood -->

    <owl:Class rdf:about="https://raw.githubusercontent.com/BOberreither/INTRO/master/INTRO_outdated.owl#Mood">
        <rdfs:subClassOf rdf:resource="https://raw.githubusercontent.com/BOberreither/INTRO/master/INTRO_outdated.owl#SemanticEntity"/>
    </owl:Class>
    


    <!-- https://raw.githubusercontent.com/BOberreither/INTRO/master/INTRO_outdated.owl#Motif -->

    <owl:Class rdf:about="https://raw.githubusercontent.com/BOberreither/INTRO/master/INTRO_outdated.owl#Motif">
        <rdfs:subClassOf rdf:resource="https://raw.githubusercontent.com/BOberreither/INTRO/master/INTRO_outdated.owl#SemanticEntity"/>
    </owl:Class>
    


    <!-- https://raw.githubusercontent.com/BOberreither/INTRO/master/INTRO_outdated.owl#Movement -->

    <owl:Class rdf:about="https://raw.githubusercontent.com/BOberreither/INTRO/master/INTRO_outdated.owl#Movement">
        <rdfs:subClassOf rdf:resource="https://raw.githubusercontent.com/BOberreither/INTRO/master/INTRO_outdated.owl#ArchitextualEntity"/>
    </owl:Class>
    


    <!-- https://raw.githubusercontent.com/BOberreither/INTRO/master/INTRO_outdated.owl#NarratologicalEntity -->

    <owl:Class rdf:about="https://raw.githubusercontent.com/BOberreither/INTRO/master/INTRO_outdated.owl#NarratologicalEntity">
        <rdfs:subClassOf rdf:resource="https://raw.githubusercontent.com/BOberreither/INTRO/master/INTRO_outdated.owl#RhetoricalEntity"/>
        <rdfs:comment>This class comprises narratological concepts.</rdfs:comment>
        <rdfs:label>Narratological Entity</rdfs:label>
    </owl:Class>
    


    <!-- https://raw.githubusercontent.com/BOberreither/INTRO/master/INTRO_outdated.owl#Numeration -->

    <owl:Class rdf:about="https://raw.githubusercontent.com/BOberreither/INTRO/master/INTRO_outdated.owl#Numeration">
        <rdfs:subClassOf rdf:resource="https://raw.githubusercontent.com/BOberreither/INTRO/master/INTRO_outdated.owl#FormalEntity"/>
    </owl:Class>
    


    <!-- https://raw.githubusercontent.com/BOberreither/INTRO/master/INTRO_outdated.owl#Oeuvre -->

    <owl:Class rdf:about="https://raw.githubusercontent.com/BOberreither/INTRO/master/INTRO_outdated.owl#Oeuvre">
        <rdfs:subClassOf rdf:resource="https://raw.githubusercontent.com/BOberreither/INTRO/master/INTRO_outdated.owl#ArchitextualEntity"/>
        <rdfs:comment>Texts that have an author as their common denominator.</rdfs:comment>
    </owl:Class>
    


    <!-- https://raw.githubusercontent.com/BOberreither/INTRO/master/INTRO_outdated.owl#Opinion -->

    <owl:Class rdf:about="https://raw.githubusercontent.com/BOberreither/INTRO/master/INTRO_outdated.owl#Opinion">
        <rdfs:subClassOf rdf:resource="https://raw.githubusercontent.com/BOberreither/INTRO/master/INTRO_outdated.owl#SemanticEntity"/>
        <rdfs:subClassOf>
            <owl:Restriction>
                <owl:onProperty rdf:resource="https://raw.githubusercontent.com/BOberreither/INTRO/master/INTRO_outdated.owl#hasOpinionObject"/>
                <owl:allValuesFrom rdf:resource="http://www.cidoc-crm.org/cidoc-crm/E70_Thing"/>
            </owl:Restriction>
        </rdfs:subClassOf>
    </owl:Class>
    


    <!-- https://raw.githubusercontent.com/BOberreither/INTRO/master/INTRO_outdated.owl#Paradigm -->

    <owl:Class rdf:about="https://raw.githubusercontent.com/BOberreither/INTRO/master/INTRO_outdated.owl#Paradigm">
        <rdfs:subClassOf rdf:resource="https://raw.githubusercontent.com/BOberreither/INTRO/master/INTRO_outdated.owl#ArchitextualEntity"/>
    </owl:Class>
    


    <!-- https://raw.githubusercontent.com/BOberreither/INTRO/master/INTRO_outdated.owl#PartSubtitle -->

    <owl:Class rdf:about="https://raw.githubusercontent.com/BOberreither/INTRO/master/INTRO_outdated.owl#PartSubtitle">
        <rdfs:subClassOf rdf:resource="https://raw.githubusercontent.com/BOberreither/INTRO/master/INTRO_outdated.owl#Subtitle"/>
    </owl:Class>
    


    <!-- https://raw.githubusercontent.com/BOberreither/INTRO/master/INTRO_outdated.owl#PartTitle -->

    <owl:Class rdf:about="https://raw.githubusercontent.com/BOberreither/INTRO/master/INTRO_outdated.owl#PartTitle">
        <rdfs:subClassOf rdf:resource="http://purl.org/spar/doco/Title"/>
    </owl:Class>
    


    <!-- https://raw.githubusercontent.com/BOberreither/INTRO/master/INTRO_outdated.owl#Plot -->

    <owl:Class rdf:about="https://raw.githubusercontent.com/BOberreither/INTRO/master/INTRO_outdated.owl#Plot">
        <rdfs:subClassOf rdf:resource="https://raw.githubusercontent.com/BOberreither/INTRO/master/INTRO_outdated.owl#SemanticEntity"/>
    </owl:Class>
    


    <!-- https://raw.githubusercontent.com/BOberreither/INTRO/master/INTRO_outdated.owl#PragmaticEntity -->

    <owl:Class rdf:about="https://raw.githubusercontent.com/BOberreither/INTRO/master/INTRO_outdated.owl#PragmaticEntity">
        <rdfs:subClassOf rdf:resource="https://raw.githubusercontent.com/BOberreither/INTRO/master/INTRO_outdated.owl#RhetoricalEntity"/>
        <rdfs:comment>This class comprises parts of a text in this regard that they pursue a certain purpose, and do so in a way that is apparent on the text surface or by application of certain conventions or handed-down standards. Subclasses can range from &apos;argument&apos; to &apos;quotation&apos; to &apos;bibliographic reference&apos;.
Subclasses of this class can be derived (or imported) from existing ontologies such as the &apos;SPAR Document Component Ontology&apos;.</rdfs:comment>
        <rdfs:label>Pragmatic Entity</rdfs:label>
    </owl:Class>
    


    <!-- https://raw.githubusercontent.com/BOberreither/INTRO/master/INTRO_outdated.owl#Quotation -->

    <owl:Class rdf:about="https://raw.githubusercontent.com/BOberreither/INTRO/master/INTRO_outdated.owl#Quotation">
        <rdfs:subClassOf rdf:resource="https://raw.githubusercontent.com/BOberreither/INTRO/master/INTRO_outdated.owl#PragmaticEntity"/>
    </owl:Class>
    


    <!-- https://raw.githubusercontent.com/BOberreither/INTRO/master/INTRO_outdated.owl#ReceptionalEntity -->

    <owl:Class rdf:about="https://raw.githubusercontent.com/BOberreither/INTRO/master/INTRO_outdated.owl#ReceptionalEntity">
        <rdfs:subClassOf rdf:resource="http://www.cidoc-crm.org/cidoc-crm/E28_Conceptual_Object"/>
        <rdfs:subClassOf>
            <owl:Restriction>
                <owl:onProperty rdf:resource="https://raw.githubusercontent.com/BOberreither/INTRO/master/INTRO_outdated.owl#definitionProvidedBy"/>
                <owl:allValuesFrom rdf:resource="https://raw.githubusercontent.com/BOberreither/INTRO/master/INTRO_outdated.owl#ActualizationOfFeature"/>
            </owl:Restriction>
        </rdfs:subClassOf>
        <rdfs:subClassOf>
            <owl:Restriction>
                <owl:onProperty rdf:resource="https://raw.githubusercontent.com/BOberreither/INTRO/master/INTRO_outdated.owl#featureActualizedIn"/>
                <owl:allValuesFrom rdf:resource="https://raw.githubusercontent.com/BOberreither/INTRO/master/INTRO_outdated.owl#ActualizationOfFeature"/>
            </owl:Restriction>
        </rdfs:subClassOf>
        <rdfs:subClassOf>
            <owl:Restriction>
                <owl:onProperty rdf:resource="https://raw.githubusercontent.com/BOberreither/INTRO/master/INTRO_outdated.owl#providesSimilarityForReference"/>
                <owl:allValuesFrom rdf:resource="https://raw.githubusercontent.com/BOberreither/INTRO/master/INTRO_outdated.owl#Reference"/>
            </owl:Restriction>
        </rdfs:subClassOf>
        <rdfs:subClassOf>
            <owl:Restriction>
                <owl:onProperty rdf:resource="https://raw.githubusercontent.com/BOberreither/INTRO/master/INTRO_outdated.owl#supportProvidedBy"/>
                <owl:allValuesFrom>
                    <owl:Class>
                        <owl:unionOf rdf:parseType="Collection">
                            <rdf:Description rdf:about="http://iflastandards.info/ns/fr/frbr/frbroo/F1_Work"/>
                            <rdf:Description rdf:about="http://iflastandards.info/ns/fr/frbr/frbroo/F22_Self-Contained_Expression"/>
                            <rdf:Description rdf:about="http://iflastandards.info/ns/fr/frbr/frbroo/F23_Expression_Fragment"/>
                            <rdf:Description rdf:about="http://iflastandards.info/ns/fr/frbr/frbroo/F2_Expression"/>
                            <rdf:Description rdf:about="http://iflastandards.info/ns/fr/frbr/frbroo/F3_Manifestation_Product_Type"/>
                            <rdf:Description rdf:about="https://raw.githubusercontent.com/BOberreither/INTRO/master/INTRO_outdated.owl#ArchitextualEntity"/>
                            <rdf:Description rdf:about="https://raw.githubusercontent.com/BOberreither/INTRO/master/INTRO_outdated.owl#ManifestationProductTypeFragment"/>
                        </owl:unionOf>
                    </owl:Class>
                </owl:allValuesFrom>
            </owl:Restriction>
        </rdfs:subClassOf>
        <rdfs:subClassOf>
            <owl:Restriction>
                <owl:onProperty rdf:resource="https://raw.githubusercontent.com/BOberreither/INTRO/master/INTRO_outdated.owl#hasParaphraseOrDefinition"/>
                <owl:allValuesFrom rdf:resource="http://www.w3.org/2001/XMLSchema#string"/>
            </owl:Restriction>
        </rdfs:subClassOf>
        <rdfs:comment>Whatever &apos;is in&apos; or &apos;can be found in&apos; or &apos;can be read out of&apos; a text, apart from the wording itself. Strictly speaking: the result of a mental process that is applied to a text and that made out distinct abstract concepts which take a specific (yet identifiable and probably individual) form in the text.
This class therefore has an extremely wide scope, its subclasses are open to additions and are to be populated from relevant reference works (e.g. the subclass &apos;Rhetorical Entity&apos; could contain concepts based on Lausberg&apos;s &apos;Handbook of Literary Rhetoric&apos;, many lemmata from the &apos;Princeton Handbook of Poetic Terms&apos; could populate the subclass &quot;Formal Entity&quot; and so on).
It is highly likely (and welcome) that the instances of subclasses or sub-subclasses of the class &apos;receptional Entity&apos; are instances or sub-subclasses of more than one subclass (e.g. that a rhetorical entity is at the same time a semantic entity as in the case of an &apos;argument&apos; or &apos;rhyme&apos;).</rdfs:comment>
        <rdfs:label>Receptional Entity</rdfs:label>
    </owl:Class>
    


    <!-- https://raw.githubusercontent.com/BOberreither/INTRO/master/INTRO_outdated.owl#Reference -->

    <owl:Class rdf:about="https://raw.githubusercontent.com/BOberreither/INTRO/master/INTRO_outdated.owl#Reference">
        <rdfs:subClassOf rdf:resource="https://raw.githubusercontent.com/BOberreither/INTRO/master/INTRO_outdated.owl#ReceptionalEntity"/>
        <rdfs:subClassOf>
            <owl:Restriction>
                <owl:onProperty rdf:resource="https://raw.githubusercontent.com/BOberreither/INTRO/master/INTRO_outdated.owl#hasType"/>
                <owl:allValuesFrom rdf:resource="https://raw.githubusercontent.com/BOberreither/INTRO/master/INTRO_outdated.owl#TypeOfIntertextualRelationship"/>
            </owl:Restriction>
        </rdfs:subClassOf>
        <rdfs:subClassOf>
            <owl:Restriction>
                <owl:onProperty rdf:resource="https://raw.githubusercontent.com/BOberreither/INTRO/master/INTRO_outdated.owl#isIdentifiedBy"/>
                <owl:allValuesFrom rdf:resource="https://raw.githubusercontent.com/BOberreither/INTRO/master/INTRO_outdated.owl#Interpretament"/>
            </owl:Restriction>
        </rdfs:subClassOf>
        <rdfs:subClassOf>
            <owl:Restriction>
                <owl:onProperty rdf:resource="https://raw.githubusercontent.com/BOberreither/INTRO/master/INTRO_outdated.owl#referenceIsBasedOnSimilarity"/>
                <owl:allValuesFrom rdf:resource="https://raw.githubusercontent.com/BOberreither/INTRO/master/INTRO_outdated.owl#ReceptionalEntity"/>
            </owl:Restriction>
        </rdfs:subClassOf>
        <rdfs:subClassOf>
            <owl:Restriction>
                <owl:onProperty rdf:resource="https://raw.githubusercontent.com/BOberreither/INTRO/master/INTRO_outdated.owl#supportProvidedBy"/>
                <owl:allValuesFrom>
                    <owl:Class>
                        <owl:unionOf rdf:parseType="Collection">
                            <rdf:Description rdf:about="http://iflastandards.info/ns/fr/frbr/frbroo/F1_Work"/>
                            <rdf:Description rdf:about="http://iflastandards.info/ns/fr/frbr/frbroo/F22_Self-Contained_Expression"/>
                            <rdf:Description rdf:about="http://iflastandards.info/ns/fr/frbr/frbroo/F23_Expression_Fragment"/>
                            <rdf:Description rdf:about="http://iflastandards.info/ns/fr/frbr/frbroo/F2_Expression"/>
                            <rdf:Description rdf:about="http://iflastandards.info/ns/fr/frbr/frbroo/F3_Manifestation_Product_Type"/>
                            <rdf:Description rdf:about="https://raw.githubusercontent.com/BOberreither/INTRO/master/INTRO_outdated.owl#ArchitextualEntity"/>
                            <rdf:Description rdf:about="https://raw.githubusercontent.com/BOberreither/INTRO/master/INTRO_outdated.owl#ManifestationProductTypeFragment"/>
                        </owl:unionOf>
                    </owl:Class>
                </owl:allValuesFrom>
            </owl:Restriction>
        </rdfs:subClassOf>
        <rdfs:subClassOf>
            <owl:Restriction>
                <owl:onProperty rdf:resource="https://raw.githubusercontent.com/BOberreither/INTRO/master/INTRO_outdated.owl#hasReferredToEntity"/>
                <owl:minQualifiedCardinality rdf:datatype="http://www.w3.org/2001/XMLSchema#nonNegativeInteger">1</owl:minQualifiedCardinality>
                <owl:onClass>
                    <owl:Class>
                        <owl:unionOf rdf:parseType="Collection">
                            <rdf:Description rdf:about="http://iflastandards.info/ns/fr/frbr/frbroo/F1_Work"/>
                            <rdf:Description rdf:about="http://iflastandards.info/ns/fr/frbr/frbroo/F22_Self-Contained_Expression"/>
                            <rdf:Description rdf:about="http://iflastandards.info/ns/fr/frbr/frbroo/F23_Expression_Fragment"/>
                            <rdf:Description rdf:about="http://iflastandards.info/ns/fr/frbr/frbroo/F2_Expression"/>
                            <rdf:Description rdf:about="http://iflastandards.info/ns/fr/frbr/frbroo/F3_Manifestation_Product_Type"/>
                            <rdf:Description rdf:about="https://raw.githubusercontent.com/BOberreither/INTRO/master/INTRO_outdated.owl#ArchitextualEntity"/>
                            <rdf:Description rdf:about="https://raw.githubusercontent.com/BOberreither/INTRO/master/INTRO_outdated.owl#ManifestationProductTypeFragment"/>
                        </owl:unionOf>
                    </owl:Class>
                </owl:onClass>
            </owl:Restriction>
        </rdfs:subClassOf>
        <rdfs:subClassOf>
            <owl:Restriction>
                <owl:onProperty rdf:resource="https://raw.githubusercontent.com/BOberreither/INTRO/master/INTRO_outdated.owl#hasReferringEntity"/>
                <owl:minQualifiedCardinality rdf:datatype="http://www.w3.org/2001/XMLSchema#nonNegativeInteger">1</owl:minQualifiedCardinality>
                <owl:onClass>
                    <owl:Class>
                        <owl:unionOf rdf:parseType="Collection">
                            <rdf:Description rdf:about="http://iflastandards.info/ns/fr/frbr/frbroo/F1_Work"/>
                            <rdf:Description rdf:about="http://iflastandards.info/ns/fr/frbr/frbroo/F22_Self-Contained_Expression"/>
                            <rdf:Description rdf:about="http://iflastandards.info/ns/fr/frbr/frbroo/F23_Expression_Fragment"/>
                            <rdf:Description rdf:about="http://iflastandards.info/ns/fr/frbr/frbroo/F2_Expression"/>
                            <rdf:Description rdf:about="http://iflastandards.info/ns/fr/frbr/frbroo/F3_Manifestation_Product_Type"/>
                            <rdf:Description rdf:about="https://raw.githubusercontent.com/BOberreither/INTRO/master/INTRO_outdated.owl#ArchitextualEntity"/>
                            <rdf:Description rdf:about="https://raw.githubusercontent.com/BOberreither/INTRO/master/INTRO_outdated.owl#ManifestationProductTypeFragment"/>
                        </owl:unionOf>
                    </owl:Class>
                </owl:onClass>
            </owl:Restriction>
        </rdfs:subClassOf>
        <rdfs:subClassOf>
            <owl:Restriction>
                <owl:onProperty rdf:resource="https://raw.githubusercontent.com/BOberreither/INTRO/master/INTRO_outdated.owl#hasParaphraseOrDefinition"/>
                <owl:allValuesFrom rdf:resource="http://www.w3.org/2001/XMLSchema#string"/>
            </owl:Restriction>
        </rdfs:subClassOf>
        <rdfs:comment>This class ismeant for the abstract notion of a reference as it is identified by a reader (and is not to be confused with the rhetorical entity &apos;quotation&apos;). Every reference has a referring and a reffered to entity, the former ranging from every part of the text up to the text as a whole (or as an abstract &apos;Work&apos;), the latter also including transtextual entitys.
A Reference is possibly identified in an interpretative.</rdfs:comment>
        <rdfs:label>Reference</rdfs:label>
    </owl:Class>
    


    <!-- https://raw.githubusercontent.com/BOberreither/INTRO/master/INTRO_outdated.owl#RhetoricalEntity -->

    <owl:Class rdf:about="https://raw.githubusercontent.com/BOberreither/INTRO/master/INTRO_outdated.owl#RhetoricalEntity">
        <rdfs:subClassOf rdf:resource="https://raw.githubusercontent.com/BOberreither/INTRO/master/INTRO_outdated.owl#ReceptionalEntity"/>
        <rdfs:subClassOf>
            <owl:Restriction>
                <owl:onProperty rdf:resource="https://raw.githubusercontent.com/BOberreither/INTRO/master/INTRO_outdated.owl#rhetoricalFeatureActualizedIn"/>
                <owl:allValuesFrom rdf:resource="https://raw.githubusercontent.com/BOberreither/INTRO/master/INTRO_outdated.owl#ActualizationOfFeature"/>
            </owl:Restriction>
        </rdfs:subClassOf>
        <rdfs:comment>This class comprises every aspect of a text that can be described in terms of rhetorics - ranging from the occurrence of rhetorical tropes (figures of speech) to parts of a e.g. research paper like &apos;introduction&apos; or &apos;quotation&apos; (pragmatic entities) to aspects of the narrative act such as &apos;voice&apos; or &apos;narrating time&apos; (narratological entities).</rdfs:comment>
        <rdfs:label>Rhetorical Entity</rdfs:label>
    </owl:Class>
    


    <!-- https://raw.githubusercontent.com/BOberreither/INTRO/master/INTRO_outdated.owl#Riffaterre -->

    <owl:Class rdf:about="https://raw.githubusercontent.com/BOberreither/INTRO/master/INTRO_outdated.owl#Riffaterre">
        <rdfs:subClassOf rdf:resource="https://raw.githubusercontent.com/BOberreither/INTRO/master/INTRO_outdated.owl#IntertextualTheory"/>
    </owl:Class>
    


    <!-- https://raw.githubusercontent.com/BOberreither/INTRO/master/INTRO_outdated.owl#Scene -->

    <owl:Class rdf:about="https://raw.githubusercontent.com/BOberreither/INTRO/master/INTRO_outdated.owl#Scene">
        <rdfs:subClassOf rdf:resource="https://raw.githubusercontent.com/BOberreither/INTRO/master/INTRO_outdated.owl#FormalEntity"/>
        <rdfs:label>Scene (Drama)</rdfs:label>
    </owl:Class>
    


    <!-- https://raw.githubusercontent.com/BOberreither/INTRO/master/INTRO_outdated.owl#School -->

    <owl:Class rdf:about="https://raw.githubusercontent.com/BOberreither/INTRO/master/INTRO_outdated.owl#School">
        <rdfs:subClassOf rdf:resource="https://raw.githubusercontent.com/BOberreither/INTRO/master/INTRO_outdated.owl#ArchitextualEntity"/>
    </owl:Class>
    


    <!-- https://raw.githubusercontent.com/BOberreither/INTRO/master/INTRO_outdated.owl#SectionSubtitle -->

    <owl:Class rdf:about="https://raw.githubusercontent.com/BOberreither/INTRO/master/INTRO_outdated.owl#SectionSubtitle">
        <rdfs:subClassOf rdf:resource="https://raw.githubusercontent.com/BOberreither/INTRO/master/INTRO_outdated.owl#Subtitle"/>
    </owl:Class>
    


    <!-- https://raw.githubusercontent.com/BOberreither/INTRO/master/INTRO_outdated.owl#SemanticEntity -->

    <owl:Class rdf:about="https://raw.githubusercontent.com/BOberreither/INTRO/master/INTRO_outdated.owl#SemanticEntity">
        <rdfs:subClassOf rdf:resource="https://raw.githubusercontent.com/BOberreither/INTRO/master/INTRO_outdated.owl#ReceptionalEntity"/>
        <rdfs:subClassOf>
            <owl:Restriction>
                <owl:onProperty rdf:resource="https://raw.githubusercontent.com/BOberreither/INTRO/master/INTRO_outdated.owl#semanticFeatureActualizedIn"/>
                <owl:allValuesFrom rdf:resource="https://raw.githubusercontent.com/BOberreither/INTRO/master/INTRO_outdated.owl#ActualizationOfFeature"/>
            </owl:Restriction>
        </rdfs:subClassOf>
        <rdfs:comment>This class comprises every semantic aspect of a text: from the common notions of &apos;plot&apos; or &apos;character&apos; up to the specific classification of forms such as &apos;situational motif&apos;.</rdfs:comment>
        <rdfs:label>Semantic Entity</rdfs:label>
    </owl:Class>
    


    <!-- https://raw.githubusercontent.com/BOberreither/INTRO/master/INTRO_outdated.owl#SituationalMotif -->

    <owl:Class rdf:about="https://raw.githubusercontent.com/BOberreither/INTRO/master/INTRO_outdated.owl#SituationalMotif">
        <rdfs:subClassOf rdf:resource="https://raw.githubusercontent.com/BOberreither/INTRO/master/INTRO_outdated.owl#Motif"/>
    </owl:Class>
    


    <!-- https://raw.githubusercontent.com/BOberreither/INTRO/master/INTRO_outdated.owl#SpatialEntity -->

    <owl:Class rdf:about="https://raw.githubusercontent.com/BOberreither/INTRO/master/INTRO_outdated.owl#SpatialEntity">
        <rdfs:subClassOf rdf:resource="https://raw.githubusercontent.com/BOberreither/INTRO/master/INTRO_outdated.owl#ArchitextualEntity"/>
        <rdfs:comment>As in: anglo-saxon, german, french, Viennese etc.</rdfs:comment>
        <rdfs:label>Spatial Entity</rdfs:label>
    </owl:Class>
    


    <!-- https://raw.githubusercontent.com/BOberreither/INTRO/master/INTRO_outdated.owl#SpatialMotif -->

    <owl:Class rdf:about="https://raw.githubusercontent.com/BOberreither/INTRO/master/INTRO_outdated.owl#SpatialMotif">
        <rdfs:subClassOf rdf:resource="https://raw.githubusercontent.com/BOberreither/INTRO/master/INTRO_outdated.owl#Motif"/>
    </owl:Class>
    


    <!-- https://raw.githubusercontent.com/BOberreither/INTRO/master/INTRO_outdated.owl#Subject -->

    <owl:Class rdf:about="https://raw.githubusercontent.com/BOberreither/INTRO/master/INTRO_outdated.owl#Subject">
        <rdfs:subClassOf rdf:resource="https://raw.githubusercontent.com/BOberreither/INTRO/master/INTRO_outdated.owl#SemanticEntity"/>
    </owl:Class>
    


    <!-- https://raw.githubusercontent.com/BOberreither/INTRO/master/INTRO_outdated.owl#Subtext -->

    <owl:Class rdf:about="https://raw.githubusercontent.com/BOberreither/INTRO/master/INTRO_outdated.owl#Subtext">
        <rdfs:subClassOf rdf:resource="https://raw.githubusercontent.com/BOberreither/INTRO/master/INTRO_outdated.owl#SemanticEntity"/>
    </owl:Class>
    


    <!-- https://raw.githubusercontent.com/BOberreither/INTRO/master/INTRO_outdated.owl#Subtitle -->

    <owl:Class rdf:about="https://raw.githubusercontent.com/BOberreither/INTRO/master/INTRO_outdated.owl#Subtitle">
        <rdfs:subClassOf rdf:resource="https://raw.githubusercontent.com/BOberreither/INTRO/master/INTRO_outdated.owl#FormalEntity"/>
    </owl:Class>
    


    <!-- https://raw.githubusercontent.com/BOberreither/INTRO/master/INTRO_outdated.owl#SupratextualEntity -->

    <owl:Class rdf:about="https://raw.githubusercontent.com/BOberreither/INTRO/master/INTRO_outdated.owl#SupratextualEntity">
        <rdfs:subClassOf rdf:resource="http://www.cidoc-crm.org/cidoc-crm/E28_Conceptual_Object"/>
        <rdfs:subClassOf>
            <owl:Restriction>
                <owl:onProperty rdf:resource="https://raw.githubusercontent.com/BOberreither/INTRO/master/INTRO_outdated.owl#definitionProvidedBy"/>
                <owl:allValuesFrom rdf:resource="https://raw.githubusercontent.com/BOberreither/INTRO/master/INTRO_outdated.owl#ActualizationOfFeature"/>
            </owl:Restriction>
        </rdfs:subClassOf>
        <rdfs:subClassOf>
            <owl:Restriction>
                <owl:onProperty rdf:resource="https://raw.githubusercontent.com/BOberreither/INTRO/master/INTRO_outdated.owl#hasParaphraseOrDefinition"/>
                <owl:allValuesFrom rdf:resource="http://www.w3.org/2001/XMLSchema#string"/>
            </owl:Restriction>
        </rdfs:subClassOf>
        <rdfs:comment>A very interesting class of textual entities. We&apos;ve never actually &apos;seen&apos; one, we&apos;ve only heard people talk about it using terms and phrases such as &apos;texte général&apos;, &apos;system&apos;, &apos;code&apos;, etc.</rdfs:comment>
        <rdfs:label>Supratextual Entity</rdfs:label>
    </owl:Class>
    


    <!-- https://raw.githubusercontent.com/BOberreither/INTRO/master/INTRO_outdated.owl#Tableau -->

    <owl:Class rdf:about="https://raw.githubusercontent.com/BOberreither/INTRO/master/INTRO_outdated.owl#Tableau">
        <rdfs:subClassOf rdf:resource="https://raw.githubusercontent.com/BOberreither/INTRO/master/INTRO_outdated.owl#FormalEntity"/>
        <rdfs:label>Tableau (Drama)</rdfs:label>
    </owl:Class>
    


    <!-- https://raw.githubusercontent.com/BOberreither/INTRO/master/INTRO_outdated.owl#TemporalEntity -->

    <owl:Class rdf:about="https://raw.githubusercontent.com/BOberreither/INTRO/master/INTRO_outdated.owl#TemporalEntity">
        <rdfs:subClassOf rdf:resource="https://raw.githubusercontent.com/BOberreither/INTRO/master/INTRO_outdated.owl#ArchitextualEntity"/>
        <rdfs:comment>As in: the 19th century, the 60ies etc.</rdfs:comment>
        <rdfs:label>Temporal Entity</rdfs:label>
    </owl:Class>
    


    <!-- https://raw.githubusercontent.com/BOberreither/INTRO/master/INTRO_outdated.owl#TemporalMotif -->

    <owl:Class rdf:about="https://raw.githubusercontent.com/BOberreither/INTRO/master/INTRO_outdated.owl#TemporalMotif">
        <rdfs:subClassOf rdf:resource="https://raw.githubusercontent.com/BOberreither/INTRO/master/INTRO_outdated.owl#Motif"/>
    </owl:Class>
    


    <!-- https://raw.githubusercontent.com/BOberreither/INTRO/master/INTRO_outdated.owl#Theme -->

    <owl:Class rdf:about="https://raw.githubusercontent.com/BOberreither/INTRO/master/INTRO_outdated.owl#Theme">
        <rdfs:subClassOf rdf:resource="https://raw.githubusercontent.com/BOberreither/INTRO/master/INTRO_outdated.owl#SemanticEntity"/>
    </owl:Class>
    


    <!-- https://raw.githubusercontent.com/BOberreither/INTRO/master/INTRO_outdated.owl#TypeMotif -->

    <owl:Class rdf:about="https://raw.githubusercontent.com/BOberreither/INTRO/master/INTRO_outdated.owl#TypeMotif">
        <rdfs:subClassOf rdf:resource="https://raw.githubusercontent.com/BOberreither/INTRO/master/INTRO_outdated.owl#Motif"/>
    </owl:Class>
    


    <!-- https://raw.githubusercontent.com/BOberreither/INTRO/master/INTRO_outdated.owl#TypeOfIntertextualRelationship -->

    <owl:Class rdf:about="https://raw.githubusercontent.com/BOberreither/INTRO/master/INTRO_outdated.owl#TypeOfIntertextualRelationship">
        <rdfs:subClassOf rdf:resource="http://www.cidoc-crm.org/cidoc-crm/E55_Type"/>
        <rdfs:subClassOf>
            <owl:Restriction>
                <owl:onProperty rdf:resource="https://raw.githubusercontent.com/BOberreither/INTRO/master/INTRO_outdated.owl#definitionProvidedBy"/>
                <owl:allValuesFrom rdf:resource="https://raw.githubusercontent.com/BOberreither/INTRO/master/INTRO_outdated.owl#ActualizationOfFeature"/>
            </owl:Restriction>
        </rdfs:subClassOf>
        <rdfs:subClassOf>
            <owl:Restriction>
                <owl:onProperty rdf:resource="https://raw.githubusercontent.com/BOberreither/INTRO/master/INTRO_outdated.owl#isTypeOf"/>
                <owl:allValuesFrom rdf:resource="https://raw.githubusercontent.com/BOberreither/INTRO/master/INTRO_outdated.owl#Reference"/>
            </owl:Restriction>
        </rdfs:subClassOf>
        <rdfs:subClassOf>
            <owl:Restriction>
                <owl:onProperty rdf:resource="https://raw.githubusercontent.com/BOberreither/INTRO/master/INTRO_outdated.owl#hasParaphraseOrDefinition"/>
                <owl:allValuesFrom rdf:resource="http://www.w3.org/2001/XMLSchema#string"/>
            </owl:Restriction>
        </rdfs:subClassOf>
        <rdfs:comment>This class comprises (as subclasses) the many classifications of intertextual relationships that can be found, for example, in specialised ontologies, in research literature, but also in greek rhetoric, in genre theory and so on.</rdfs:comment>
        <rdfs:label>Type of Intertextual Relationship</rdfs:label>
    </owl:Class>
    


    <!-- https://raw.githubusercontent.com/BOberreither/INTRO/master/INTRO_outdated.owl#VarietyOfText -->

    <owl:Class rdf:about="https://raw.githubusercontent.com/BOberreither/INTRO/master/INTRO_outdated.owl#VarietyOfText">
        <rdfs:subClassOf rdf:resource="https://raw.githubusercontent.com/BOberreither/INTRO/master/INTRO_outdated.owl#ArchitextualEntity"/>
        <rdfs:comment>As in: essay, letter, nvoel, grocery list etc.</rdfs:comment>
        <rdfs:label>Variety of Text</rdfs:label>
    </owl:Class>
    


    <!-- 
    ///////////////////////////////////////////////////////////////////////////////////////
    //
    // Individuals
    //
    ///////////////////////////////////////////////////////////////////////////////////////
     -->

    


    <!-- https://raw.githubusercontent.com/BOberreither/INTRO/master/INTRO_outdated.owl#CarettaCaretta_1stEd -->

    <owl:NamedIndividual rdf:about="https://raw.githubusercontent.com/BOberreither/INTRO/master/INTRO_outdated.owl#CarettaCaretta_1stEd">
        <rdf:type rdf:resource="http://iflastandards.info/ns/fr/frbr/frbroo/F3_Manifestation_Product_Type"/>
        <frbroo:R4i_comprises_carriers_of rdf:resource="https://raw.githubusercontent.com/BOberreither/INTRO/master/INTRO_outdated.owl#Caretta_Book"/>
        <hasProductTypeFragment rdf:resource="https://raw.githubusercontent.com/BOberreither/INTRO/master/INTRO_outdated.owl#CarettaCaretta_Passage1"/>
        <isAppurtenantElement rdf:resource="https://raw.githubusercontent.com/BOberreither/INTRO/master/INTRO_outdated.owl#TransT_OeuvreOfPaulusHochgatterer"/>
        <isDiscussedIn rdf:resource="https://raw.githubusercontent.com/BOberreither/INTRO/master/INTRO_outdated.owl#SomeDissertation_Interpretament2"/>
        <showsActualization rdf:resource="https://raw.githubusercontent.com/BOberreither/INTRO/master/INTRO_outdated.owl#CarettaCaretta_JudgementFashion"/>
        <hasBibliographicalData>Hochgatterer, Paulus: Caretta Caretta. A Novel. Transl. and with an afterword by Todd C. Hanlin. Riverside, CA: Ariadne Press 2010 (Studies in Austrian Literature, Culture and Thought. Translation Series).</hasBibliographicalData>
        <rdfs:label>&quot;CC&quot; - Buchausgabe</rdfs:label>
    </owl:NamedIndividual>
    


    <!-- https://raw.githubusercontent.com/BOberreither/INTRO/master/INTRO_outdated.owl#CarettaCaretta_Characteristic1 -->

    <owl:NamedIndividual rdf:about="https://raw.githubusercontent.com/BOberreither/INTRO/master/INTRO_outdated.owl#CarettaCaretta_Characteristic1">
        <rdf:type rdf:resource="https://raw.githubusercontent.com/BOberreither/INTRO/master/INTRO_outdated.owl#Characteristic"/>
        <characteristicShownBy rdf:resource="https://raw.githubusercontent.com/BOberreither/INTRO/master/INTRO_outdated.owl#CarettaCaretta_1stEd"/>
        <consistsIn rdf:resource="https://raw.githubusercontent.com/BOberreither/INTRO/master/INTRO_outdated.owl#CarettaCaretta_ThemeFashion"/>
        <isIdentifiedBy rdf:resource="https://raw.githubusercontent.com/BOberreither/INTRO/master/INTRO_outdated.owl#SomeDissertation_Interpretament1"/>
        <supportsAffiliationTo rdf:resource="https://raw.githubusercontent.com/BOberreither/INTRO/master/INTRO_outdated.owl#TransT_EpochGermanPopliterature"/>
        <hasParaphraseOrDefinition>The book (or: this edition of) &apos;Caretta Caretta&apos; thematising fashion is a characteristic supporting the novel&apos;s affiliation to the &apos;epoch&apos; of German pop literature.</hasParaphraseOrDefinition>
        <rdfs:label>&quot;CC&quot; - Charakteristikum 1</rdfs:label>
    </owl:NamedIndividual>
    


    <!-- https://raw.githubusercontent.com/BOberreither/INTRO/master/INTRO_outdated.owl#CarettaCaretta_Characteristic2 -->

    <owl:NamedIndividual rdf:about="https://raw.githubusercontent.com/BOberreither/INTRO/master/INTRO_outdated.owl#CarettaCaretta_Characteristic2">
        <rdf:type rdf:resource="https://raw.githubusercontent.com/BOberreither/INTRO/master/INTRO_outdated.owl#Characteristic"/>
        <characteristicShownBy rdf:resource="https://raw.githubusercontent.com/BOberreither/INTRO/master/INTRO_outdated.owl#CarettaCaretta_1stEd"/>
        <consistsIn rdf:resource="https://raw.githubusercontent.com/BOberreither/INTRO/master/INTRO_outdated.owl#CarettaCaretta_JudgementFashion"/>
        <isIdentifiedBy rdf:resource="https://raw.githubusercontent.com/BOberreither/INTRO/master/INTRO_outdated.owl#SomeDissertation_Interpretament1"/>
        <supportsNonAffiliationTo rdf:resource="https://raw.githubusercontent.com/BOberreither/INTRO/master/INTRO_outdated.owl#TransT_EpochGermanPopliterature"/>
        <hasParaphraseOrDefinition>The book (or: this edition of) &apos;Caretta Caretta&apos;s specific judgement of fashion as a part of youth culture is a characteristic distinguishing the novel from most of the representative novel&apos;s of the &apos;epoch&apos; of German pop literature, thus supporting the novel&apos;s non-affiliation to this architextual entity.</hasParaphraseOrDefinition>
        <rdfs:label>&quot;CC&quot; - Charakteristikum 2</rdfs:label>
    </owl:NamedIndividual>
    


    <!-- https://raw.githubusercontent.com/BOberreither/INTRO/master/INTRO_outdated.owl#CarettaCaretta_Fragment1 -->

    <owl:NamedIndividual rdf:about="https://raw.githubusercontent.com/BOberreither/INTRO/master/INTRO_outdated.owl#CarettaCaretta_Fragment1">
        <rdf:type rdf:resource="http://iflastandards.info/ns/fr/frbr/frbroo/F23_Expression_Fragment"/>
        <frbroo:R15i_is_fragment_of rdf:resource="https://raw.githubusercontent.com/BOberreither/INTRO/master/INTRO_outdated.owl#Caretta_Book"/>
        <rdfs:label>&quot;CC&quot; - Passage</rdfs:label>
    </owl:NamedIndividual>
    


    <!-- https://raw.githubusercontent.com/BOberreither/INTRO/master/INTRO_outdated.owl#CarettaCaretta_JudgementFashion -->

    <owl:NamedIndividual rdf:about="https://raw.githubusercontent.com/BOberreither/INTRO/master/INTRO_outdated.owl#CarettaCaretta_JudgementFashion">
        <rdf:type rdf:resource="https://raw.githubusercontent.com/BOberreither/INTRO/master/INTRO_outdated.owl#ActualizationOfFeature"/>
        <actualizationFoundOn rdf:resource="https://raw.githubusercontent.com/BOberreither/INTRO/master/INTRO_outdated.owl#CarettaCaretta_1stEd"/>
        <actualizesSemanticFeature rdf:resource="https://raw.githubusercontent.com/BOberreither/INTRO/master/INTRO_outdated.owl#SemEnt_JudgementFashion"/>
        <rdfs:label>&quot;CC&quot; - Urteil Modefetisch</rdfs:label>
    </owl:NamedIndividual>
    


    <!-- https://raw.githubusercontent.com/BOberreither/INTRO/master/INTRO_outdated.owl#CarettaCaretta_Passage1 -->

    <owl:NamedIndividual rdf:about="https://raw.githubusercontent.com/BOberreither/INTRO/master/INTRO_outdated.owl#CarettaCaretta_Passage1">
        <rdf:type rdf:resource="https://raw.githubusercontent.com/BOberreither/INTRO/master/INTRO_outdated.owl#ManifestationProductTypeFragment"/>
        <comprisesFragmentCarriersOf rdf:resource="https://raw.githubusercontent.com/BOberreither/INTRO/master/INTRO_outdated.owl#CarettaCaretta_Fragment1"/>
        <isDiscussedIn rdf:resource="https://raw.githubusercontent.com/BOberreither/INTRO/master/INTRO_outdated.owl#SomeDissertation_Interpretament2"/>
        <isProductTypeFragmentOf rdf:resource="https://raw.githubusercontent.com/BOberreither/INTRO/master/INTRO_outdated.owl#CarettaCaretta_1stEd"/>
        <isReferringEntity rdf:resource="https://raw.githubusercontent.com/BOberreither/INTRO/master/INTRO_outdated.owl#CarettaCaretta_Reference_ItsAMagicalWorld1"/>
        <hasLocation>pp. 222f.</hasLocation>
        <hasWording>First I plopped down on the mat and [...] read my Calvin &amp; Hobbes all the way through: Calvin is standing in a downpour, in complete uniform, with an umbrella, boots, and a hood with full facemask: and when the sun comes out after three minutes, he&apos;s still standing there, just as before. [...] &apos;And so he stood there for the rest of the day in his grotesque outfit.&apos; Shit.</hasWording>
        <rdfs:label>&quot;CC&quot; - Passage Buchausgabe</rdfs:label>
    </owl:NamedIndividual>
    


    <!-- https://raw.githubusercontent.com/BOberreither/INTRO/master/INTRO_outdated.owl#CarettaCaretta_Reference_ItsAMagicalWorld1 -->

    <owl:NamedIndividual rdf:about="https://raw.githubusercontent.com/BOberreither/INTRO/master/INTRO_outdated.owl#CarettaCaretta_Reference_ItsAMagicalWorld1">
        <rdf:type rdf:resource="https://raw.githubusercontent.com/BOberreither/INTRO/master/INTRO_outdated.owl#Reference"/>
        <hasReferredToEntity rdf:resource="https://raw.githubusercontent.com/BOberreither/INTRO/master/INTRO_outdated.owl#ItsAMagicalWorld_Passage1"/>
        <hasReferringEntity rdf:resource="https://raw.githubusercontent.com/BOberreither/INTRO/master/INTRO_outdated.owl#CarettaCaretta_Passage1"/>
        <hasType rdf:resource="https://raw.githubusercontent.com/BOberreither/INTRO/master/INTRO_outdated.owl#Genette_1_Intertextuality"/>
        <isIdentifiedBy rdf:resource="https://raw.githubusercontent.com/BOberreither/INTRO/master/INTRO_outdated.owl#SomeDissertation_Interpretament2"/>
        <rdfs:label>Verweis &quot;CC&quot; - &quot;MW&quot;</rdfs:label>
    </owl:NamedIndividual>
    


    <!-- https://raw.githubusercontent.com/BOberreither/INTRO/master/INTRO_outdated.owl#CarettaCaretta_ThemeFashion -->

    <owl:NamedIndividual rdf:about="https://raw.githubusercontent.com/BOberreither/INTRO/master/INTRO_outdated.owl#CarettaCaretta_ThemeFashion">
        <rdf:type rdf:resource="https://raw.githubusercontent.com/BOberreither/INTRO/master/INTRO_outdated.owl#ActualizationOfFeature"/>
        <actualizationFoundOn rdf:resource="https://raw.githubusercontent.com/BOberreither/INTRO/master/INTRO_outdated.owl#CarettaCaretta_1stEd"/>
        <actualizesSemanticFeature rdf:resource="https://raw.githubusercontent.com/BOberreither/INTRO/master/INTRO_outdated.owl#SemEnt_ThemeFashion"/>
        <rdfs:label>&quot;CC&quot; - Modefetisch</rdfs:label>
    </owl:NamedIndividual>
    


    <!-- https://raw.githubusercontent.com/BOberreither/INTRO/master/INTRO_outdated.owl#Caretta_Book -->

    <owl:NamedIndividual rdf:about="https://raw.githubusercontent.com/BOberreither/INTRO/master/INTRO_outdated.owl#Caretta_Book">
        <rdf:type rdf:resource="http://iflastandards.info/ns/fr/frbr/frbroo/F22_Self-Contained_Expression"/>
        <frbroo:R3i_realises rdf:resource="https://raw.githubusercontent.com/BOberreither/INTRO/master/INTRO_outdated.owl#Caretta_Work"/>
        <hasBibliographicalData>Hochgatterer, Paulus: Caretta Caretta</hasBibliographicalData>
        <rdfs:label>&quot;CC&quot; - Buch</rdfs:label>
    </owl:NamedIndividual>
    


    <!-- https://raw.githubusercontent.com/BOberreither/INTRO/master/INTRO_outdated.owl#Caretta_Work -->

    <owl:NamedIndividual rdf:about="https://raw.githubusercontent.com/BOberreither/INTRO/master/INTRO_outdated.owl#Caretta_Work">
        <rdf:type rdf:resource="http://iflastandards.info/ns/fr/frbr/frbroo/F1_Work"/>
        <frbroo:R3_is_realised_in rdf:resource="https://raw.githubusercontent.com/BOberreither/INTRO/master/INTRO_outdated.owl#Caretta_Book"/>
        <hasBibliographicalData>(Hochgatterer, Paulus): (Caretta Caretta)</hasBibliographicalData>
        <rdfs:label>&quot;CC&quot; - [platon.] &apos;Werk&apos;</rdfs:label>
    </owl:NamedIndividual>
    


    <!-- https://raw.githubusercontent.com/BOberreither/INTRO/master/INTRO_outdated.owl#Genette_1_Intertextuality -->

    <owl:NamedIndividual rdf:about="https://raw.githubusercontent.com/BOberreither/INTRO/master/INTRO_outdated.owl#Genette_1_Intertextuality">
        <rdf:type rdf:resource="https://raw.githubusercontent.com/BOberreither/INTRO/master/INTRO_outdated.owl#Genette"/>
        <definitionProvidedBy rdf:resource="https://raw.githubusercontent.com/BOberreither/INTRO/master/INTRO_outdated.owl#Palimpsests_ActualizationDefinitionInt"/>
        <isTypeOf rdf:resource="https://raw.githubusercontent.com/BOberreither/INTRO/master/INTRO_outdated.owl#CarettaCaretta_Reference_ItsAMagicalWorld1"/>
        <rdfs:label>&quot;Intertext.&quot; nach Genette</rdfs:label>
    </owl:NamedIndividual>
    


    <!-- https://raw.githubusercontent.com/BOberreither/INTRO/master/INTRO_outdated.owl#ItsAMagicalWorld_1stEd -->

    <owl:NamedIndividual rdf:about="https://raw.githubusercontent.com/BOberreither/INTRO/master/INTRO_outdated.owl#ItsAMagicalWorld_1stEd">
        <rdf:type rdf:resource="http://iflastandards.info/ns/fr/frbr/frbroo/F3_Manifestation_Product_Type"/>
        <frbroo:R4i_comprises_carriers_of rdf:resource="https://raw.githubusercontent.com/BOberreither/INTRO/master/INTRO_outdated.owl#ItsAMagicalWorld_Book"/>
        <hasProductTypeFragment rdf:resource="https://raw.githubusercontent.com/BOberreither/INTRO/master/INTRO_outdated.owl#ItsAMagicalWorld_Passage1"/>
        <isAppurtenantElement rdf:resource="https://raw.githubusercontent.com/BOberreither/INTRO/master/INTRO_outdated.owl#TransT_OeuvreOfBillWatterson"/>
        <hasBibliographicalData>Watterson, Bill (1996): It&apos;s a Magical World. London: Andrews McMeel Books.</hasBibliographicalData>
        <rdfs:label>&quot;MW&quot; - Buchausgabe</rdfs:label>
    </owl:NamedIndividual>
    


    <!-- https://raw.githubusercontent.com/BOberreither/INTRO/master/INTRO_outdated.owl#ItsAMagicalWorld_Book -->

    <owl:NamedIndividual rdf:about="https://raw.githubusercontent.com/BOberreither/INTRO/master/INTRO_outdated.owl#ItsAMagicalWorld_Book">
        <rdf:type rdf:resource="http://iflastandards.info/ns/fr/frbr/frbroo/F2_Expression"/>
        <frbroo:R3i_realises rdf:resource="https://raw.githubusercontent.com/BOberreither/INTRO/master/INTRO_outdated.owl#ItsAMagicalWorld_Work"/>
        <hasBibliographicalData>Watterson, Bill: It&apos;s a Magical World</hasBibliographicalData>
        <rdfs:label>&quot;MW&quot; - Buch</rdfs:label>
    </owl:NamedIndividual>
    


    <!-- https://raw.githubusercontent.com/BOberreither/INTRO/master/INTRO_outdated.owl#ItsAMagicalWorld_Fragment1 -->

    <owl:NamedIndividual rdf:about="https://raw.githubusercontent.com/BOberreither/INTRO/master/INTRO_outdated.owl#ItsAMagicalWorld_Fragment1">
        <rdf:type rdf:resource="http://iflastandards.info/ns/fr/frbr/frbroo/F23_Expression_Fragment"/>
        <frbroo:R15i_is_fragment_of rdf:resource="https://raw.githubusercontent.com/BOberreither/INTRO/master/INTRO_outdated.owl#ItsAMagicalWorld_Book"/>
        <isAppurtenantElement rdf:resource="https://raw.githubusercontent.com/BOberreither/INTRO/master/INTRO_outdated.owl#TransT_DiscourseOnFashion"/>
        <rdfs:label>&quot;MW&quot; - Passage</rdfs:label>
    </owl:NamedIndividual>
    


    <!-- https://raw.githubusercontent.com/BOberreither/INTRO/master/INTRO_outdated.owl#ItsAMagicalWorld_Passage1 -->

    <owl:NamedIndividual rdf:about="https://raw.githubusercontent.com/BOberreither/INTRO/master/INTRO_outdated.owl#ItsAMagicalWorld_Passage1">
        <rdf:type rdf:resource="https://raw.githubusercontent.com/BOberreither/INTRO/master/INTRO_outdated.owl#ManifestationProductTypeFragment"/>
        <comprisesFragmentCarriersOf rdf:resource="https://raw.githubusercontent.com/BOberreither/INTRO/master/INTRO_outdated.owl#ItsAMagicalWorld_Fragment1"/>
        <isAppurtenantElement rdf:resource="https://raw.githubusercontent.com/BOberreither/INTRO/master/INTRO_outdated.owl#TransT_DiscourseOnFashion"/>
        <hasBibliographicalData>Watterson, Bill (1996): It&apos;s a Magical World. London: Andrews McMeel books, p. SEITENZAHL</hasBibliographicalData>
        <hasLocation>somewhere in CaH</hasLocation>
        <hasWording>Some words from CaH</hasWording>
        <rdfs:label>&quot;MW&quot; - Passage Buchausgabe</rdfs:label>
    </owl:NamedIndividual>
    


    <!-- https://raw.githubusercontent.com/BOberreither/INTRO/master/INTRO_outdated.owl#ItsAMagicalWorld_Work -->

    <owl:NamedIndividual rdf:about="https://raw.githubusercontent.com/BOberreither/INTRO/master/INTRO_outdated.owl#ItsAMagicalWorld_Work">
        <rdf:type rdf:resource="http://iflastandards.info/ns/fr/frbr/frbroo/F1_Work"/>
        <isAppurtenantElement rdf:resource="https://raw.githubusercontent.com/BOberreither/INTRO/master/INTRO_outdated.owl#TransT_OeuvreOfBillWatterson"/>
        <hasBibliographicalData>(Watterson, Bill): (It&apos;s a magical World)</hasBibliographicalData>
        <rdfs:label>&quot;MW&quot; - [platon] &apos;Werk&apos;</rdfs:label>
    </owl:NamedIndividual>
    


    <!-- https://raw.githubusercontent.com/BOberreither/INTRO/master/INTRO_outdated.owl#Palimpsests_1stEd -->

    <owl:NamedIndividual rdf:about="https://raw.githubusercontent.com/BOberreither/INTRO/master/INTRO_outdated.owl#Palimpsests_1stEd">
        <rdf:type rdf:resource="http://iflastandards.info/ns/fr/frbr/frbroo/F3_Manifestation_Product_Type"/>
        <hasProductTypeFragment rdf:resource="https://raw.githubusercontent.com/BOberreither/INTRO/master/INTRO_outdated.owl#Palimpsests_Passage1"/>
        <hasBibliographicalData>Genette, Gérard: Palimpsests. Literature in the Second Degree. Transl. by Channa Newman &amp; Claude Doubinsky. Foreword by Gerald Price. Lincoln and London: Univ. of Nebraska Press 1997.</hasBibliographicalData>
        <rdfs:label>&quot;P&quot; - Buchausgabe</rdfs:label>
    </owl:NamedIndividual>
    


    <!-- https://raw.githubusercontent.com/BOberreither/INTRO/master/INTRO_outdated.owl#Palimpsests_ActualizationDefinitionInt -->

    <owl:NamedIndividual rdf:about="https://raw.githubusercontent.com/BOberreither/INTRO/master/INTRO_outdated.owl#Palimpsests_ActualizationDefinitionInt">
        <rdf:type rdf:resource="https://raw.githubusercontent.com/BOberreither/INTRO/master/INTRO_outdated.owl#ActualizationOfFeature"/>
        <actualizationFoundOn rdf:resource="https://raw.githubusercontent.com/BOberreither/INTRO/master/INTRO_outdated.owl#Palimpsests_Passage1"/>
        <actualizesFeature rdf:resource="https://raw.githubusercontent.com/BOberreither/INTRO/master/INTRO_outdated.owl#SemEnt_Definition_GenetteIntertextuality"/>
        <rdfs:label>&quot;P&quot; - Definition</rdfs:label>
    </owl:NamedIndividual>
    


    <!-- https://raw.githubusercontent.com/BOberreither/INTRO/master/INTRO_outdated.owl#Palimpsests_Book -->

    <owl:NamedIndividual rdf:about="https://raw.githubusercontent.com/BOberreither/INTRO/master/INTRO_outdated.owl#Palimpsests_Book">
        <rdf:type rdf:resource="http://iflastandards.info/ns/fr/frbr/frbroo/F22_Self-Contained_Expression"/>
        <frbroo:R3i_realises rdf:resource="https://raw.githubusercontent.com/BOberreither/INTRO/master/INTRO_outdated.owl#Palimpsests_Work"/>
        <hasBibliographicalData>Genette, Gérard: Palimpsests</hasBibliographicalData>
        <rdfs:label>&quot;P&quot; - Buch</rdfs:label>
    </owl:NamedIndividual>
    


    <!-- https://raw.githubusercontent.com/BOberreither/INTRO/master/INTRO_outdated.owl#Palimpsests_Fragment1 -->

    <owl:NamedIndividual rdf:about="https://raw.githubusercontent.com/BOberreither/INTRO/master/INTRO_outdated.owl#Palimpsests_Fragment1">
        <rdf:type rdf:resource="http://iflastandards.info/ns/fr/frbr/frbroo/F23_Expression_Fragment"/>
        <frbroo:R15i_is_fragment_of rdf:resource="https://raw.githubusercontent.com/BOberreither/INTRO/master/INTRO_outdated.owl#Palimpsests_Book"/>
        <fragmentCarriersProvidedBy rdf:resource="https://raw.githubusercontent.com/BOberreither/INTRO/master/INTRO_outdated.owl#Palimpsests_Passage1"/>
        <rdfs:label>&quot;P&quot; - Passage</rdfs:label>
    </owl:NamedIndividual>
    


    <!-- https://raw.githubusercontent.com/BOberreither/INTRO/master/INTRO_outdated.owl#Palimpsests_Passage1 -->

    <owl:NamedIndividual rdf:about="https://raw.githubusercontent.com/BOberreither/INTRO/master/INTRO_outdated.owl#Palimpsests_Passage1">
        <rdf:type rdf:resource="https://raw.githubusercontent.com/BOberreither/INTRO/master/INTRO_outdated.owl#ManifestationProductTypeFragment"/>
        <comprisesFragmentCarriersOf rdf:resource="https://raw.githubusercontent.com/BOberreither/INTRO/master/INTRO_outdated.owl#Palimpsests_Fragment1"/>
        <isProductTypeFragmentOf rdf:resource="https://raw.githubusercontent.com/BOberreither/INTRO/master/INTRO_outdated.owl#Palimpsests_1stEd"/>
        <hasLocation>pp. 1f.</hasLocation>
        <hasWording>The first type was explored some years ago by Julia Kristeva, under the name of [i]intertextuality[/i] [...]. For my part I define it, no doubt in a amore restrictive sens, as a relationship of copresence between two texts or among several texts: that is to say, eidetically and typically as the actual presence of one text within another. In its  most explicit and literal form, it is the traditional practice of [i]quoting[/i] (with quotation marks, with or without specific referendes). In another less explicit and canonical form, it is the practice of [i]plagiarism[/i] [...], which is an undeclared but still literal borrowing. Again, in still less explicit and lessl iteral guise, it is the practice of [i]allusion[/i]:  that is an enunciation whose full meaning presupposes the perception of relantionship between it and another text, to which it necessarily refers by some inflections that otherwise remain unintelligible.</hasWording>
        <rdfs:label>&quot;P&quot; - Passage Buchausgabe</rdfs:label>
    </owl:NamedIndividual>
    


    <!-- https://raw.githubusercontent.com/BOberreither/INTRO/master/INTRO_outdated.owl#Palimpsests_Work -->

    <owl:NamedIndividual rdf:about="https://raw.githubusercontent.com/BOberreither/INTRO/master/INTRO_outdated.owl#Palimpsests_Work">
        <rdf:type rdf:resource="http://iflastandards.info/ns/fr/frbr/frbroo/F1_Work"/>
        <frbroo:R3_is_realised_in rdf:resource="https://raw.githubusercontent.com/BOberreither/INTRO/master/INTRO_outdated.owl#Palimpsests_Book"/>
        <hasBibliographicalData>(Genette, Gérard): (Palimpsests)</hasBibliographicalData>
        <rdfs:label>&quot;P&quot; - [quasiplaton.] &apos;Werk&apos;</rdfs:label>
    </owl:NamedIndividual>
    


    <!-- https://raw.githubusercontent.com/BOberreither/INTRO/master/INTRO_outdated.owl#SemEnt_Definition_GenetteIntertextuality -->

    <owl:NamedIndividual rdf:about="https://raw.githubusercontent.com/BOberreither/INTRO/master/INTRO_outdated.owl#SemEnt_Definition_GenetteIntertextuality">
        <rdf:type rdf:resource="https://raw.githubusercontent.com/BOberreither/INTRO/master/INTRO_outdated.owl#Definition"/>
        <featureActualizedIn rdf:resource="https://raw.githubusercontent.com/BOberreither/INTRO/master/INTRO_outdated.owl#Palimpsests_ActualizationDefinitionInt"/>
        <rdfs:label>Def. &quot;Intertextualität&quot;</rdfs:label>
    </owl:NamedIndividual>
    


    <!-- https://raw.githubusercontent.com/BOberreither/INTRO/master/INTRO_outdated.owl#SemEnt_JudgementFashion -->

    <owl:NamedIndividual rdf:about="https://raw.githubusercontent.com/BOberreither/INTRO/master/INTRO_outdated.owl#SemEnt_JudgementFashion">
        <rdf:type rdf:resource="https://raw.githubusercontent.com/BOberreither/INTRO/master/INTRO_outdated.owl#Opinion"/>
        <hasOpinionObject rdf:resource="https://raw.githubusercontent.com/BOberreither/INTRO/master/INTRO_outdated.owl#SemEnt_ThemeFashion"/>
        <semanticFeatureActualizedIn rdf:resource="https://raw.githubusercontent.com/BOberreither/INTRO/master/INTRO_outdated.owl#CarettaCaretta_JudgementFashion"/>
        <rdfs:label>Urteil Mode (Sem.)</rdfs:label>
    </owl:NamedIndividual>
    


    <!-- https://raw.githubusercontent.com/BOberreither/INTRO/master/INTRO_outdated.owl#SemEnt_TextInterpretation -->

    <owl:NamedIndividual rdf:about="https://raw.githubusercontent.com/BOberreither/INTRO/master/INTRO_outdated.owl#SemEnt_TextInterpretation">
        <rdf:type rdf:resource="https://raw.githubusercontent.com/BOberreither/INTRO/master/INTRO_outdated.owl#Interpretation"/>
        <featureActualizedIn rdf:resource="https://raw.githubusercontent.com/BOberreither/INTRO/master/INTRO_outdated.owl#SomeDissertation_ActualizationInt_1"/>
        <featureActualizedIn rdf:resource="https://raw.githubusercontent.com/BOberreither/INTRO/master/INTRO_outdated.owl#SomeDissertation_ActualizationInt_2"/>
        <rdfs:label>Textanalyse (Sem.)</rdfs:label>
    </owl:NamedIndividual>
    


    <!-- https://raw.githubusercontent.com/BOberreither/INTRO/master/INTRO_outdated.owl#SemEnt_ThemeFashion -->

    <owl:NamedIndividual rdf:about="https://raw.githubusercontent.com/BOberreither/INTRO/master/INTRO_outdated.owl#SemEnt_ThemeFashion">
        <rdf:type rdf:resource="https://raw.githubusercontent.com/BOberreither/INTRO/master/INTRO_outdated.owl#Theme"/>
        <featureActualizedIn rdf:resource="https://raw.githubusercontent.com/BOberreither/INTRO/master/INTRO_outdated.owl#CarettaCaretta_ThemeFashion"/>
        <supportProvidedBy rdf:resource="https://raw.githubusercontent.com/BOberreither/INTRO/master/INTRO_outdated.owl#SomeHandbookPass1"/>
        <rdfs:label>Thema Mode (Sem.)</rdfs:label>
    </owl:NamedIndividual>
    


    <!-- https://raw.githubusercontent.com/BOberreither/INTRO/master/INTRO_outdated.owl#SomeDissertationFrag1 -->

    <owl:NamedIndividual rdf:about="https://raw.githubusercontent.com/BOberreither/INTRO/master/INTRO_outdated.owl#SomeDissertationFrag1">
        <rdf:type rdf:resource="http://iflastandards.info/ns/fr/frbr/frbroo/F23_Expression_Fragment"/>
        <frbroo:R15i_is_fragment_of rdf:resource="https://raw.githubusercontent.com/BOberreither/INTRO/master/INTRO_outdated.owl#SomeDissertation_Book"/>
        <rdfs:label>Diss. - Passage1</rdfs:label>
    </owl:NamedIndividual>
    


    <!-- https://raw.githubusercontent.com/BOberreither/INTRO/master/INTRO_outdated.owl#SomeDissertationFrag2 -->

    <owl:NamedIndividual rdf:about="https://raw.githubusercontent.com/BOberreither/INTRO/master/INTRO_outdated.owl#SomeDissertationFrag2">
        <rdf:type rdf:resource="http://iflastandards.info/ns/fr/frbr/frbroo/F23_Expression_Fragment"/>
        <frbroo:R15i_is_fragment_of rdf:resource="https://raw.githubusercontent.com/BOberreither/INTRO/master/INTRO_outdated.owl#SomeDissertation_Book"/>
        <rdfs:label>Diss. - Passage 2</rdfs:label>
    </owl:NamedIndividual>
    


    <!-- https://raw.githubusercontent.com/BOberreither/INTRO/master/INTRO_outdated.owl#SomeDissertationPass_1 -->

    <owl:NamedIndividual rdf:about="https://raw.githubusercontent.com/BOberreither/INTRO/master/INTRO_outdated.owl#SomeDissertationPass_1">
        <rdf:type rdf:resource="https://raw.githubusercontent.com/BOberreither/INTRO/master/INTRO_outdated.owl#ManifestationProductTypeFragment"/>
        <comprisesFragmentCarriersOf rdf:resource="https://raw.githubusercontent.com/BOberreither/INTRO/master/INTRO_outdated.owl#SomeDissertationFrag1"/>
        <isProductTypeFragmentOf rdf:resource="https://raw.githubusercontent.com/BOberreither/INTRO/master/INTRO_outdated.owl#SomeDissertation_1stEd"/>
        <rdfs:label>Diss. - Passage Buchausg.1</rdfs:label>
    </owl:NamedIndividual>
    


    <!-- https://raw.githubusercontent.com/BOberreither/INTRO/master/INTRO_outdated.owl#SomeDissertationPass_2 -->

    <owl:NamedIndividual rdf:about="https://raw.githubusercontent.com/BOberreither/INTRO/master/INTRO_outdated.owl#SomeDissertationPass_2">
        <rdf:type rdf:resource="https://raw.githubusercontent.com/BOberreither/INTRO/master/INTRO_outdated.owl#ManifestationProductTypeFragment"/>
        <comprisesFragmentCarriersOf rdf:resource="https://raw.githubusercontent.com/BOberreither/INTRO/master/INTRO_outdated.owl#SomeDissertationFrag2"/>
        <holdsInterpretament rdf:resource="https://raw.githubusercontent.com/BOberreither/INTRO/master/INTRO_outdated.owl#SomeDissertation_Interpretament2"/>
        <isProductTypeFragmentOf rdf:resource="https://raw.githubusercontent.com/BOberreither/INTRO/master/INTRO_outdated.owl#SomeDissertation_1stEd"/>
        <hasLocation>p. 196</hasLocation>
        <hasWording>Hier werden zudem zwei wichtige Intertexte verwoben. Swordfishtrombones ist das Album von Tom Waits von 1983, das Dominik von seinem Betreuer (Cord-Blouson und Doc Martens) geschenkt bekommen hat; Calvin &amp; Hobbes bezeichnet die letzte der be-treffenden Comicsammlungen von Bill Watterson (It’s a magical World, dt.: Eine Welt voller Wunder).
Im ersten Intertext – Down down down – ist von der unaufhaltsamen Höllenfahrt eines als „boy“ titulierten Missetäters die Rede. So weit, so naheliegend die Identifikationsleistung Dominiks; verschränkt wird die Idee von der Höllenfahrt allerdings mit dem vermeintlich geringeren Verhängnis des Kindes (Calvin), das bemerken muss, falsch angezogen zu sein, genauer: mit der Regenkleidung eine Ausrüstung gewählt zu haben, die für die unmittelbare Vergangenheit zwar unumgänglich war (drei Minuten starker Re-gen), in Zukunft (bei Sonnenschein) jedoch vor allem hinderlich sein würde.</hasWording>
        <rdfs:label>Diss. - Passage Buchausg. 2</rdfs:label>
    </owl:NamedIndividual>
    


    <!-- https://raw.githubusercontent.com/BOberreither/INTRO/master/INTRO_outdated.owl#SomeDissertation_1stEd -->

    <owl:NamedIndividual rdf:about="https://raw.githubusercontent.com/BOberreither/INTRO/master/INTRO_outdated.owl#SomeDissertation_1stEd">
        <rdf:type rdf:resource="http://iflastandards.info/ns/fr/frbr/frbroo/F3_Manifestation_Product_Type"/>
        <frbroo:R4i_comprises_carriers_of rdf:resource="https://raw.githubusercontent.com/BOberreither/INTRO/master/INTRO_outdated.owl#SomeDissertation_Book"/>
        <hasBibliographicalData>SomePhDStudent: SomeDissertation. University. Year.</hasBibliographicalData>
        <rdfs:label>Diss. - Buchausgabe</rdfs:label>
    </owl:NamedIndividual>
    


    <!-- https://raw.githubusercontent.com/BOberreither/INTRO/master/INTRO_outdated.owl#SomeDissertation_ActualizationInt_1 -->

    <owl:NamedIndividual rdf:about="https://raw.githubusercontent.com/BOberreither/INTRO/master/INTRO_outdated.owl#SomeDissertation_ActualizationInt_1">
        <rdf:type rdf:resource="https://raw.githubusercontent.com/BOberreither/INTRO/master/INTRO_outdated.owl#ActualizationOfFeature"/>
        <actualizesSemanticFeature rdf:resource="https://raw.githubusercontent.com/BOberreither/INTRO/master/INTRO_outdated.owl#SemEnt_TextInterpretation"/>
        <rdfs:label>Diss. - Textanalyse</rdfs:label>
    </owl:NamedIndividual>
    


    <!-- https://raw.githubusercontent.com/BOberreither/INTRO/master/INTRO_outdated.owl#SomeDissertation_ActualizationInt_2 -->

    <owl:NamedIndividual rdf:about="https://raw.githubusercontent.com/BOberreither/INTRO/master/INTRO_outdated.owl#SomeDissertation_ActualizationInt_2">
        <rdf:type rdf:resource="https://raw.githubusercontent.com/BOberreither/INTRO/master/INTRO_outdated.owl#ActualizationOfFeature"/>
        <actualizationFoundOn rdf:resource="https://raw.githubusercontent.com/BOberreither/INTRO/master/INTRO_outdated.owl#SomeDissertationPass_2"/>
        <actualizesSemanticFeature rdf:resource="https://raw.githubusercontent.com/BOberreither/INTRO/master/INTRO_outdated.owl#SemEnt_TextInterpretation"/>
        <rdfs:label>Diss. - 2. Textanalyse</rdfs:label>
    </owl:NamedIndividual>
    


    <!-- https://raw.githubusercontent.com/BOberreither/INTRO/master/INTRO_outdated.owl#SomeDissertation_Book -->

    <owl:NamedIndividual rdf:about="https://raw.githubusercontent.com/BOberreither/INTRO/master/INTRO_outdated.owl#SomeDissertation_Book">
        <rdf:type rdf:resource="http://iflastandards.info/ns/fr/frbr/frbroo/F22_Self-Contained_Expression"/>
        <frbroo:R3i_realises rdf:resource="https://raw.githubusercontent.com/BOberreither/INTRO/master/INTRO_outdated.owl#SomeDissertation_Work"/>
        <rdfs:label>Diss. - Buch</rdfs:label>
    </owl:NamedIndividual>
    


    <!-- https://raw.githubusercontent.com/BOberreither/INTRO/master/INTRO_outdated.owl#SomeDissertation_Interpretament1 -->

    <owl:NamedIndividual rdf:about="https://raw.githubusercontent.com/BOberreither/INTRO/master/INTRO_outdated.owl#SomeDissertation_Interpretament1">
        <rdf:type rdf:resource="https://raw.githubusercontent.com/BOberreither/INTRO/master/INTRO_outdated.owl#Interpretament"/>
        <consistsIn rdf:resource="https://raw.githubusercontent.com/BOberreither/INTRO/master/INTRO_outdated.owl#SomeDissertation_ActualizationInt_1"/>
        <identifies rdf:resource="https://raw.githubusercontent.com/BOberreither/INTRO/master/INTRO_outdated.owl#CarettaCaretta_Characteristic1"/>
        <identifies rdf:resource="https://raw.githubusercontent.com/BOberreither/INTRO/master/INTRO_outdated.owl#CarettaCaretta_Characteristic2"/>
        <interpretamentOriginatingIn rdf:resource="https://raw.githubusercontent.com/BOberreither/INTRO/master/INTRO_outdated.owl#SomeDissertationPass_1"/>
        <rdfs:label>Diss. - 1. Int.-Akt</rdfs:label>
    </owl:NamedIndividual>
    


    <!-- https://raw.githubusercontent.com/BOberreither/INTRO/master/INTRO_outdated.owl#SomeDissertation_Interpretament2 -->

    <owl:NamedIndividual rdf:about="https://raw.githubusercontent.com/BOberreither/INTRO/master/INTRO_outdated.owl#SomeDissertation_Interpretament2">
        <rdf:type rdf:resource="https://raw.githubusercontent.com/BOberreither/INTRO/master/INTRO_outdated.owl#Interpretament"/>
        <consistsIn rdf:resource="https://raw.githubusercontent.com/BOberreither/INTRO/master/INTRO_outdated.owl#SomeDissertation_ActualizationInt_2"/>
        <discusses rdf:resource="https://raw.githubusercontent.com/BOberreither/INTRO/master/INTRO_outdated.owl#CarettaCaretta_Passage1"/>
        <discusses rdf:resource="https://raw.githubusercontent.com/BOberreither/INTRO/master/INTRO_outdated.owl#ItsAMagicalWorld_Passage1"/>
        <identifies rdf:resource="https://raw.githubusercontent.com/BOberreither/INTRO/master/INTRO_outdated.owl#CarettaCaretta_Reference_ItsAMagicalWorld1"/>
        <interpretamentOriginatingIn rdf:resource="https://raw.githubusercontent.com/BOberreither/INTRO/master/INTRO_outdated.owl#SomeDissertationPass_2"/>
        <rdfs:label>Diss. - 2. Int.-Akt</rdfs:label>
    </owl:NamedIndividual>
    


    <!-- https://raw.githubusercontent.com/BOberreither/INTRO/master/INTRO_outdated.owl#SomeDissertation_Work -->

    <owl:NamedIndividual rdf:about="https://raw.githubusercontent.com/BOberreither/INTRO/master/INTRO_outdated.owl#SomeDissertation_Work">
        <rdf:type rdf:resource="http://iflastandards.info/ns/fr/frbr/frbroo/F1_Work"/>
        <rdfs:label>Diss. - [platon]. Werk</rdfs:label>
    </owl:NamedIndividual>
    


    <!-- https://raw.githubusercontent.com/BOberreither/INTRO/master/INTRO_outdated.owl#SomeHandbookFrag1 -->

    <owl:NamedIndividual rdf:about="https://raw.githubusercontent.com/BOberreither/INTRO/master/INTRO_outdated.owl#SomeHandbookFrag1">
        <rdf:type rdf:resource="http://iflastandards.info/ns/fr/frbr/frbroo/F23_Expression_Fragment"/>
        <frbroo:R15i_is_fragment_of rdf:resource="https://raw.githubusercontent.com/BOberreither/INTRO/master/INTRO_outdated.owl#SomeHandbook_Book"/>
    </owl:NamedIndividual>
    


    <!-- https://raw.githubusercontent.com/BOberreither/INTRO/master/INTRO_outdated.owl#SomeHandbookPass1 -->

    <owl:NamedIndividual rdf:about="https://raw.githubusercontent.com/BOberreither/INTRO/master/INTRO_outdated.owl#SomeHandbookPass1">
        <rdf:type rdf:resource="https://raw.githubusercontent.com/BOberreither/INTRO/master/INTRO_outdated.owl#ManifestationProductTypeFragment"/>
        <comprisesFragmentCarriersOf rdf:resource="https://raw.githubusercontent.com/BOberreither/INTRO/master/INTRO_outdated.owl#SomeHandbookFrag1"/>
        <isProductTypeFragmentOf rdf:resource="https://raw.githubusercontent.com/BOberreither/INTRO/master/INTRO_outdated.owl#SomeHandbook_1stEd"/>
    </owl:NamedIndividual>
    


    <!-- https://raw.githubusercontent.com/BOberreither/INTRO/master/INTRO_outdated.owl#SomeHandbook_1stEd -->

    <owl:NamedIndividual rdf:about="https://raw.githubusercontent.com/BOberreither/INTRO/master/INTRO_outdated.owl#SomeHandbook_1stEd">
        <rdf:type rdf:resource="http://iflastandards.info/ns/fr/frbr/frbroo/F3_Manifestation_Product_Type"/>
        <frbroo:R4i_comprises_carriers_of rdf:resource="https://raw.githubusercontent.com/BOberreither/INTRO/master/INTRO_outdated.owl#SomeHandbook_Book"/>
    </owl:NamedIndividual>
    


    <!-- https://raw.githubusercontent.com/BOberreither/INTRO/master/INTRO_outdated.owl#SomeHandbook_Book -->

    <owl:NamedIndividual rdf:about="https://raw.githubusercontent.com/BOberreither/INTRO/master/INTRO_outdated.owl#SomeHandbook_Book">
        <rdf:type rdf:resource="http://iflastandards.info/ns/fr/frbr/frbroo/F22_Self-Contained_Expression"/>
        <frbroo:R3i_realises rdf:resource="https://raw.githubusercontent.com/BOberreither/INTRO/master/INTRO_outdated.owl#SomeHandbook_Work"/>
    </owl:NamedIndividual>
    


    <!-- https://raw.githubusercontent.com/BOberreither/INTRO/master/INTRO_outdated.owl#SomeHandbook_Work -->

    <owl:NamedIndividual rdf:about="https://raw.githubusercontent.com/BOberreither/INTRO/master/INTRO_outdated.owl#SomeHandbook_Work">
        <rdf:type rdf:resource="http://iflastandards.info/ns/fr/frbr/frbroo/F1_Work"/>
    </owl:NamedIndividual>
    


    <!-- https://raw.githubusercontent.com/BOberreither/INTRO/master/INTRO_outdated.owl#TransT_DiscourseOnFashion -->

    <owl:NamedIndividual rdf:about="https://raw.githubusercontent.com/BOberreither/INTRO/master/INTRO_outdated.owl#TransT_DiscourseOnFashion">
        <rdf:type rdf:resource="https://raw.githubusercontent.com/BOberreither/INTRO/master/INTRO_outdated.owl#Discourse"/>
        <hasAppurtenantElement rdf:resource="https://raw.githubusercontent.com/BOberreither/INTRO/master/INTRO_outdated.owl#CarettaCaretta_1stEd"/>
        <rdfs:label>Diskurs zur Mode</rdfs:label>
    </owl:NamedIndividual>
    


    <!-- https://raw.githubusercontent.com/BOberreither/INTRO/master/INTRO_outdated.owl#TransT_DiscourseScholarlyDiscourseOnLiterature -->

    <owl:NamedIndividual rdf:about="https://raw.githubusercontent.com/BOberreither/INTRO/master/INTRO_outdated.owl#TransT_DiscourseScholarlyDiscourseOnLiterature">
        <rdf:type rdf:resource="https://raw.githubusercontent.com/BOberreither/INTRO/master/INTRO_outdated.owl#Discourse"/>
        <hasAppurtenantElement rdf:resource="https://raw.githubusercontent.com/BOberreither/INTRO/master/INTRO_outdated.owl#SomeDissertation_1stEd"/>
        <hasAppurtenantElement rdf:resource="https://raw.githubusercontent.com/BOberreither/INTRO/master/INTRO_outdated.owl#SomeHandbook_1stEd"/>
        <hasAppurtenantElement rdf:resource="https://raw.githubusercontent.com/BOberreither/INTRO/master/INTRO_outdated.owl#SomeHandbook_Book"/>
        <hasAppurtenantElement rdf:resource="https://raw.githubusercontent.com/BOberreither/INTRO/master/INTRO_outdated.owl#SomeHandbook_Work"/>
        <rdfs:label>Literaturwiss. Diskurs</rdfs:label>
    </owl:NamedIndividual>
    


    <!-- https://raw.githubusercontent.com/BOberreither/INTRO/master/INTRO_outdated.owl#TransT_EpochGermanPopliterature -->

    <owl:NamedIndividual rdf:about="https://raw.githubusercontent.com/BOberreither/INTRO/master/INTRO_outdated.owl#TransT_EpochGermanPopliterature">
        <rdf:type rdf:resource="https://raw.githubusercontent.com/BOberreither/INTRO/master/INTRO_outdated.owl#Epoch"/>
        <rdfs:label>Epoche Popliteratur</rdfs:label>
    </owl:NamedIndividual>
    


    <!-- https://raw.githubusercontent.com/BOberreither/INTRO/master/INTRO_outdated.owl#TransT_LiteraryTheory -->

    <owl:NamedIndividual rdf:about="https://raw.githubusercontent.com/BOberreither/INTRO/master/INTRO_outdated.owl#TransT_LiteraryTheory">
        <rdf:type rdf:resource="https://raw.githubusercontent.com/BOberreither/INTRO/master/INTRO_outdated.owl#Discipline"/>
        <hasAppurtenantElement rdf:resource="https://raw.githubusercontent.com/BOberreither/INTRO/master/INTRO_outdated.owl#Palimpsests_1stEd"/>
        <rdfs:label>Disz. Literaturtheorie</rdfs:label>
    </owl:NamedIndividual>
    


    <!-- https://raw.githubusercontent.com/BOberreither/INTRO/master/INTRO_outdated.owl#TransT_OeuvreOfBillWatterson -->

    <owl:NamedIndividual rdf:about="https://raw.githubusercontent.com/BOberreither/INTRO/master/INTRO_outdated.owl#TransT_OeuvreOfBillWatterson">
        <rdf:type rdf:resource="https://raw.githubusercontent.com/BOberreither/INTRO/master/INTRO_outdated.owl#Oeuvre"/>
        <hasAppurtenantElement rdf:resource="https://raw.githubusercontent.com/BOberreither/INTRO/master/INTRO_outdated.owl#ItsAMagicalWorld_1stEd"/>
        <rdfs:label>Oeuvre Watterson</rdfs:label>
    </owl:NamedIndividual>
    


    <!-- https://raw.githubusercontent.com/BOberreither/INTRO/master/INTRO_outdated.owl#TransT_OeuvreOfPaulusHochgatterer -->

    <owl:NamedIndividual rdf:about="https://raw.githubusercontent.com/BOberreither/INTRO/master/INTRO_outdated.owl#TransT_OeuvreOfPaulusHochgatterer">
        <rdf:type rdf:resource="https://raw.githubusercontent.com/BOberreither/INTRO/master/INTRO_outdated.owl#Oeuvre"/>
        <hasAppurtenantElement rdf:resource="https://raw.githubusercontent.com/BOberreither/INTRO/master/INTRO_outdated.owl#CarettaCaretta_1stEd"/>
        <rdfs:label>Oeuvre Hochgatterer</rdfs:label>
    </owl:NamedIndividual>
    


    <!-- 
    ///////////////////////////////////////////////////////////////////////////////////////
    //
    // General axioms
    //
    ///////////////////////////////////////////////////////////////////////////////////////
     -->

    <rdf:Description>
        <rdf:type rdf:resource="http://www.w3.org/2002/07/owl#AllDisjointClasses"/>
        <owl:members rdf:parseType="Collection">
            <rdf:Description rdf:about="http://purl.org/spar/doco/Abstract"/>
            <rdf:Description rdf:about="http://purl.org/spar/doco/Afterword"/>
            <rdf:Description rdf:about="http://purl.org/spar/doco/Appendix"/>
            <rdf:Description rdf:about="http://purl.org/spar/doco/Colophon"/>
            <rdf:Description rdf:about="http://purl.org/spar/doco/Foreword"/>
            <rdf:Description rdf:about="http://purl.org/spar/doco/Glossary"/>
            <rdf:Description rdf:about="http://purl.org/spar/doco/Index"/>
            <rdf:Description rdf:about="http://purl.org/spar/doco/ListOfFigures"/>
            <rdf:Description rdf:about="http://purl.org/spar/doco/ListOfTables"/>
            <rdf:Description rdf:about="http://purl.org/spar/doco/Preface"/>
            <rdf:Description rdf:about="http://purl.org/spar/doco/TableOfContents"/>
        </owl:members>
    </rdf:Description>
    <rdf:Description>
        <rdf:type rdf:resource="http://www.w3.org/2002/07/owl#AllDisjointClasses"/>
        <owl:members rdf:parseType="Collection">
            <rdf:Description rdf:about="http://purl.org/spar/doco/BackMatter"/>
            <rdf:Description rdf:about="http://purl.org/spar/doco/BodyMatter"/>
            <rdf:Description rdf:about="http://purl.org/spar/doco/CaptionedBox"/>
            <rdf:Description rdf:about="http://purl.org/spar/doco/Chapter"/>
            <rdf:Description rdf:about="http://purl.org/spar/doco/ComplexRunInQuotation"/>
            <rdf:Description rdf:about="http://purl.org/spar/doco/Footnote"/>
            <rdf:Description rdf:about="http://purl.org/spar/doco/Formula"/>
            <rdf:Description rdf:about="http://purl.org/spar/doco/FormulaBox"/>
            <rdf:Description rdf:about="http://purl.org/spar/doco/FrontMatter"/>
            <rdf:Description rdf:about="http://purl.org/spar/doco/List"/>
            <rdf:Description rdf:about="http://purl.org/spar/doco/Part"/>
            <rdf:Description rdf:about="http://purl.org/spar/doco/Section"/>
            <rdf:Description rdf:about="http://purl.org/spar/doco/Table"/>
        </owl:members>
    </rdf:Description>
    <rdf:Description>
        <rdf:type rdf:resource="http://www.w3.org/2002/07/owl#AllDisjointClasses"/>
        <owl:members rdf:parseType="Collection">
            <rdf:Description rdf:about="http://purl.org/spar/doco/ListOfAuthors"/>
            <rdf:Description rdf:about="http://purl.org/spar/doco/ListOfContributors"/>
            <rdf:Description rdf:about="http://purl.org/spar/doco/ListOfOrganizations"/>
        </owl:members>
    </rdf:Description>
</rdf:RDF>



<!-- Generated by the OWL API (version 4.2.8.20170104-2310) https://github.com/owlcs/owlapi -->

